@prefix : <http://www.semanticweb.org/matte/ontologies/2025/10/untitled-ontology-4#> .
@prefix owl: <http://www.w3.org/2002/07/owl#> .
@prefix rdf: <http://www.w3.org/1999/02/22-rdf-syntax-ns#> .
@prefix xml: <http://www.w3.org/XML/1998/namespace> .
@prefix xsd: <http://www.w3.org/2001/XMLSchema#> .
@prefix rdfs: <http://www.w3.org/2000/01/rdf-schema#> .
@base <http://www.semanticweb.org/matte/ontologies/2025/10/untitled-ontology-4#> .

<http://www.semanticweb.org/matte/ontologies/2025/10/untitled-ontology-4> rdf:type owl:Ontology .

#################################################################
#    Annotation properties
#################################################################

###  http://purl.obolibrary.org/obo/IAO_0000114
<http://purl.obolibrary.org/obo/IAO_0000114> rdf:type owl:AnnotationProperty ;
                                             rdfs:label "has curation status"@en ,
                                                        "has curation status" .


###  http://purl.obolibrary.org/obo/IAO_0000412
<http://purl.obolibrary.org/obo/IAO_0000412> rdf:type owl:AnnotationProperty ;
                                             rdfs:label "imported from"@en .


###  http://rdfs.org/ns/void#inDataset
<http://rdfs.org/ns/void#inDataset> rdf:type owl:AnnotationProperty .


###  http://www.beerecipe.com/ontology#ebc
<http://www.beerecipe.com/ontology#ebc> rdf:type owl:AnnotationProperty .


###  http://www.geneontology.org/formats/oboInOwl#hasDbXref
<http://www.geneontology.org/formats/oboInOwl#hasDbXref> rdf:type owl:AnnotationProperty ;
                                                         rdfs:label "database_cross_reference" .


###  http://www.w3.org/2000/01/rdf-schema#label
rdfs:label rdfs:label "label"@en ,
                      "label" .


###  http://www.w3.org/2004/02/skos/core#definition
<http://www.w3.org/2004/02/skos/core#definition> rdf:type owl:AnnotationProperty .


###  http://www.w3.org/2004/02/skos/core#example
<http://www.w3.org/2004/02/skos/core#example> rdf:type owl:AnnotationProperty .


###  http://www.w3.org/2004/02/skos/core#historyNote
<http://www.w3.org/2004/02/skos/core#historyNote> rdf:type owl:AnnotationProperty .


###  http://www.w3.org/2004/02/skos/core#note
<http://www.w3.org/2004/02/skos/core#note> rdf:type owl:AnnotationProperty .


###  http://www.w3.org/ns/prov#hadPrimarySource
<http://www.w3.org/ns/prov#hadPrimarySource> rdf:type owl:AnnotationProperty .


###  http://xmlns.com/foaf/0.1/isPrimaryTopicOf
<http://xmlns.com/foaf/0.1/isPrimaryTopicOf> rdf:type owl:AnnotationProperty .


###  http://xmlns.com/foaf/0.1/name
<http://xmlns.com/foaf/0.1/name> rdf:type owl:AnnotationProperty .


###  https://rdf.ag/o/hops#alphaAcidsContent
<https://rdf.ag/o/hops#alphaAcidsContent> rdf:type owl:AnnotationProperty .


###  https://rdf.ag/o/hops#betaAcidsContent
<https://rdf.ag/o/hops#betaAcidsContent> rdf:type owl:AnnotationProperty .


###  https://rdf.ag/o/hops#perceivedAroma
<https://rdf.ag/o/hops#perceivedAroma> rdf:type owl:AnnotationProperty .


###  https://rdf.ag/o/hops#substitute
<https://rdf.ag/o/hops#substitute> rdf:type owl:AnnotationProperty .


###  https://rdf.ag/o/hops#totalOilContent
<https://rdf.ag/o/hops#totalOilContent> rdf:type owl:AnnotationProperty .


#################################################################
#    Datatypes
#################################################################

###  http://www.beerecipe.com/ontology#Cereal
<http://www.beerecipe.com/ontology#Cereal> rdf:type rdfs:Datatype .


###  http://www.beerecipe.com/ontology#Hop
<http://www.beerecipe.com/ontology#Hop> rdf:type rdfs:Datatype .


###  http://www.beerecipe.com/ontology#Malt
<http://www.beerecipe.com/ontology#Malt> rdf:type rdfs:Datatype .


###  http://www.semanticweb.org/matte/ontologies/2025/10/untitled-ontology-4#BrewingStep
:BrewingStep rdf:type rdfs:Datatype .


###  http://www.semanticweb.org/matte/ontologies/2025/10/untitled-ontology-4#Water
:Water rdf:type rdfs:Datatype .


###  http://www.semanticweb.org/matte/ontologies/2025/10/untitled-ontology-4#Yeast
:Yeast rdf:type rdfs:Datatype .


###  http://www.w3.org/2001/XMLSchema#date
xsd:date rdf:type rdfs:Datatype .


###  http://www.w3.org/2001/XMLSchema#float
xsd:float rdf:type rdfs:Datatype .


#################################################################
#    Object Properties
#################################################################

###  http://www.beerecipe.com/ontology#hasBeerStyle
<http://www.beerecipe.com/ontology#hasBeerStyle> rdf:type owl:ObjectProperty ;
                                                 rdfs:domain <https://rdf.ag/o/beer#Beer> ;
                                                 rdfs:range <http://www.beerecipe.com/ontology#BeerStyle> ;
                                                 owl:propertyChainAxiom ( <http://www.beerecipe.com/ontology#isProducedBy>
                                                                          <http://www.beerecipe.com/ontology#hasStyle>
                                                                        ) ;
                                                 rdfs:comment "Style of the beer, inferred from the recipe that produces it" ;
                                                 rdfs:label "has beer style" .


###  http://www.beerecipe.com/ontology#hasBrewingStep
<http://www.beerecipe.com/ontology#hasBrewingStep> rdf:type owl:ObjectProperty ;
                                                   owl:inverseOf <http://www.beerecipe.com/ontology#isStepOf> ;
                                                   rdfs:domain <http://www.beerecipe.com/ontology#Recipe> ;
                                                   rdfs:range <http://www.beerecipe.com/ontology#BrewingStep> .


###  http://www.beerecipe.com/ontology#hasCereal
<http://www.beerecipe.com/ontology#hasCereal> rdf:type owl:ObjectProperty ;
                                              rdfs:subPropertyOf <http://www.beerecipe.com/ontology#hasIngredient> ;
                                              owl:inverseOf <http://www.beerecipe.com/ontology#isCerealOf> ;
                                              rdfs:domain <http://www.beerecipe.com/ontology#Recipe> ;
                                              rdfs:range :Cereal .


###  http://www.beerecipe.com/ontology#hasDifficultyLevel
<http://www.beerecipe.com/ontology#hasDifficultyLevel> rdf:type owl:ObjectProperty ,
                                                                owl:FunctionalProperty ;
                                                       rdfs:domain <http://www.beerecipe.com/ontology#Recipe> ;
                                                       rdfs:range <http://www.beerecipe.com/ontology#DifficultyLevel> ;
                                                       rdfs:comment "Connects a recipe to its difficulty level classification" ;
                                                       rdfs:label "has difficulty level" .


###  http://www.beerecipe.com/ontology#hasFlavorProfile
<http://www.beerecipe.com/ontology#hasFlavorProfile> rdf:type owl:ObjectProperty ;
                                                     owl:inverseOf <http://www.beerecipe.com/ontology#isFlavorOf> ;
                                                     rdf:type owl:FunctionalProperty ;
                                                     rdfs:domain <http://www.beerecipe.com/ontology#Ingredient> ;
                                                     rdfs:range <http://www.beerecipe.com/ontology#FlavorProfile> ;
                                                     rdfs:comment "Connects an ingredient to its flavor profile (citrus, pine, floral, etc.)" ;
                                                     rdfs:label "has flavor profile" .


###  http://www.beerecipe.com/ontology#hasHop
<http://www.beerecipe.com/ontology#hasHop> rdf:type owl:ObjectProperty ;
                                           rdfs:subPropertyOf <http://www.beerecipe.com/ontology#hasIngredient> ;
                                           owl:inverseOf <http://www.beerecipe.com/ontology#isHopOf> ;
                                           rdfs:domain <http://www.beerecipe.com/ontology#Recipe> ;
                                           rdfs:range <https://rdf.ag/o/hops#Hops> .


###  http://www.beerecipe.com/ontology#hasIngredient
<http://www.beerecipe.com/ontology#hasIngredient> rdf:type owl:ObjectProperty ;
                                                  owl:inverseOf <http://www.beerecipe.com/ontology#isIngredientOf> ;
                                                  rdfs:domain <http://www.beerecipe.com/ontology#Recipe> ;
                                                  rdfs:range <http://www.beerecipe.com/ontology#Ingredient> .


###  http://www.beerecipe.com/ontology#hasMalt
<http://www.beerecipe.com/ontology#hasMalt> rdf:type owl:ObjectProperty ;
                                            rdfs:subPropertyOf <http://www.beerecipe.com/ontology#hasIngredient> ;
                                            owl:inverseOf <http://www.beerecipe.com/ontology#isMaltOf> ;
                                            rdfs:domain <http://www.beerecipe.com/ontology#Recipe> ;
                                            rdfs:range <https://rdf.ag/o/malt#Malt> .


###  http://www.beerecipe.com/ontology#hasOriginCountry
<http://www.beerecipe.com/ontology#hasOriginCountry> rdf:type owl:ObjectProperty ;
                                                     owl:inverseOf <http://www.beerecipe.com/ontology#isOriginOf> ;
                                                     rdf:type owl:FunctionalProperty ;
                                                     rdfs:domain <http://www.beerecipe.com/ontology#Ingredient> ;
                                                     rdfs:range <http://www.beerecipe.com/ontology#Country> ;
                                                     rdfs:comment "Connects an ingredient to its country of origin" ;
                                                     rdfs:label "has origin country" .


###  http://www.beerecipe.com/ontology#hasStyle
<http://www.beerecipe.com/ontology#hasStyle> rdf:type owl:ObjectProperty ;
                                             owl:inverseOf <http://www.beerecipe.com/ontology#isStyleOf> ;
                                             rdf:type owl:FunctionalProperty ;
                                             rdfs:domain <http://www.beerecipe.com/ontology#Recipe> ;
                                             rdfs:range <http://www.beerecipe.com/ontology#BeerStyle> .


###  http://www.beerecipe.com/ontology#hasYeast
<http://www.beerecipe.com/ontology#hasYeast> rdf:type owl:ObjectProperty ;
                                             rdfs:subPropertyOf <http://www.beerecipe.com/ontology#hasIngredient> ;
                                             owl:inverseOf <http://www.beerecipe.com/ontology#isYeastOf> ;
                                             rdfs:domain <http://www.beerecipe.com/ontology#Recipe> ;
                                             rdfs:range <http://www.beerecipe.com/ontology#Yeast> .


###  http://www.beerecipe.com/ontology#isCerealOf
<http://www.beerecipe.com/ontology#isCerealOf> rdf:type owl:ObjectProperty ;
                                               rdfs:domain :Cereal ;
                                               rdfs:range <http://www.beerecipe.com/ontology#Recipe> .


###  http://www.beerecipe.com/ontology#isFlavorOf
<http://www.beerecipe.com/ontology#isFlavorOf> rdf:type owl:ObjectProperty ;
                                               rdfs:domain <http://www.beerecipe.com/ontology#FlavorProfile> ;
                                               rdfs:range <http://www.beerecipe.com/ontology#Ingredient> ;
                                               rdfs:comment "Indicates which ingredients have this flavor profile" ;
                                               rdfs:label "is flavor of" .


###  http://www.beerecipe.com/ontology#isHopOf
<http://www.beerecipe.com/ontology#isHopOf> rdf:type owl:ObjectProperty ;
                                            rdfs:domain <https://rdf.ag/o/hops#Hops> ;
                                            rdfs:range <http://www.beerecipe.com/ontology#Recipe> .


###  http://www.beerecipe.com/ontology#isIngredientOf
<http://www.beerecipe.com/ontology#isIngredientOf> rdf:type owl:ObjectProperty ;
                                                   rdfs:domain <http://www.beerecipe.com/ontology#Ingredient> ;
                                                   rdfs:range <http://www.beerecipe.com/ontology#Recipe> .


###  http://www.beerecipe.com/ontology#isMaltOf
<http://www.beerecipe.com/ontology#isMaltOf> rdf:type owl:ObjectProperty ;
                                             rdfs:domain <https://rdf.ag/o/malt#Malt> ;
                                             rdfs:range <http://www.beerecipe.com/ontology#Recipe> .


###  http://www.beerecipe.com/ontology#isOriginOf
<http://www.beerecipe.com/ontology#isOriginOf> rdf:type owl:ObjectProperty ;
                                               rdfs:domain <http://www.beerecipe.com/ontology#Country> ;
                                               rdfs:range <http://www.beerecipe.com/ontology#Ingredient> .


###  http://www.beerecipe.com/ontology#isProducedBy
<http://www.beerecipe.com/ontology#isProducedBy> rdf:type owl:ObjectProperty ;
                                                 owl:inverseOf <http://www.beerecipe.com/ontology#producesBeer> ;
                                                 rdfs:range <http://www.beerecipe.com/ontology#Recipe> .


###  http://www.beerecipe.com/ontology#isRequiredBy
<http://www.beerecipe.com/ontology#isRequiredBy> rdf:type owl:ObjectProperty ;
                                                 owl:inverseOf <http://www.beerecipe.com/ontology#requiresEquipment> ;
                                                 rdfs:domain <http://www.beerecipe.com/ontology#Equipment> ;
                                                 rdfs:range <http://www.beerecipe.com/ontology#Recipe> .


###  http://www.beerecipe.com/ontology#isSimilarTo
<http://www.beerecipe.com/ontology#isSimilarTo> rdf:type owl:ObjectProperty ,
                                                         owl:SymmetricProperty ,
                                                         owl:TransitiveProperty ;
                                                rdfs:domain <http://www.beerecipe.com/ontology#Recipe> ;
                                                rdfs:range <http://www.beerecipe.com/ontology#Recipe> .


###  http://www.beerecipe.com/ontology#isStepOf
<http://www.beerecipe.com/ontology#isStepOf> rdf:type owl:ObjectProperty ;
                                             rdfs:domain <http://www.beerecipe.com/ontology#BrewingStep> ;
                                             rdfs:range <http://www.beerecipe.com/ontology#Recipe> .


###  http://www.beerecipe.com/ontology#isStyleOf
<http://www.beerecipe.com/ontology#isStyleOf> rdf:type owl:ObjectProperty ;
                                              rdfs:domain <http://www.beerecipe.com/ontology#BeerStyle> ;
                                              rdfs:range <http://www.beerecipe.com/ontology#Recipe> .


###  http://www.beerecipe.com/ontology#isSubstituteOf
<http://www.beerecipe.com/ontology#isSubstituteOf> rdf:type owl:ObjectProperty ,
                                                            owl:SymmetricProperty ;
                                                   rdfs:domain <http://www.beerecipe.com/ontology#Ingredient> ;
                                                   rdfs:range <http://www.beerecipe.com/ontology#Ingredient> ;
                                                   rdfs:comment "Indicates that one ingredient can substitute another. This is a symmetric property." ;
                                                   rdfs:label "is substitute of" .


###  http://www.beerecipe.com/ontology#isSuitableFor
<http://www.beerecipe.com/ontology#isSuitableFor> rdf:type owl:ObjectProperty ;
                                                  rdfs:domain <http://www.beerecipe.com/ontology#Recipe> ;
                                                  rdfs:range <http://www.beerecipe.com/ontology#DietaryRequirement> ;
                                                  rdfs:comment "Indicates dietary requirements that a recipe is suitable for (vegan, gluten-free, etc.)" ;
                                                  rdfs:label "is suitable for" .


###  http://www.beerecipe.com/ontology#isYeastOf
<http://www.beerecipe.com/ontology#isYeastOf> rdf:type owl:ObjectProperty ;
                                              rdfs:domain <http://www.beerecipe.com/ontology#Yeast> ;
                                              rdfs:range <http://www.beerecipe.com/ontology#Recipe> .


###  http://www.beerecipe.com/ontology#producesBeer
<http://www.beerecipe.com/ontology#producesBeer> rdf:type owl:ObjectProperty ,
                                                          owl:FunctionalProperty ;
                                                 rdfs:domain <http://www.beerecipe.com/ontology#Recipe> ;
                                                 rdfs:range <https://rdf.ag/o/beer#Beer> .


###  http://www.beerecipe.com/ontology#requiresEquipment
<http://www.beerecipe.com/ontology#requiresEquipment> rdf:type owl:ObjectProperty ,
                                                               owl:TransitiveProperty ;
                                                      rdfs:domain <http://www.beerecipe.com/ontology#Recipe> ;
                                                      rdfs:range <http://www.beerecipe.com/ontology#Equipment> ;
                                                      rdfs:comment "Connects a recipe to the equipment required" ;
                                                      rdfs:label "requires equipment" .


###  http://www.semanticweb.org/matte/ontologies/2025/10/untitled-ontology-4#hasWater
:hasWater rdf:type owl:ObjectProperty ;
          rdfs:subPropertyOf <http://www.beerecipe.com/ontology#hasIngredient> ;
          rdfs:domain <http://www.beerecipe.com/ontology#Recipe> ;
          rdfs:range :Water .


#################################################################
#    Data properties
#################################################################

###  http://www.beerecipe.com/ontology#additionTime
<http://www.beerecipe.com/ontology#additionTime> rdf:type owl:DatatypeProperty ;
                                                 rdfs:domain <https://rdf.ag/o/hops#Hops> ;
                                                 rdfs:range xsd:int ;
                                                 rdfs:comment "Time of addition in minutes from start of boil (e.g., 60, 15, 0)" ;
                                                 rdfs:label "addition time" .


###  http://www.beerecipe.com/ontology#alphaAcidPercentage
<http://www.beerecipe.com/ontology#alphaAcidPercentage> rdf:type owl:DatatypeProperty ;
                                                        rdfs:domain <https://rdf.ag/o/hops#Hops> ;
                                                        rdfs:range xsd:float ;
                                                        rdfs:comment "Alpha acid percentage of the hop" ;
                                                        rdfs:label "alpha acid percentage" .


###  http://www.beerecipe.com/ontology#author
<http://www.beerecipe.com/ontology#author> rdf:type owl:DatatypeProperty ;
                                           rdfs:domain <http://www.beerecipe.com/ontology#Recipe> ;
                                           rdfs:range xsd:string ;
                                           rdfs:comment "The author or creator of the recipe" ;
                                           rdfs:label "author" .


###  http://www.beerecipe.com/ontology#batchSize
<http://www.beerecipe.com/ontology#batchSize> rdf:type owl:DatatypeProperty ;
                                              rdfs:domain <http://www.beerecipe.com/ontology#Recipe> ;
                                              rdfs:range xsd:float ;
                                              rdfs:comment "Volume of beer produced in liters" ;
                                              rdfs:label "batch size" .


###  http://www.beerecipe.com/ontology#boilingTime
<http://www.beerecipe.com/ontology#boilingTime> rdf:type owl:DatatypeProperty ;
                                                rdfs:domain <http://www.beerecipe.com/ontology#Recipe> ;
                                                rdfs:range xsd:int ;
                                                rdfs:comment "Duration of the boiling step in minutes" ;
                                                rdfs:label "boiling time" .


###  http://www.beerecipe.com/ontology#cerealName
<http://www.beerecipe.com/ontology#cerealName> rdf:type owl:DatatypeProperty ;
                                               rdfs:domain :Cereal ;
                                               rdfs:range xsd:string ;
                                               rdfs:comment "The name of the cereal" ;
                                               rdfs:label "cereal name" .


###  http://www.beerecipe.com/ontology#conditioningDuration
<http://www.beerecipe.com/ontology#conditioningDuration> rdf:type owl:DatatypeProperty ;
                                                         rdfs:domain <http://www.beerecipe.com/ontology#Recipe> ;
                                                         rdfs:range xsd:int ;
                                                         rdfs:comment "Duration of conditioning in days" ;
                                                         rdfs:label "conditioning duration" .


###  http://www.beerecipe.com/ontology#creationDate
<http://www.beerecipe.com/ontology#creationDate> rdf:type owl:DatatypeProperty ;
                                                 rdfs:domain <http://www.beerecipe.com/ontology#Recipe> ;
                                                 rdfs:range xsd:date ;
                                                 rdfs:comment "The date when the recipe was created" ;
                                                 rdfs:label "creation date" .


###  http://www.beerecipe.com/ontology#difficultyLevel
<http://www.beerecipe.com/ontology#difficultyLevel> rdf:type owl:DatatypeProperty ;
                                                    rdfs:domain <http://www.beerecipe.com/ontology#Recipe> ;
                                                    rdfs:range xsd:string ;
                                                    rdfs:comment "Difficulty level: beginner, intermediate, advanced, or expert" ;
                                                    rdfs:label "difficulty level" .


###  http://www.beerecipe.com/ontology#ebcColor
<http://www.beerecipe.com/ontology#ebcColor> rdf:type owl:DatatypeProperty ;
                                             rdfs:domain <https://rdf.ag/o/malt#Malt> ;
                                             rdfs:range xsd:int ;
                                             rdfs:comment "Color contribution in EBC units" ;
                                             rdfs:label "EBC color" .


###  http://www.beerecipe.com/ontology#estimatedABV
<http://www.beerecipe.com/ontology#estimatedABV> rdf:type owl:DatatypeProperty ;
                                                 rdfs:domain <http://www.beerecipe.com/ontology#Recipe> ;
                                                 rdfs:range xsd:float ;
                                                 rdfs:comment "Estimated Alcohol By Volume percentage" ;
                                                 rdfs:label "estimated ABV" .


###  http://www.beerecipe.com/ontology#estimatedEBC
<http://www.beerecipe.com/ontology#estimatedEBC> rdf:type owl:DatatypeProperty ;
                                                 rdfs:domain <http://www.beerecipe.com/ontology#Recipe> ;
                                                 rdfs:range xsd:int ;
                                                 rdfs:comment "Estimated color in European Brewery Convention units" ;
                                                 rdfs:label "estimated EBC" .


###  http://www.beerecipe.com/ontology#estimatedIBU
<http://www.beerecipe.com/ontology#estimatedIBU> rdf:type owl:DatatypeProperty ;
                                                 rdfs:domain <http://www.beerecipe.com/ontology#Recipe> ;
                                                 rdfs:range xsd:int ;
                                                 rdfs:comment "Estimated International Bitterness Units" ;
                                                 rdfs:label "estimated IBU" .


###  http://www.beerecipe.com/ontology#fermentationDuration
<http://www.beerecipe.com/ontology#fermentationDuration> rdf:type owl:DatatypeProperty ;
                                                         rdfs:domain <http://www.beerecipe.com/ontology#Recipe> ;
                                                         rdfs:range xsd:int ;
                                                         rdfs:comment "Duration of fermentation in days" ;
                                                         rdfs:label "fermentation duration" .


###  http://www.beerecipe.com/ontology#finalGravity
<http://www.beerecipe.com/ontology#finalGravity> rdf:type owl:DatatypeProperty ;
                                                 rdfs:domain <http://www.beerecipe.com/ontology#Recipe> ;
                                                 rdfs:range xsd:float ;
                                                 rdfs:comment "Final gravity of the beer after fermentation" ;
                                                 rdfs:label "final gravity" .


###  http://www.beerecipe.com/ontology#glutenContent
<http://www.beerecipe.com/ontology#glutenContent> rdf:type owl:DatatypeProperty ;
                                                  rdfs:domain :Cereal ;
                                                  rdfs:range xsd:boolean ;
                                                  rdfs:comment "Indicates if the cereal contains gluten" ;
                                                  rdfs:label "gluten content" .


###  http://www.beerecipe.com/ontology#hasBrewingStep
<http://www.beerecipe.com/ontology#hasBrewingStep> rdf:type owl:DatatypeProperty ;
                                                   rdfs:range :BrewingStep .


###  http://www.beerecipe.com/ontology#hasCereal
<http://www.beerecipe.com/ontology#hasCereal> rdf:type owl:DatatypeProperty ;
                                              rdfs:range <http://www.beerecipe.com/ontology#Cereal> .


###  http://www.beerecipe.com/ontology#hasHop
<http://www.beerecipe.com/ontology#hasHop> rdf:type owl:DatatypeProperty ;
                                           rdfs:range <http://www.beerecipe.com/ontology#Hop> .


###  http://www.beerecipe.com/ontology#hasIngredient
<http://www.beerecipe.com/ontology#hasIngredient> rdf:type owl:DatatypeProperty .


###  http://www.beerecipe.com/ontology#hasMalt
<http://www.beerecipe.com/ontology#hasMalt> rdf:type owl:DatatypeProperty ;
                                            rdfs:range <http://www.beerecipe.com/ontology#Malt> .


###  http://www.beerecipe.com/ontology#hasStyle
<http://www.beerecipe.com/ontology#hasStyle> rdf:type owl:DatatypeProperty ,
                                                      owl:FunctionalProperty .


###  http://www.beerecipe.com/ontology#hopName
<http://www.beerecipe.com/ontology#hopName> rdf:type owl:DatatypeProperty ;
                                            rdfs:domain <https://rdf.ag/o/hops#Hops> ;
                                            rdfs:range xsd:string ;
                                            rdfs:comment "The name of the hop variety" ;
                                            rdfs:label "hop name" .


###  http://www.beerecipe.com/ontology#ingredientName
<http://www.beerecipe.com/ontology#ingredientName> rdf:type owl:DatatypeProperty ;
                                                   rdfs:domain <http://www.beerecipe.com/ontology#Ingredient> ;
                                                   rdfs:range xsd:string ;
                                                   rdfs:comment "The name of the ingredient" ;
                                                   rdfs:label "ingredient name" .


###  http://www.beerecipe.com/ontology#isCerealOf
<http://www.beerecipe.com/ontology#isCerealOf> rdf:type owl:DatatypeProperty .


###  http://www.beerecipe.com/ontology#isGlutenFree
<http://www.beerecipe.com/ontology#isGlutenFree> rdf:type owl:DatatypeProperty ;
                                                 rdfs:domain <http://www.beerecipe.com/ontology#Recipe> ;
                                                 rdfs:range xsd:boolean ;
                                                 rdfs:comment "Indicates if the recipe is gluten-free" ;
                                                 rdfs:label "is gluten free" .


###  http://www.beerecipe.com/ontology#isHopOf
<http://www.beerecipe.com/ontology#isHopOf> rdf:type owl:DatatypeProperty .


###  http://www.beerecipe.com/ontology#isIngredientOf
<http://www.beerecipe.com/ontology#isIngredientOf> rdf:type owl:DatatypeProperty .


###  http://www.beerecipe.com/ontology#isMaltOf
<http://www.beerecipe.com/ontology#isMaltOf> rdf:type owl:DatatypeProperty .


###  http://www.beerecipe.com/ontology#isOriginOf
<http://www.beerecipe.com/ontology#isOriginOf> rdf:type owl:DatatypeProperty .


###  http://www.beerecipe.com/ontology#isProducedBy
<http://www.beerecipe.com/ontology#isProducedBy> rdf:type owl:DatatypeProperty .


###  http://www.beerecipe.com/ontology#isRequiredBy
<http://www.beerecipe.com/ontology#isRequiredBy> rdf:type owl:DatatypeProperty .


###  http://www.beerecipe.com/ontology#isSimilarTo
<http://www.beerecipe.com/ontology#isSimilarTo> rdf:type owl:DatatypeProperty .


###  http://www.beerecipe.com/ontology#isStepOf
<http://www.beerecipe.com/ontology#isStepOf> rdf:type owl:DatatypeProperty .


###  http://www.beerecipe.com/ontology#isStyleOf
<http://www.beerecipe.com/ontology#isStyleOf> rdf:type owl:DatatypeProperty .


###  http://www.beerecipe.com/ontology#isVegan
<http://www.beerecipe.com/ontology#isVegan> rdf:type owl:DatatypeProperty ;
                                            rdfs:domain <http://www.beerecipe.com/ontology#Recipe> ;
                                            rdfs:range xsd:boolean ;
                                            rdfs:comment "Indicates if the recipe is suitable for vegans" ;
                                            rdfs:label "is vegan" .


###  http://www.beerecipe.com/ontology#isYeastOf
<http://www.beerecipe.com/ontology#isYeastOf> rdf:type owl:DatatypeProperty .


###  http://www.beerecipe.com/ontology#maltName
<http://www.beerecipe.com/ontology#maltName> rdf:type owl:DatatypeProperty ;
                                             rdfs:range xsd:string ;
                                             rdfs:comment "The name of the malt" ;
                                             rdfs:label "malt name" .


###  http://www.beerecipe.com/ontology#mashingTime
<http://www.beerecipe.com/ontology#mashingTime> rdf:type owl:DatatypeProperty ;
                                                rdfs:domain <http://www.beerecipe.com/ontology#Recipe> ;
                                                rdfs:range xsd:int ;
                                                rdfs:comment "Duration of the mashing step in minutes" ;
                                                rdfs:label "mashing time" .


###  http://www.beerecipe.com/ontology#maxABV
<http://www.beerecipe.com/ontology#maxABV> rdf:type owl:DatatypeProperty ;
                                           rdfs:domain <http://www.beerecipe.com/ontology#BeerStyle> ;
                                           rdfs:range xsd:float ;
                                           rdfs:comment "Maximum ABV for this beer style" ;
                                           rdfs:label "maximum ABV" .


###  http://www.beerecipe.com/ontology#maxAttenuation
<http://www.beerecipe.com/ontology#maxAttenuation> rdf:type owl:DatatypeProperty ;
                                                   rdfs:domain <http://www.beerecipe.com/ontology#Yeast> ;
                                                   rdfs:range xsd:decimal ;
                                                   rdfs:comment "Maximum expected attenuation as percentage (numeric value)."@en ;
                                                   rdfs:label "maxAttenuation"@en .


###  http://www.beerecipe.com/ontology#maxIBU
<http://www.beerecipe.com/ontology#maxIBU> rdf:type owl:DatatypeProperty ;
                                           rdfs:domain <http://www.beerecipe.com/ontology#BeerStyle> ;
                                           rdfs:range xsd:int ;
                                           rdfs:comment "Maximum IBU for this beer style" ;
                                           rdfs:label "maximum IBU" .


###  http://www.beerecipe.com/ontology#minABV
<http://www.beerecipe.com/ontology#minABV> rdf:type owl:DatatypeProperty ;
                                           rdfs:domain <http://www.beerecipe.com/ontology#BeerStyle> ;
                                           rdfs:range xsd:float ;
                                           rdfs:comment "Minimum ABV for this beer style" ;
                                           rdfs:label "minimum ABV" .


###  http://www.beerecipe.com/ontology#minAttenuation
<http://www.beerecipe.com/ontology#minAttenuation> rdf:type owl:DatatypeProperty ;
                                                   rdfs:domain <http://www.beerecipe.com/ontology#Yeast> ;
                                                   rdfs:range xsd:decimal ;
                                                   rdfs:comment "Minimum expected attenuation as percentage (numeric value, e.g. 68 or 0.68 depending on convention)."@en ;
                                                   rdfs:label "minAttenuation"@en .


###  http://www.beerecipe.com/ontology#minIBU
<http://www.beerecipe.com/ontology#minIBU> rdf:type owl:DatatypeProperty ;
                                           rdfs:domain <http://www.beerecipe.com/ontology#BeerStyle> ;
                                           rdfs:range xsd:int ;
                                           rdfs:comment "Minimum IBU for this beer style" ;
                                           rdfs:label "minimum IBU" .


###  http://www.beerecipe.com/ontology#optimalTemperature
<http://www.beerecipe.com/ontology#optimalTemperature> rdf:type owl:DatatypeProperty ;
                                                       rdfs:domain <http://www.beerecipe.com/ontology#Yeast> ;
                                                       rdfs:range xsd:float ;
                                                       rdfs:comment "Optimal fermentation temperature (degrees Celsius)."@en ;
                                                       rdfs:label "optimalTemperature"@en .


###  http://www.beerecipe.com/ontology#originalGravity
<http://www.beerecipe.com/ontology#originalGravity> rdf:type owl:DatatypeProperty ;
                                                    rdfs:domain <http://www.beerecipe.com/ontology#Recipe> ;
                                                    rdfs:range xsd:float ;
                                                    rdfs:comment "Original gravity of the wort before fermentation" ;
                                                    rdfs:label "original gravity" .


###  http://www.beerecipe.com/ontology#producesBeer
<http://www.beerecipe.com/ontology#producesBeer> rdf:type owl:DatatypeProperty ,
                                                          owl:FunctionalProperty .


###  http://www.beerecipe.com/ontology#quantity
<http://www.beerecipe.com/ontology#quantity> rdf:type owl:DatatypeProperty ;
                                             rdfs:domain <http://www.beerecipe.com/ontology#Ingredient> ;
                                             rdfs:range xsd:float ;
                                             rdfs:comment "Quantity of ingredient used" ;
                                             rdfs:label "quantity" .


###  http://www.beerecipe.com/ontology#recipeDescription
<http://www.beerecipe.com/ontology#recipeDescription> rdf:type owl:DatatypeProperty ;
                                                      rdfs:domain <http://www.beerecipe.com/ontology#Recipe> ;
                                                      rdfs:range xsd:string ;
                                                      rdfs:comment "A textual description of the recipe" ;
                                                      rdfs:label "recipe description" .


###  http://www.beerecipe.com/ontology#recipeName
<http://www.beerecipe.com/ontology#recipeName> rdf:type owl:DatatypeProperty ;
                                               rdfs:domain <http://www.beerecipe.com/ontology#Recipe> ;
                                               rdfs:range xsd:string ;
                                               rdfs:comment "The name of the recipe" ;
                                               rdfs:label "recipe name" .


###  http://www.beerecipe.com/ontology#servingTemperature
<http://www.beerecipe.com/ontology#servingTemperature> rdf:type owl:DatatypeProperty ;
                                                       rdfs:domain <http://www.beerecipe.com/ontology#Recipe> ;
                                                       rdfs:range xsd:float ;
                                                       rdfs:comment "Recommended serving temperature in Celsius" ;
                                                       rdfs:label "serving temperature" .


###  http://www.beerecipe.com/ontology#stepDuration
<http://www.beerecipe.com/ontology#stepDuration> rdf:type owl:DatatypeProperty ;
                                                 rdfs:domain <http://www.beerecipe.com/ontology#BrewingStep> ;
                                                 rdfs:range xsd:int ;
                                                 rdfs:comment "Duration of the step in minutes" ;
                                                 rdfs:label "step duration" .


###  http://www.beerecipe.com/ontology#stepInstructions
<http://www.beerecipe.com/ontology#stepInstructions> rdf:type owl:DatatypeProperty ;
                                                     rdfs:domain <http://www.beerecipe.com/ontology#BrewingStep> ;
                                                     rdfs:range xsd:string ;
                                                     rdfs:comment "Detailed instructions for the brewing step" ;
                                                     rdfs:label "step instructions" .


###  http://www.beerecipe.com/ontology#stepName
<http://www.beerecipe.com/ontology#stepName> rdf:type owl:DatatypeProperty ;
                                             rdfs:domain <http://www.beerecipe.com/ontology#BrewingStep> ;
                                             rdfs:range xsd:string ;
                                             rdfs:comment "The name of the brewing step" ;
                                             rdfs:label "step name" .


###  http://www.beerecipe.com/ontology#stepOrder
<http://www.beerecipe.com/ontology#stepOrder> rdf:type owl:DatatypeProperty ;
                                              rdfs:domain <http://www.beerecipe.com/ontology#BrewingStep> ;
                                              rdfs:range xsd:int ;
                                              rdfs:comment "Order of the step in the brewing process (1, 2, 3...)" ;
                                              rdfs:label "step order" .


###  http://www.beerecipe.com/ontology#stepTemperature
<http://www.beerecipe.com/ontology#stepTemperature> rdf:type owl:DatatypeProperty ;
                                                    rdfs:domain <http://www.beerecipe.com/ontology#BrewingStep> ;
                                                    rdfs:range xsd:float ;
                                                    rdfs:comment "Temperature of the step in Celsius" ;
                                                    rdfs:label "step temperature" .


###  http://www.beerecipe.com/ontology#styleDescription
<http://www.beerecipe.com/ontology#styleDescription> rdf:type owl:DatatypeProperty ;
                                                     rdfs:domain <http://www.beerecipe.com/ontology#BeerStyle> ;
                                                     rdfs:range xsd:string ;
                                                     rdfs:comment "Description of the beer style characteristics" ;
                                                     rdfs:label "style description" .


###  http://www.beerecipe.com/ontology#styleName
<http://www.beerecipe.com/ontology#styleName> rdf:type owl:DatatypeProperty ;
                                              rdfs:domain <http://www.beerecipe.com/ontology#BeerStyle> ;
                                              rdfs:range xsd:string ;
                                              rdfs:comment "The name of the beer style" ;
                                              rdfs:label "style name" .


###  http://www.beerecipe.com/ontology#totalBrewingTime
<http://www.beerecipe.com/ontology#totalBrewingTime> rdf:type owl:DatatypeProperty ;
                                                     rdfs:domain <http://www.beerecipe.com/ontology#Recipe> ;
                                                     rdfs:range xsd:int ;
                                                     rdfs:comment "Total brewing time in minutes" ;
                                                     rdfs:label "total brewing time" .


###  http://www.beerecipe.com/ontology#unit
<http://www.beerecipe.com/ontology#unit> rdf:type owl:DatatypeProperty ;
                                         rdfs:domain <http://www.beerecipe.com/ontology#Ingredient> ;
                                         rdfs:range xsd:string ;
                                         rdfs:comment "Unit of measurement: grams, kg, liters, ml, oz, lbs" ;
                                         rdfs:label "unit" .


###  http://www.beerecipe.com/ontology#yeastDescription
<http://www.beerecipe.com/ontology#yeastDescription> rdf:type owl:DatatypeProperty ;
                                                     rdfs:domain <http://www.beerecipe.com/ontology#Yeast> ;
                                                     rdfs:range xsd:string ;
                                                     rdfs:comment "Short description of yeast characteristics, flavors and typical uses."@en ;
                                                     rdfs:label "yeastDescription"@en .


###  http://www.beerecipe.com/ontology#yeastName
<http://www.beerecipe.com/ontology#yeastName> rdf:type owl:DatatypeProperty ;
                                              rdfs:domain <http://www.beerecipe.com/ontology#Yeast> ;
                                              rdfs:range xsd:string ;
                                              rdfs:comment "Human-readable name of the yeast strain."@en ;
                                              rdfs:label "yeastName"@en .


#################################################################
#    Classes
#################################################################

###  http://purl.obolibrary.org/obo/FOODON_00001178
<http://purl.obolibrary.org/obo/FOODON_00001178> rdf:type owl:Class ;
                                                 rdfs:subClassOf :FoodIngredient ;
                                                 <http://purl.obolibrary.org/obo/IAO_0000412> "http://purl.obolibrary.org/obo/foodon/releases/2025-08-01/foodon.owl" ;
                                                 rdfs:label "honey food product"@en .


###  http://purl.obolibrary.org/obo/FOODON_00001260
<http://purl.obolibrary.org/obo/FOODON_00001260> rdf:type owl:Class ;
                                                 owl:equivalentClass <https://rdf.ag/o/beer#Beer> .


###  http://purl.obolibrary.org/obo/FOODON_03301475
<http://purl.obolibrary.org/obo/FOODON_03301475> rdf:type owl:Class ;
                                                 rdfs:subClassOf :FoodIngredient ;
                                                 <http://purl.obolibrary.org/obo/IAO_0000114> <http://purl.obolibrary.org/obo/IAO_0000428> ;
                                                 <http://purl.obolibrary.org/obo/IAO_0000412> "http://purl.obolibrary.org/obo/foodon/releases/2025-08-01/foodon.owl" ;
                                                 <http://www.geneontology.org/formats/oboInOwl#hasDbXref> <https://bioregistry.io/reference/siren:F1475> ;
                                                 rdfs:comment """SIREN DB annotation:
* crystal FOODON:03430143
* fully heat-treated FOODON:03440014
* sugar FOODON:03420108
* acidified FOODON:03460200
* food hydrolyzation process FOODON:03460277"""@en ;
                                                 rdfs:label "corn sugar"@en .


###  http://www.beerecipe.com/ontology#BeerStyle
<http://www.beerecipe.com/ontology#BeerStyle> rdf:type owl:Class ;
                                              rdfs:comment "A beer style is a classification of beer based on various factors including appearance, flavor, ingredients, production method, history, and origin. Beer styles provide guidelines for acceptable ranges of characteristics such as color, bitterness, alcohol content, and aroma."@en ;
                                              rdfs:label "Beer Style"@en ;
                                              <http://www.w3.org/2004/02/skos/core#definition> "A categorization system for beer that defines characteristic ranges for properties like ABV, IBU, color (EBC/SRM), and typical flavor profiles. Styles are often defined by brewing organizations like BJCP or Brewers Association."@en ;
                                              <http://www.w3.org/2004/02/skos/core#example> "American IPA: 5.5-7.5% ABV, 40-70 IBU, characterized by prominent hop bitterness and citrus aroma from American hop varieties."@en ;
                                              <http://www.w3.org/2004/02/skos/core#note> "Beer styles evolve over time and may vary between different classification systems. Modern craft brewing has also created many hybrid and experimental styles."@en .


###  http://www.beerecipe.com/ontology#BoilStep
<http://www.beerecipe.com/ontology#BoilStep> rdf:type owl:Class ;
                                             rdfs:subClassOf <http://www.beerecipe.com/ontology#BrewingStep> ;
                                             rdfs:comment "Step where wort is boiled to sterilize and isomerize hop alpha acids."@en ;
                                             rdfs:label "Boil Step" .


###  http://www.beerecipe.com/ontology#BrewingStep
<http://www.beerecipe.com/ontology#BrewingStep> rdf:type owl:Class ;
                                                rdfs:comment "A brewing step represents a specific stage in the beer production process. Each step has defined parameters including duration, temperature, and specific instructions. Common steps include mashing, lautering, boiling, fermentation, and conditioning."@en ;
                                                rdfs:label "Brewing Step"@en ;
                                                <http://www.w3.org/2004/02/skos/core#definition> "An individual procedural stage in the brewing process, characterized by specific time duration, temperature, order of execution, and detailed instructions that must be followed to achieve desired beer characteristics."@en ;
                                                <http://www.w3.org/2004/02/skos/core#example> "Mashing step: 66°C for 60 minutes, converting starches to fermentable sugars. Boiling step: 100°C for 60 minutes, sterilizing the wort and extracting hop bitterness."@en ;
                                                <http://www.w3.org/2004/02/skos/core#note> "The order and precise execution of brewing steps is critical to achieving consistent, high-quality beer. Each step affects the final product's flavor, aroma, appearance, and stability."@en .


###  http://www.beerecipe.com/ontology#ConditioningStep
<http://www.beerecipe.com/ontology#ConditioningStep> rdf:type owl:Class ;
                                                     rdfs:subClassOf <http://www.beerecipe.com/ontology#BrewingStep> ;
                                                     rdfs:comment "Maturation phase where beer flavors develop, clarifies, and stabilizes."@en ;
                                                     rdfs:label "Conditioning Step" .


###  http://www.beerecipe.com/ontology#CoolingStep
<http://www.beerecipe.com/ontology#CoolingStep> rdf:type owl:Class ;
                                                rdfs:subClassOf <http://www.beerecipe.com/ontology#BrewingStep> ;
                                                rdfs:comment "Step to cool wort to yeast pitching temperature."@en ;
                                                rdfs:label "Cooling Step" .


###  http://www.beerecipe.com/ontology#Country
<http://www.beerecipe.com/ontology#Country> rdf:type owl:Class ;
                                            rdfs:comment "A country represents a geographical and political entity that is the origin of brewing ingredients, beer styles, or brewing traditions. Different countries have distinct brewing histories, indigenous ingredients, and characteristic beer styles."@en ;
                                            rdfs:label "Country"@en ;
                                            <http://www.w3.org/2004/02/skos/core#definition> "A nation state or geographical region that serves as the origin or source for brewing ingredients (hops, malts, yeast strains) or beer styles, often influencing the characteristics and traditions of beer production."@en ;
                                            <http://www.w3.org/2004/02/skos/core#example> "Germany: Origin of noble hops like Hallertau and Tettnanger, and beer styles like Pilsner and Weissbier. United States: Origin of high alpha acid hops like Cascade and Centennial, and styles like American IPA."@en ;
                                            <http://www.w3.org/2004/02/skos/core#note> "Terroir and climate significantly affect the characteristics of brewing ingredients, particularly hops and barley varieties, making the country of origin an important attribute for ingredient selection."@en .


###  http://www.beerecipe.com/ontology#DietaryRequirement
<http://www.beerecipe.com/ontology#DietaryRequirement> rdf:type owl:Class ;
                                                       rdfs:comment "Dietary requirements represent specific nutritional, health, or ethical restrictions that individuals may have regarding food and beverage consumption. In brewing, this includes considerations for allergens, animal products, and specific ingredients that certain populations avoid."@en ;
                                                       rdfs:label "Dietary Requirement"@en ;
                                                       <http://www.w3.org/2004/02/skos/core#definition> "A classification of dietary restrictions or preferences that a beer recipe may satisfy, including but not limited to vegan, gluten-free, organic, low-calorie, or allergen-free requirements."@en ;
                                                       <http://www.w3.org/2004/02/skos/core#example> "Gluten-free: Beer made with gluten-free grains like sorghum, rice, or certified gluten-free oats. Vegan: Beer produced without using animal-derived fining agents like isinglass or gelatin."@en ;
                                                       <http://www.w3.org/2004/02/skos/core#note> "Traditional beer brewing often uses animal-derived products for clarification (isinglass, gelatin) and may contain allergens (gluten from barley/wheat). Modern brewing techniques allow for production of beers meeting various dietary requirements."@en .


###  http://www.beerecipe.com/ontology#DifficultyLevel
<http://www.beerecipe.com/ontology#DifficultyLevel> rdf:type owl:Class ;
                                                    rdfs:comment "The difficulty level of a beer recipe indicates the complexity of the brewing process, the precision required, the equipment needed, and the brewing experience necessary to successfully execute the recipe. It helps brewers select appropriate recipes for their skill level."@en ;
                                                    rdfs:label "Difficulty Level"@en ;
                                                    <http://www.w3.org/2004/02/skos/core#definition> "A classification of brewing complexity typically ranging from beginner to expert, based on factors such as number of ingredients, precision of temperature control required, complexity of brewing steps, fermentation management, and specialized equipment needs."@en ;
                                                    <http://www.w3.org/2004/02/skos/core#example> "Beginner: Simple pale ale with single malt, single hop, basic fermentation. Intermediate: Multi-grain beer with hop schedule and temperature-controlled fermentation. Advanced: Barrel-aged sour beer with multiple microorganism fermentation and extended aging. Expert: Spontaneously fermented lambic with coolship and multi-year aging in wood."@en ;
                                                    <http://www.w3.org/2004/02/skos/core#note> "Difficulty assessment considers technical complexity, time commitment, equipment requirements, ingredient sourcing, and margin for error. Some styles like lagers may be technically simple but require extended time and precise temperature control."@en .


###  http://www.beerecipe.com/ontology#Equipment
<http://www.beerecipe.com/ontology#Equipment> rdf:type owl:Class ;
                                              rdfs:comment "Brewing equipment encompasses all tools, vessels, and instruments required to execute a beer recipe. Equipment ranges from basic household items for beginner brewing to specialized professional-grade machinery for advanced techniques and commercial production."@en ;
                                              rdfs:label "Equipment"@en ;
                                              <http://www.w3.org/2004/02/skos/core#definition> "Physical tools, vessels, instruments, and machinery used in the beer brewing process, including items for mashing, boiling, fermentation, temperature control, filtration, carbonation, and packaging."@en ;
                                              <http://www.w3.org/2004/02/skos/core#example> "Basic equipment: Brew kettle, fermentation bucket, airlock, thermometer, hydrometer, bottles. Advanced equipment: Temperature-controlled fermentation chamber, counterflow chiller, conical fermenter, kegging system, pH meter. Professional equipment: Automated mash tun, brewhouse control system, bright beer tanks, centrifuge."@en ;
                                              <http://www.w3.org/2004/02/skos/core#note> "Equipment quality and capability directly impact beer quality, consistency, and the range of styles that can be produced. Some beer styles require specific equipment (e.g., lagers need temperature control, certain ales benefit from conical fermenters for dry hopping)."@en .


###  http://www.beerecipe.com/ontology#FermentationStep
<http://www.beerecipe.com/ontology#FermentationStep> rdf:type owl:Class ;
                                                     rdfs:subClassOf <http://www.beerecipe.com/ontology#BrewingStep> ;
                                                     rdfs:comment "Yeast converts sugars into alcohol and CO2; primary fermentation phase."@en ;
                                                     rdfs:label "Fermentation Step" .


###  http://www.beerecipe.com/ontology#FlavorProfile
<http://www.beerecipe.com/ontology#FlavorProfile> rdf:type owl:Class ;
                                                  rdfs:comment "A flavor profile describes the characteristic tastes, aromas, and sensory attributes of an ingredient or finished beer. For ingredients, it indicates the contribution they make to the final beer. Flavor profiles help brewers select appropriate ingredients to achieve desired beer characteristics."@en ;
                                                  rdfs:label "Flavor Profile"@en ;
                                                  <http://www.w3.org/2004/02/skos/core#definition> "A structured description of sensory characteristics including taste (bitter, sweet, sour, salty, umami), aroma compounds (fruity, floral, piney, spicy, earthy), mouthfeel, and overall flavor impression contributed by an ingredient or present in a finished beer."@en ;
                                                  <http://www.w3.org/2004/02/skos/core#example> "Cascade hops: Citrus (grapefruit, orange), floral, slightly spicy aroma with moderate bitterness. Munich malt: Bread crust, toasty, slightly sweet malt flavor with amber color contribution. Saison yeast: Fruity esters (banana, pear), peppery phenols, dry finish."@en ;
                                                  <http://www.w3.org/2004/02/skos/core#note> "Flavor profiles are subjective and can vary based on usage levels, combination with other ingredients, and brewing techniques. Professional flavor profiling uses standardized vocabulary from systems like the Beer Flavor Wheel or Sensory Lexicon."@en .


###  http://www.beerecipe.com/ontology#Ingredient
<http://www.beerecipe.com/ontology#Ingredient> rdf:type owl:Class ;
                                               rdfs:comment "An ingredient is any substance added during the brewing process that contributes to the final beer's characteristics. The four essential ingredients are water, malt (or other fermentable grains), hops, and yeast, though many additional ingredients can be used for flavor, color, or functional purposes."@en ;
                                               rdfs:label "Ingredient"@en ;
                                               <http://www.w3.org/2004/02/skos/core#definition> "A component substance used in beer production that contributes to flavor, aroma, color, body, fermentable sugars, bitterness, preservation, or other characteristics of the finished beer. Ingredients include malted and unmalted grains, hops, yeast, water, and adjuncts."@en ;
                                               <http://www.w3.org/2004/02/skos/core#example> "Primary ingredients: Pale malt (base fermentables and flavor), Cascade hops (bitterness and aroma), ale yeast (fermentation and esters), water (solvent and mineral content). Adjuncts: Lactose (body and sweetness), coriander (spice flavor), orange peel (citrus aroma), oak chips (wood character)."@en ;
                                               <http://www.w3.org/2004/02/skos/core#note> "The German Reinheitsgebot (Beer Purity Law of 1516) traditionally limited beer ingredients to water, barley, and hops (yeast was not yet understood). Modern brewing uses a vast array of ingredients, though some traditional styles still adhere to these restrictions."@en .


###  http://www.beerecipe.com/ontology#MashOutStep
<http://www.beerecipe.com/ontology#MashOutStep> rdf:type owl:Class ;
                                                rdfs:subClassOf <http://www.beerecipe.com/ontology#MashStep> ;
                                                rdfs:comment "Step to stop enzymatic activity and raise mash temperature before lautering."@en ;
                                                rdfs:label "MashOut Step" .


###  http://www.beerecipe.com/ontology#MashStep
<http://www.beerecipe.com/ontology#MashStep> rdf:type owl:Class ;
                                             rdfs:subClassOf <http://www.beerecipe.com/ontology#BrewingStep> ,
                                                             [ rdf:type owl:Restriction ;
                                                               owl:onProperty <http://www.beerecipe.com/ontology#stepTemperature> ;
                                                               owl:someValuesFrom xsd:float
                                                             ] ;
                                             rdfs:comment "Step where starches in the malt are converted into fermentable sugars."@en ;
                                             rdfs:label "Mash Step" .


###  http://www.beerecipe.com/ontology#Recipe
<http://www.beerecipe.com/ontology#Recipe> rdf:type owl:Class ;
                                           rdfs:subClassOf [ owl:intersectionOf ( <http://www.beerecipe.com/ontology#Recipe>
                                                                                  [ rdf:type owl:Restriction ;
                                                                                    owl:onProperty <http://www.beerecipe.com/ontology#hasCereal> ;
                                                                                    owl:minQualifiedCardinality "1"^^xsd:nonNegativeInteger ;
                                                                                    owl:onClass :Cereal
                                                                                  ]
                                                                                  [ rdf:type owl:Restriction ;
                                                                                    owl:onProperty <http://www.beerecipe.com/ontology#hasHop> ;
                                                                                    owl:minQualifiedCardinality "1"^^xsd:nonNegativeInteger ;
                                                                                    owl:onClass <https://rdf.ag/o/hops#Hops>
                                                                                  ]
                                                                                  [ rdf:type owl:Restriction ;
                                                                                    owl:onProperty <http://www.beerecipe.com/ontology#hasMalt> ;
                                                                                    owl:minQualifiedCardinality "1"^^xsd:nonNegativeInteger ;
                                                                                    owl:onClass <https://rdf.ag/o/malt#Malt>
                                                                                  ]
                                                                                  [ rdf:type owl:Restriction ;
                                                                                    owl:onProperty :hasWater ;
                                                                                    owl:minQualifiedCardinality "1"^^xsd:nonNegativeInteger ;
                                                                                    owl:onClass :Water
                                                                                  ]
                                                                                  [ rdf:type owl:Restriction ;
                                                                                    owl:onProperty <http://www.beerecipe.com/ontology#hasYeast> ;
                                                                                    owl:qualifiedCardinality "1"^^xsd:nonNegativeInteger ;
                                                                                    owl:onClass <http://www.beerecipe.com/ontology#Yeast>
                                                                                  ]
                                                                                ) ;
                                                             rdf:type owl:Class
                                                           ] ,
                                                           [ rdf:type owl:Restriction ;
                                                             owl:onProperty <http://www.beerecipe.com/ontology#hasStyle> ;
                                                             owl:qualifiedCardinality "1"^^xsd:nonNegativeInteger ;
                                                             owl:onClass <http://www.beerecipe.com/ontology#BeerStyle>
                                                           ] ;
                                           rdfs:comment "A beer recipe describes the complete process and ingredients needed to produce a specific type of beer. It includes information about malts, hops, yeast, water chemistry, brewing steps, and expected characteristics of the final product."@en ;
                                           rdfs:label "Recipe"@en ;
                                           <http://www.w3.org/2004/02/skos/core#definition> "A structured set of instructions and ingredients for brewing beer, including quantities, temperatures, timings, and expected beer characteristics such as ABV, IBU, and color."@en ;
                                           <http://www.w3.org/2004/02/skos/core#example> "Easy Pale Ale: A beginner-friendly recipe using pale ale malt, Cascade hops, producing a 4.8% ABV beer with 30 IBU."@en .


###  http://www.beerecipe.com/ontology#SpargeStep
<http://www.beerecipe.com/ontology#SpargeStep> rdf:type owl:Class ;
                                               rdfs:subClassOf <http://www.beerecipe.com/ontology#BrewingStep> ;
                                               rdfs:comment "Rinse the grains to extract remaining sugars and increase wort yield."@en ;
                                               rdfs:label "Sparge Step" .


###  http://www.beerecipe.com/ontology#WhirlpoolStep
<http://www.beerecipe.com/ontology#WhirlpoolStep> rdf:type owl:Class ;
                                                  rdfs:subClassOf <http://www.beerecipe.com/ontology#BrewingStep> ;
                                                  rdfs:comment "Clarifies wort by separating hops and trub after boiling."@en ;
                                                  rdfs:label "Whirlpool Step" .


###  http://www.beerecipe.com/ontology#Yeast
<http://www.beerecipe.com/ontology#Yeast> rdf:type owl:Class ;
                                          rdfs:subClassOf <http://www.beerecipe.com/ontology#Ingredient> ;
                                          owl:disjointWith <https://rdf.ag/o/malt#Malt> ;
                                          rdfs:comment "Yeast is a single-celled microorganism (fungus) essential for beer fermentation. Yeast converts fermentable sugars into alcohol and carbon dioxide, while producing flavor compounds (esters, phenols) that significantly influence the beer's character. Different yeast strains produce distinct flavor profiles and are categorized primarily into ale yeasts (Saccharomyces cerevisiae) and lager yeasts (Saccharomyces pastorianus)."@en ;
                                          rdfs:label "Yeast"@en ;
                                          <http://www.w3.org/2004/02/skos/core#definition> "A living microorganism ingredient used to ferment wort into beer, converting sugars to alcohol and CO2, while contributing characteristic flavors, aromas, and determining fermentation characteristics such as temperature range, attenuation, and flocculation."@en ;
                                          <http://www.w3.org/2004/02/skos/core#example> "Ale yeast (S. cerevisiae): Ferments at 15-24°C, produces fruity esters, top-fermenting. Lager yeast (S. pastorianus): Ferments at 7-13°C, produces clean flavor profile, bottom-fermenting. Belgian yeast: Produces spicy phenols and fruity esters. Kveik: Norwegian farmhouse yeast, ferments at high temperatures (25-40°C)."@en ;
                                          <http://www.w3.org/2004/02/skos/core#note> "Yeast is often called the most important ingredient in brewing as it not only produces alcohol but dramatically influences the beer's flavor profile. Wild yeasts and bacteria (Brettanomyces, Lactobacillus, Pediococcus) are used in sour and wild beer production."@en .


###  http://www.semanticweb.org/matte/ontologies/2025/10/untitled-ontology-4#AdvancedRecipe
:AdvancedRecipe rdf:type owl:Class ;
                owl:equivalentClass [ owl:intersectionOf ( <http://www.beerecipe.com/ontology#Recipe>
                                                           [ rdf:type owl:Restriction ;
                                                             owl:onProperty <http://www.beerecipe.com/ontology#difficultyLevel> ;
                                                             owl:hasValue "advanced"
                                                           ]
                                                         ) ;
                                      rdf:type owl:Class
                                    ] ;
                rdfs:subClassOf <http://www.beerecipe.com/ontology#Recipe> .


###  http://www.semanticweb.org/matte/ontologies/2025/10/untitled-ontology-4#BeginnerRecipe
:BeginnerRecipe rdf:type owl:Class ;
                owl:equivalentClass [ owl:intersectionOf ( <http://www.beerecipe.com/ontology#Recipe>
                                                           [ rdf:type owl:Restriction ;
                                                             owl:onProperty <http://www.beerecipe.com/ontology#difficultyLevel> ;
                                                             owl:hasValue "beginner"
                                                           ]
                                                         ) ;
                                      rdf:type owl:Class
                                    ] ;
                rdfs:subClassOf <http://www.beerecipe.com/ontology#Recipe> .


###  http://www.semanticweb.org/matte/ontologies/2025/10/untitled-ontology-4#Cereal
:Cereal rdf:type owl:Class ;
        rdfs:subClassOf <http://www.beerecipe.com/ontology#Ingredient> ;
        owl:disjointWith <https://rdf.ag/o/malt#Malt> .


###  http://www.semanticweb.org/matte/ontologies/2025/10/untitled-ontology-4#ExpertRecipe
:ExpertRecipe rdf:type owl:Class ;
              owl:equivalentClass [ owl:intersectionOf ( <http://www.beerecipe.com/ontology#Recipe>
                                                         [ rdf:type owl:Restriction ;
                                                           owl:onProperty <http://www.beerecipe.com/ontology#difficultyLevel> ;
                                                           owl:hasValue "expert"
                                                         ]
                                                       ) ;
                                    rdf:type owl:Class
                                  ] ;
              rdfs:subClassOf <http://www.beerecipe.com/ontology#Recipe> .


###  http://www.semanticweb.org/matte/ontologies/2025/10/untitled-ontology-4#FoodIngredient
:FoodIngredient rdf:type owl:Class ;
                rdfs:subClassOf <http://www.beerecipe.com/ontology#Ingredient> .


###  http://www.semanticweb.org/matte/ontologies/2025/10/untitled-ontology-4#GlutenFreeRecipe
:GlutenFreeRecipe rdf:type owl:Class ;
                  owl:equivalentClass [ owl:intersectionOf ( <http://www.beerecipe.com/ontology#Recipe>
                                                             [ rdf:type owl:Restriction ;
                                                               owl:onProperty <http://www.beerecipe.com/ontology#hasCereal> ;
                                                               owl:someValuesFrom [ rdf:type owl:Restriction ;
                                                                                    owl:onProperty <http://www.beerecipe.com/ontology#glutenContent> ;
                                                                                    owl:hasValue "false"^^xsd:boolean
                                                                                  ]
                                                             ]
                                                           ) ;
                                        rdf:type owl:Class
                                      ] ;
                  rdfs:subClassOf <http://www.beerecipe.com/ontology#Recipe> .


###  http://www.semanticweb.org/matte/ontologies/2025/10/untitled-ontology-4#IPARecipe
:IPARecipe rdf:type owl:Class ;
           rdfs:subClassOf <http://www.beerecipe.com/ontology#Recipe> ,
                           [ owl:intersectionOf ( <http://www.beerecipe.com/ontology#Recipe>
                                                  [ rdf:type owl:Restriction ;
                                                    owl:onProperty <http://www.beerecipe.com/ontology#hasHop> ;
                                                    owl:minQualifiedCardinality "2"^^xsd:nonNegativeInteger ;
                                                    owl:onClass <https://rdf.ag/o/hops#Hops>
                                                  ]
                                                ) ;
                             rdf:type owl:Class
                           ] .


###  http://www.semanticweb.org/matte/ontologies/2025/10/untitled-ontology-4#ImperialBeer
:ImperialBeer rdf:type owl:Class ;
              owl:equivalentClass [ owl:intersectionOf ( <http://www.beerecipe.com/ontology#Recipe>
                                                         [ rdf:type owl:Restriction ;
                                                           owl:onProperty <http://www.beerecipe.com/ontology#estimatedABV> ;
                                                           owl:someValuesFrom [ rdf:type rdfs:Datatype ;
                                                                                owl:onDatatype xsd:float ;
                                                                                owl:withRestrictions ( [ xsd:minExclusive "10.0"^^xsd:float
                                                                                                       ]
                                                                                                     )
                                                                              ]
                                                         ]
                                                       ) ;
                                    rdf:type owl:Class
                                  ] ;
              rdfs:subClassOf <http://www.beerecipe.com/ontology#Recipe> .


###  http://www.semanticweb.org/matte/ontologies/2025/10/untitled-ontology-4#IntermediateRecipe
:IntermediateRecipe rdf:type owl:Class ;
                    owl:equivalentClass [ owl:intersectionOf ( <http://www.beerecipe.com/ontology#Recipe>
                                                               [ rdf:type owl:Restriction ;
                                                                 owl:onProperty <http://www.beerecipe.com/ontology#difficultyLevel> ;
                                                                 owl:hasValue "intermediate"
                                                               ]
                                                             ) ;
                                          rdf:type owl:Class
                                        ] ;
                    rdfs:subClassOf <http://www.beerecipe.com/ontology#Recipe> .


###  http://www.semanticweb.org/matte/ontologies/2025/10/untitled-ontology-4#LowAlcoholBeer
:LowAlcoholBeer rdf:type owl:Class ;
                owl:equivalentClass [ owl:intersectionOf ( <http://www.beerecipe.com/ontology#Recipe>
                                                           [ rdf:type owl:Restriction ;
                                                             owl:onProperty <http://www.beerecipe.com/ontology#estimatedABV> ;
                                                             owl:someValuesFrom [ rdf:type rdfs:Datatype ;
                                                                                  owl:onDatatype xsd:float ;
                                                                                  owl:withRestrictions ( [ xsd:maxExclusive "4.0"^^xsd:float
                                                                                                         ]
                                                                                                       )
                                                                                ]
                                                           ]
                                                         ) ;
                                      rdf:type owl:Class
                                    ] ;
                rdfs:subClassOf <http://www.beerecipe.com/ontology#Recipe> .


###  http://www.semanticweb.org/matte/ontologies/2025/10/untitled-ontology-4#RiceWheat
:RiceWheat rdf:type owl:Class ;
           rdfs:subClassOf :Cereal .


###  http://www.semanticweb.org/matte/ontologies/2025/10/untitled-ontology-4#SessionBeer
:SessionBeer rdf:type owl:Class ;
             owl:equivalentClass [ owl:intersectionOf ( <http://www.beerecipe.com/ontology#Recipe>
                                                        [ rdf:type owl:Restriction ;
                                                          owl:onProperty <http://www.beerecipe.com/ontology#estimatedABV> ;
                                                          owl:someValuesFrom [ rdf:type rdfs:Datatype ;
                                                                               owl:onDatatype xsd:float ;
                                                                               owl:withRestrictions ( [ xsd:minInclusive "4.0"^^xsd:float
                                                                                                      ]
                                                                                                      [ xsd:maxInclusive "5.0"^^xsd:float
                                                                                                      ]
                                                                                                    )
                                                                             ]
                                                        ]
                                                      ) ;
                                   rdf:type owl:Class
                                 ] ;
             rdfs:subClassOf <http://www.beerecipe.com/ontology#Recipe> .


###  http://www.semanticweb.org/matte/ontologies/2025/10/untitled-ontology-4#StandardBeer
:StandardBeer rdf:type owl:Class ;
              owl:equivalentClass [ owl:intersectionOf ( <http://www.beerecipe.com/ontology#Recipe>
                                                         [ rdf:type owl:Restriction ;
                                                           owl:onProperty <http://www.beerecipe.com/ontology#estimatedABV> ;
                                                           owl:someValuesFrom [ rdf:type rdfs:Datatype ;
                                                                                owl:onDatatype xsd:float ;
                                                                                owl:withRestrictions ( [ xsd:minInclusive "5.0"^^xsd:float
                                                                                                       ]
                                                                                                       [ xsd:maxInclusive "7.0"^^xsd:float
                                                                                                       ]
                                                                                                     )
                                                                              ]
                                                         ]
                                                       ) ;
                                    rdf:type owl:Class
                                  ] ;
              rdfs:subClassOf <http://www.beerecipe.com/ontology#Recipe> .


###  http://www.semanticweb.org/matte/ontologies/2025/10/untitled-ontology-4#StrongBeer
:StrongBeer rdf:type owl:Class ;
            owl:equivalentClass [ owl:intersectionOf ( <http://www.beerecipe.com/ontology#Recipe>
                                                       [ rdf:type owl:Restriction ;
                                                         owl:onProperty <http://www.beerecipe.com/ontology#estimatedABV> ;
                                                         owl:someValuesFrom [ rdf:type rdfs:Datatype ;
                                                                              owl:onDatatype xsd:float ;
                                                                              owl:withRestrictions ( [ xsd:minInclusive "7.0"^^xsd:float
                                                                                                     ]
                                                                                                     [ xsd:maxInclusive "10.0"^^xsd:float
                                                                                                     ]
                                                                                                   )
                                                                            ]
                                                       ]
                                                     ) ;
                                  rdf:type owl:Class
                                ] ;
            rdfs:subClassOf <http://www.beerecipe.com/ontology#Recipe> .


###  http://www.semanticweb.org/matte/ontologies/2025/10/untitled-ontology-4#Water
:Water rdf:type owl:Class ;
       rdfs:subClassOf <http://www.beerecipe.com/ontology#Ingredient> .


###  https://rdf.ag/o/MaltingActivity
<https://rdf.ag/o/MaltingActivity> rdf:type owl:Class .


###  https://rdf.ag/o/beer#Ale
<https://rdf.ag/o/beer#Ale> rdf:type owl:Class ;
                            rdfs:subClassOf <https://rdf.ag/o/beer#Beer> ;
                            <http://rdfs.org/ns/void#inDataset> <https://rdf.ag/o/beer#datasetdefinition> ;
                            rdfs:isDefinedBy <https://rdf.ag/o/beer-2024-02-21> ;
                            rdfs:label "Ale"@en ;
                            <http://www.w3.org/2004/02/skos/core#definition> """La principale caractéristique distinctive d'un Ale est le type de levure utilisé dans le processus de brassage, Saccharomyces cerevisiae. S. cerevisiae préfère généralement une gamme de brassage plus chaude et n'a pas la capacité de métaboliser les sucres complexes: mélibiose et raffinose.
         
         Les Ales sont généralement fermentées, en fonction bien sûr de la souche de levure, à 16-24°C (60-75°F). Ce qui est généralement, mais pas exclusivement, plus chaud que la fermentation de lager.
         
         Les Ales ne subissent pas non plus de phase de conditionnement à froid. Cependant, il n'est pas rare que certaines lagers ne subissent pas de phase froide."""@fr ,
                                                                             """The main distinguishing feature of an ale is the type of yeast used in the brewing process, Saccharomyces cerevisiae. S. cerevisiae typically prefers a warmer brewing range and lacks the ability to metabolize the complex sugars: melibiose and raffinose.
         
         Ales are typically fermented, depending of course on the strain yeast, at 16-24˚C (60-75˚F) temperature range. Which is typically, but not exclusively, warmer than lager fermentation.
         
         Ales also do not undergo a cold-conditioning phase. However it is not uncommon for some lagers to not undergo a cold phase."""@en ;
                            <http://xmlns.com/foaf/0.1/name> "Ale" .


###  https://rdf.ag/o/beer#Altbier
<https://rdf.ag/o/beer#Altbier> rdf:type owl:Class ;
                                rdfs:subClassOf <https://rdf.ag/o/beer#AmberBitterEuropeanBeer> ,
                                                <https://rdf.ag/o/beer#GermanBeer> ;
                                <http://rdfs.org/ns/void#inDataset> <https://rdf.ag/o/beer#datasetdefinition> ;
                                rdfs:isDefinedBy <http://rdf.ag/o/beer-2024-02-21> ;
                                rdfs:label "Altbier"@en ,
                                           "Altbier"@fr ;
                                <http://www.w3.org/2004/02/skos/core#definition> "Ces bières sont traditionnellement brassées près de Düsseldorf, en Allemagne. L'Altbier est une bière de style ancien qui est typiquement de couleur ambrée, maltée et quelque peu amère."@fr ,
                                                                                 "These beers are traditionally brewed near Düsseldorf, Germany. Altbier is an old style of beer that is typically amber colored, malty and somewhat bitter."@en ;
                                <http://xmlns.com/foaf/0.1/name> "Altbier" .


###  https://rdf.ag/o/beer#AlternativeFermentablesBeer
<https://rdf.ag/o/beer#AlternativeFermentablesBeer> rdf:type owl:Class ;
                                                    rdfs:subClassOf <https://rdf.ag/o/beer#Beer> ;
                                                    <http://rdfs.org/ns/void#inDataset> <https://rdf.ag/o/beer#datasetdefinition> ;
                                                    rdfs:isDefinedBy <http://rdf.ag/o/beer-2024-02-21> ;
                                                    rdfs:label "Alternative Fermentables Beer"@en ,
                                                               "Bière Fermentable Alternative"@fr ;
                                                    <http://www.w3.org/2004/02/skos/core#definition> "Ce sont des bières spéciales qui utilisent des ingrédients supplémentaires pour ajouter des arômes distincts tels que des céréales ou du sucre."@fr ,
                                                                                                     "These are specialty beers that use additional ingredients to add distinct flavoring such as grain or sugar."@en ;
                                                    <http://xmlns.com/foaf/0.1/name> "Alternative Fermentables Beer" .


###  https://rdf.ag/o/beer#AmberBitterEuropeanBeer
<https://rdf.ag/o/beer#AmberBitterEuropeanBeer> rdf:type owl:Class ;
                                                rdfs:subClassOf <https://rdf.ag/o/beer#Beer> ,
                                                                <https://rdf.ag/o/beer#EuropeanBeer> ;
                                                <http://rdfs.org/ns/void#inDataset> <https://rdf.ag/o/beer#datasetdefinition> ;
                                                rdfs:isDefinedBy <http://rdf.ag/o/beer-2024-02-21> ;
                                                rdfs:label "Amber Bitter European Beer"@en ,
                                                           "Bière Européenne Ambrée Amère"@fr ;
                                                <http://www.w3.org/2004/02/skos/core#definition> "Ces bières sont d'origine allemande ou autrichienne, sont de couleur ambrée et vont de même à amères équilibrées."@fr ,
                                                                                                 "These beers are German or Austrian in origin, are amber colored, and range from even to bitter balanced."@en ;
                                                <http://xmlns.com/foaf/0.1/name> "Amber Bitter European Beer" .


###  https://rdf.ag/o/beer#AmberMaltyEuropeanLager
<https://rdf.ag/o/beer#AmberMaltyEuropeanLager> rdf:type owl:Class ;
                                                rdfs:subClassOf <https://rdf.ag/o/beer#Beer> ;
                                                <http://rdfs.org/ns/void#inDataset> <https://rdf.ag/o/beer#datasetdefinition> ;
                                                rdfs:isDefinedBy <http://rdf.ag/o/beer-2024-02-21> ;
                                                rdfs:label "Amber Malty European Lager"@en ,
                                                           "Lager Européenne Maltée Ambrée"@fr ;
                                                <http://www.w3.org/2004/02/skos/core#definition> "Ces types de bières sont des lagers, ou bières de fermentation basse, d'origine allemande qui se distinguent par leur couleur ambrée et par leur caractère malté, puissant et corsé (vollbier à starkbier)."@fr ,
                                                                                                 "These types of beers are lagers, or bottom-fermenting beers, that are German in origin and are distinguished by their amber color and for being malty, strong and fullbodied (vollbier to starkbier)."@en ;
                                                <http://xmlns.com/foaf/0.1/name> "Amber Malty European Lager" .


###  https://rdf.ag/o/beer#AmericanPorterandStout
<https://rdf.ag/o/beer#AmericanPorterandStout> rdf:type owl:Class ;
                                               rdfs:subClassOf <https://rdf.ag/o/beer#Stout> .


###  https://rdf.ag/o/beer#AmericanWildAle
<https://rdf.ag/o/beer#AmericanWildAle> rdf:type owl:Class ;
                                        rdfs:subClassOf <https://rdf.ag/o/beer#Ale> ,
                                                        <https://rdf.ag/o/beer#PaleAle> ;
                                        <http://rdfs.org/ns/void#inDataset> <https://rdf.ag/o/beer#datasetdefinition> ;
                                        rdfs:isDefinedBy <http://rdf.ag/o/beer-2024-02-21> ;
                                        rdfs:label "Ale Sauvage Américain"@fr ,
                                                   "American Wild Ale"@en ;
                                        <http://www.w3.org/2004/02/skos/core#definition> "Le terme 'sauvage' dans le nom de cette catégorie est lié au fait que les saveurs de ces bières sont davantage influencées par des processus microbiens que par les levures de bière traditionnelles. Ce sont des bières de spécialité qui couvrent une grande variété de styles qui ne correspondent pas aux styles traditionnels mais qui ont des ingrédients et des profils de fermentation similaires."@fr ,
                                                                                         "The term 'Wild' in the name of this category has to do with the fact that the flavors of these beers are influenced more by microbial processes rather than by the traditional brewer's yeasts. These are specialty beers that cover a wide variety of styles that don't fit traditional styles but have similar fermentation ingredients and profiles."@en ;
                                        <http://xmlns.com/foaf/0.1/name> "American Wild Ale" .


###  https://rdf.ag/o/beer#BDG
<https://rdf.ag/o/beer#BDG> rdf:type owl:Class ;
                            rdfs:subClassOf <https://rdf.ag/o/beer#FarmhouseAle> ;
                            <http://rdfs.org/ns/void#inDataset> <https://rdf.ag/o/beer#datasetdefinition> ;
                            rdfs:isDefinedBy <https://rdf.ag/o/beer-2024-02-21> ;
                            rdfs:label "Bière de Garde"@en ,
                                       "Bière de Garde"@fr ;
                            <http://www.w3.org/2004/02/skos/core#definition> "Semblables aux bières de saison, les bières de garde sont des bières de saison qui sont généralement appréciées pendant l'été jusqu'à la fin des vendanges. Elles étaient traditionnellement brassées dans la région Nord-Pas-de-Calais en France. Les saisons sont généralement sèches et/ou épicées, cependant, contrairement à sa cousine, la bière de garde est généralement plus douce et maltée."@fr ,
                                                                             "Similar to saison beers, bière de garde beers are seasonal beers that are typically enjoyed during the summer until the end of harvest. They were traditionally brewed in the Nord-Pas-de-Calais region of France. Saisons are typically dry and or spicy, however, unlike its cousin, bière de gardes are typically sweeter and maltier."@en ;
                            <http://xmlns.com/foaf/0.1/name> "Bière de Garde" .


###  https://rdf.ag/o/beer#Beer
<https://rdf.ag/o/beer#Beer> rdf:type owl:Class ;
                             rdfs:subClassOf <https://rdf.ag/o/beer#MaltBeverage> ,
                                             <https://schema.org/ProductGroup> ;
                             owl:disjointWith <https://rdf.ag/o/beer#Cider> ,
                                              <https://rdf.ag/o/beer#Mead> ;
                             <http://rdfs.org/ns/void#inDataset> <https://rdf.ag/o/beer#datasetdefinition> ;
                             rdfs:isDefinedBy <https://rdf.ag/o/beer-2024-02-21> ;
                             rdfs:label "Beer"@en ,
                                        "Bière"@fr ;
                             <http://www.w3.org/2004/02/skos/core#definition> "Beer a drink that is created as a result of the fermentation of yeast malt and is flavored with hops. The fermentation process results in alcohol, however there are some beers that are specifically brewed to be non-alcoholic."@en ,
                                                                              "La bière est une boisson créée à la suite de la fermentation du malt de levure et aromatisée au houblon. Le processus de fermentation donne de l'alcool, mais certaines bières sont spécifiquement brassées pour être non alcoolisées."@fr .


###  https://rdf.ag/o/beer#BelgianAle
<https://rdf.ag/o/beer#BelgianAle> rdf:type owl:Class ;
                                   rdfs:subClassOf <https://rdf.ag/o/beer#Ale> ,
                                                   <https://rdf.ag/o/beer#BelgianBeer> ;
                                   <http://rdfs.org/ns/void#inDataset> <https://rdf.ag/o/beer#datasetdefinition> ;
                                   rdfs:isDefinedBy <http://rdf.ag/o/beer-2024-02-21> ;
                                   rdfs:label "Belgian Ale"@en ,
                                              "Bière Belge"@fr ,
                                              "French Ale"@en ;
                                   <http://www.w3.org/2004/02/skos/core#definition> "Belgian Ales are flavorful Belgian and French Ales that range from being balanced to malty."@en ,
                                                                                    "Les bières belges sont des bières belges et françaises savoureuses qui vont de l'équilibre au malté."@fr ;
                                   <http://xmlns.com/foaf/0.1/name> "Belgian Ale" .


###  https://rdf.ag/o/beer#BelgianBeer
<https://rdf.ag/o/beer#BelgianBeer> rdf:type owl:Class ;
                                    rdfs:subClassOf <https://rdf.ag/o/beer#EuropeanBeer> ;
                                    <http://rdfs.org/ns/void#inDataset> <https://rdf.ag/o/beer#datasetdefinition> ;
                                    rdfs:isDefinedBy <https://rdf.ag/o/beer-2024-02-21> ;
                                    rdfs:label "Belgian Beer"@en ,
                                               "Bière Belge"@fr ,
                                               "French Beer"@en ;
                                    <http://www.w3.org/2004/02/skos/core#definition> "Belgian beers are a grouping of beer styles produced in Belgium or in the Belgian style. These styles are mostly ales that use fruity yeasts and malts. French beers are also included in this categorization."@en ,
                                                                                     "Les bières belges sont un regroupement de styles de bières produits en Belgique ou dans le style belge. Ces styles sont principalement des ales qui utilisent des levures et des malts fruités. Les bières françaises sont également incluses dans cette catégorisation."@fr ;
                                    <http://xmlns.com/foaf/0.1/name> "Belgian Beer" .


###  https://rdf.ag/o/beer#BritishBeer
<https://rdf.ag/o/beer#BritishBeer> rdf:type owl:Class ;
                                    rdfs:subClassOf <https://rdf.ag/o/beer#EuropeanBeer> ;
                                    <http://rdfs.org/ns/void#inDataset> <https://rdf.ag/o/beer#datasetdefinition> ;
                                    rdfs:isDefinedBy <http://rdf.ag/o/beer-2024-02-21> ;
                                    rdfs:label "Bière Anglaise"@fr ,
                                               "British Beer"@en ,
                                               "English Beer"@en ;
                                    <http://www.w3.org/2004/02/skos/core#definition> "Beers whose style originated from Great Britain or countries that are part of the British Commonwealth."@en ,
                                                                                     "Bières dont le style est originaire de Grande-Bretagne ou de pays faisant partie du Commonwealth britannique."@fr ;
                                    <http://xmlns.com/foaf/0.1/name> "British Beer" .


###  https://rdf.ag/o/beer#BritishBitter
<https://rdf.ag/o/beer#BritishBitter> rdf:type owl:Class ;
                                      rdfs:subClassOf <https://rdf.ag/o/beer#Beer> ,
                                                      <https://rdf.ag/o/beer#BritishBeer> ;
                                      <http://rdfs.org/ns/void#inDataset> <https://rdf.ag/o/beer#datasetdefinition> ;
                                      rdfs:isDefinedBy <http://rdf.ag/o/beer-2024-02-21> ;
                                      rdfs:label "Amer Britannique"@fr ,
                                                 "British Bitter"@en ;
                                      <http://www.w3.org/2004/02/skos/core#definition> "Les bières dans le style des amères britanniques ne reflètent pas les formulations d'exportation d'une amère britannique, mais plutôt la version « vraie bière » de ce type de bière. Ce style couvre une large gamme de bières allant des bières brunes et sucrées sans mousse aux pâles, houblonnées et très mousseuses."@fr ,
                                                                                       "The beers in the style of British bitters are not reflective of the export formulations of a British Bitter, rather the 'real ale' version of this type of beer. This style covers a wide range of beers ranging from dark, sweet beers with no head to pale, hoppy and very foamy."@en ;
                                      <http://xmlns.com/foaf/0.1/name> "British Bitter" .


###  https://rdf.ag/o/beer#BrownBritishBeer
<https://rdf.ag/o/beer#BrownBritishBeer> rdf:type owl:Class ;
                                         rdfs:subClassOf <https://rdf.ag/o/beer#Beer> ,
                                                         <https://rdf.ag/o/beer#BritishBeer> ;
                                         <http://rdfs.org/ns/void#inDataset> <https://rdf.ag/o/beer#datasetdefinition> ;
                                         rdfs:isDefinedBy <http://rdf.ag/o/beer-2024-02-21> ;
                                         rdfs:label "Bière Brune Britannique"@fr ,
                                                    "Brown British Beer"@en ;
                                         <http://www.w3.org/2004/02/skos/core#definition> "Bien que ces bières n'aient aucune relation historique entre elles, elles sont regroupées dans le style Brown British Beer en raison de leurs similitudes concernant leur couleur sombre, leur force modérée, leur origine britannique et leur équilibre malté."@fr ,
                                                                                          "While these beers have no historic relationship with each other, they are grouped in the Brown British Beer style due to their similarites regarding their dark color, moderate strength, British origin and malty balance."@en ;
                                         <http://xmlns.com/foaf/0.1/name> "Brown British Beer" .


###  https://rdf.ag/o/beer#Cider
<https://rdf.ag/o/beer#Cider> rdf:type owl:Class .


###  https://rdf.ag/o/beer#CreamAle
<https://rdf.ag/o/beer#CreamAle> rdf:type owl:Class ;
                                 rdfs:subClassOf <https://rdf.ag/o/beer#Ale> ,
                                                 <https://rdf.ag/o/beer#PaleAle> ;
                                 <http://rdfs.org/ns/void#inDataset> <https://rdf.ag/o/beer#datasetdefinition> ;
                                 rdfs:isDefinedBy <https://rdf.ag/o/beer-2024-02-21> ;
                                 rdfs:label "Cream Ale"@en ;
                                 <http://www.w3.org/2004/02/skos/core#definition> """Bien que considérées comme des ales, les bières à la crème ressemblent davantage à des lagers légères en termes de goût. Contrairement à leur nom, les bières à la crème ne contiennent pas nécessairement de crème ou d'autres produits laitiers ou dérivés. Ils contiennent cependant des ingrédients adjuvants qui pourraient contenir du lactose ou du sucre de lait mais qui pourraient être des fruits, du café, de la menthe, de la vanille, d'autres céréales ou même du gaz azoté qui donne une texture plus «crémeuse». Ces bières sont généralement plus alcoolisées et amères que les autres bières légères.
         
         Les bières à la crème utilisent des levures qui sont généralement utilisées pour les bières blondes, mais peuvent parfois inclure des levures pour les bières. Même avec une levure de bière blonde, la bière est fermentée à une température plus élevée, ce qui est typique des ales."""@fr ,
                                                                                  """While considered ales, cream beers more closely resemble light lagers in terms of taste. Contrary to the name, cream beers do not necessarily contain cream or other milk products or derivatives. They do however contain adjuct ingredients which could contain lactose or milk sugar but could be fruit, coffee, mint, vanilla, other grains, or even nitrogenated gas that attributes to a more 'creamy' texture. These beers are typically more alcoholic and bitter compared to other light ales.
         
         Cream ales use yeasts that are typically used for lagers, but could sometimes include yeasts for ales. Even with a lager yeast, the beer is fermented at a higher temperature, which is typical for ales."""@en .


###  https://rdf.ag/o/beer#CzechLager
<https://rdf.ag/o/beer#CzechLager> rdf:type owl:Class ;
                                   rdfs:subClassOf <https://rdf.ag/o/beer#EuropeanBeer> ,
                                                   <https://rdf.ag/o/beer#Lager> ;
                                   <http://rdfs.org/ns/void#inDataset> <https://rdf.ag/o/beer#datasetdefinition> ;
                                   rdfs:isDefinedBy <http://rdf.ag/o/beer-2024-02-21> ;
                                   rdfs:label "Czech Lager"@en ,
                                              "Lager Tchèque"@fr ;
                                   <http://www.w3.org/2004/02/skos/core#definition> "Czech lagers are less attenuated than German lagers which results in a higher finishing gravity. They are also usually fermented at cooler temperatures (7-10˚C) and for longer and use decoction, mostly double decoction, mashes."@en ,
                                                                                    "Les lagers tchèques sont moins atténuées que les lagers allemandes, ce qui se traduit par une densité de finition plus élevée. Ils sont également généralement fermentés à des températures plus fraîches (7-10°C) et plus longtemps et utilisent des purées en décoction, principalement en double décoction."@fr ;
                                   <http://xmlns.com/foaf/0.1/name> "Czech Lager" .


###  https://rdf.ag/o/beer#DarkBritishBeer
<https://rdf.ag/o/beer#DarkBritishBeer> rdf:type owl:Class ;
                                        rdfs:subClassOf <https://rdf.ag/o/beer#BritishBeer> ,
                                                        <https://rdf.ag/o/beer#Stout> ;
                                        <http://rdfs.org/ns/void#inDataset> <https://rdf.ag/o/beer#datasetdefinition> ;
                                        rdfs:isDefinedBy <http://rdf.ag/o/beer-2024-02-21> ;
                                        rdfs:label "Dark British Beer"@en ;
                                        <http://www.w3.org/2004/02/skos/core#definition> "Ces bières sont généralement des stouts forts qui vont du sucré à l'amer. 'Britannique' dans cette catégorie fait référence aux îles britanniques au sens large plutôt qu'à la Grande-Bretagne, c'est pourquoi certaines bières irlandaises sont incluses dans ce style de bière."@fr ,
                                                                                         "These beers are typically strong stouts that range from being sweet to bitter. 'British' in this category refers to the broader British Isles rather than Great Britain, which is why some Irish beers are included in this beer style."@en ;
                                        <http://xmlns.com/foaf/0.1/name> "Dark British Beer" .


###  https://rdf.ag/o/beer#DarkEuropeanLager
<https://rdf.ag/o/beer#DarkEuropeanLager> rdf:type owl:Class ;
                                          rdfs:subClassOf <https://rdf.ag/o/beer#EuropeanBeer> ,
                                                          <https://rdf.ag/o/beer#Lager> ;
                                          <http://rdfs.org/ns/void#inDataset> <https://rdf.ag/o/beer#datasetdefinition> ;
                                          rdfs:isDefinedBy <http://rdf.ag/o/beer-2024-02-21> ;
                                          rdfs:label "Dark European Lager"@en ,
                                                     "Lager Européenne Foncée"@fr ;
                                          <http://www.w3.org/2004/02/skos/core#definition> "Ce style de bière comprend des bières blondes fortes (vollbier) de couleur plus foncée que les bières de couleur brun ambré."@fr ,
                                                                                           "This style of beer includes strong (vollbier) lager that are darker in color than amber-brown colored beers."@en ;
                                          <http://xmlns.com/foaf/0.1/name> "Dark European Lager" .


###  https://rdf.ag/o/beer#EnglishPaleAle
<https://rdf.ag/o/beer#EnglishPaleAle> rdf:type owl:Class ;
                                       rdfs:subClassOf <https://rdf.ag/o/beer#EnglishStyleAle> ,
                                                       <https://rdf.ag/o/beer#PaleAle> ;
                                       <http://rdfs.org/ns/void#inDataset> <https://rdf.ag/o/beer#datasetdefinition> ;
                                       rdfs:isDefinedBy <https://rdf.ag/o/beer-2024-02-21> ;
                                       rdfs:label "British Pale Ale"@en ,
                                                  "English Pale Ale"@en ,
                                                  "English-Style Pale Ale"@en ;
                                       <http://www.w3.org/2004/02/skos/core#definition> "English Pale Ale is a type of pale ale that is brewed in the English style, usually more with more hop flavor and bitterness."@en ,
                                                                                        "La Pale Ale anglaise est un type de ale pâle brassée dans le style anglais, généralement plus avec plus de saveur de houblon et d'amertume."@fr ;
                                       <http://xmlns.com/foaf/0.1/name> "English Pale Ale" .


###  https://rdf.ag/o/beer#EnglishStyleAle
<https://rdf.ag/o/beer#EnglishStyleAle> rdf:type owl:Class ;
                                        rdfs:subClassOf <https://rdf.ag/o/beer#Ale> ,
                                                        <https://rdf.ag/o/beer#BritishBeer> ;
                                        <http://rdfs.org/ns/void#inDataset> <https://rdf.ag/o/beer#datasetdefinition> ;
                                        rdfs:isDefinedBy <https://rdf.ag/o/beer-2024-02-21> ;
                                        rdfs:label "British Style Ale"@en ,
                                                   "English Style Ale"@en ,
                                                   "Style Anglais"@fr ;
                                        <http://www.w3.org/2004/02/skos/core#definition> "English Style Ales are ales are that are brewed in the English style."@en ,
                                                                                         "Les ales à l'anglaise sont des ales brassées dans le style Anglais."@fr ;
                                        <http://xmlns.com/foaf/0.1/name> "English Style Ale" .


###  https://rdf.ag/o/beer#EuropeanBeer
<https://rdf.ag/o/beer#EuropeanBeer> rdf:type owl:Class ;
                                     rdfs:subClassOf <https://rdf.ag/o/beer#Beer> ;
                                     <http://rdfs.org/ns/void#inDataset> <https://rdf.ag/o/beer#datasetdefinition> ;
                                     rdfs:isDefinedBy <http://rdf.ag/o/beer-2024-02-21> ;
                                     rdfs:label "Bière Européenne"@fr ,
                                                "European Beer"@en ;
                                     <http://www.w3.org/2004/02/skos/core#definition> "Beers whose style originated from Europe."@en ,
                                                                                      "Des bières dont le style est originaire d'Europe."@fr ;
                                     <http://xmlns.com/foaf/0.1/name> "European Beer" .


###  https://rdf.ag/o/beer#EuropeanSourAle
<https://rdf.ag/o/beer#EuropeanSourAle> rdf:type owl:Class ;
                                        rdfs:subClassOf <https://rdf.ag/o/beer#Ale> ,
                                                        <https://rdf.ag/o/beer#EuropeanBeer> ,
                                                        <https://rdf.ag/o/beer#SourBeer> ;
                                        <http://rdfs.org/ns/void#inDataset> <https://rdf.ag/o/beer#datasetdefinition> ;
                                        rdfs:isDefinedBy <http://rdf.ag/o/beer-2024-02-21> ;
                                        rdfs:label "Ale Aigre Européenn"@fr ,
                                                   "European Sour Ale"@en ;
                                        <http://www.w3.org/2004/02/skos/core#definition> "Ces bières représentent les bières acidulées traditionnelles d'Europe qui ont pour la plupart une base de blé et une faible amertume."@fr ,
                                                                                         "These beers represent the traditional sour beers of Europe that have a wheat base for the most part and low bitterness."@en ;
                                        <http://xmlns.com/foaf/0.1/name> "European Sour Ale" .


###  https://rdf.ag/o/beer#FarmhouseAle
<https://rdf.ag/o/beer#FarmhouseAle> rdf:type owl:Class ;
                                     rdfs:subClassOf <https://rdf.ag/o/beer#Ale> ,
                                                     <https://rdf.ag/o/beer#BelgianBeer> ;
                                     <http://rdfs.org/ns/void#inDataset> <https://rdf.ag/o/beer#datasetdefinition> ;
                                     rdfs:isDefinedBy <https://rdf.ag/o/beer-2024-02-21> ;
                                     rdfs:label "Ale de Ferme"@fr ,
                                                "Farmhouse Ale"@en ;
                                     <http://www.w3.org/2004/02/skos/core#definition> "Farmhouse ales are traditionally brewed during the winter with leftover crops from the harvest and are drunk by seasonal farmhands, or 'saisonniers' in French, when working on the farm throughout the following season. This classification of beer encompasses a number of styles."@en ,
                                                                                      "Les bières de ferme sont traditionnellement brassées pendant l'hiver avec les restes de récolte et sont bues par les ouvriers agricoles saisonniers, ou «saisonniers» en français, lorsqu'ils travaillent à la ferme tout au long de la saison suivante. Cette classification de la bière englobe un certain nombre de styles."@fr ;
                                     <http://xmlns.com/foaf/0.1/name> "Farmhouse Ale" .


###  https://rdf.ag/o/beer#FruitBeer
<https://rdf.ag/o/beer#FruitBeer> rdf:type owl:Class ;
                                  rdfs:subClassOf <https://rdf.ag/o/beer#Beer> ;
                                  <http://rdfs.org/ns/void#inDataset> <https://rdf.ag/o/beer#datasetdefinition> ;
                                  rdfs:isDefinedBy <http://rdf.ag/o/beer-2024-02-21> ;
                                  rdfs:label "Bière aux Fruits"@fr ,
                                             "Fruit Beer"@en ;
                                  <http://www.w3.org/2004/02/skos/core#definition> "Fruit beers involve the use of fruit in the beer brewing process. It is important to note that the culinary definition of 'fruit' is used, which are plant structures that are sweet or sour, have a seed or seeds and can be eaten raw."@en ,
                                                                                   "Les bières aux fruits impliquent l'utilisation de fruits dans le processus de brassage de la bière. Il est important de noter que la définition culinaire de «fruit» est utilisée, qui sont des structures végétales aigre-douces, ont une graine ou des graines et peuvent être consommées crues."@fr ;
                                  <http://xmlns.com/foaf/0.1/name> "Fruit Beer" .


###  https://rdf.ag/o/beer#GermanBeer
<https://rdf.ag/o/beer#GermanBeer> rdf:type owl:Class ;
                                   rdfs:subClassOf <https://rdf.ag/o/beer#EuropeanBeer> ;
                                   <http://rdfs.org/ns/void#inDataset> <https://rdf.ag/o/beer#datasetdefinition> ;
                                   rdfs:isDefinedBy <http://rdf.ag/o/beer-2024-02-21> ;
                                   rdfs:label "Bière Allemande"@fr ,
                                              "German Beer"@en ;
                                   <http://www.w3.org/2004/02/skos/core#definition> "Beers whose style originated from Germany."@en ,
                                                                                    "Bières dont le style est originaire d'Allemagne."@fr ;
                                   <http://xmlns.com/foaf/0.1/name> "German Beer" .


###  https://rdf.ag/o/beer#GermanPurityLawBeer
<https://rdf.ag/o/beer#GermanPurityLawBeer> rdf:type owl:Class ;
                                            rdfs:subClassOf <https://rdf.ag/o/beer#Beer> ,
                                                            <https://rdf.ag/o/beer#EuropeanBeer> ;
                                            <http://rdfs.org/ns/void#inDataset> <https://rdf.ag/o/Sundby2013> ,
                                                                                <https://rdf.ag/o/beer#datasetdefinition> ;
                                            rdfs:isDefinedBy <http://rdf.ag/o/beer-2024-02-21> ;
                                            rdfs:label "Bière Pureté Allemande"@fr ,
                                                       "German Purity Law Beer"@en ,
                                                       "Reinheitsgebot"@de ;
                                            <http://www.w3.org/2004/02/skos/core#definition> "A beer that meets the requirements of the German Beer Purity Law of 1516 where beer was made exclusively from water, barley, hops and yeast."@en ,
                                                                                             "Une bière qui répond aux exigences de la loi allemande sur la pureté de la bière de 1516, où la bière était fabriquée exclusivement à partir d'eau, d'orge, de houblon et de levure."@fr .


###  https://rdf.ag/o/beer#GermanWheatBeer
<https://rdf.ag/o/beer#GermanWheatBeer> rdf:type owl:Class ;
                                        rdfs:subClassOf <https://rdf.ag/o/beer#GermanBeer> ,
                                                        <https://rdf.ag/o/beer#WheatBeer> ;
                                        <http://rdfs.org/ns/void#inDataset> <https://rdf.ag/o/beer#datasetdefinition> ;
                                        rdfs:isDefinedBy <http://rdf.ag/o/beer-2024-02-21> ;
                                        rdfs:label "Bière de Blé Allemande"@fr ,
                                                   "German Wheat Beer"@en ;
                                        <http://www.w3.org/2004/02/skos/core#definition> "Ces bières de blé sont fortes et corsées (vollbier et starkbier). Ils peuvent être de couleur foncée ou pâle et n'avoir aucune aigreur."@fr ,
                                                                                         "These wheat beers are strong and full bodied (vollbier and starkbier). They can be dark or pale colored and have no sourness to them."@en ;
                                        <http://xmlns.com/foaf/0.1/name> "German Wheat Beer" .


###  https://rdf.ag/o/beer#GlutenFreeBeer
<https://rdf.ag/o/beer#GlutenFreeBeer> rdf:type owl:Class ;
                                       rdfs:subClassOf <https://rdf.ag/o/beer#Beer> ;
                                       <http://rdfs.org/ns/void#inDataset> <https://rdf.ag/o/beer#datasetdefinition> ;
                                       rdfs:isDefinedBy <http://rdf.ag/o/beer-2024-02-21> ;
                                       <http://www.w3.org/2004/02/skos/core#definition> "Beer that was brewed with no gluten products, specifically using gluten-free malts."@en ,
                                                                                        "Bière brassée sans produits sans gluten, en particulier avec des malts sans gluten."@fr .


###  https://rdf.ag/o/beer#GlutenReducedBeer
<https://rdf.ag/o/beer#GlutenReducedBeer> rdf:type owl:Class ;
                                          rdfs:subClassOf <https://rdf.ag/o/beer#Beer> ;
                                          <http://rdfs.org/ns/void#inDataset> <https://rdf.ag/o/beer#datasetdefinition> ;
                                          rdfs:isDefinedBy <http://rdf.ag/o/beer-2024-02-21> ;
                                          <http://www.w3.org/2004/02/skos/core#definition> "Beer that was brewed with ingredients containing gluten but had undergone another process to remove the gluten. Since there are gluten ingredients involved, there might still be traces of gluten that are lower than the FDA detectable gluten amount for labelling purposes but may still be present all the same."@en ,
                                                                                           "Bière brassée avec des ingrédients contenant du gluten mais ayant subi un autre processus pour éliminer le gluten. Étant donné qu'il y a des ingrédients de gluten impliqués, il peut toujours y avoir des traces de gluten qui sont inférieures à la quantité de gluten détectable par la FDA à des fins d'étiquetage, mais qui peuvent tout de même être présentes."@fr .


###  https://rdf.ag/o/beer#HistoricalBeer
<https://rdf.ag/o/beer#HistoricalBeer> rdf:type owl:Class ;
                                       rdfs:subClassOf <https://rdf.ag/o/beer#Beer> ;
                                       <http://rdfs.org/ns/void#inDataset> <https://rdf.ag/o/beer#datasetdefinition> ;
                                       rdfs:isDefinedBy <http://rdf.ag/o/beer-2024-02-21> ;
                                       rdfs:label "Bière Historique"@fr ,
                                                  "Historical Beer"@en ;
                                       <http://www.w3.org/2004/02/skos/core#definition> "Cette catégorie de styles de bière comprend les bières qui sont des recréations et redécouvertes de bières traditionnelles mais aussi des styles de bière qui ont disparu et ne sont plus en production aujourd'hui."@fr ,
                                                                                        "This category of beer styles includes beer that are recreations and rediscoveries of traditional beers but also beer styles that have died out and are no longer in production today."@en ;
                                       <http://xmlns.com/foaf/0.1/name> "Historical Beer" .


###  https://rdf.ag/o/beer#ImperialStout
<https://rdf.ag/o/beer#ImperialStout> rdf:type owl:Class ;
                                      rdfs:subClassOf <https://rdf.ag/o/beer#AmericanPorterandStout> ,
                                                      <https://rdf.ag/o/beer#Stout> ;
                                      <http://rdfs.org/ns/void#inDataset> <https://rdf.ag/o/beer#datasetdefinition> ;
                                      rdfs:isDefinedBy <http://rdf.ag/o/beer-2024-02-21> ;
                                      <http://www.w3.org/2004/02/skos/core#definition> "A very dark beer style with a high ABV. An intense and complex flavored stout that relies on roasted malts."@en ,
                                                                                       "Un style de bière très sombre avec un ABV élevé. Une stout au goût intense et complexe qui repose sur des malts torréfiés."@fr .


###  https://rdf.ag/o/beer#IndiaPaleAle
<https://rdf.ag/o/beer#IndiaPaleAle> rdf:type owl:Class ;
                                     rdfs:subClassOf <https://rdf.ag/o/beer#EnglishPaleAle> ;
                                     <http://rdfs.org/ns/void#inDataset> <https://rdf.ag/o/beer#datasetdefinition> ;
                                     rdfs:isDefinedBy <https://rdf.ag/o/beer-2024-02-21> ;
                                     rdfs:label "IPA"@en ;
                                     <http://www.w3.org/2004/02/skos/core#definition> "India Pale Ale is actually a type of pale ale that is brewed in the \"English\" style, contrary to its name. It was originally brewed for the Indian market which is where it got its name. It's origins are still debated to this day but this beer is known for its use of English hops and yeast."@en ,
                                                                                      "L'Inde Pale Ale est en fait un type de ale pâle qui est brassée dans le style \"anglais\", contrairement à son nom. Il était à l'origine brassé pour le marché indien, d'où il tire son nom. Ses origines sont encore débattues à ce jour, mais cette bière est connue pour son utilisation de houblon anglais et de levure."@fr ;
                                     <http://xmlns.com/foaf/0.1/name> "India Pale Ale" .


###  https://rdf.ag/o/beer#IrishBeer
<https://rdf.ag/o/beer#IrishBeer> rdf:type owl:Class ;
                                  rdfs:subClassOf <https://rdf.ag/o/beer#Beer> ,
                                                  <https://rdf.ag/o/beer#BritishBeer> ;
                                  <http://rdfs.org/ns/void#inDataset> <https://rdf.ag/o/beer#datasetdefinition> ;
                                  rdfs:isDefinedBy <http://rdf.ag/o/beer-2024-02-21> ;
                                  rdfs:label "Bière Irlandaise"@fr ,
                                             "Irish Beer"@en ;
                                  <http://www.w3.org/2004/02/skos/core#definition> "Ce style de bières contient des bières irlandaises traditionnelles à fermentation haute qui vont d'ambrées à foncées, et modérées à légèrement fortes."@fr ,
                                                                                   "This style of beers contains traditional Irish top-fermenting beers that range from being amber to dark, and moderate to being slightly strong."@en ;
                                  <http://xmlns.com/foaf/0.1/name> "Irish Beer" .


###  https://rdf.ag/o/beer#Kolsch
<https://rdf.ag/o/beer#Kolsch> rdf:type owl:Class ;
                               rdfs:subClassOf <https://rdf.ag/o/beer#GermanBeer> ,
                                               <https://rdf.ag/o/beer#GermanPurityLawBeer> ,
                                               <https://rdf.ag/o/beer#PaleBitterEuropeanBeer> ;
                               <http://rdfs.org/ns/void#inDataset> <https://rdf.ag/o/beer#datasetdefinition> ;
                               rdfs:isDefinedBy <http://rdf.ag/o/beer-2024-02-21> ;
                               rdfs:label "Kölsch Beer"@en ,
                                          "Kölsch Bier"@de ;
                               <http://www.w3.org/2004/02/skos/core#definition> "Kölsch beer is beer that has been brewed within 50 km of the city of Cologne, Germany and brewed according to the Kölsch Konvention as defined by the Kölner Brauerei-Verband, or the Cologne Brewers Association, and it also must confer to the Reinheitsgebot requirements."@en ,
                                                                                "La bière Kölsch est une bière brassée à moins de 50 km de la ville de Cologne, en Allemagne, et brassée selon la Kölsch Konvention telle que définie par le Kölner Brauerei-Verband, ou l'Association des brasseurs de Cologne, et elle doit également répondre aux exigences Reinheitsgebot."@fr .


###  https://rdf.ag/o/beer#Lager
<https://rdf.ag/o/beer#Lager> rdf:type owl:Class ;
                              rdfs:subClassOf <https://rdf.ag/o/beer#Beer> .


###  https://rdf.ag/o/beer#MaltBeverage
<https://rdf.ag/o/beer#MaltBeverage> rdf:type owl:Class .


###  https://rdf.ag/o/beer#Mead
<https://rdf.ag/o/beer#Mead> rdf:type owl:Class .


###  https://rdf.ag/o/beer#MilkStout
<https://rdf.ag/o/beer#MilkStout> rdf:type owl:Class ;
                                  rdfs:subClassOf <https://rdf.ag/o/beer#Stout> ;
                                  <http://rdfs.org/ns/void#inDataset> <https://rdf.ag/o/beer#datasetdefinition> ;
                                  rdfs:comment "Any stouts that that use milk or any milk product as an ingredient is an instance of this class despite the UK Food Labelling Regulations of 1996 to ensure that consumers are aware of a possibility of lactose in their beer."@en ,
                                               "Toute stout qui utilise du lait ou tout produit laitier comme ingrédient est un exemple de cette classe malgré les réglementations britanniques sur l'étiquetage des aliments de 1996 pour s'assurer que les consommateurs sont conscients d'une possibilité de lactose dans leur bière."@fr ;
                                  rdfs:isDefinedBy <https://rdf.ag/o/beer-2024-02-21> ;
                                  rdfs:label "Milk Stout"@en ,
                                             "Milk Stout"@fr ;
                                  <http://www.w3.org/2004/02/skos/core#definition> "Les stouts de lait sont un type de stouts qui ont été édulcorés par l'ajout de lait ou de produits laitiers."@fr ,
                                                                                   "Milk stouts are a type of stouts that have been sweetened by the addition of milk or milk products."@en ;
                                  <http://www.w3.org/2004/02/skos/core#historyNote> "Au Royaume-Uni, le Food Labelling Regulations de 1996 stipule que les stouts de lait ne peuvent pas être décrits comme contenant du «lait», étant donné que les éléments nutritifs du lait sont détruits ou transformés dans le processus de brassage et que ce qui reste n'est pas du «lait»."@fr ,
                                                                                    "In the United Kingdom, the Food Labelling Regulations of 1996 state that milk stouts cannot be described as containing 'milk', since the milk nutrients are destroyed or transformed in the brewing process and what is left is not 'milk'."@en ;
                                  <http://xmlns.com/foaf/0.1/name> "Milk Stout" .


###  https://rdf.ag/o/beer#MunichHelles
<https://rdf.ag/o/beer#MunichHelles> rdf:type owl:Class ;
                                     rdfs:subClassOf <https://rdf.ag/o/beer#GermanBeer> ,
                                                     <https://rdf.ag/o/beer#PaleMaltyEuropeanLager> ;
                                     <http://rdfs.org/ns/void#inDataset> <https://rdf.ag/o/beer#datasetdefinition> ;
                                     rdfs:isDefinedBy <http://rdf.ag/o/beer-2024-02-21> ;
                                     rdfs:label "Helles"@en ,
                                                "Munich Helles"@en ;
                                     <http://www.w3.org/2004/02/skos/core#definition> "La Munich Helles est un type de bière lager légère brassée en Allemagne qui a été créée pour concurrencer la pilsner tchèque. Ce style de bière utilise généralement du houblon Hallertau et met davantage l'accent sur les malts que la pilsner tchèque."@fr ,
                                                                                      "Munich Helles is a type of light lager brewed in Germany that was created in order to compete with Czech Pilsners. This style of beer typically uses Hallertau hops and has more of an amphasis on malts than the Czech Pilsners."@en ;
                                     <http://xmlns.com/foaf/0.1/name> "Munich Helles" .


###  https://rdf.ag/o/beer#NonAlcoholicBeer
<https://rdf.ag/o/beer#NonAlcoholicBeer> rdf:type owl:Class ;
                                         rdfs:subClassOf <https://rdf.ag/o/beer#Beer> ,
                                                         <https://rdf.ag/o/beer#NonAlcoholicDrink> ,
                                                         <https://schema.org/ProductGroup> ;
                                         <http://rdfs.org/ns/void#inDataset> <https://rdf.ag/o/beer#datasetdefinition> ;
                                         rdfs:isDefinedBy <https://rdf.ag/o/beer-2024-02-21> ;
                                         rdfs:label "Bière sans alcool"@fr ,
                                                    "Cereal Beverage"@en ,
                                                    "Non Alcoholic Beer"@en ;
                                         <http://www.w3.org/2004/02/skos/core#definition> "A malt beverage that has less than 0.5 percent alcohol by volume. According to the FDA and the Alcohol Tax and Trade Bureau, non-alcoholic beers are not treated as beers under the International Revenue Code (IRC) because they have less than 0.5% alcohol by volume. A non-alcoholic beer must use the term \"dealcoholized\" or \"alcohol-removed\" before 'beer' on its statement of identity and must be in equal font. \"Non-alcoholic\" can be used as an additional label but it cannot be used instead of \"dealcoholized\" or \"alcohol-removed\"."@en ,
                                                                                          "Une boisson maltée qui a moins de 0,5 pour cent d'alcool par volume. Selon la FDA et l'Alcool Tax and Trade Bureau, les bières non alcoolisées ne sont pas traitées comme des bières en vertu du Code international des revenus (IRC) car elles contiennent moins de 0,5% d'alcool en volume. Une bière sans alcool doit utiliser le terme \"désalcoolisé\" ou \"sans alcool\" avant \"bière\" sur sa déclaration d'identité et doit être dans la même police. \"Sans alcool\" peut être utilisé comme étiquette supplémentaire, mais il ne peut pas être utilisé à la place de \"désalcoolisé\" ou \"sans alcool\"."@fr .


###  https://rdf.ag/o/beer#NonAlcoholicDrink
<https://rdf.ag/o/beer#NonAlcoholicDrink> rdf:type owl:Class .


###  https://rdf.ag/o/beer#NorthAmericanBeer
<https://rdf.ag/o/beer#NorthAmericanBeer> rdf:type owl:Class ;
                                          rdfs:subClassOf <https://rdf.ag/o/beer#Beer> ;
                                          <http://rdfs.org/ns/void#inDataset> <https://rdf.ag/o/beer#datasetdefinition> ;
                                          rdfs:isDefinedBy <http://rdf.ag/o/beer-2024-02-21> ;
                                          rdfs:label "Bière Nord-Américaine"@fr ,
                                                     "North American Beer"@en ;
                                          <http://www.w3.org/2004/02/skos/core#definition> "Beers whose style originated from North America."@en ,
                                                                                           "Des bières dont le style est originaire d'Amérique du Nord."@fr ;
                                          <http://xmlns.com/foaf/0.1/name> "North American Beer" .


###  https://rdf.ag/o/beer#Oktoberfestbier
<https://rdf.ag/o/beer#Oktoberfestbier> rdf:type owl:Class ;
                                        rdfs:subClassOf <https://rdf.ag/o/beer#GermanBeer> ,
                                                        <https://rdf.ag/o/beer#Lager> ;
                                        <http://rdfs.org/ns/void#inDataset> <https://rdf.ag/o/beer#datasetdefinition> ;
                                        rdfs:comment "According to German Law, Oktoberfestbier is legally reserved for the six breweries who are allowed to serve their beer at the Munich Oktoberfest. Those brewers are: Augustiner, Hacker-Pschorr, Hofbräuhaus, Löwenbräu, Paulaner, and Spaten. However, German Law does not extend beyond the German borders so the märzen/oktoberfest is used as a label for a beer style elsewhere, particulary among craft brewers."@en ,
                                                     "According to German Law, Oktoberfestbier is legally reserved for the six breweries who are allowed to serve their beer at the Munich Oktoberfest. Those brewers are: Augustiner, Hacker-Pschorr, Hofbräuhaus, Löwenbräu, Paulaner, and Spaten. However, German Law does not extend beyond the German borders so the märzen/oktoberfest is used as a label for a beer style elsewhere, particulary among craft brewers."@fr ;
                                        rdfs:isDefinedBy <https://rdf.ag/o/beer-2024-02-21> ;
                                        rdfs:label "Märzen"@en ,
                                                   "Oktoberfest Beer"@en ;
                                        <http://www.w3.org/2004/02/skos/core#definition> """Les bières de style Märzen sont des lagers légères qui sont généralement brassées avec des malts de Vienne, de Munich et parfois Pilsner et du houblon allemand traditionnel à faible teneur en acide alpha comme Hallertau et Tettnanger, mais peuvent être remplacés par le mont. Hood ou Saaz. L'arôme de Märzen est légèrement amer et pas trop houblonné, de sorte que la saveur du malt de Vienne et de Munich est plus prononcée. Cette bière a généralement une teneur en alcool plus élevée que les lagers allemandes traditionnelles à environ 5-6% abv. L'arôme est comparable à le Lager de Vienne.
         
         Historiquement, ce style de bière était brassé en mars, d'où le Märzen signifiant «mars» en allemand. En raison du manque de réfrigération à l'époque, le duc bavarois Albrecht V a décrété qu'aucun brassage ne devrait avoir lieu entre le 23 avril et le 29 septembre pour réduire la détérioration de la bière. Par conséquent, les bières ont été brassées en mars et mises en bière (conservées au frais) jusqu'à l'Oktoberfest. Traditionnellement, ces bières étaient plus foncées mais sont devenues de plus en plus légères pour correspondre aux goûts modernes."""@fr ,
                                                                                         "Märzen-style beers are light lagers that are typically brewed with Vienna, Munich and sometimes Pilsner malts and traditional German hops with low alpha acid contents such as Hallertau and Tettnanger but can substituted with Mt. Hood or Saaz. The aroma of Märzen is slightly bitter and not overly hoppy so that the Vienna and Munich malt flavor is more promenant. This beer is typically higher in alcohol content than traditional German lagers at around 5-6% abv. The aroma is comparable to Vienna lager."@en ;
                                        <http://xmlns.com/foaf/0.1/name> "Oktoberfest Beer"@en ,
                                                                         "Oktoberfestbier"@de ,
                                                                         "Märzenbier" .


###  https://rdf.ag/o/beer#PaleAle
<https://rdf.ag/o/beer#PaleAle> rdf:type owl:Class ;
                                rdfs:subClassOf <https://rdf.ag/o/beer#Ale> ;
                                <http://rdfs.org/ns/void#inDataset> <https://rdf.ag/o/beer#datasetdefinition> ;
                                rdfs:isDefinedBy <https://rdf.ag/o/beer-2024-02-21> ;
                                rdfs:label "Ale Pâle"@en ,
                                           "Pale Ale"@en ,
                                           "Une Blonde"@fr ;
                                <http://www.w3.org/2004/02/skos/core#definition> """Les Pale Ales sont un style de bière généralement de couleur claire, aux saveurs de houblon fort et à faible teneur en alcool. Ce terme générique comprend les IPA, les APA et les Ales Pâle Anglaises.
         
         La plupart des Pale Ales sont de style anglais, car elles sont devenues très populaires, de nombreux pays ont développé leurs propres versions de pâles ales qui provenaient du style anglais de brassage de bière.
         
         Samuel Allsopp à Burton, au Royaume-Uni, a brassé la première Ale Pâle pour le marché indien en 1822 et elle a été expédiée en 1823 en Inde, ce qui a eu un impact durable qui a conduit à l'essor des India Pale Ales.
         
         Les ales pâles étaient autrefois appelées «bitter ales», mais maintenant elles sont devenues trois versions «ordinaires» qui vont de 3% -4% ABV, «spéciales» et «extra spéciales» qui vont de 4,5-5% ABV."""@fr ,
                                                                                 """Pale Ales are a style of beer that are typically light in color, have stong hop flavors, and low in alcohol content. This umbrella term includes IPAs, APAs and English pale ales.
      
      Most Pale Ales are english-style, since it has become quite popular, many countries developed their own versions of pale ales that originated from English style of brewing beer.
      
      Samuel Allsopp in Burton, UK brewed the first pale ale for the Indian market in 1822 and it was shipped in 1823 to India which had a lasting impact that lead to the rise of India Pale Ales.
      
     Pale ales used to be called \"bitter ales\" in the past but now it has become three versions being \"ordinary\" that range in 3%-4% ABV, \"special\" and \"extra special\" that range 4.5-5% ABV."""@en ;
                                <http://xmlns.com/foaf/0.1/name> "Pale Ale" .


###  https://rdf.ag/o/beer#PaleBitterEuropeanBeer
<https://rdf.ag/o/beer#PaleBitterEuropeanBeer> rdf:type owl:Class ;
                                               rdfs:subClassOf <https://rdf.ag/o/beer#Beer> ,
                                                               <https://rdf.ag/o/beer#EuropeanBeer> ;
                                               <http://rdfs.org/ns/void#inDataset> <https://rdf.ag/o/beer#datasetdefinition> ;
                                               rdfs:isDefinedBy <http://rdf.ag/o/beer-2024-02-21> ;
                                               rdfs:label "Bière Européenne Amère Pâle"@fr ,
                                                          "Pale Bitter European Beer"@en ;
                                               <http://www.w3.org/2004/02/skos/core#definition> "Ces bières sont pâles et amères avec un arôme de houblon doux à modérément fort. Ces bières sont bien atténuées et sont généralement lagerées ou de fermentation basse."@fr ,
                                                                                                "These beers are pale and bitter with a mild to moderately strong hoppy aroma. These beers are well attenuated and are usually lagered, or bottom-fermented."@en ;
                                               <http://xmlns.com/foaf/0.1/name> "Pale Bitter European Beer" .


###  https://rdf.ag/o/beer#PaleCommonwealthBeer
<https://rdf.ag/o/beer#PaleCommonwealthBeer> rdf:type owl:Class ;
                                             rdfs:subClassOf <https://rdf.ag/o/beer#Beer> ,
                                                             <https://rdf.ag/o/beer#BritishBeer> ;
                                             <http://rdfs.org/ns/void#inDataset> <https://rdf.ag/o/beer#datasetdefinition> ;
                                             rdfs:isDefinedBy <http://rdf.ag/o/beer-2024-02-21> ;
                                             rdfs:label "Bière Pâle du Commonwealth"@fr ,
                                                        "Pale Commonwealth Beer"@en ;
                                             <http://www.w3.org/2004/02/skos/core#definition> "Ces bières proviennent toutes de pays ayant appartenu à l'ancien Empire britannique. Ils sont de couleur claire, sautent en avant, amers et modérément forts."@fr ,
                                                                                              "These beers are all from countries that once belonged to the former British Empire. They are light in color, hop forward, bitter, and moderately strong."@en ;
                                             <http://xmlns.com/foaf/0.1/name> "Pale Commonwealth Beer" .


###  https://rdf.ag/o/beer#PaleMaltyEuropeanLager
<https://rdf.ag/o/beer#PaleMaltyEuropeanLager> rdf:type owl:Class ;
                                               rdfs:subClassOf <https://rdf.ag/o/beer#EuropeanBeer> ,
                                                               <https://rdf.ag/o/beer#Lager> ;
                                               <http://rdfs.org/ns/void#inDataset> <https://rdf.ag/o/beer#datasetdefinition> ;
                                               rdfs:isDefinedBy <http://rdf.ag/o/beer-2024-02-21> ;
                                               rdfs:label "Lager Européenne Pâle et Maltée"@fr ,
                                                          "Pale Malty European Lager"@en ;
                                               <http://www.w3.org/2004/02/skos/core#definition> "Ce style comprend principalement des lagers allemandes qui utilisent des malts Pilsner et bien qu'elles soient maltées, elles sont toujours bien atténuées."@fr ,
                                                                                                "This style includes mostly German lagers that use Pilsner malts and while they are malty, they are still well attenuated."@en ;
                                               <http://xmlns.com/foaf/0.1/name> "Pale Malty European Lager" .


###  https://rdf.ag/o/beer#Pilsner_GermanStyle
<https://rdf.ag/o/beer#Pilsner_GermanStyle> rdf:type owl:Class ;
                                            rdfs:subClassOf <https://rdf.ag/o/beer#GermanBeer> ;
                                            <http://rdfs.org/ns/void#inDataset> <https://rdf.ag/o/beer#datasetdefinition> ;
                                            rdfs:isDefinedBy <https://rdf.ag/o/beer-2024-02-21> ;
                                            rdfs:label "German Style Pilsner"@en ;
                                            <http://www.w3.org/2004/02/skos/core#definition> "Ce style pilsner se caractérise par rapport aux pilsners tchèques en ayant utilisé des malts pilsner allemands et souvent un ou plusieurs des quatre houblons allemands 'nobles': Hallertau, Tettnanger, Spalt et Hersbrucker."@fr ,
                                                                                             "This style pilsner is characterized from Czech pilsners by having used German pilsner malts and often one or more of the four \"noble\" German hops: Hallertau, Tettnanger, Spalt and Hersbrucker."@en ;
                                            <http://xmlns.com/foaf/0.1/name> "German Style Pilsner" .


###  https://rdf.ag/o/beer#Saison
<https://rdf.ag/o/beer#Saison> rdf:type owl:Class ;
                               rdfs:subClassOf <https://rdf.ag/o/beer#FarmhouseAle> ;
                               <http://rdfs.org/ns/void#inDataset> <https://rdf.ag/o/beer#datasetdefinition> ;
                               rdfs:isDefinedBy <https://rdf.ag/o/beer-2024-02-21> ;
                               rdfs:label "Saison"@en ,
                                          "Saison"@fr ;
                               <http://www.w3.org/2004/02/skos/core#definition> "Les bières de saison sont des bières de saison qui sont généralement appréciées pendant l'été jusqu'à la fin de la récolte. Il existe une grande variété de saisons brassées à la mode, choisies à la discrétion du brasseur. Les saisons sont généralement plus fruitées et plus faibles en alcool que les bières typiques. Alors que les saisons sont originaires de Belgique, il y a une popularité croissante parmi les brasseurs artisanaux américains pour produire leurs propres saisons."@fr ,
                                                                                "Saison beers are seasonal beers that are typically enjoyed during the summer until the end of harvest. There are a wide variety of saisons brewed in the fasion as choosen at the brewer's discretion. Saisons are typically fruitier and lower in alcohol content than typical beers. While saisons originated in Belgium, there is increasing popularity among American craft brewers to produce their own saisons."@en ;
                               <http://xmlns.com/foaf/0.1/name> "Saison" .


###  https://rdf.ag/o/beer#Schwarzbier
<https://rdf.ag/o/beer#Schwarzbier> rdf:type owl:Class ;
                                    rdfs:subClassOf <https://rdf.ag/o/beer#DarkEuropeanLager> ,
                                                    <https://rdf.ag/o/beer#GermanBeer> ;
                                    <http://rdfs.org/ns/void#inDataset> <https://rdf.ag/o/beer#datasetdefinition> ;
                                    rdfs:isDefinedBy <https://rdf.ag/o/beer-2024-02-21> ;
                                    rdfs:label "Schwarzbier"@en ;
                                    <http://www.w3.org/2004/02/skos/core#definition> "La Schwarzbier est un type de Lager allemande qui est fabriquée à partir de malts torréfiés, semblable à un stout, ce qui lui donne sa coloration foncée. Des notes de chocolat ou de café peuvent être déduites des malts torréfiés utilisés dans son brassage."@fr ,
                                                                                     "Schwarzbier is a type of German Lager that is made from roasted malts, similar to a stout, which gives it its dark coloring. Hints of chocolate or coffee can be decerned from the roasted malts used in its brewing."@en ;
                                    <http://xmlns.com/foaf/0.1/name> "Schwarzbier" .


###  https://rdf.ag/o/beer#ScottishBeer
<https://rdf.ag/o/beer#ScottishBeer> rdf:type owl:Class ;
                                     rdfs:subClassOf <https://rdf.ag/o/beer#Beer> ,
                                                     <https://rdf.ag/o/beer#BritishBeer> ;
                                     <http://rdfs.org/ns/void#inDataset> <https://rdf.ag/o/beer#datasetdefinition> ;
                                     rdfs:isDefinedBy <http://rdf.ag/o/beer-2024-02-21> ;
                                     rdfs:label "Bière Écossaise"@fr ,
                                                "Scottish Beer"@en ;
                                     <http://www.w3.org/2004/02/skos/core#definition> "Les bières Écossaises étaient autrefois décrites en shillings - ou le prix d'un baril de bière - elles sont maintenant divisées en trois sous-catégories: Léger, Lourd et Exportation. Ces bières sont généralement houblonnées, utilisant des houblons plus caramélisés et ont généralement des ABV à l'extrémité inférieure."@fr ,
                                                                                      "Scottish Beers used to be described in shillings - or the price of a barrel of beer - now they are divided into three subcategories: Light, Heavy and Export. These beers are usually hop forward, using more caramelized hops, and usually have ABVs on the lower end."@en ;
                                     <http://xmlns.com/foaf/0.1/name> "Scottish Beer" .


###  https://rdf.ag/o/beer#SmokedBeer
<https://rdf.ag/o/beer#SmokedBeer> rdf:type owl:Class ;
                                   rdfs:subClassOf <https://rdf.ag/o/beer#Beer> ;
                                   <http://rdfs.org/ns/void#inDataset> <https://rdf.ag/o/beer#datasetdefinition> ;
                                   rdfs:isDefinedBy <http://rdf.ag/o/beer-2024-02-21> ;
                                   rdfs:label "Bière Fumée"@fr ,
                                              "Smoked Beer"@en ;
                                   <http://www.w3.org/2004/02/skos/core#definition> "Ce sont des bières de spécialité qui ont un arôme fumé distinct."@fr ,
                                                                                    "These are specialty beers that have a distinct smokey aroma."@en ;
                                   <http://xmlns.com/foaf/0.1/name> "Smoked Beer" .


###  https://rdf.ag/o/beer#SourBeer
<https://rdf.ag/o/beer#SourBeer> rdf:type owl:Class ;
                                 rdfs:subClassOf <https://rdf.ag/o/beer#Beer> ;
                                 <http://rdfs.org/ns/void#inDataset> <https://rdf.ag/o/beer#datasetdefinition> ;
                                 rdfs:isDefinedBy <https://rdf.ag/o/beer-2024-02-21> ;
                                 rdfs:label "Sour Beer"@en ;
                                 <http://www.w3.org/2004/02/skos/core#definition> "Les bières aigres sont un groupe de bières au goût aigre, acide ou acidulé. Ils proviennent d'une variété de styles et d'ingrédients. Cette acidité provient de la bactérie Pediococcus Lactobacillus, qui produit de l'acide lactique ainsi que de petites quantités d'acide acédique ou de vinaigre."@fr ,
                                                                                  "Sour beers are a grouping of beers that taste sour, acidic or tart. They come about from a variety of styles and ingredients. This acidity comes from the Pediococcus Lactobacillus bacteria, which produce lactic acid as well as some small amounts of acedic acid, or vinegar."@en ;
                                 <http://xmlns.com/foaf/0.1/name> "Sour Beer" .


###  https://rdf.ag/o/beer#SpecialtyBeer
<https://rdf.ag/o/beer#SpecialtyBeer> rdf:type owl:Class ;
                                      rdfs:subClassOf <https://rdf.ag/o/beer#Beer> ;
                                      <http://rdfs.org/ns/void#inDataset> <https://rdf.ag/o/beer#datasetdefinition> ;
                                      rdfs:isDefinedBy <http://rdf.ag/o/beer-2024-02-21> ;
                                      rdfs:label "Bière de Spécialité"@fr ,
                                                 "Hybrid/Mixed Beer"@en ,
                                                 "Specialty Beer"@en ;
                                      <http://www.w3.org/2004/02/skos/core#definition> "Ce sont des bières de spécialité qui ne rentrent dans aucune autre catégorie de bière."@fr ,
                                                                                       "These are specialty beers that do not fit in any other category of beer."@en ;
                                      <http://xmlns.com/foaf/0.1/name> "Specialty Beer" .


###  https://rdf.ag/o/beer#SpicedBeer
<https://rdf.ag/o/beer#SpicedBeer> rdf:type owl:Class ;
                                   rdfs:subClassOf <https://rdf.ag/o/beer#Beer> ;
                                   <http://rdfs.org/ns/void#inDataset> <https://rdf.ag/o/beer#datasetdefinition> ;
                                   rdfs:isDefinedBy <http://rdf.ag/o/beer-2024-02-21> ;
                                   rdfs:label "Bière Épicée"@fr ,
                                              "Spiced Beer"@en ;
                                   <http://www.w3.org/2004/02/skos/core#definition> "Ce sont des bières brassées avec les définitions culinaires des légumes, des herbes et des épices. Dans ce cas, le 'légume' est défini comme une partie d'une plante qui est moins sucrée que le fruit d'une plante, salée et peut parfois être consommée crue. Les 'herbes' sont les parties feuillues des plantes utilisées pour aromatiser les aliments tels que les pétales, les fleurs et les tiges. Les 'épices' sont les parties séchées et non feuillues des plantes utilisées pour aromatiser et peuvent inclure les graines, l'écorce, les racines et les fruits."@fr ,
                                                                                    "These are beers that a brewed with the culinary definitions of vegetable, herbs, and spices. In this instance 'vegetable' is defined as a part of a plant that is less sweet than the fruit of a plant, savory and can sometimes be eaten raw. 'Herbs' are the leafy parts of plants used for flavoring food such as petals, flowers, and stalks. 'Spices' are the dried, non-leafy parts of plants used for flavoring and can include seeds, bark, roots and fruit."@en ;
                                   <http://xmlns.com/foaf/0.1/name> "Spiced Beer" .


###  https://rdf.ag/o/beer#Stout
<https://rdf.ag/o/beer#Stout> rdf:type owl:Class ;
                              rdfs:subClassOf <https://rdf.ag/o/beer#Ale> ;
                              <http://rdfs.org/ns/void#inDataset> <https://rdf.ag/o/beer#datasetdefinition> ;
                              rdfs:isDefinedBy <https://rdf.ag/o/beer-2024-02-21> ;
                              rdfs:label "Stout"@en ,
                                         "Stout"@fr ;
                              <http://www.w3.org/2004/02/skos/core#definition> "Les stouts sont un type de bière noire qui utilise une orge «fumée» ou maltée, qui donne son arôme distinctif de «café» ou de «chocolat». Les stouts sont similaires aux porteurs mais sont généralement plus épais et plus sains."@fr ,
                                                                               "Stouts are a dark type of ale that use a 'smoked' or malted barley, which give its distinctive 'coffee' or 'chocolate' flavored. Stouts are similar to porters but are usually thicker and healthier."@en ;
                              <http://xmlns.com/foaf/0.1/name> "Stout" .


###  https://rdf.ag/o/beer#StrongAmericanAle
<https://rdf.ag/o/beer#StrongAmericanAle> rdf:type owl:Class ;
                                          rdfs:subClassOf <https://rdf.ag/o/beer#Ale> ,
                                                          <https://rdf.ag/o/beer#PaleAle> ;
                                          <http://rdfs.org/ns/void#inDataset> <https://rdf.ag/o/beer#datasetdefinition> ;
                                          rdfs:isDefinedBy <http://rdf.ag/o/beer-2024-02-21> ;
                                          rdfs:label "Ale Américaine Forte"@fr ,
                                                     "Strong American Ale"@en ;
                                          <http://www.w3.org/2004/02/skos/core#definition> "Ces bières se caractérisent par leurs profils forts qui ont des ABV élevés et manquent de torréfaction."@fr ,
                                                                                           "These beers are characterized by their strong profiles that have high ABVs and lacking roast."@en ;
                                          <http://xmlns.com/foaf/0.1/name> "Strong American Ale" .


###  https://rdf.ag/o/beer#StrongBelgianAle
<https://rdf.ag/o/beer#StrongBelgianAle> rdf:type owl:Class ;
                                         rdfs:subClassOf <https://rdf.ag/o/beer#BelgianAle> ;
                                         <http://rdfs.org/ns/void#inDataset> <https://rdf.ag/o/beer#datasetdefinition> ;
                                         rdfs:isDefinedBy <http://rdf.ag/o/beer-2024-02-21> ,
                                                          <https://rdf.ag/o/beer-2024-02-21> ;
                                         rdfs:label "Ale Belge Forte"@fr ,
                                                    "Strong Belgian Ale"@en ;
                                         <http://www.w3.org/2004/02/skos/core#definition> "Belgian Ales are ales are that are brewed in the Belgian style."@en ,
                                                                                          "Les Strong Belgian Ales sont les versions les plus fortes des Belgian Ales, elles reposent davantage sur la levure pour leur saveur plutôt que sur les malts comme pour la plupart des Belges Ales et ont généralement une teneur en alcool plus élevée."@fr ,
                                                                                          "Les bières belges sont des bières brassées dans le style belge."@fr ,
                                                                                          "Strong Belgian Ales are the stronger versions of Belgian Ales, they rely more on yeast for their flavor rather than malts as for most Belgian Ales and generally have higher alcohol content."@en ;
                                         <http://xmlns.com/foaf/0.1/name> "Strong Belgian Ale" .


###  https://rdf.ag/o/beer#StrongBritishAle
<https://rdf.ag/o/beer#StrongBritishAle> rdf:type owl:Class ;
                                         rdfs:subClassOf <https://rdf.ag/o/beer#Ale> ,
                                                         <https://rdf.ag/o/beer#BritishBeer> ;
                                         <http://rdfs.org/ns/void#inDataset> <https://rdf.ag/o/beer#datasetdefinition> ;
                                         rdfs:isDefinedBy <http://rdf.ag/o/beer-2024-02-21> ;
                                         rdfs:label "Ale Britannique Forte"@fr ,
                                                    "Strong British Ale"@en ;
                                         <http://www.w3.org/2004/02/skos/core#definition> "Ces bières proviennent des îles britanniques et sont généralement fortes et non torréfiées."@fr ,
                                                                                          "These beers are from the British Isles and are typically strong and non-roasty."@en ;
                                         <http://xmlns.com/foaf/0.1/name> "Strong British Ale" .


###  https://rdf.ag/o/beer#StrongEuropeanBeer
<https://rdf.ag/o/beer#StrongEuropeanBeer> rdf:type owl:Class ;
                                           rdfs:subClassOf <https://rdf.ag/o/beer#Beer> ,
                                                           <https://rdf.ag/o/beer#EuropeanBeer> ;
                                           <http://rdfs.org/ns/void#inDataset> <https://rdf.ag/o/beer#datasetdefinition> ;
                                           rdfs:isDefinedBy <http://rdf.ag/o/beer-2024-02-21> ;
                                           rdfs:label "Bière Européenne Forte"@fr ,
                                                      "Strong European Beer"@en ;
                                           <http://www.w3.org/2004/02/skos/core#definition> "Ce sont des bières blondes d'Allemagne et des régions baltes d'Europe et ont généralement une teneur en alcool plus élevée et sont plus fortes que les autres bières de la région. Ils ne se limitent pas aux bières de couleur foncée."@fr ,
                                                                                            "These are lagers from Germany and the Baltic regions of Europe and usually have higher alcohol contents and are stronger than other beers from the region. They are not limited to just dark colored beers."@en ;
                                           <http://xmlns.com/foaf/0.1/name> "Strong European Beer" .


###  https://rdf.ag/o/beer#SummerAle
<https://rdf.ag/o/beer#SummerAle> rdf:type owl:Class ;
                                  rdfs:subClassOf <https://rdf.ag/o/beer#Ale> ;
                                  <http://rdfs.org/ns/void#inDataset> <https://rdf.ag/o/beer#datasetdefinition> ;
                                  rdfs:isDefinedBy <https://rdf.ag/o/beer-2024-02-21> ;
                                  rdfs:label "Ale d'Été"@fr ,
                                             "Summer Ale"@en ;
                                  <http://www.w3.org/2004/02/skos/core#definition> "Les bières d'été sont généralement caractérisées comme une bière d'été aux agrumes et rafraîchissante. Ils sont le plus souvent une forme de bière de blé américaine, mais peuvent inclure d'autres styles de bière."@fr ,
                                                                                   "Summer Ales are typically characterized as citrus-y and refreshing summer beer. They are most commonly a form of American Wheat beer or English-style summer ale, but can include other styles of ale."@en ;
                                  <http://xmlns.com/foaf/0.1/name> "Summer Ale" .


###  https://rdf.ag/o/beer#TraditionalOktoberfestbier
<https://rdf.ag/o/beer#TraditionalOktoberfestbier> rdf:type owl:Class ;
                                                   rdfs:subClassOf <https://rdf.ag/o/beer#GermanBeer> ,
                                                                   <https://rdf.ag/o/beer#Lager> ;
                                                   <http://rdfs.org/ns/void#inDataset> <https://rdf.ag/o/beer#datasetdefinition> ;
                                                   rdfs:comment "According to German Law, Oktoberfestbier is legally reserved for the six breweries who are allowed to serve their beer at the Munich Oktoberfest. Those brewers are: Augustiner, Hacker-Pschorr, Hofbräuhaus, Löwenbräu, Paulaner, and Spaten. However, German Law does not extend beyond the German borders so the märzen/oktoberfest is used as a label for a beer style elsewhere, particulary among craft brewers."@en ,
                                                                "According to German Law, Oktoberfestbier is legally reserved for the six breweries who are allowed to serve their beer at the Munich Oktoberfest. Those brewers are: Augustiner, Hacker-Pschorr, Hofbräuhaus, Löwenbräu, Paulaner, and Spaten. However, German Law does not extend beyond the German borders so the märzen/oktoberfest is used as a label for a beer style elsewhere, particulary among craft brewers."@fr ;
                                                   rdfs:isDefinedBy <https://rdf.ag/o/beer-2024-02-21> ;
                                                   rdfs:label "Traditional Märzenbier"@en ,
                                                              "Traditional Oktoberfest Beer"@en ;
                                                   <http://www.w3.org/2004/02/skos/core#definition> """Historically, this style of beer was brewed in March, hence the Märzen meaning 'March' in German. Due to the lack of refrigeration at the time, the Bavarian Duke Albrecht V decreed that no brewing should occur between April 23 and September 29th to reduce beer spoilage. Therefore the beers were brewed in March and lagered (stored cool) until Oktoberfest. Traditionally these beers were darker but have now become increasing lighter to match modern tastes.
         
         The first lager that was officially labelled 'Märzenbier' was brewed in 1841 by the Spaten Brewery of Munich and was introduced at that year's Oktoberfest. In 1872 Spaten was the first to label their märzen-style lager as Oktoberfestbier, and the recipe Spaten uses today is still largely based on the one used in 1872."""@en ,
                                                                                                    """Historiquement, ce style de bière était brassé en mars, d'où le Märzen signifiant «mars» en allemand. En raison du manque de réfrigération à l'époque, le duc bavarois Albrecht V a décrété qu'aucun brassage ne devrait avoir lieu entre le 23 avril et le 29 septembre pour réduire la détérioration de la bière. Par conséquent, les bières ont été brassées en mars et conservées au frais jusqu'à l'Oktoberfest. Traditionnellement, ces bières étaient plus foncées mais sont devenues de plus en plus légères pour correspondre aux goûts modernes.
     
         La première lager officiellement étiquetée «Märzenbier» a été brassée en 1841 par la brasserie Spaten de Munich et a été présentée à l'Oktoberfest de cette année-là. En 1872, Spaten fut le premier à étiqueter son lager de style märzen comme Oktoberfestbier, et la recette que Spaten utilise aujourd'hui est encore largement basée sur celle utilisée en 1872."""@fr ;
                                                   <http://xmlns.com/foaf/0.1/name> "Traditional Oktoberfest Beer"@en ,
                                                                                    "Traditional Märzenbier" .


###  https://rdf.ag/o/beer#TrappistAle
<https://rdf.ag/o/beer#TrappistAle> rdf:type owl:Class ;
                                    rdfs:subClassOf <https://rdf.ag/o/beer#Ale> ;
                                    <http://rdfs.org/ns/void#inDataset> <https://rdf.ag/o/beer#datasetdefinition> ;
                                    rdfs:isDefinedBy <http://rdf.ag/o/beer-2024-02-21> ;
                                    rdfs:label "Bière Trappiste"@fr ,
                                               "Trappist Ale"@en ;
                                    <http://www.w3.org/2004/02/skos/core#definition> "Le terme 'Trappiste' utilisé pour décrire la bière est une appellation protégée qui n'est utilisée que par les monastères trappistes brasseurs de bière. Les Trappist Ales sont caractérisées comme étant hautement carbonatées et atténuées avec un fort caractère de levure."@fr ,
                                                                                     "The term 'Trappist' used to describe beer is a protected appelation  to be used only by the beer-brewing Trappists monastaries. Trappist Ales are characterized as being highly carbonated and attenuated with a strong yeast character."@en ;
                                    <http://xmlns.com/foaf/0.1/name> "Trappist Ale" .


###  https://rdf.ag/o/beer#WheatBeer
<https://rdf.ag/o/beer#WheatBeer> rdf:type owl:Class ;
                                  rdfs:subClassOf <https://rdf.ag/o/beer#Beer> ;
                                  <http://rdfs.org/ns/void#inDataset> <https://rdf.ag/o/beer#datasetdefinition> ;
                                  rdfs:isDefinedBy <https://rdf.ag/o/beer-2024-02-21> ;
                                  rdfs:label "Bière de Blé"@fr ,
                                             "Wheat Beer"@en ;
                                  <http://www.w3.org/2004/02/skos/core#definition> "Les bières de blé sont originaires d'Allemagne et sont généralement des ales pâles. Le style Ahe se caractérise par un pourcentage élevé de blé malté ou non."@fr ,
                                                                                   "Wheat beers are characterized by having a large percentage of malted or unmalted wheat. They originated in Germany and are usually brewed in the style of pale ales."@en ;
                                  <http://xmlns.com/foaf/0.1/name> "Wheat Beer" .


###  https://rdf.ag/o/beer#WoodBeer
<https://rdf.ag/o/beer#WoodBeer> rdf:type owl:Class ;
                                 rdfs:subClassOf <https://rdf.ag/o/beer#Beer> ;
                                 <http://rdfs.org/ns/void#inDataset> <https://rdf.ag/o/beer#datasetdefinition> ;
                                 rdfs:isDefinedBy <http://rdf.ag/o/beer-2024-02-21> ;
                                 rdfs:label "Bière De Bois"@fr ,
                                            "Wood Beer"@en ;
                                 <http://www.w3.org/2004/02/skos/core#definition> "Ce sont des bières de spécialité qui ont un arôme de bois vieilli."@fr ,
                                                                                  "These are specialty beers that have a wood-aged aroma."@en ;
                                 <http://xmlns.com/foaf/0.1/name> "Wood Beer" .


###  https://rdf.ag/o/cerealstoo#ADU
<https://rdf.ag/o/cerealstoo#ADU> rdf:type owl:Class ;
                                  rdfs:subClassOf <https://rdf.ag/o/cerealstoo#DUWH> ;
                                  <http://rdfs.org/ns/void#inDataset> <https://rdf.ag/o/cerealstoo#datasetdefinition> ;
                                  rdfs:isDefinedBy <https://rdf.ag/o/cerealstoo-2021-02-18> ;
                                  rdfs:label "Amber Durum Wheat"@en ,
                                             "Blé Dur Ambré"@fr ;
                                  <http://www.w3.org/2004/02/skos/core#definition> "Blé contenant moins de 75% mais plus de 60% de grains constitués de grains vitreux et durs de blé dur de couleur ambrée."@fr ,
                                                                                   "Wheat which has less than 75% but more than 60% of kernels consisting of vitreous and hard kernels of amber colored durum."@en ;
                                  <http://www.w3.org/ns/prov#hadPrimarySource> <https://rdf.ag/o/cerealstoo#USDA2014StandardsforWheat> ;
                                  <http://xmlns.com/foaf/0.1/name> "ADU" .


###  https://rdf.ag/o/cerealstoo#CEHRW
<https://rdf.ag/o/cerealstoo#CEHRW> rdf:type owl:Class ;
                                    rdfs:subClassOf <https://rdf.ag/o/cerealstoo#HardWheat> ,
                                                    <https://rdf.ag/o/cerealstoo#RedWheat> ,
                                                    <https://rdf.ag/o/cerealstoo#WinterWheat> ;
                                    <http://rdfs.org/ns/void#inDataset> <https://rdf.ag/o/cerealstoo#datasetdefinition> ;
                                    rdfs:isDefinedBy <https://rdf.ag/o/cerealstoo-2021-02-18> ;
                                    rdfs:label "Blé de Force Rouge d'Hiver de l'Est Canadien"@fr ,
                                               "Canada Eastern Hard Red Winter Wheat"@en ;
                                    <http://www.w3.org/2004/02/skos/core#definition> "CEHRWs have good milling and baking quality and has three milling grades. Wheats in this class are primarily used for noodles, steamed breads, French breads and flat breads."@en ,
                                                                                     "CEHRWs have good milling and baking quality and has three milling grades. Wheats in this class are primarily used for noodles, steamed breads, French breads and flat breads."@fr ;
                                    <http://www.w3.org/ns/prov#hadPrimarySource> <https://rdf.ag/o/cerealstoo#CanadianGrainCommission2019Canadian-Wheat-Classes> ;
                                    <http://xmlns.com/foaf/0.1/name> "CEHRW" .


###  https://rdf.ag/o/cerealstoo#CERS
<https://rdf.ag/o/cerealstoo#CERS> rdf:type owl:Class ;
                                   rdfs:subClassOf <https://rdf.ag/o/cerealstoo#RedWheat> ,
                                                   <https://rdf.ag/o/cerealstoo#SpringWheat> ;
                                   <http://rdfs.org/ns/void#inDataset> <https://rdf.ag/o/cerealstoo#datasetdefinition> ;
                                   rdfs:isDefinedBy <https://rdf.ag/o/cerealstoo-2021-02-18> ;
                                   rdfs:label "Blé Roux de Printemps de l'Est Canadien"@fr ,
                                              "Canada Eastern Red Spring Wheat"@en ;
                                   <http://www.w3.org/2004/02/skos/core#definition> "CERS wheats are used for the production of high volume pan bread, which can be used as it is or blended with other wheats to produce pasta, steamed bread, flat bread, noodles and hearth bread. This class has three milling grades and has superior milling and baking quality."@en ,
                                                                                    "Les blés CERS sont utilisés pour la production de pain de mie à grand volume, qui peut être utilisé tel quel ou mélangé avec d'autres blés pour produire des pâtes, du pain cuit à la vapeur, du pain plat, des nouilles et du pain de cuisine. Cette classe a trois grades de fraisage et a une qualité de fraisage et de cuisson supérieure."@fr ;
                                   <http://www.w3.org/ns/prov#hadPrimarySource> <https://rdf.ag/o/cerealstoo#CanadianGrainCommission2019Canadian-Wheat-Classes> ;
                                   <http://xmlns.com/foaf/0.1/name> "CERS" .


###  https://rdf.ag/o/cerealstoo#CESRW
<https://rdf.ag/o/cerealstoo#CESRW> rdf:type owl:Class ;
                                    rdfs:subClassOf <https://rdf.ag/o/cerealstoo#RedWheat> ,
                                                    <https://rdf.ag/o/cerealstoo#SoftWheat> ,
                                                    <https://rdf.ag/o/cerealstoo#SpringWheat> ;
                                    <http://rdfs.org/ns/void#inDataset> <https://rdf.ag/o/cerealstoo#datasetdefinition> ;
                                    rdfs:isDefinedBy <https://rdf.ag/o/cerealstoo-2021-02-18> ;
                                    rdfs:label "Blé Tendre Rouge d'Hiver de l'Est Canadien"@fr ,
                                               "Canada Eastern Soft Red Winter"@en ;
                                    <http://www.w3.org/2004/02/skos/core#definition> "CESRS wheats are wheats that are low in protein and are primarily used for patries, cakes, biscuits, cereal, filling and crackers."@en ,
                                                                                     "Les blés CESRS sont des blés pauvres en protéines et sont principalement utilisés pour les pâtisseries, les gâteaux, les biscuits, les céréales, la garniture et les craquelins."@fr ;
                                    <http://www.w3.org/ns/prov#hadPrimarySource> <https://rdf.ag/o/cerealstoo#CanadianGrainCommission2019Canadian-Wheat-Classes> ;
                                    <http://xmlns.com/foaf/0.1/name> "CESRW" .


###  https://rdf.ag/o/cerealstoo#CEWW
<https://rdf.ag/o/cerealstoo#CEWW> rdf:type owl:Class ;
                                   rdfs:subClassOf <https://rdf.ag/o/cerealstoo#SoftWheat> ,
                                                   <https://rdf.ag/o/cerealstoo#WhiteWheat> ,
                                                   <https://rdf.ag/o/cerealstoo#WinterWheat> ;
                                   <http://rdfs.org/ns/void#inDataset> <https://rdf.ag/o/cerealstoo#datasetdefinition> ;
                                   rdfs:isDefinedBy <https://rdf.ag/o/cerealstoo-2021-02-18> ;
                                   rdfs:label "Blé Blanc d'Hiver de l'Est Canadien"@fr ,
                                              "Canada Eastern White Winter Wheat"@en ;
                                   <http://www.w3.org/2004/02/skos/core#definition> "CEWW are soft, white winter wheats that are low in protein primarily used for biscuits, cakes, crackers, cereal, filling and pastries."@en ,
                                                                                    "Les CEWW sont des blés d'hiver doux et blancs à faible teneur en protéines, principalement utilisés pour les biscuits, les gâteaux, les craquelins, les céréales, la garniture et les pâtisseries."@fr ;
                                   <http://www.w3.org/ns/prov#hadPrimarySource> <https://rdf.ag/o/cerealstoo#CanadianGrainCommission2019Canadian-Wheat-Classes> ;
                                   <http://xmlns.com/foaf/0.1/name> "CEWW" .


###  https://rdf.ag/o/cerealstoo#CNHR
<https://rdf.ag/o/cerealstoo#CNHR> rdf:type owl:Class ;
                                   rdfs:subClassOf <https://rdf.ag/o/cerealstoo#HardWheat> ,
                                                   <https://rdf.ag/o/cerealstoo#RedWheat> ,
                                                   <https://rdf.ag/o/cerealstoo#SpringWheat> ;
                                   <http://rdfs.org/ns/void#inDataset> <https://rdf.ag/o/cerealstoo#datasetdefinition> ;
                                   rdfs:isDefinedBy <https://rdf.ag/o/cerealstoo-2021-02-18> ;
                                   rdfs:label "Blé de Force Rouge du Nord Canadien"@fr ,
                                              "Canada North Hard Red"@en ;
                                   <http://www.w3.org/2004/02/skos/core#definition> "CNHR wheats are red, spring wheats that have medium to hard kernels and medium gluten strength. These wheats have very good milling quality and have three milling grades. They are primarily used for steamed breads, flat breads, hearth breads and noodles."@en ,
                                                                                    "Les blés CNHR sont des blés rouges de printemps qui ont des grains moyens à durs et une force de gluten moyenne. Ces blés ont une très bonne qualité de mouture et ont trois grades de mouture. Ils sont principalement utilisés pour les pains cuits à la vapeur, les pains plats, les pains de foyer et les nouilles."@fr ;
                                   <http://www.w3.org/ns/prov#hadPrimarySource> <https://rdf.ag/o/cerealstoo#CanadianGrainCommission2019Canadian-Wheat-Classes> ;
                                   <http://xmlns.com/foaf/0.1/name> "CNHR" .


###  https://rdf.ag/o/cerealstoo#CPSR
<https://rdf.ag/o/cerealstoo#CPSR> rdf:type owl:Class ;
                                   rdfs:subClassOf <https://rdf.ag/o/cerealstoo#RedWheat> ,
                                                   <https://rdf.ag/o/cerealstoo#SpringWheat> ;
                                   <http://rdfs.org/ns/void#inDataset> <https://rdf.ag/o/cerealstoo#datasetdefinition> ;
                                   rdfs:isDefinedBy <https://rdf.ag/o/cerealstoo-2021-02-18> ;
                                   rdfs:label "Blé Roux de Printemps Canada Prairie"@fr ,
                                              "Canada Prairie Spring Red"@en ;
                                   <http://www.w3.org/2004/02/skos/core#definition> "CPSR wheats are red, spring wheats that have medium hard kernels, two milling grades and medium dough strangth. They are primarily used for steamed breads, hearth breads, noodles and flat breads."@en ,
                                                                                    "Les blés CPSR sont des blés rouges de printemps qui ont des grains moyennement durs, deux grades de mouture et une pâte moyenne. Ils sont principalement utilisés pour les pains cuits à la vapeur, les pains de foyer, les nouilles et les pains plats."@fr ;
                                   <http://www.w3.org/ns/prov#hadPrimarySource> <https://rdf.ag/o/cerealstoo#CanadianGrainCommission2019Canadian-Wheat-Classes> ;
                                   <http://xmlns.com/foaf/0.1/name> "CPSR" .


###  https://rdf.ag/o/cerealstoo#CPSW
<https://rdf.ag/o/cerealstoo#CPSW> rdf:type owl:Class ;
                                   rdfs:subClassOf <https://rdf.ag/o/cerealstoo#SpringWheat> ,
                                                   <https://rdf.ag/o/cerealstoo#WhiteWheat> ;
                                   <http://rdfs.org/ns/void#inDataset> <https://rdf.ag/o/cerealstoo#datasetdefinition> ;
                                   rdfs:isDefinedBy <https://rdf.ag/o/cerealstoo-2021-02-18> ;
                                   rdfs:label "Blé Blanc de Printemps Canada Prairie"@fr ,
                                              "Canada Prairie Spring White"@en ;
                                   <http://www.w3.org/2004/02/skos/core#definition> "CPSW are white spring wheats with two milling grades and have medium dough strength. They are primarily used for chapatis, noodles and flat breads."@en ,
                                                                                    "Les CPSW sont des blés de printemps blancs avec deux grades de mouture et une pâte moyenne. Ils sont principalement utilisés pour les chapatis, les nouilles et les pains plats."@fr ;
                                   <http://www.w3.org/ns/prov#hadPrimarySource> <https://rdf.ag/o/cerealstoo#CanadianGrainCommission2019Canadian-Wheat-Classes> ;
                                   <http://xmlns.com/foaf/0.1/name> "CPSW" .


###  https://rdf.ag/o/cerealstoo#CWES
<https://rdf.ag/o/cerealstoo#CWES> rdf:type owl:Class ;
                                   rdfs:subClassOf <https://rdf.ag/o/cerealstoo#HardWheat> ,
                                                   <https://rdf.ag/o/cerealstoo#RedWheat> ,
                                                   <https://rdf.ag/o/cerealstoo#SpringWheat> ;
                                   <http://rdfs.org/ns/void#inDataset> <https://rdf.ag/o/cerealstoo#datasetdefinition> ;
                                   rdfs:isDefinedBy <https://rdf.ag/o/cerealstoo-2021-02-18> ;
                                   rdfs:label "Blé Extra Fort de l'Ouest Canadien"@fr ,
                                              "Canada Western Extra Strong"@en ;
                                   <http://www.w3.org/2004/02/skos/core#definition> "CERS wheats are hard, red spring wheats that have two milling grades and extra strong gluten. Wheats in this class are ideal for adding extra gluten strength to speciality products."@en ,
                                                                                    "Les blés CERS sont des blés de printemps durs rouges qui ont deux grades de mouture et du gluten extra fort. Les blés de cette classe sont idéaux pour ajouter une force de gluten supplémentaire aux produits de spécialité."@fr ;
                                   <http://www.w3.org/ns/prov#hadPrimarySource> <https://rdf.ag/o/cerealstoo#CanadianGrainCommission2019Canadian-Wheat-Classes> ;
                                   <http://xmlns.com/foaf/0.1/name> "CWES" .


###  https://rdf.ag/o/cerealstoo#CWHWS
<https://rdf.ag/o/cerealstoo#CWHWS> rdf:type owl:Class ;
                                    rdfs:subClassOf <https://rdf.ag/o/cerealstoo#HardWheat> ,
                                                    <https://rdf.ag/o/cerealstoo#SpringWheat> ,
                                                    <https://rdf.ag/o/cerealstoo#WhiteWheat> ;
                                    <http://rdfs.org/ns/void#inDataset> <https://rdf.ag/o/cerealstoo#datasetdefinition> ;
                                    rdfs:isDefinedBy <https://rdf.ag/o/cerealstoo-2021-02-18> ;
                                    rdfs:label "Blé de Force Blanc de Printemps de l'Ouest Canadien"@fr ,
                                               "Canadian Western Hard White Spring"@en ;
                                    <http://www.w3.org/2004/02/skos/core#definition> "CWHWS wheats are hard, white spring wheats that have superior milling quality, three milling grades and produce flour with excellent color. They are primarily used for noodles and breadmaking."@en ,
                                                                                     "Les blés CWHWS sont des blés de force blanc de printemps qui ont une qualité de mouture supérieure, trois grades de mouture et produisent une farine avec une excellente couleur. Ils sont principalement utilisés pour les nouilles et la panification."@fr ;
                                    <http://www.w3.org/ns/prov#hadPrimarySource> <https://rdf.ag/o/cerealstoo#CanadianGrainCommission2019Canadian-Wheat-Classes> ;
                                    <http://xmlns.com/foaf/0.1/name> "CWHWS" .


###  https://rdf.ag/o/cerealstoo#CWRS
<https://rdf.ag/o/cerealstoo#CWRS> rdf:type owl:Class ;
                                   rdfs:subClassOf <https://rdf.ag/o/cerealstoo#HardWheat> ,
                                                   <https://rdf.ag/o/cerealstoo#RedWheat> ,
                                                   <https://rdf.ag/o/cerealstoo#SpringWheat> ;
                                   <http://rdfs.org/ns/void#inDataset> <https://rdf.ag/o/cerealstoo#datasetdefinition> ;
                                   rdfs:isDefinedBy <https://rdf.ag/o/cerealstoo-2021-02-18> ;
                                   rdfs:label "Blé Roux de Printemps de l'Ouest Canadien"@fr ,
                                              "Canadian Western Red Spring"@en ;
                                   <http://www.w3.org/2004/02/skos/core#definition> "CWRS wheats are hard, red spring wheats that have superior milling, baking qualitymthree milling grades, and  various protein levels. They are commonly used alone or in blends with other wheats for the production of pan bread in high volumes. They can also be used for hearth breads, pasta, noodles, steamed and flat breads."@en ,
                                                                                    "Les blés CWRS sont des blés de force roux de printemps qui ont une qualité de mouture et de boulangerie supérieure avec trois grades de mouture et divers niveaux de protéines. Ils sont couramment utilisés seuls ou en mélanges avec d'autres blés pour la production de pain pané en grandes quantités. Ils peuvent également être utilisés pour les pains de foyer, les pâtes, les nouilles, les pains cuits à la vapeur et plats."@fr ;
                                   <http://www.w3.org/ns/prov#hadPrimarySource> <https://rdf.ag/o/cerealstoo#CanadianGrainCommission2019Canadian-Wheat-Classes> ;
                                   <http://xmlns.com/foaf/0.1/name> "CWRS" .


###  https://rdf.ag/o/cerealstoo#CWRW
<https://rdf.ag/o/cerealstoo#CWRW> rdf:type owl:Class ;
                                   rdfs:subClassOf <https://rdf.ag/o/cerealstoo#HardWheat> ,
                                                   <https://rdf.ag/o/cerealstoo#RedWheat> ,
                                                   <https://rdf.ag/o/cerealstoo#WinterWheat> ;
                                   <http://rdfs.org/ns/void#inDataset> <https://rdf.ag/o/cerealstoo#datasetdefinition> ;
                                   rdfs:isDefinedBy <https://rdf.ag/o/cerealstoo-2021-02-18> ;
                                   rdfs:label "Blé Rouge d'Hiver de l'Ouest Canadien"@fr ,
                                              "Canada Western Red Winter"@en ;
                                   <http://www.w3.org/2004/02/skos/core#definition> "Les Blés Rouges d'Hiver de l'Ouest Canadien ont trois grades de mouture et une très bonne qualité de mouture. Il est couramment utilisé pour la cuisson de pains plats et français, de nouilles et de pains cuits à la vapeur."@fr ,
                                                                                    "The CWRW wheat class has three milling grades and very good milling quality. These wheats are commonly used for baking flat and french breads, noodles, and for steamed breads."@en ;
                                   <http://www.w3.org/ns/prov#hadPrimarySource> <https://rdf.ag/o/cerealstoo#CanadianGrainCommission2019Canadian-Wheat-Classes> ;
                                   <http://xmlns.com/foaf/0.1/name> "CWRW" .


###  https://rdf.ag/o/cerealstoo#CWSWS
<https://rdf.ag/o/cerealstoo#CWSWS> rdf:type owl:Class ;
                                    rdfs:subClassOf <https://rdf.ag/o/cerealstoo#SoftWheat> ,
                                                    <https://rdf.ag/o/cerealstoo#SpringWheat> ,
                                                    <https://rdf.ag/o/cerealstoo#WhiteWheat> ;
                                    <http://rdfs.org/ns/void#inDataset> <https://rdf.ag/o/cerealstoo#datasetdefinition> ;
                                    rdfs:isDefinedBy <https://rdf.ag/o/cerealstoo-2021-02-18> ;
                                    rdfs:label "Blé Tendre Blanc de Printemps de l'Ouest Canadien"@fr ,
                                               "Canada Western Soft White Spring"@en ;
                                    <http://www.w3.org/2004/02/skos/core#definition> "CWSWS wheats have three milling grades, low protein content and are primarily used in cookies, pastries, cakes,  noodles, chapatis, steamed and flat breads."@en ,
                                                                                     "Les Blés Tendres Blancs de Printemps de l'Ouest Canadien ont trois grades de mouture, une faible teneur en protéines et sont principalement utilisés dans les pâtisseries, les biscuits, les gâteaux, les chapatis, les nouilles, les pains cuits à la vapeur et les pains plats."@fr ;
                                    <http://www.w3.org/ns/prov#hadPrimarySource> <https://rdf.ag/o/cerealstoo#CanadianGrainCommission2019Canadian-Wheat-Classes> ;
                                    <http://xmlns.com/foaf/0.1/name> "CWSWS" .


###  https://rdf.ag/o/cerealstoo#DU
<https://rdf.ag/o/cerealstoo#DU> rdf:type owl:Class ;
                                 rdfs:subClassOf <https://rdf.ag/o/cerealstoo#DUWH> ;
                                 <http://rdfs.org/ns/void#inDataset> <https://rdf.ag/o/cerealstoo#datasetdefinition> ;
                                 rdfs:isDefinedBy <https://rdf.ag/o/cerealstoo-2021-02-18> ;
                                 rdfs:label "Amber Durum Wheat"@en ,
                                            "Blé Dur Ambré"@fr ;
                                 <http://www.w3.org/2004/02/skos/core#definition> "Blé dont moins de 60% de grains sont constitués de grains vitreux et durs de blé dur de couleur ambrée."@fr ,
                                                                                  "Wheat which has less than 60% of kernels consisting of vitreous and hard kernels of amber colored durum."@en ;
                                 <http://www.w3.org/ns/prov#hadPrimarySource> <https://rdf.ag/o/cerealstoo#USDA2014StandardsforWheat> ;
                                 <http://xmlns.com/foaf/0.1/name> "DU" .


###  https://rdf.ag/o/cerealstoo#DUWH
<https://rdf.ag/o/cerealstoo#DUWH> rdf:type owl:Class ;
                                   rdfs:subClassOf :Cereal ;
                                   <http://rdfs.org/ns/void#inDataset> <https://rdf.ag/o/cerealstoo#datasetdefinition> ;
                                   rdfs:isDefinedBy <https://rdf.ag/o/cerealstoo-2021-02-18> ;
                                   rdfs:label "Blé Dur"@fr ,
                                              "Durum Wheat"@en ;
                                   <http://www.w3.org/2004/02/skos/core#definition> "Cette classe comprend toutes les variétés de blé dur."@fr ,
                                                                                    "This class includes all durum varieties of wheat."@en ;
                                   <http://www.w3.org/ns/prov#hadPrimarySource> <https://rdf.ag/o/cerealstoo#USDA2014StandardsforWheat> ;
                                   <http://xmlns.com/foaf/0.1/name> "DUWH" .


###  https://rdf.ag/o/cerealstoo#HADU
<https://rdf.ag/o/cerealstoo#HADU> rdf:type owl:Class ;
                                   rdfs:subClassOf <https://rdf.ag/o/cerealstoo#DUWH> ;
                                   <http://rdfs.org/ns/void#inDataset> <https://rdf.ag/o/cerealstoo#datasetdefinition> ;
                                   rdfs:isDefinedBy <https://rdf.ag/o/cerealstoo-2021-02-18> ;
                                   rdfs:label "Blé Dur Ambré de Force"@fr ,
                                              "Hard Amber Durum Wheat"@en ;
                                   <http://www.w3.org/2004/02/skos/core#definition> "Blé qui a au moins 75% de grains sont constitués de grains vitreux et durs de blé dur de couleur ambrée."@fr ,
                                                                                    "Wheat which has at least 75% of kernels consisting of vitreous and hard kernels of amber colored durum."@en ;
                                   <http://www.w3.org/ns/prov#hadPrimarySource> <https://rdf.ag/o/cerealstoo#USDA2014StandardsforWheat> ;
                                   <http://xmlns.com/foaf/0.1/name> "HADU" .


###  https://rdf.ag/o/cerealstoo#HardWheat
<https://rdf.ag/o/cerealstoo#HardWheat> rdf:type owl:Class ;
                                        rdfs:subClassOf :Cereal ;
                                        <http://rdfs.org/ns/void#inDataset> <https://rdf.ag/o/cerealstoo#datasetdefinition> ;
                                        rdfs:isDefinedBy <https://rdf.ag/o/cerealstoo-2021-02-18> ;
                                        rdfs:label "Blé de Force"@fr-ca ,
                                                   "Hard Wheat"@en ;
                                        <http://www.w3.org/2004/02/skos/core#definition> "Les blés considérés comme «durs» ont une teneur en protéines plus élevée que les blés «tendres». Cela signifie que ces blés contiennent plus de gluten, ce qui les rend idéaux pour les produits de boulangerie levés car le gluten fournit le composant élastique de la pâte et ce qui permet au pain d'avoir une texture spongieuse."@fr ,
                                                                                         "Wheats that are considered 'Hard' have a higher protein content relative to 'Soft' wheats. This means that these wheats have more gluten, which makes them ideal for baked goods that are yeast-leavened as the gluten provides the elastic component of dough and what allows bread to have a spongy texture."@en ;
                                        <http://www.w3.org/ns/prov#hadPrimarySource> <https://rdf.ag/o/cerealstoo#Gramene2013> ,
                                                                                     <https://rdf.ag/o/cerealstoo#HRUSKOVA2009> .


###  https://rdf.ag/o/cerealstoo#RedWheat
<https://rdf.ag/o/cerealstoo#RedWheat> rdf:type owl:Class ;
                                       rdfs:subClassOf :Cereal ;
                                       <http://rdfs.org/ns/void#inDataset> <https://rdf.ag/o/cerealstoo#datasetdefinition> ;
                                       rdfs:isDefinedBy <https://rdf.ag/o/cerealstoo-2021-02-18> ;
                                       rdfs:label "Blé Rouge"@fr ,
                                                  "Red Wheat"@en ;
                                       <http://www.w3.org/2004/02/skos/core#definition> "Il y a trois caractéristiques qui classent généralement les blés: printemps / hiver, rouge / blanc, dur / mou. Il n'est pas toujours facile de décerner la couleur des grains de blé, mais les grains de blé rouge présentent une pigmentation (souvent rougeâtre) dans le son du grain. Ce sont les gènes de la plante de blé qui déterminent la présence de pigments dans le son."@fr ,
                                                                                        "There are three characteristics that typically categorize wheats: spring/winter, red/white, hard/soft. It is not always easy to decern color in wheat kernels, but red wheat kernels show pigmentation (often reddish) in the bran of the grain. The genes of the wheat plant are what determines if there is a presence of pigments in the bran."@en ;
                                       <http://www.w3.org/ns/prov#hadPrimarySource> <https://rdf.ag/o/cerealstoo#Wang1999> .


###  https://rdf.ag/o/cerealstoo#SoftWheat
<https://rdf.ag/o/cerealstoo#SoftWheat> rdf:type owl:Class ;
                                        rdfs:subClassOf :Cereal ;
                                        <http://rdfs.org/ns/void#inDataset> <https://rdf.ag/o/cerealstoo#datasetdefinition> ;
                                        rdfs:isDefinedBy <https://rdf.ag/o/cerealstoo-2021-02-18> ;
                                        rdfs:label "Blé Tendre"@fr ,
                                                   "Soft Wheat"@en ;
                                        <http://www.w3.org/2004/02/skos/core#definition> "Les blés classés comme «tendres» ont un pourcentage plus élevé de glucides que les protéines (gluten), ce qui rend cette classification de blé idéale pour les pâtisseries et les gâteaux. Les blés tendres sont principalement classés comme blés «d'hiver»."@fr ,
                                                                                         "Wheats that are classified as 'Soft' have a larger percentage of carbohydrates than protein (gluten), which makes this classification of wheat ideal for pasties and cakes. Soft wheats are mostly categorized as 'Winter' wheats."@en ;
                                        <http://www.w3.org/ns/prov#hadPrimarySource> <https://rdf.ag/o/cerealstoo#Gramene2013> ,
                                                                                     <https://rdf.ag/o/cerealstoo#HRUSKOVA2009> .


###  https://rdf.ag/o/cerealstoo#SpringWheat
<https://rdf.ag/o/cerealstoo#SpringWheat> rdf:type owl:Class ;
                                          rdfs:subClassOf :Cereal ;
                                          <http://rdfs.org/ns/void#inDataset> <https://rdf.ag/o/cerealstoo#datasetdefinition> ;
                                          rdfs:isDefinedBy <https://rdf.ag/o/cerealstoo-2021-02-18> ;
                                          rdfs:label "Blé de Printemps"@fr ,
                                                     "Spring Wheat"@en ;
                                          <http://www.w3.org/2004/02/skos/core#definition> "Certain wheats varieties that have been bred, or have a genetic disposition, to produce higher yields when planted in the spring. This class can also include wheats that have not been bred to be spring wheats but wheats that produce good yields when planted in the spring, under ideal conditions."@en ,
                                                                                           "Certaines variétés de blé qui ont été sélectionnées ou qui ont une disposition génétique pour produire des rendements plus élevés lorsqu'elles sont plantées au printemps. Cette classe peut également inclure des blés qui n'ont pas été élevés pour être des blés de printemps mais des blés qui produisent de bons rendements lorsqu'ils sont plantés au printemps, dans des conditions idéales."@fr ;
                                          <http://www.w3.org/ns/prov#hadPrimarySource> <https://rdf.ag/o/cerealstoo#CerealsCanada2017-Review> .


###  https://rdf.ag/o/cerealstoo#WhiteWheat
<https://rdf.ag/o/cerealstoo#WhiteWheat> rdf:type owl:Class ;
                                         rdfs:subClassOf :Cereal ;
                                         <http://rdfs.org/ns/void#inDataset> <https://rdf.ag/o/cerealstoo#datasetdefinition> ;
                                         rdfs:isDefinedBy <https://rdf.ag/o/cerealstoo-2021-02-18> ;
                                         rdfs:label "Blé Blanc"@fr ,
                                                    "White Wheat"@en ;
                                         <http://www.w3.org/2004/02/skos/core#definition> "Les blés blancs sont des blés qui n'ont pas de pigments dans le son de leurs grains. Cette absence de pigmentation est due à la constitution génétique de la plante."@fr ,
                                                                                          "White wheats are wheat that have an absence of pigments in the bran of their kernels. This absence of pigmentation is due to the genetic make up of the plant."@en ;
                                         <http://www.w3.org/ns/prov#hadPrimarySource> <https://rdf.ag/o/cerealstoo#Wang1999> .


###  https://rdf.ag/o/cerealstoo#WinterWheat
<https://rdf.ag/o/cerealstoo#WinterWheat> rdf:type owl:Class ;
                                          rdfs:subClassOf :Cereal ;
                                          <http://rdfs.org/ns/void#inDataset> <https://rdf.ag/o/cerealstoo#datasetdefinition> ;
                                          rdfs:isDefinedBy <https://rdf.ag/o/cerealstoo-2021-02-18> ;
                                          rdfs:label "Blé d'Hiver"@fr ,
                                                     "Winter Wheat"@en ;
                                          <http://www.w3.org/2004/02/skos/core#definition> "Le blé d'hiver sont des cultivars de blé qui sont sélectionnés, ou qui ont une disposition génétique, pour produire de meilleurs rendements lorsqu'ils sont plantés à l'automne, laissés à hiverner puis récoltés au printemps. Cependant, d'autres variétés peuvent également produire de bons rendements (dans des conditions idéales) si elles sont également plantées à l'automne; même s'ils ne sont généralement pas considérés comme du blé d'hiver, ils peuvent être utilisés comme blé d'hiver."@fr ,
                                                                                           "Winter wheat are wheat cultivars that are bred, or have a genetic disposition, to produce better yields when they are planted in the fall, left to overwinter and then harvested in the spring. However, other varieties can also produce good yields (under ideal conditions) if they are planted in the fall as well; even if they aren't considered typically a winter wheat they can be used as winter wheat."@en ;
                                          <http://www.w3.org/ns/prov#hadPrimarySource> <https://rdf.ag/o/cerealstoo#CerealsCanada2017-Review> .


###  https://rdf.ag/o/hops#CTZ
<https://rdf.ag/o/hops#CTZ> rdf:type owl:Class ;
                            rdfs:subClassOf <https://rdf.ag/o/hops#HopsColumbus> ,
                                            <https://rdf.ag/o/hops#HopsTomahawk> ,
                                            <https://rdf.ag/o/hops#HopsZeus> ;
                            <http://rdfs.org/ns/void#inDataset> <https://rdf.ag/o/hops#datasetdefinition> ;
                            rdfs:isDefinedBy <https://rdf.ag/o/hops-2021-07-30> ;
                            rdfs:label "CTZ"@en ;
                            <http://www.w3.org/2004/02/skos/core#definition> "CTZ signifie Columbus, Tomahawk et Zeus, qui est un mélange de ces trois houblons car ces trois houblons ont une teneur élevée en acide alpha."@fr ,
                                                                             "CTZ stands for Columbus, Tomahawk and Zeus, which is a blend of these three hops since all three of these hops have high alpha acid contents."@en ;
                            <http://xmlns.com/foaf/0.1/name> "CTZ" .


###  https://rdf.ag/o/hops#Hops
<https://rdf.ag/o/hops#Hops> rdf:type owl:Class ;
                             rdfs:subClassOf <http://www.beerecipe.com/ontology#Ingredient> ;
                             owl:disjointWith <https://rdf.ag/o/malt#Malt> ;
                             <http://rdfs.org/ns/void#inDataset> <https://rdf.ag/o/hops#datasetdefinition> ;
                             rdfs:isDefinedBy <https://rdf.ag/o/hops-2021-07-30> ;
                             rdfs:label "Houblon"@fr ;
                             <http://www.w3.org/2004/02/skos/core#definition> "H. lupulus a le plus de valeur de ce genre car les fleurs ou le houblon sont un ingrédient clé de la bière. Cette espèce est principalement cultivée dans l'hémisphère nord (entre 35˚ et 55˚N) mais elle est également cultivée en Australie, en Nouvelle-Zélande et en Afrique du Sud."@fr ,
                                                                              "H. lupulus has the most value of this genus as the flowers or 'hops' are a key ingredient in beer. This species is mostly grown in the Northern Hemisphere (between 35˚ and 55˚N) but it is also cultivated in Australia, New Zealand and South Africa."@en ;
                             <http://xmlns.com/foaf/0.1/name> "H. lupulus"@la ,
                                                              "Hops"@en .


###  https://rdf.ag/o/hops#HopsAdmiral
<https://rdf.ag/o/hops#HopsAdmiral> rdf:type owl:Class ;
                                    rdfs:subClassOf <https://rdf.ag/o/hops#Hops> ;
                                    <http://rdfs.org/ns/void#inDataset> <https://rdf.ag/o/hops#datasetdefinition> ;
                                    rdfs:isDefinedBy <https://rdf.ag/o/hops-2021-07-30> ;
                                    rdfs:label "Admiral"@en ;
                                    <http://www.w3.org/2004/02/skos/core#definition> "Admiral a été élevé au Wye College au Royaume-Uni pour sa teneur élevée en acide alpha. Il est sorti en 1998 et descend très probablement de Challenger et Northdown. Admiral est principalement utilisé comme houblon amer."@fr ,
                                                                                     "Admiral was bred a Wye College in the UK for its high alpha acid content. It was released in 1998 and most likely descended from Challenger and Northdown. Admiral is mostly used as a bittering hop."@en ;
                                    <http://xmlns.com/foaf/0.1/name> "Admiral" ;
                                    <https://rdf.ag/o/hops#alphaAcidsContent> "13-16.2" ;
                                    <https://rdf.ag/o/hops#betaAcidsContent> "4.8-6.1" ;
                                    <https://rdf.ag/o/hops#perceivedAroma> "Agrumes, Amer, Herbal"@fr ,
                                                                           "Bitter, Citrus, Herbal"@en ;
                                    <https://rdf.ag/o/hops#totalOilContent> "1-1.7" .


###  https://rdf.ag/o/hops#HopsAhtanum
<https://rdf.ag/o/hops#HopsAhtanum> rdf:type owl:Class ;
                                    rdfs:subClassOf <https://rdf.ag/o/hops#Hops> ;
                                    <http://rdfs.org/ns/void#inDataset> <https://rdf.ag/o/hops#datasetdefinition> ;
                                    rdfs:isDefinedBy <https://rdf.ag/o/hops-2021-07-30> ;
                                    rdfs:label "Ahtanum™"@en ;
                                    <http://www.w3.org/2004/02/skos/core#definition> "Ahtanum™ a été élevé par C. E. Zimmermann et est une marque déposée de Yakima Chief Ranches LLC en 2017. Il est souvent décrit comme ayant un arôme floral, terreux et pamplemousse. Ahtanum est connu pour être résistant au mildiou et au Peronospora avec des cônes petits et compacts."@fr ,
                                                                                     "Ahtanum™ was bred by C. E. Zimmermann and is trademarked by Yakima Chief Ranches LLC in 2017. It is often secribed as having a floral, earthy and grapfruity aroma. Ahtanum is known to be resistant to downy mildew and Peronospora with small and compact cones."@en ;
                                    <http://xmlns.com/foaf/0.1/name> "Ahtanum™" ;
                                    <https://rdf.ag/o/hops#alphaAcidsContent> "4-6.3" ;
                                    <https://rdf.ag/o/hops#betaAcidsContent> "5-6.5" ;
                                    <https://rdf.ag/o/hops#perceivedAroma> "Earthy, Floral, Grapefruit"@en ,
                                                                           "Floral, Pamplemousse, Terreux"@fr ;
                                    <https://rdf.ag/o/hops#totalOilContent> "0.8-1.2" .


###  https://rdf.ag/o/hops#HopsAmarillo
<https://rdf.ag/o/hops#HopsAmarillo> rdf:type owl:Class ;
                                     rdfs:subClassOf <https://rdf.ag/o/hops#Hops> ;
                                     <http://rdfs.org/ns/void#inDataset> <https://rdf.ag/o/hops#datasetdefinition> ;
                                     rdfs:isDefinedBy <https://rdf.ag/o/hops-2021-07-30> ;
                                     rdfs:label "Amarillo®"@en ;
                                     <http://www.w3.org/2004/02/skos/core#definition> "Amarillo® est une variété déposée de Virgil Gamache Farms, Inc. Il est souvent décrit comme ayant un arôme de orange, citron, de pamplemousse, de thé noir, de pêche, de melon et d'abricot. Il est également connu pour avoir une teneur élevée en acide alpha, des cônes petits et compacts et une sotrabilité élevée."@fr ,
                                                                                      "Amarillo® is a trademarked variety of Virgil Gamache Farms, Inc. It is often described as having an aroma of orange, lemon, grapefruit, black tea, peach, melon and apricot. It is also known for having a high alpha acid content, small and compact cones, and high sotrability."@en ;
                                     <http://xmlns.com/foaf/0.1/name> "Amarillo® VGXP01" ;
                                     <https://rdf.ag/o/hops#alphaAcidsContent> "8-11" ;
                                     <https://rdf.ag/o/hops#betaAcidsContent> "6-7" ;
                                     <https://rdf.ag/o/hops#perceivedAroma> "Abricot, Citron, Melon, Orange, Pamplemousse, Pêche, Thé Noir"@fr ,
                                                                            "Apricot, Black Tea, Grapefruit, Lemon, Melon, Orange, Peach"@en ;
                                     <https://rdf.ag/o/hops#totalOilContent> "1.5-1.9" .


###  https://rdf.ag/o/hops#HopsApollo
<https://rdf.ag/o/hops#HopsApollo> rdf:type owl:Class ;
                                   rdfs:subClassOf <https://rdf.ag/o/hops#Hops> ;
                                   <http://rdfs.org/ns/void#inDataset> <https://rdf.ag/o/hops#datasetdefinition> ;
                                   rdfs:isDefinedBy <https://rdf.ag/o/hops-2021-07-30> ;
                                   rdfs:label "Apollo™"@en ;
                                   <http://www.w3.org/2004/02/skos/core#definition> "Apollo ™ a été développé par Hopsteiner et breveté en 2009. Il est dérivé de Zeus, Galena et Nugget, et a été élevé pour ses niveaux élevés d'acide alpha, sa capacité de stockage et ses faibles niveaux de cohumulone."@fr ,
                                                                                    "Apollo™ was developed by Hopsteiner and patented in 2009. It is derived from Zeus, Galena and Nugget, and was bred for its high alpha acid levels, storability and low cohumulone levels."@en ;
                                   <http://xmlns.com/foaf/0.1/name> "Apollo™" ;
                                   <https://rdf.ag/o/hops#alphaAcidsContent> "15-20" ;
                                   <https://rdf.ag/o/hops#betaAcidsContent> "5.5-8" ;
                                   <https://rdf.ag/o/hops#perceivedAroma> "Herbal, Grapefruit, Resinous"@en ,
                                                                          "Herbal, Pamplemousse, Résineux"@fr ;
                                   <https://rdf.ag/o/hops#totalOilContent> "1.5-2.5" .


###  https://rdf.ag/o/hops#HopsAquila
<https://rdf.ag/o/hops#HopsAquila> rdf:type owl:Class ;
                                   rdfs:subClassOf <https://rdf.ag/o/hops#Hops> ;
                                   <http://rdfs.org/ns/void#inDataset> <https://rdf.ag/o/hops#datasetdefinition> ;
                                   rdfs:comment "As of 1996, this hop cultivar is no longer being sold commercially due to its high cohumulone content."@en ,
                                                "Depuis 1996, ce cultivar de houblon n'est plus commercialisé en raison de sa forte teneur en cohumulone."@fr ;
                                   rdfs:isDefinedBy <https://rdf.ag/o/hops-2021-07-30> ;
                                   rdfs:label "Aquila"@en ;
                                   <http://www.w3.org/2004/02/skos/core#definition> "Aquila is a US aromatic hop that was developed by in 1970 by Dr. Robert R. Romanko at Parma, Idaho and was released in 1994."@en ,
                                                                                    "L'Aquila est un houblon aromatique américain développé en 1970 par le Dr Robert R. Romanko à Parma, Idaho et sorti en 1994."@fr ;
                                   <http://xmlns.com/foaf/0.1/name> "Aquila" ;
                                   <https://rdf.ag/o/hops#alphaAcidsContent> "6.7-8.9" ;
                                   <https://rdf.ag/o/hops#betaAcidsContent> "4.1-4.9" ;
                                   <https://rdf.ag/o/hops#totalOilContent> "1.45" .


###  https://rdf.ag/o/hops#HopsAramis
<https://rdf.ag/o/hops#HopsAramis> rdf:type owl:Class ;
                                   rdfs:subClassOf <https://rdf.ag/o/hops#Hops> ;
                                   <http://rdfs.org/ns/void#inDataset> <https://rdf.ag/o/hops#datasetdefinition> ;
                                   rdfs:isDefinedBy <https://rdf.ag/o/hops-2021-07-30> ;
                                   rdfs:label "Aramis"@en ;
                                   <http://www.w3.org/2004/02/skos/core#definition> "Aramis est un houblon français qui a été élevé en 2002 à partir d'un croisement entre Strisselspalt et Whitbread Golding par le programme de sélection du Comptoir Agricole."@fr ,
                                                                                    "Aramis is a French hop that was bred in 2002 from a cross between Strisselspalt and Whitbread Golding by the Comptoir Agricole breeding program."@en ;
                                   <http://xmlns.com/foaf/0.1/name> "Aramis" ;
                                   <https://rdf.ag/o/hops#alphaAcidsContent> "7.9-8.3" ;
                                   <https://rdf.ag/o/hops#betaAcidsContent> "3.8-4.5" ;
                                   <https://rdf.ag/o/hops#perceivedAroma> "Agrumes, Épices, Herbal, Sucré"@fr ,
                                                                          "Citrus, Herbal, Spice, Sweet"@en ;
                                   <https://rdf.ag/o/hops#totalOilContent> "1.2-1.6" .


###  https://rdf.ag/o/hops#HopsBanner
<https://rdf.ag/o/hops#HopsBanner> rdf:type owl:Class ;
                                   rdfs:subClassOf <https://rdf.ag/o/hops#Hops> ;
                                   rdfs:comment "Due to severe mildew problems, this hop has been abandoned from further research."@en ,
                                                "En raison de graves problèmes de moisissure, ce houblon a été abandonné des recherches ultérieures."@fr ;
                                   rdfs:label "Banner"@en ;
                                   <http://www.w3.org/2004/02/skos/core#definition> "Banner est un descendant de Brewer's Gold par pollinisation libre pour sa teneur élevée en acide alpha dans les années 1970 et sorti en 1996."@fr ,
                                                                                    "Banner is descendant of Brewer's Gold through open pollination for its high alpha acid content in the 1970s and released in 1996."@en ;
                                   <http://xmlns.com/foaf/0.1/isPrimaryTopicOf> <https://rdf.ag/o/hops#1996.0011183X003600050070x> ;
                                   <http://xmlns.com/foaf/0.1/name> "Banner" ;
                                   <https://rdf.ag/o/hops#alphaAcidsContent> "8.4-13" ;
                                   <https://rdf.ag/o/hops#betaAcidsContent> "5.3-8" ;
                                   <https://rdf.ag/o/hops#totalOilContent> "2.17" .


###  https://rdf.ag/o/hops#HopsBelma
<https://rdf.ag/o/hops#HopsBelma> rdf:type owl:Class ;
                                  rdfs:subClassOf <https://rdf.ag/o/hops#Hops> ;
                                  <http://rdfs.org/ns/void#inDataset> <https://rdf.ag/o/hops#datasetdefinition> ;
                                  rdfs:isDefinedBy <https://rdf.ag/o/hops-2021-07-30> ;
                                  rdfs:label "Belma®"@en ;
                                  <http://www.w3.org/2004/02/skos/core#definition> "Belma® est un houblon à double usage qui a été récemment lancé en 2012 par Puterbaugh Farms, Hops Direct, LLC. Il est connu pour son arôme fruité."@fr ,
                                                                                   "Belma® is a dual-purpose hop that was recently released in 2012 by Puterbaugh Farms, Hops Direct, LLC in Washington, US. It is known for its fruity aroma."@en ;
                                  <http://xmlns.com/foaf/0.1/name> "Belma®" ;
                                  <https://rdf.ag/o/hops#alphaAcidsContent> "8.5-12.1" ;
                                  <https://rdf.ag/o/hops#betaAcidsContent> "4-8" ;
                                  <https://rdf.ag/o/hops#perceivedAroma> "Ananas, Floral, Fraise, Melon, Pamplemousse, Orange"@fr ,
                                                                         "Floral, Grapefruit, Melon, Orange, Pineapple, Strawberry"@en ;
                                  <https://rdf.ag/o/hops#totalOilContent> "1-2.5" .


###  https://rdf.ag/o/hops#HopsBobek
<https://rdf.ag/o/hops#HopsBobek> rdf:type owl:Class ;
                                  rdfs:subClassOf <https://rdf.ag/o/hops#Hops> ;
                                  <http://rdfs.org/ns/void#inDataset> <https://rdf.ag/o/hops#datasetdefinition> ;
                                  rdfs:isDefinedBy <https://rdf.ag/o/hops-2021-07-30> ;
                                  rdfs:label "Bobek"@en ,
                                             "Styrian Bobek"@en ,
                                             "Styrian Golding B"@en ;
                                  <http://www.w3.org/2004/02/skos/core#definition> "Belma® est un houblon à double usage qui a été récemment lancé en 2012 par Puterbaugh Farms, Hops Direct, LLC. Il est connu pour son arôme fruité."@fr ,
                                                                                   "Bobek was bred in Slovenia from a cross between Northern Brewer and a Slovenian male to produce an aromatic hop with high alpha acid content."@en ;
                                  <http://xmlns.com/foaf/0.1/name> "Bobek" ;
                                  <https://rdf.ag/o/hops#alphaAcidsContent> "3.2-9.3" ;
                                  <https://rdf.ag/o/hops#betaAcidsContent> "4-6.6" ;
                                  <https://rdf.ag/o/hops#perceivedAroma> "Citron, Épicé, Floral, Pin"@fr ,
                                                                         "Lemon, Floral, Pine, Spicy"@en ;
                                  <https://rdf.ag/o/hops#totalOilContent> "0.7-4" .


###  https://rdf.ag/o/hops#HopsBramlingCross
<https://rdf.ag/o/hops#HopsBramlingCross> rdf:type owl:Class ;
                                          rdfs:subClassOf <https://rdf.ag/o/hops#Hops> ;
                                          <http://rdfs.org/ns/void#inDataset> <https://rdf.ag/o/hops#datasetdefinition> ;
                                          rdfs:isDefinedBy <https://rdf.ag/o/hops-2021-07-30> ;
                                          rdfs:label "Bramling Cross"@en ;
                                          <http://www.w3.org/2004/02/skos/core#definition> "Brambling Cross est une variété principalement utilisée au Royaume-Uni pour les bières conditionnées en fût. C'est un cors entre Golding et un houblon canadien sauvage et a été récolté pour la première fois au Wye College en 1927. Cette variété est connue pour son arôme de citron, de mûres, de prunes, et de cassis."@fr ,
                                                                                           "Brambling Cross is a variety mostly used in the UK for cask-conditioned beers. It is a cross between Golding and a wild Canadian hop and was first harvested at Wye College in 1927. This variety is known for its aroma of lemon, blackberries, plums, and blackcurrant."@en ;
                                          <http://xmlns.com/foaf/0.1/name> "Bramling Cross" ;
                                          <https://rdf.ag/o/hops#alphaAcidsContent> "5-7" ;
                                          <https://rdf.ag/o/hops#betaAcidsContent> "3-4" ;
                                          <https://rdf.ag/o/hops#perceivedAroma> "Blackberry, Blackcurrent, Lemon, Plum"@en ,
                                                                                 "Cassis, Citron, Mûre, Prune"@fr ;
                                          <https://rdf.ag/o/hops#totalOilContent> "0.83" .


###  https://rdf.ag/o/hops#HopsBravo
<https://rdf.ag/o/hops#HopsBravo> rdf:type owl:Class ;
                                  rdfs:subClassOf <https://rdf.ag/o/hops#Hops> ;
                                  rdfs:label "Bravo"@en ;
                                  <http://www.w3.org/2004/02/skos/core#definition> "Bravo a été développé par Hopsteiner au Golden Gate Roza Hop Ranches à Prosser, Washington, États-Unis, breveté et publié en 2006 pour son profil alpha élevé."@fr ,
                                                                                   "Bravo was developed by Hopsteiner at Golden Gate Roza Hop Ranches in Prosser, Washington, US, patented and released in 2006 for its high alpha profile."@en ;
                                  <http://xmlns.com/foaf/0.1/name> "Bravo" ;
                                  <https://rdf.ag/o/hops#alphaAcidsContent> "14-17" ;
                                  <https://rdf.ag/o/hops#betaAcidsContent> "3-5" ;
                                  <https://rdf.ag/o/hops#perceivedAroma> "Earthy, Floral, Pine, Resinous, Spicy"@en ,
                                                                         "Épicé, Floral, Pin, Résineux, Terreux"@fr ;
                                  <https://rdf.ag/o/hops#totalOilContent> "1.6-2.4" .


###  https://rdf.ag/o/hops#HopsBrewersGold
<https://rdf.ag/o/hops#HopsBrewersGold> rdf:type owl:Class ;
                                        rdfs:subClassOf <https://rdf.ag/o/hops#Hops> ;
                                        <http://rdfs.org/ns/void#inDataset> <https://rdf.ag/o/hops#datasetdefinition> ;
                                        rdfs:isDefinedBy <https://rdf.ag/o/hops-2021-07-30> ;
                                        rdfs:label "Brewer's Gold"@en ;
                                        <http://www.w3.org/2004/02/skos/core#definition> "Brewer's Gold a été sélectionné de manière sélective par le professeur E.F. Salmon du Wye College en Angleterre en 1894. Depuis lors, ce houblon a été utilisé pour l'amertume et la production d'autres variétés de houblon très amer. En termes d'arôme, on dit qu'il a des notes de cassis et d'épices. L'or de Brewer a également de petits cônes compacts et est résistant à la flétrissure verticillienne et modérément résistant au mildiou."@fr ,
                                                                                         "Brewer's Gold was selectively bred by Professor E.F. Salmon of Wye College in England in 1894. Since then, this hop has been used for bittering and producing other high bitter hop varieties. In terms of aroma, it is said to have notes of blackcurrant, and spice. Brewer's Gold also has small, compact cones and is resistant to verticillium wilt and moderately resistant to downy mildew."@en ;
                                        <http://xmlns.com/foaf/0.1/name> "Brewer's Gold" ;
                                        <https://rdf.ag/o/hops#alphaAcidsContent> "9.2" ;
                                        <https://rdf.ag/o/hops#betaAcidsContent> "4.8" ;
                                        <https://rdf.ag/o/hops#perceivedAroma> "Blackcurrent, Spicy"@en ,
                                                                               "Cassis, Epicé"@fr ;
                                        <https://rdf.ag/o/hops#totalOilContent> "1.96" .


###  https://rdf.ag/o/hops#HopsBullion
<https://rdf.ag/o/hops#HopsBullion> rdf:type owl:Class ;
                                    rdfs:subClassOf <https://rdf.ag/o/hops#Hops> ;
                                    <http://rdfs.org/ns/void#inDataset> <https://rdf.ag/o/hops#datasetdefinition> ;
                                    rdfs:isDefinedBy <https://rdf.ag/o/hops-2021-07-30> ;
                                    rdfs:label "Bullion"@en ;
                                    <http://www.w3.org/2004/02/skos/core#definition> "Bullion est une variété créée pour la première fois en 1919 par le professeur E.S. Saumon d'un houblon canadien sauvage et d'un houblon anglais inconnu. Il est principalement cultivé aux États-Unis en petites quantités et est la sœur de Brewer's Gold. Il n'est pas autant utilisé en faveur d'autres variétés d'acide alpha supérieur et de la capacité de stockage et aussi parce qu'il est sensible à la plupart des virus. L'arôme de Bullion est connu pour avoir un arôme d'épices et de fruits noirs."@fr ,
                                                                                     "Bullion is variety first bred in 1919 by Professor E.S. Salmon from a wild Canadian hop and an unknown English hop. It is mostly grown in the US in small quantities and is the sister to Brewer's Gold. It is not used as much in favor of other higher alpha acid varieties and storability and also since it is susceptible to most viruses. Bullion's aroma is known for having an aroma of spices and dark fruits."@en ;
                                    <http://xmlns.com/foaf/0.1/name> "Bullion" ;
                                    <https://rdf.ag/o/hops#alphaAcidsContent> "10" ;
                                    <https://rdf.ag/o/hops#betaAcidsContent> "4.8" ;
                                    <https://rdf.ag/o/hops#perceivedAroma> "Dark Fruit, Spicy"@en ,
                                                                           "Fruits noirs, Épicé"@fr ;
                                    <https://rdf.ag/o/hops#totalOilContent> "1.65" .


###  https://rdf.ag/o/hops#HopsCalypso
<https://rdf.ag/o/hops#HopsCalypso> rdf:type owl:Class ;
                                    rdfs:subClassOf <https://rdf.ag/o/hops#Hops> ;
                                    <http://rdfs.org/ns/void#inDataset> <https://rdf.ag/o/hops#datasetdefinition> ;
                                    rdfs:isDefinedBy <https://rdf.ag/o/hops-2021-07-30> ;
                                    rdfs:label "Calypso™"@en ;
                                    <http://www.w3.org/2004/02/skos/core#definition> "Calypso™ est un houblon breveté en 2014 par Hopsteiner, plus précisément Roger D. Jeske et Paul D. Matthews à Yakima, Washington, États-Unis. Ce houblon a été sélectionné pour ses qualités aromatiques, mais il a également une teneur élevée en acide alpha."@fr ,
                                                                                     "Calypso™ is a hop patented in 2014 by Hopsteiner, specifically Roger D. Jeske and Paul D. Matthews at Yakima, Washington, US. This hop was bred for its aromatic qualities, but it also has a high alpha acid content as well."@en ;
                                    <http://xmlns.com/foaf/0.1/name> "Calypso™" ;
                                    <https://rdf.ag/o/hops#alphaAcidsContent> "12-14" ;
                                    <https://rdf.ag/o/hops#betaAcidsContent> "5-6" ;
                                    <https://rdf.ag/o/hops#perceivedAroma> "Apple, Lime, Pear, Stone Fruit"@en ,
                                                                           "Citron vert, Fruit à noyau, Poire, Pomme"@fr .


###  https://rdf.ag/o/hops#HopsCanterburyGolding
<https://rdf.ag/o/hops#HopsCanterburyGolding> rdf:type owl:Class ;
                                              owl:equivalentClass <https://rdf.ag/o/hops#HopsEastKentGolding> ;
                                              rdfs:subClassOf <https://rdf.ag/o/hops#HopsGolding> ;
                                              <http://rdfs.org/ns/void#inDataset> <https://rdf.ag/o/hops#datasetdefinition> ;
                                              rdfs:isDefinedBy <https://rdf.ag/o/hops-2021-07-30> ;
                                              rdfs:label "Canterbury Golding"@en ;
                                              <http://www.w3.org/2004/02/skos/core#definition> "Canterbury Golding est identique à East Kent Golding."@fr ,
                                                                                               "Canterbury Golding is identical to East Kent Golding."@en ;
                                              <http://xmlns.com/foaf/0.1/name> "Canterbury Golding" .


###  https://rdf.ag/o/hops#HopsCascade
<https://rdf.ag/o/hops#HopsCascade> rdf:type owl:Class ;
                                    rdfs:subClassOf <https://rdf.ag/o/hops#Hops> ;
                                    <http://rdfs.org/ns/void#inDataset> <https://rdf.ag/o/hops#datasetdefinition> ;
                                    rdfs:isDefinedBy <https://rdf.ag/o/hops-2021-07-30> ;
                                    rdfs:label "Cascade"@en ;
                                    <http://www.w3.org/2004/02/skos/core#definition> """Cascade est l'une des variétés de houblon les plus cultivées aux États-Unis, du nom de la chaîne de montagnes Cascades, avec un profil aromatique d'agrumes, de pamplemousse, de fleurs et de notes épicées. Les caractéristiques notables sont de longs cônes vert foncé et une faible teneur en acide alpha par rapport aux autres houblons.
      
      Cascade a été relâchée pour la culture en 1972 par un programme de sélection de l'USDA à Corvallis, Oregon et c'est un descendant de Fuggle."""@fr ,
                                                                                     """Cascade is one of the most widely cultivated US hop variety, named after the Cascades Mountain range, with an aroma profile of citrus, grapefruit, floral and spicy notes. Notable characteristics are long, dark green cones and a low alpha acid content relative to other hops.
      
      Cascade was released for cultivation in 1972 by a USDA breeding program in Corvallis, Oregon and it is a descendant of Fuggle."""@en ;
                                    <http://xmlns.com/foaf/0.1/name> "Cascade" ;
                                    <https://rdf.ag/o/hops#alphaAcidsContent> "6.2" ;
                                    <https://rdf.ag/o/hops#betaAcidsContent> "5.0" ;
                                    <https://rdf.ag/o/hops#totalOilContent> "1.27" .


###  https://rdf.ag/o/hops#HopsCascadeUS
<https://rdf.ag/o/hops#HopsCascadeUS> rdf:type owl:Class ;
                                      rdfs:subClassOf <https://rdf.ag/o/hops#HopsCascade> ;
                                      <http://rdfs.org/ns/void#inDataset> <https://rdf.ag/o/hops#datasetdefinition> ;
                                      rdfs:isDefinedBy <https://rdf.ag/o/hops-2021-07-30> ;
                                      rdfs:label "Cascade (US)"@en ,
                                                 "Cascade (US)"@fr ;
                                      <http://www.w3.org/2004/02/skos/core#definition> "Cascade (US) est génétiquement identique à Cascade, cependant Cascade (US) fait référence au terroir cultivé aux États-Unis (ou en Amérique du Nord)."@fr ,
                                                                                       "Cascade (US) is genetically identical to Cascade, however Cascade (US) refers to the terroir from being grown in the US (or North America)."@en ;
                                      <http://xmlns.com/foaf/0.1/name> "Cascade (US)" ;
                                      <https://rdf.ag/o/hops#alphaAcidsContent> "4.5–7.0" ;
                                      <https://rdf.ag/o/hops#betaAcidsContent> "4.8–7.0" ;
                                      <https://rdf.ag/o/hops#perceivedAroma> "Agrumes, Épicé, Floral, Fruité, Pamplemousse"@fr ,
                                                                             "Citrus, Floral, Fruity, Grapefruit, Spicy"@en ;
                                      <https://rdf.ag/o/hops#totalOilContent> "0.7-1.4" .


###  https://rdf.ag/o/hops#HopsCashmere
<https://rdf.ag/o/hops#HopsCashmere> rdf:type owl:Class ;
                                     rdfs:subClassOf <https://rdf.ag/o/hops#Hops> ;
                                     <http://rdfs.org/ns/void#inDataset> <https://rdf.ag/o/hops#datasetdefinition> ;
                                     rdfs:isDefinedBy <https://rdf.ag/o/hops-2021-07-30> ;
                                     rdfs:label "Cashmere"@en ,
                                                "Cashmere"@fr ;
                                     <http://www.w3.org/2004/02/skos/core#definition> """Cashmere est le résultat du croisement entre Cascade et Northern Brewer, publié par l'Université de l'État de Washington en 2013.
      
      On dit que c'est un bon houblon à double usage pour l'amertume et l'arôme."""@fr ,
                                                                                      """Cashmere is a result of the cross between Cascade and Northern Brewer, released by Washington State University in 2013.
      
      It is said to be a good dual-purpose hop for bittering and aroma."""@en ;
                                     <http://xmlns.com/foaf/0.1/name> "Cashmere" ;
                                     <https://rdf.ag/o/hops#alphaAcidsContent> "7.7–9.1" ;
                                     <https://rdf.ag/o/hops#betaAcidsContent> "6.4–7.1" ;
                                     <https://rdf.ag/o/hops#perceivedAroma> "Ananas, Épicé, Citron, Fruitée, Noix de Coco, Melon, Zeste de Lime"@fr ,
                                                                            "Coconut, Fruity, Lemon, Lime Peel, Melon, Pineapple, Spicy"@en ;
                                     <https://rdf.ag/o/hops#totalOilContent> "1.2-1.4" .


###  https://rdf.ag/o/hops#HopsCeleia
<https://rdf.ag/o/hops#HopsCeleia> rdf:type owl:Class ;
                                   rdfs:subClassOf <https://rdf.ag/o/hops#Hops> ;
                                   <http://rdfs.org/ns/void#inDataset> <https://rdf.ag/o/hops#datasetdefinition> ;
                                   rdfs:isDefinedBy <https://rdf.ag/o/hops-2021-07-30> ;
                                   rdfs:label "Celeia"@en ;
                                   <http://www.w3.org/2004/02/skos/core#definition> "Celeia est une descendante de Styrian Golding et Aurora et est un houblon triploïde. Il est principalement utilisé comme houblon aromatique."@fr ,
                                                                                    "Celeia is a descendant of Styrian Golding and Aurora and is a triploid hop. It is mostly used as an aromatic hop."@en ;
                                   <http://xmlns.com/foaf/0.1/name> "Celeia" ;
                                   <https://rdf.ag/o/hops#alphaAcidsContent> "5-6" ;
                                   <https://rdf.ag/o/hops#betaAcidsContent> "3-4" ;
                                   <https://rdf.ag/o/hops#perceivedAroma> "Agrumes, Floral"@fr ,
                                                                          "Citrus, Floral"@en ;
                                   <https://rdf.ag/o/hops#totalOilContent> "1.31" .


###  https://rdf.ag/o/hops#HopsCentennial
<https://rdf.ag/o/hops#HopsCentennial> rdf:type owl:Class ;
                                       rdfs:subClassOf <https://rdf.ag/o/hops#Hops> ;
                                       <http://rdfs.org/ns/void#inDataset> <https://rdf.ag/o/hops#datasetdefinition> ;
                                       rdfs:isDefinedBy <https://rdf.ag/o/hops-2021-07-30> ;
                                       rdfs:label "Centennial"@en ,
                                                  "Centennial"@fr ,
                                                  "Super Cascade"@en ;
                                       <http://www.w3.org/2004/02/skos/core#definition> """Parfois appelé «Super Cascade», ce houblon est connu comme un houblon à double usage pour son arôme et son effet amer dans les bières. Sa popularité ne cesse de croître parmi les brasseurs artisanaux.
      
      Anciennement connu sous le nom de Hop W415-90, il a été hybride en 1974 au Centre de recherche et de vulgarisation en agriculture irriguée de Brewer's Gold, Fuggle et East Kent Golding. Ce houblon a été rebaptisé «Centennial» pour le 100e anniversaire de l'État de Washington en 1989. Il a été cultivé à titre expérimental pendant quelques années, c'est pourquoi l'USDA a attribué son numéro d'accession 1987, lorsqu'il a reçu le nom de Centennial en 1989."""@fr ,
                                                                                        """Sometimes referred to as 'Super Cascade', this hop is known as a dual-purpose hop for its aroma and bittering affect in brews. Its popularity has been increasing among craft brewers.
         
         Formerly known as Hop W415-90, that was hybridized in 1974 at the Irrigated Agriculture Research and Extension Center from Brewer's Gold, Fuggle and East Kent Golding. This hop was renamed 'Centennial' for the 100th anniversary of Washington's statehood in 1989. It was grown experimentally for a few years, which is why the USDA assigned its accession number 1987, when it got the name Centennial in 1989."""@en ;
                                       <http://xmlns.com/foaf/0.1/isPrimaryTopicOf> <https://rdf.ag/o/hops#doi:10.2135/cropsci1986.0011183X002600010049x> ;
                                       <http://xmlns.com/foaf/0.1/name> "Centennial" ;
                                       <https://rdf.ag/o/hops#alphaAcidsContent> "9.5–11.5" ;
                                       <https://rdf.ag/o/hops#betaAcidsContent> "3.5–4.5" ;
                                       <https://rdf.ag/o/hops#perceivedAroma> "Agrumes, Floral"@fr ,
                                                                              "Citrus, Floral"@en ;
                                       <https://rdf.ag/o/hops#totalOilContent> "1.5-2.5" .


###  https://rdf.ag/o/hops#HopsChallenger
<https://rdf.ag/o/hops#HopsChallenger> rdf:type owl:Class ;
                                       rdfs:subClassOf <https://rdf.ag/o/hops#Hops> ;
                                       <http://rdfs.org/ns/void#inDataset> <https://rdf.ag/o/hops#datasetdefinition> ;
                                       rdfs:isDefinedBy <https://rdf.ag/o/hops-2021-07-30> ;
                                       rdfs:label "Challenger"@en ,
                                                  "Wye Challenger"@en ;
                                       <http://www.w3.org/2004/02/skos/core#definition> "Cette variété de houblon a été lancée en 1972 par le Wye College et est issue d'un croisement entre Northern Brewer et Zattler. C'était un houblon très populaire au Royaume-Uni des années 1980 aux années 1990."@fr ,
                                                                                        "This hop variety was released in 1972 from Wye College and is derived from a cross between Northern Brewer and Zattler. It was a very popular hop in the UK from the 1980s to 1990s."@en ;
                                       <http://xmlns.com/foaf/0.1/name> "Challenger" ;
                                       <https://rdf.ag/o/hops#alphaAcidsContent> "6.5-9" ;
                                       <https://rdf.ag/o/hops#betaAcidsContent> "3.2-4.5" ;
                                       <https://rdf.ag/o/hops#perceivedAroma> "Cedar, Green Tea, Spicy"@en ,
                                                                              "Cèdre, Épicé, Thé Vert"@en ;
                                       <https://rdf.ag/o/hops#totalOilContent> "1-1.7" .


###  https://rdf.ag/o/hops#HopsChinook
<https://rdf.ag/o/hops#HopsChinook> rdf:type owl:Class ;
                                    rdfs:subClassOf <https://rdf.ag/o/hops#Hops> ;
                                    <http://rdfs.org/ns/void#inDataset> <https://rdf.ag/o/hops#datasetdefinition> ;
                                    rdfs:isDefinedBy <https://rdf.ag/o/hops-2021-07-30> ;
                                    rdfs:label "Chinook"@en ;
                                    <http://www.w3.org/2004/02/skos/core#definition> """Chinook, anciennement W415-90, est un houblon issu du croisement entre Petham Golding x Brewer's Gold - Utah 526-4 68052 x 63012M grâce à un programme de sélection USDA dans l'État de Washington en 1985.
      
         Il a gagné en popularité parmi les brasseurs artisanaux, mais il est également très respecté parmi les grandes brasseries pour sa teneur élevée en acide alpha et ses notes d'agrumes et de pin."""@fr ,
                                                                                     """Chinook, formerly W415-90, is a hop that came about from the cross between Petham Golding x Brewer's Gold - Utah 526-4 68052 x 63012M through a USDA breeding program in Washington state in 1985.
      
         It has grown in popularity among craft brewers but is also highly respected among larger breweries for its high alpha acid content and notes of citrus and pine."""@en ;
                                    <http://xmlns.com/foaf/0.1/isPrimaryTopicOf> <https://rdf.ag/o/hops#cropsci1986.0011183X002600010049x> ;
                                    <http://xmlns.com/foaf/0.1/name> "Chinook" ;
                                    <https://rdf.ag/o/hops#alphaAcidsContent> "12.0–14.0" ;
                                    <https://rdf.ag/o/hops#betaAcidsContent> "3.0–4.0" ;
                                    <https://rdf.ag/o/hops#perceivedAroma> "Grapefruit, Pine, Spicy"@en ,
                                                                           "Épicé, Pamplemousse, Pin"@fr ;
                                    <https://rdf.ag/o/hops#totalOilContent> "0.7-1.4" .


###  https://rdf.ag/o/hops#HopsCitra
<https://rdf.ag/o/hops#HopsCitra> rdf:type owl:Class ;
                                  rdfs:subClassOf <https://rdf.ag/o/hops#Hops> ;
                                  <http://rdfs.org/ns/void#inDataset> <https://rdf.ag/o/hops#datasetdefinition> ;
                                  rdfs:isDefinedBy <https://rdf.ag/o/hops-2021-07-30> ;
                                  rdfs:label "Citra®"@en ;
                                  <http://www.w3.org/2004/02/skos/core#definition> "Citra® a été créé dans une coentreprise de John I. Haas, Inc. et Select Botanicals Group et sorti en 2008. Gene Probasco est crédité d'avoir élevé Citra® pour la première fois en 1990. Il a une lignée complexe impliquant Brewer's Gold, Hallertau Mittelfrüh, East Kent Golding et Tettnanger. Citra® est connu pour avoir un arôme de fruits tropicaux, d'agrumes et d'amer."@fr ,
                                                                                   "Citra® was created in a joint venture of John I. Haas, Inc. and Select Botanicals Group and released in 2008. Gene Probasco is credited with having first bred Citra® in 1990. It has a complex lineage involving Brewer’s Gold, Hallertau Mittelfrüh, East Kent Golding, and Tettnanger. Citra® is known for having a tropical fruit aroma, citrus-y and bitter aroma."@en ;
                                  <http://xmlns.com/foaf/0.1/name> "Citra®" ;
                                  <https://rdf.ag/o/hops#alphaAcidsContent> "10-15" ;
                                  <https://rdf.ag/o/hops#betaAcidsContent> "3–4.5" ;
                                  <https://rdf.ag/o/hops#perceivedAroma> "Amer, Agrumes, Citron Vert, Fruits Tropicaux, Pamplemousse"@fr ,
                                                                         "Bitter, Citrus, Grapefruit, Lime, Tropical Fruit"@en ;
                                  <https://rdf.ag/o/hops#totalOilContent> "1.5-3" .


###  https://rdf.ag/o/hops#HopsCluster
<https://rdf.ag/o/hops#HopsCluster> rdf:type owl:Class ;
                                    rdfs:subClassOf <https://rdf.ag/o/hops#Hops> ;
                                    <http://rdfs.org/ns/void#inDataset> <https://rdf.ag/o/hops#datasetdefinition> ;
                                    rdfs:isDefinedBy <https://rdf.ag/o/hops-2021-07-30> ;
                                    rdfs:label "Cluster"@en ;
                                    <http://www.w3.org/2004/02/skos/core#definition> "Cluster hops are a grouping of American hops that have mutated from interactions with local varieties. The origins of these hops are vague at best as these hops are some of the oldest grown hops in the United States. Cluster hops can be separated into two groups: Early Cluster and Late Cluster, which references the time of maturity."@en ,
                                                                                     "Le houblon Cluster est un groupe de houblon américain qui a muté à la suite d'interactions avec des variétés locales. Les origines de ces houblons sont au mieux vagues, car ces houblons sont parmi les plus anciens houblons cultivés aux États-Unis. Les houblons Cluster peuvent être séparés en deux groupes: Early Cluster et Late Cluster, qui font référence au moment de maturité."@fr ;
                                    <http://xmlns.com/foaf/0.1/name> "Cluster" ;
                                    <https://rdf.ag/o/hops#alphaAcidsContent> "5.5-9" ;
                                    <https://rdf.ag/o/hops#betaAcidsContent> "4-6" ;
                                    <https://rdf.ag/o/hops#perceivedAroma> "Floral, Pin"@fr ,
                                                                           "Floral, Pine"@en ;
                                    <https://rdf.ag/o/hops#totalOilContent> "0.4-0.8" .


###  https://rdf.ag/o/hops#HopsCluster_AUS
<https://rdf.ag/o/hops#HopsCluster_AUS> rdf:type owl:Class ;
                                        rdfs:subClassOf <https://rdf.ag/o/hops#HopsCluster> ;
                                        <http://rdfs.org/ns/void#inDataset> <https://rdf.ag/o/hops#datasetdefinition> ;
                                        rdfs:isDefinedBy <https://rdf.ag/o/hops-2021-07-30> ;
                                        rdfs:label "Austrailian Cluster"@en ,
                                                   "Cluster (AUS)"@en ;
                                        <http://www.w3.org/2004/02/skos/core#definition> "Cluster (AUS) hops are Cluster hops (originally from the US) that are grown in Australia and therefore have slightly different properties due to the difference in terroir."@en ,
                                                                                         "Les houblons Cluster (AUS) sont des houblons Cluster (originaires des États-Unis) qui sont cultivés en Australie et ont donc des propriétés légèrement différentes en raison de la différence de terroir."@fr ;
                                        <http://xmlns.com/foaf/0.1/name> "Cluster (AUS)" ;
                                        <https://rdf.ag/o/hops#alphaAcidsContent> "5.5-8.5" ;
                                        <https://rdf.ag/o/hops#betaAcidsContent> "4.5-5.5" ;
                                        <https://rdf.ag/o/hops#perceivedAroma> "Herbal, Resinous"@en ,
                                                                               "Herbal, Résineux"@fr ;
                                        <https://rdf.ag/o/hops#totalOilContent> "0.4-1" .


###  https://rdf.ag/o/hops#HopsCluster_California
<https://rdf.ag/o/hops#HopsCluster_California> rdf:type owl:Class ;
                                               rdfs:subClassOf <https://rdf.ag/o/hops#HopsCluster> ;
                                               <http://rdfs.org/ns/void#inDataset> <https://rdf.ag/o/hops#datasetdefinition> ;
                                               rdfs:isDefinedBy <https://rdf.ag/o/hops-2021-07-30> ;
                                               rdfs:label "California Cluster"@en ;
                                               <http://www.w3.org/2004/02/skos/core#definition> "La lignée de California Cluster n'est pas tout à fait claire, mais la ferme à houblon, Hops-Meister, de Clearlake, en Californie, a déposé deux variantes de Cluster de Californie : Ivanhoe et Gargoyle."@fr ,
                                                                                                "The lineage of California Cluster is not entirely clear, however the hop farm, Hops-Meister, from Clearlake, California have trademarked two variations of Cluster from California: Ivanhoe and Gargoyle."@en ;
                                               <http://xmlns.com/foaf/0.1/name> "California Cluster" ;
                                               <https://rdf.ag/o/hops#alphaAcidsContent> "5.5-8.5" ;
                                               <https://rdf.ag/o/hops#betaAcidsContent> "4.5-5.5" ;
                                               <https://rdf.ag/o/hops#perceivedAroma> "Agrumes, Mangue"@fr ,
                                                                                      "Citrus, Mango"@en .


###  https://rdf.ag/o/hops#HopsCluster_EarlyCluster
<https://rdf.ag/o/hops#HopsCluster_EarlyCluster> rdf:type owl:Class ;
                                                 rdfs:subClassOf <https://rdf.ag/o/hops#HopsCluster> ;
                                                 <http://rdfs.org/ns/void#inDataset> <https://rdf.ag/o/hops#datasetdefinition> ;
                                                 rdfs:isDefinedBy <https://rdf.ag/o/hops-2021-07-30> ;
                                                 rdfs:label "Early Cluster"@en ;
                                                 <http://www.w3.org/2004/02/skos/core#definition> "Ce type de houblon mûrit plus tôt dans la saison que les autres variétés de houblon Cluster."@fr ,
                                                                                                  "This type of hop matures earlier in the season than other varieties of Cluster hops."@en ;
                                                 <http://xmlns.com/foaf/0.1/name> "Early Cluster" ;
                                                 <https://rdf.ag/o/hops#alphaAcidsContent> "6.4" ;
                                                 <https://rdf.ag/o/hops#betaAcidsContent> "4.4" ;
                                                 <https://rdf.ag/o/hops#totalOilContent> "0.79" .


###  https://rdf.ag/o/hops#HopsCluster_Gargoyle
<https://rdf.ag/o/hops#HopsCluster_Gargoyle> rdf:type owl:Class ;
                                             rdfs:subClassOf <https://rdf.ag/o/hops#HopsCluster_California> ;
                                             <http://rdfs.org/ns/void#inDataset> <https://rdf.ag/o/hops#datasetdefinition> ;
                                             rdfs:isDefinedBy <https://rdf.ag/o/hops-2021-07-30> ;
                                             rdfs:label "Gargoyle"@en ;
                                             <http://www.w3.org/2004/02/skos/core#definition> "Semblable à Ivanhoe, le houblon Gargoyle est une variété de cluster qui a été déposée par la ferme de houblon californienne Hops-Meister. Cependant, contrairement à Ivanhoe, Gargoyle est connu pour avoir un arôme plus de mangue et d'agrumes."@fr ,
                                                                                              "Similar to Ivanhoe, Gargoyle hops is a variety of Cluster that has been trademarked by the Californian hop farm Hops-Meister. However, unlike Ivanhoe, Gargoyle is known for having a more mango and citrus aroma."@en ;
                                             <http://xmlns.com/foaf/0.1/name> "Gargoyle" ;
                                             <https://rdf.ag/o/hops#alphaAcidsContent> "7.5" ;
                                             <https://rdf.ag/o/hops#perceivedAroma> "Agrumes, Mangue"@fr ,
                                                                                    "Citrus, Mango"@en .


###  https://rdf.ag/o/hops#HopsCluster_Ivanhoe
<https://rdf.ag/o/hops#HopsCluster_Ivanhoe> rdf:type owl:Class ;
                                            rdfs:subClassOf <https://rdf.ag/o/hops#HopsCluster_California> ;
                                            <http://rdfs.org/ns/void#inDataset> <https://rdf.ag/o/hops#datasetdefinition> ;
                                            rdfs:isDefinedBy <https://rdf.ag/o/hops-2021-07-30> ;
                                            rdfs:label "Ivanhoe"@en ;
                                            <http://www.w3.org/2004/02/skos/core#definition> "Comme Gargoyle, Ivanhoe est une variété de Cluster qui a été déposée par la ferme de houblon californienne Hops-Meister. Cependant, contrairement à Gargoyle, Ivanhoe est connu pour avoir un arôme d'agrumes et de pin qui n'est pas différent de Cascade."@fr ,
                                                                                             "Like Gargoyle, Ivanhoe is a variety of Cluster that has been trademarked by the Californian hop farm Hops-Meister. However, unlike Gargoyle, Ivanhoe is known for having a citrus and pine aroma not dissimilar to Cascade."@en ;
                                            <http://xmlns.com/foaf/0.1/name> "Ivanhoe" ;
                                            <https://rdf.ag/o/hops#alphaAcidsContent> "7.3-8" ;
                                            <https://rdf.ag/o/hops#betaAcidsContent> "4.6" ;
                                            <https://rdf.ag/o/hops#perceivedAroma> "Agrumes, Pin"@fr ,
                                                                                   "Citrus, Pine"@en .


###  https://rdf.ag/o/hops#HopsCluster_L16
<https://rdf.ag/o/hops#HopsCluster_L16> rdf:type owl:Class ;
                                        rdfs:subClassOf <https://rdf.ag/o/hops#HopsCluster_Yakima> ;
                                        <http://rdfs.org/ns/void#inDataset> <https://rdf.ag/o/hops#datasetdefinition> ;
                                        rdfs:isDefinedBy <https://rdf.ag/o/hops-2021-07-30> ;
                                        rdfs:label "Late Cluster L16"@en ,
                                                   "Late Cluster selection L16"@en ;
                                        <http://www.w3.org/2004/02/skos/core#definition> "A selection of a Yakima hop plant from 1950."@en ,
                                                                                         "Ce type de houblon Cluster préfère le climat plus sec de la vallée de Yakima, dans l'État de Washington."@fr ;
                                        <http://xmlns.com/foaf/0.1/name> "Late Cluster L16" ;
                                        <https://rdf.ag/o/hops#alphaAcidsContent> "5.8" ;
                                        <https://rdf.ag/o/hops#betaAcidsContent> "4.2" ;
                                        <https://rdf.ag/o/hops#totalOilContent> "0.5" .


###  https://rdf.ag/o/hops#HopsCluster_Yakima
<https://rdf.ag/o/hops#HopsCluster_Yakima> rdf:type owl:Class ;
                                           rdfs:subClassOf <https://rdf.ag/o/hops#HopsCluster> ;
                                           <http://rdfs.org/ns/void#inDataset> <https://rdf.ag/o/hops#datasetdefinition> ;
                                           rdfs:isDefinedBy <https://rdf.ag/o/hops-2021-07-30> ;
                                           rdfs:label "Late Cluster L8"@en ,
                                                      "Yakima Cluster"@en ;
                                           <http://www.w3.org/2004/02/skos/core#definition> "Ce type de houblon Cluster préfère le climat plus sec de la vallée de Yakima, dans l'État de Washington."@fr ,
                                                                                            "This type of Cluster hop prefers the drier climate of Yakima Valley, Washington."@en ;
                                           <http://xmlns.com/foaf/0.1/name> "Yakima Cluster" ;
                                           <https://rdf.ag/o/hops#alphaAcidsContent> "4.4-9.8" ;
                                           <https://rdf.ag/o/hops#betaAcidsContent> "3-6.1" ;
                                           <https://rdf.ag/o/hops#totalOilContent> "0.24-0.90" .


###  https://rdf.ag/o/hops#HopsColumbia
<https://rdf.ag/o/hops#HopsColumbia> rdf:type owl:Class ;
                                     rdfs:subClassOf <https://rdf.ag/o/hops#Hops> ;
                                     <http://rdfs.org/ns/void#inDataset> <https://rdf.ag/o/hops#datasetdefinition> ;
                                     rdfs:isDefinedBy <https://rdf.ag/o/hops-2021-07-30> ;
                                     rdfs:label "Columbia"@en ;
                                     <http://www.w3.org/2004/02/skos/core#definition> "Columbia est un houblon qui était plus favorisé dans les années 1980 mais a ensuite été abandonné au profit de sa sœur triploïde, Willamette. Avec l'essor de la brasserie artisanale, Columbia a commencé à regagner sa popularité."@fr ,
                                                                                      "Columbia is a hop that was more favored in the 1980s but was then discontinued in favor of its triploid sister, Willamette. With the rise of craft brewing, Columbia has started to regain its popularity."@en ;
                                     <http://xmlns.com/foaf/0.1/isPrimaryTopicOf> <https://rdf.ag/o/hops#cropsci1976.0011183X00160005004> ;
                                     <http://xmlns.com/foaf/0.1/name> "Columbia" ;
                                     <https://rdf.ag/o/hops#alphaAcidsContent> "8.8" ;
                                     <https://rdf.ag/o/hops#betaAcidsContent> "4" ;
                                     <https://rdf.ag/o/hops#perceivedAroma> "Citron, Fruité, Terreux"@fr ,
                                                                            "Earthy, Lemon, Fruity"@en ;
                                     <https://rdf.ag/o/hops#totalOilContent> "1.21" .


###  https://rdf.ag/o/hops#HopsColumbus
<https://rdf.ag/o/hops#HopsColumbus> rdf:type owl:Class ;
                                     rdfs:subClassOf <https://rdf.ag/o/hops#Hops> ;
                                     <http://rdfs.org/ns/void#inDataset> <https://rdf.ag/o/hops#datasetdefinition> ;
                                     rdfs:isDefinedBy <https://rdf.ag/o/hops-2021-07-30> ;
                                     rdfs:label "Columbus"@en ;
                                     <http://www.w3.org/2004/02/skos/core#definition> "La lignée de Colombus n'est pas connue. Il est génétiquement identique à Tomahawk®, mais en raison d'un différend juridique entre Hopunion et Yakima Chief, les deux noms ont été enregistrés lorsque les deux parties ont tenté de breveter indépendamment la même variété. Columbus/Tomahawk® a été élevé pour sa teneur élevée en acide alpha et est souvent vendu avec Zeus en tant que CTZ."@fr ,
                                                                                      "The lineage of Columbus is not known. It is genetically identical to Tomahawk®, however due to a legal dispute between Hopunion and Yakima Chief both names were registered when the two parties tried to independently patent the same variety. Columbus/Tomahawk® was bred for its high alpha acid content and is often sold with Zeus as CTZ."@en ;
                                     <http://xmlns.com/foaf/0.1/name> "Columbus" ;
                                     <https://rdf.ag/o/hops#alphaAcidsContent> "14-18" ;
                                     <https://rdf.ag/o/hops#betaAcidsContent> "4.5-6" ;
                                     <https://rdf.ag/o/hops#totalOilContent> "1.5-4.5" .


###  https://rdf.ag/o/hops#HopsComet
<https://rdf.ag/o/hops#HopsComet> rdf:type owl:Class ;
                                  rdfs:subClassOf <https://rdf.ag/o/hops#Hops> ;
                                  <http://rdfs.org/ns/void#inDataset> <https://rdf.ag/o/hops#datasetdefinition> ;
                                  rdfs:isDefinedBy <https://rdf.ag/o/hops-2021-07-30> ;
                                  rdfs:label "Comet"@en ;
                                  <http://www.w3.org/2004/02/skos/core#definition> "Comet est le résultat d'un croisement entre le houblon anglais Sunshine et une variété amérindienne dans la recherche d'un houblon alpha acide à plus haut rendement. Il a été publié en 1974 par l'USDA."@fr ,
                                                                                   "Comet is the result of a cross between the English hop Sunshine and a native American variety in the search for a higher yielding alpha acid hop. It was released in 1974 by the USDA."@en ;
                                  <http://xmlns.com/foaf/0.1/isPrimaryTopicOf> <https://rdf.ag/o/hops#10.2135cropsci1975.0011183X0015000100> ;
                                  <http://xmlns.com/foaf/0.1/name> "Comet" ;
                                  <https://rdf.ag/o/hops#alphaAcidsContent> "9.4-12.4" ;
                                  <https://rdf.ag/o/hops#betaAcidsContent> "3-6.1" ;
                                  <https://rdf.ag/o/hops#perceivedAroma> "Agrumes, Pamplemousse, Résineux"@fr ,
                                                                         "Citrus, Grapefruit, Resinous"@en ;
                                  <https://rdf.ag/o/hops#totalOilContent> "1.98" .


###  https://rdf.ag/o/hops#HopsCrystal
<https://rdf.ag/o/hops#HopsCrystal> rdf:type owl:Class ;
                                    rdfs:subClassOf <https://rdf.ag/o/hops#Hops> ;
                                    <http://rdfs.org/ns/void#inDataset> <https://rdf.ag/o/hops#datasetdefinition> ;
                                    rdfs:isDefinedBy <https://rdf.ag/o/hops-2021-07-30> ;
                                    rdfs:label "Crystal"@en ;
                                    <http://www.w3.org/2004/02/skos/core#definition> "Crystal, publié par l'USDA en 1993, a une lignée qui comprend Hallertau, Cascade, Brewer's Gold et Early Green. C'est la demi-soeur triploïde du mont. Hood et Liberty et est un houblon très polyvalent."@fr ,
                                                                                     "Crystal, released by the USDA in 1993, has a lineage that includes Hallertau, Cascade, Brewer’s Gold and Early Green. It is the triploid half-sister to Mt. Hood and Liberty and is a very versatile hop."@en ;
                                    <http://xmlns.com/foaf/0.1/isPrimaryTopicOf> <https://rdf.ag/o/hops#cropsci1995.0011183X003500010053x> ;
                                    <http://xmlns.com/foaf/0.1/name> "Crystal" ;
                                    <https://rdf.ag/o/hops#alphaAcidsContent> "2.8-4.4" ;
                                    <https://rdf.ag/o/hops#betaAcidsContent> "5.8-7" ;
                                    <https://rdf.ag/o/hops#perceivedAroma> "Boisé, Cannelle, Floral, Fruité, Noix de muscade, Poivre Noir"@fr ,
                                                                           "Cinnamon, Black Pepper, Floral, Fruity, Nutmeg, Woody"@en ;
                                    <https://rdf.ag/o/hops#totalOilContent> "0.82" .


###  https://rdf.ag/o/hops#HopsDana
<https://rdf.ag/o/hops#HopsDana> rdf:type owl:Class ;
                                 rdfs:subClassOf <https://rdf.ag/o/hops#Hops> ;
                                 <http://rdfs.org/ns/void#inDataset> <https://rdf.ag/o/hops#datasetdefinition> ;
                                 rdfs:isDefinedBy <https://rdf.ag/o/hops-2021-07-30> ;
                                 rdfs:label "Dana"@en ,
                                            "Extra Styrian Dana"@en ;
                                 <http://www.w3.org/2004/02/skos/core#definition> "Dana a été élevée par l'Institute of Hop Research de Zalec, en Slovénie, à partir d'un croisement entre Hallertau Magnum et un houblon slovène local."@fr ,
                                                                                  "Dana was bred by the Institute of Hop Research in Zalec, Slovenia from a cross between Hallertau Magnum and a local Slovenian hop."@en ;
                                 <http://xmlns.com/foaf/0.1/isPrimaryTopicOf> <https://rdf.ag/o/hops#jpr2011.08.0403crc> ;
                                 <http://xmlns.com/foaf/0.1/name> "Dana" ;
                                 <https://rdf.ag/o/hops#alphaAcidsContent> "11-16" ;
                                 <https://rdf.ag/o/hops#betaAcidsContent> "4-6" ;
                                 <https://rdf.ag/o/hops#perceivedAroma> "Citron, Floral, Pin"@fr ,
                                                                        "Floral, Lemon, Pine"@en ;
                                 <https://rdf.ag/o/hops#totalOilContent> "2.4-3.9" .


###  https://rdf.ag/o/hops#HopsDelta
<https://rdf.ag/o/hops#HopsDelta> rdf:type owl:Class ;
                                  rdfs:subClassOf <https://rdf.ag/o/hops#Hops> ;
                                  <http://rdfs.org/ns/void#inDataset> <https://rdf.ag/o/hops#datasetdefinition> ;
                                  rdfs:isDefinedBy <https://rdf.ag/o/hops-2021-07-30> ;
                                  rdfs:label "Delta"@en ,
                                             "Hopsteiner 04188"@en ;
                                  <http://www.w3.org/2004/02/skos/core#definition> "Delta est sorti en 2009 de Hopsteiner et est un croisement entre Fuggle et un mâle dérivé de Cascade."@fr ,
                                                                                   "Delta was released in 2009 from Hopsteiner and is a cross between Fuggle and a male derived from Cascade."@en ;
                                  <http://xmlns.com/foaf/0.1/name> "Delta" ;
                                  <https://rdf.ag/o/hops#alphaAcidsContent> "5.5-7" ;
                                  <https://rdf.ag/o/hops#betaAcidsContent> "5.5-7" ;
                                  <https://rdf.ag/o/hops#perceivedAroma> "Agrumes, Ananas, Épicé, Melon, Poire"@fr ,
                                                                         "Citrus, Melon, Pear, Pineapple, Spicy"@en ;
                                  <https://rdf.ag/o/hops#totalOilContent> "0.5-1.1" .


###  https://rdf.ag/o/hops#HopsEastKentGolding
<https://rdf.ag/o/hops#HopsEastKentGolding> rdf:type owl:Class ;
                                            rdfs:subClassOf <https://rdf.ag/o/hops#HopsGolding> ;
                                            <http://rdfs.org/ns/void#inDataset> <https://rdf.ag/o/hops#datasetdefinition> ;
                                            rdfs:isDefinedBy <https://rdf.ag/o/hops-2021-07-30> ;
                                            rdfs:label "British Kent Golding"@en ,
                                                       "EKG"@en ,
                                                       "East Kent Golding"@en ,
                                                       "Kent Golding"@en ;
                                            <http://www.w3.org/2004/02/skos/core#definition> """East Kent Golding est l'une des plus anciennes variétés de Golding, cultivée exclusivement dans (et nommée d'après) des villes du Kent, en Angleterre. Cette variété est un descendant de la variété Canterbury Whitebine.
      
      Il est identique à Canterbury Golding, car les Goldings portent généralement le nom de la ville dans laquelle ils ont été cultivés. East Kent fait référence à la variété de houblon de la région du Kent et Canterbury est une ville du Kent. La variété est surtout connue sous le nom d'East Kent Golding."""@fr ,
                                                                                             """East Kent Golding is one of the oldest variety of Golding, grown exclusively from (and named after) towns in Kent, England. This variety is a descendant of the Canterbury Whitebine variety.
      
      It is identical to Canterbury Golding, as Goldings are typically named from the town that they were grown in. East Kent refers to the hop variety from the Kent area and Canterbury is a town in Kent. The variety is mostly known as East Kent Golding."""@en ;
                                            <http://xmlns.com/foaf/0.1/name> "East Kent Golding" ;
                                            <https://rdf.ag/o/hops#alphaAcidsContent> "5–6" ;
                                            <https://rdf.ag/o/hops#betaAcidsContent> "2.0–3.0" ;
                                            <https://rdf.ag/o/hops#perceivedAroma> "Earthy, Honey, Lavender, Spice, Thyme"@en ,
                                                                                   "Épice, Miel, Lavande, Terreux, Thym"@en ;
                                            <https://rdf.ag/o/hops#totalOilContent> "0.85" .


###  https://rdf.ag/o/hops#HopsEastwellGolding
<https://rdf.ag/o/hops#HopsEastwellGolding> rdf:type owl:Class ;
                                            rdfs:subClassOf <https://rdf.ag/o/hops#HopsGolding> ;
                                            <http://rdfs.org/ns/void#inDataset> <https://rdf.ag/o/hops#datasetdefinition> ;
                                            rdfs:isDefinedBy <https://rdf.ag/o/hops-2021-07-30> ;
                                            rdfs:label "Eastwell Golding"@en ;
                                            <http://www.w3.org/2004/02/skos/core#definition> "Eastwell Golding est une variété de houblon d'Eastwell Park (près d'Ashford, Kent au Royaume-Uni) et a été créée via une section clonale en 1889. Elle est généralement utilisée comme houblon aromatique pour les bières anglaises et belges. Ce houblon a été utilisé pour l'élevage de Target."@fr ,
                                                                                             "Eastwell Golding is a hop variety from Eastwell Park (near Ashford, Kent in the UK) and was created via clonal section in 1889. It is usually used as an aroma hop for English and Belgian ales. This hop was used for breeding Target."@en ;
                                            <http://xmlns.com/foaf/0.1/name> "Eastwell Golding" ;
                                            <https://rdf.ag/o/hops#alphaAcidsContent> "6" ;
                                            <https://rdf.ag/o/hops#betaAcidsContent> "3.0" ;
                                            <https://rdf.ag/o/hops#totalOilContent> "1.5" .


###  https://rdf.ag/o/hops#HopsEkuanot
<https://rdf.ag/o/hops#HopsEkuanot> rdf:type owl:Class ;
                                    rdfs:subClassOf <https://rdf.ag/o/hops#Hops> ;
                                    <http://rdfs.org/ns/void#inDataset> <https://rdf.ag/o/hops#datasetdefinition> ;
                                    rdfs:isDefinedBy <https://rdf.ag/o/hops-2021-07-30> ;
                                    rdfs:label "Ekuanot®"@en ,
                                               "Equinox"@en ,
                                               "HBC 366"@en ;
                                    <http://www.w3.org/2004/02/skos/core#definition> "Ekuanot®, anciennement Equinox après un litige de marque, a été élevé par Eugene G. Probasco et Jason Perrault de Hop Breeding Company, LLC., Yakima, WA (États-Unis)."@fr ,
                                                                                     "Ekuanot®, formerly Equinox after a trademark dispute, was bred by Eugene G. Probasco and Jason Perrault from Hop Breeding Company, LLC., Yakima, WA (US)."@en ;
                                    <http://xmlns.com/foaf/0.1/name> "Ekuanot®" ;
                                    <https://rdf.ag/o/hops#alphaAcidsContent> "14.5-15.5" ;
                                    <https://rdf.ag/o/hops#betaAcidsContent> "4.5-5.5" ;
                                    <https://rdf.ag/o/hops#perceivedAroma> "Apple, Green Pepper, Herbal, Lemon, Lime, Papaya"@en ,
                                                                           "Citron, Citron Vert, Herbes, Papaye, Poivron Vert, Pomme"@fr ;
                                    <https://rdf.ag/o/hops#totalOilContent> "2.5-4.5" .


###  https://rdf.ag/o/hops#HopsElDorado
<https://rdf.ag/o/hops#HopsElDorado> rdf:type owl:Class ;
                                     rdfs:subClassOf <https://rdf.ag/o/hops#Hops> ;
                                     <http://rdfs.org/ns/void#inDataset> <https://rdf.ag/o/hops#datasetdefinition> ;
                                     rdfs:isDefinedBy <https://rdf.ag/o/hops-2021-07-30> ;
                                     rdfs:label "El Dorado"@en ;
                                     <http://www.w3.org/2004/02/skos/core#definition> """El Dorado est un houblon américain créé par CLS Farms, LLC en 2008 et rendu public en 2010.
      
      Ce houblon est bon pour l'amertume et pour l'ajout d'arôme en raison de sa forte teneur en acide alpha et en huile."""@fr ,
                                                                                      """El Dorado is an American hops created by CLS Farms, LLC in 2008 and released to the public in 2010.
      
      This hop is good for bittering and for adding aroma due to its high alpha acid and oil content."""@en ;
                                     <http://xmlns.com/foaf/0.1/name> "El Dorado" ;
                                     <https://rdf.ag/o/hops#alphaAcidsContent> "13-17" ;
                                     <https://rdf.ag/o/hops#betaAcidsContent> "7-8" ;
                                     <https://rdf.ag/o/hops#perceivedAroma> "Fruits Tropicaux, Poire, Fruits à Noyau"@fr ,
                                                                            "Tropical Fruit, Pear, Stone Fruit"@en ;
                                     <https://rdf.ag/o/hops#totalOilContent> "2.50-3.3" .


###  https://rdf.ag/o/hops#HopsEroica
<https://rdf.ag/o/hops#HopsEroica> rdf:type owl:Class ;
                                   rdfs:subClassOf <https://rdf.ag/o/hops#Hops> ;
                                   <http://rdfs.org/ns/void#inDataset> <https://rdf.ag/o/hops#datasetdefinition> ;
                                   rdfs:isDefinedBy <https://rdf.ag/o/hops-2021-07-30> ;
                                   rdfs:label "Eroica"@en ;
                                   <http://www.w3.org/2004/02/skos/core#definition> "Eroica a été élevé aux côtés de sa sœur Galena en 1968 et il a été rendu public en 1979 par les stations d'expérimentation agricole de l'Idaho et de l'Oregon en collaboration avec l'USDA. Il a été dérivé de Brewer's Gold par pollinisation libre."@fr ,
                                                                                    "Eroica was bred alongside its sister Galena in 1968 and it was released to the public in 1979 by both the Idaho and Oregon Agricultural Experiment Stations in conjunction the USDA. It was derived from Brewer's Gold through open pollenation."@en ;
                                   <http://xmlns.com/foaf/0.1/isPrimaryTopicOf> <https://rdf.ag/o/hops#cropsci1982.0011183X002200060052x> ;
                                   <http://xmlns.com/foaf/0.1/name> "Eroica" ;
                                   <https://rdf.ag/o/hops#alphaAcidsContent> "12.3" ;
                                   <https://rdf.ag/o/hops#betaAcidsContent> "4.5" ;
                                   <https://rdf.ag/o/hops#perceivedAroma> "Amer, Fruité"@fr ,
                                                                          "Bitter, Fruity"@en ;
                                   <https://rdf.ag/o/hops#totalOilContent> "0.8-1.3" .


###  https://rdf.ag/o/hops#HopsEroica_vf
<https://rdf.ag/o/hops#HopsEroica_vf> rdf:type owl:Class ;
                                      rdfs:subClassOf <https://rdf.ag/o/hops#HopsEroica> ;
                                      <http://rdfs.org/ns/void#inDataset> <https://rdf.ag/o/hops#datasetdefinition> ;
                                      rdfs:isDefinedBy <https://rdf.ag/o/hops-2021-07-30> ;
                                      rdfs:label "Eroica vf"@en ;
                                      <http://www.w3.org/2004/02/skos/core#definition> "La version 'sans virus' d'Eroica Hops."@fr ,
                                                                                       "The 'virus-free' version of Eroica Hops."@en ;
                                      <http://xmlns.com/foaf/0.1/name> "Eroica vf" ;
                                      <https://rdf.ag/o/hops#alphaAcidsContent> "12.3" ;
                                      <https://rdf.ag/o/hops#betaAcidsContent> "4.7" ;
                                      <https://rdf.ag/o/hops#perceivedAroma> "Amer, Fruité"@fr ,
                                                                             "Bitter, Fruity"@en ;
                                      <https://rdf.ag/o/hops#totalOilContent> "1.10" .


###  https://rdf.ag/o/hops#HopsFalconersFlight
<https://rdf.ag/o/hops#HopsFalconersFlight> rdf:type owl:Class ;
                                            rdfs:subClassOf <https://rdf.ag/o/hops#HopsCascade> ,
                                                            <https://rdf.ag/o/hops#HopsCentennial> ,
                                                            <https://rdf.ag/o/hops#HopsChinook> ,
                                                            <https://rdf.ag/o/hops#HopsCitra> ,
                                                            <https://rdf.ag/o/hops#HopsCluster> ,
                                                            <https://rdf.ag/o/hops#HopsColumbus> ,
                                                            <https://rdf.ag/o/hops#HopsCrystal> ;
                                            rdfs:label "Falconer's Flight®"@en ;
                                            <http://www.w3.org/2004/02/skos/core#definition> "Falconer's Flight® est le mélange exclusif de Hopunion LLC des houblons \"7 C\" du nord-ouest du Pacifique, ainsi que quelques autres variétés expérimentales qui ont également été développées par Hopunion. Les houblons \"7 C\" sont: Cascade, Centennial, Chinook, Citra®, Cluster, Columbus et Crystal."@fr ,
                                                                                             "Falconer's Flight® is Hopunion LLC's proprietary blend of 'the 7C' hops of the Pacific Northwest, along with a few other experimental varieties that were also developed by Hopunion. The '7 C' hops are: Cascade, Centennial, Chinook, Citra®, Cluster, Columbus and Crystal."@en ;
                                            <http://xmlns.com/foaf/0.1/name> "Falconer's Flight®" ;
                                            <https://rdf.ag/o/hops#alphaAcidsContent> "9.5-12" ;
                                            <https://rdf.ag/o/hops#betaAcidsContent> "4-5" ;
                                            <https://rdf.ag/o/hops#perceivedAroma> "Citron, Floral, Pamplemousse"@fr ,
                                                                                   "Floral, Grapefruit, Lemon"@en ;
                                            <https://rdf.ag/o/hops#totalOilContent> "1.6-4.6" .


###  https://rdf.ag/o/hops#HopsFirstGold
<https://rdf.ag/o/hops#HopsFirstGold> rdf:type owl:Class ;
                                      rdfs:subClassOf <https://rdf.ag/o/hops#Hops> ;
                                      <http://rdfs.org/ns/void#inDataset> <https://rdf.ag/o/hops#datasetdefinition> ;
                                      rdfs:isDefinedBy <https://rdf.ag/o/hops-2021-07-30> ;
                                      rdfs:label "First Gold"@en ;
                                      <http://www.w3.org/2004/02/skos/core#definition> "First Gold est un descendant de Brewer's Gold et un mâle nain du Wye College au Royaume-Uni et a été lancé en 1995. C'est aussi le premier houblon de haie d'Angleterre."@fr ,
                                                                                       "First Gold is a descendant of Brewer's Gold and a dwarf male from Wye College in the UK and was released in 1995. It is also England's first hedgerow hop."@en ;
                                      <http://xmlns.com/foaf/0.1/name> "First Gold" ;
                                      <https://rdf.ag/o/hops#alphaAcidsContent> "5.6-9.3" ;
                                      <https://rdf.ag/o/hops#betaAcidsContent> "2.3-4.1" ;
                                      <https://rdf.ag/o/hops#perceivedAroma> "Cannelle, Mandarine, Marmelade, Orange"@fr ,
                                                                             "Cinnamon, Marmalade, Orange, Tangerine"@en ;
                                      <https://rdf.ag/o/hops#totalOilContent> "0.7-1.5" .


###  https://rdf.ag/o/hops#HopsFuggle
<https://rdf.ag/o/hops#HopsFuggle> rdf:type owl:Class ;
                                   rdfs:subClassOf <https://rdf.ag/o/hops#Hops> ;
                                   <http://rdfs.org/ns/void#inDataset> <https://rdf.ag/o/hops#datasetdefinition> ;
                                   rdfs:isDefinedBy <https://rdf.ag/o/hops-2021-07-30> ;
                                   rdfs:label "Fuggle"@en ,
                                              "Fuggles"@en ;
                                   <http://www.w3.org/2004/02/skos/core#definition> "Fuggle a été introduit et nommé par Richard Fuggle en 1875 après avoir été découvert pour la première fois dans une houblonnière du Kent appartenant à George Stace. Il était plus populaire en tant que houblon à double usage il y a 100 ans, mais aujourd'hui, il est principalement utilisé pour son arôme."@fr ,
                                                                                    "Fuggle was introduced and named by Richard Fuggle in 1875 after first being discovered in a Kent hopyard owned by George Stace. It was more popular as a dual-use hops 100 years ago but today it is mostly used for its aroma."@en ;
                                   <http://xmlns.com/foaf/0.1/name> "Fuggle" .


###  https://rdf.ag/o/hops#HopsFuggle_H
<https://rdf.ag/o/hops#HopsFuggle_H> rdf:type owl:Class ;
                                     rdfs:subClassOf <https://rdf.ag/o/hops#HopsFuggle_US> ;
                                     <http://rdfs.org/ns/void#inDataset> <https://rdf.ag/o/hops#datasetdefinition> ;
                                     rdfs:isDefinedBy <https://rdf.ag/o/hops-2021-07-30> ;
                                     rdfs:label "Fuggle H"@en ;
                                     <http://www.w3.org/2004/02/skos/core#definition> "Fuggle H a été développé à l'OSU East Farm à Corvallis, en Oregon, grâce à la reproduction sélective de Fuggle à haut rendement à partir de la variété Fuggle originale du Royaume-Uni."@fr ,
                                                                                      "Fuggle H was developed in 1961 at OSU East Farm in Corvallis, Oregon through selective breeding of high yielding Fuggle from the original Fuggle variety from the UK."@en ;
                                     <http://xmlns.com/foaf/0.1/name> "Fuggle H" ;
                                     <https://rdf.ag/o/hops#alphaAcidsContent> "2.8" ;
                                     <https://rdf.ag/o/hops#betaAcidsContent> "2.8" ;
                                     <https://rdf.ag/o/hops#totalOilContent> "0.9" .


###  https://rdf.ag/o/hops#HopsFuggle_Tetraploid
<https://rdf.ag/o/hops#HopsFuggle_Tetraploid> rdf:type owl:Class ;
                                              rdfs:subClassOf <https://rdf.ag/o/hops#HopsFuggle_US> ;
                                              <http://rdfs.org/ns/void#inDataset> <https://rdf.ag/o/hops#datasetdefinition> ;
                                              rdfs:isDefinedBy <https://rdf.ag/o/hops-2021-07-30> ;
                                              rdfs:label "Fuggle Tetraploid"@en ;
                                              <http://www.w3.org/2004/02/skos/core#definition> "Fuggle Tetraploid a été développé en 1966 à OSU East Farm à Corvallis, Oregon, grâce au traitement à la colchicine de la variété Fuggle originale du Royaume-Uni."@fr ,
                                                                                               "Fuggle Tetraploid was developed in 1966 at OSU East Farm in Corvallis, Oregon through colchicine treatment of the original Fuggle variety from the UK."@en ;
                                              <http://xmlns.com/foaf/0.1/name> "Fuggle Tetraploid" ;
                                              <https://rdf.ag/o/hops#alphaAcidsContent> "5" ;
                                              <https://rdf.ag/o/hops#betaAcidsContent> "2.4" ;
                                              <https://rdf.ag/o/hops#totalOilContent> "0.93" .


###  https://rdf.ag/o/hops#HopsFuggle_UK
<https://rdf.ag/o/hops#HopsFuggle_UK> rdf:type owl:Class ;
                                      rdfs:subClassOf <https://rdf.ag/o/hops#HopsFuggle> ;
                                      <http://rdfs.org/ns/void#inDataset> <https://rdf.ag/o/hops#datasetdefinition> ;
                                      rdfs:isDefinedBy <https://rdf.ag/o/hops-2021-07-30> ;
                                      rdfs:label "Fuggle (UK)"@en ;
                                      <http://www.w3.org/2004/02/skos/core#definition> "Fuggle (UK) est génétiquement identique au houblon Fuggle, mais ses propriétés peuvent différer des autres houblons Fuggle car il a été cultivé au Royaume-Uni et a donc un terroir différent."@fr ,
                                                                                       "Fuggle (UK) is genetically identical to Fuggle hops, but its properties may differ from other Fuggle hops as it was grown in the UK and therefore has a different terroir."@en ;
                                      <http://xmlns.com/foaf/0.1/name> "Fuggle (UK)" ;
                                      <https://rdf.ag/o/hops#alphaAcidsContent> "2.4-6.1" ;
                                      <https://rdf.ag/o/hops#betaAcidsContent> "2.1-2.8" ;
                                      <https://rdf.ag/o/hops#perceivedAroma> "Boisé, Floral, Herbeux, Menthe"@fr ,
                                                                             "Floral, Grassy, Minty, Woody"@en ;
                                      <https://rdf.ag/o/hops#totalOilContent> "0.44-0.83" .


###  https://rdf.ag/o/hops#HopsFuggle_US
<https://rdf.ag/o/hops#HopsFuggle_US> rdf:type owl:Class ;
                                      rdfs:subClassOf <https://rdf.ag/o/hops#HopsFuggle> ;
                                      <http://rdfs.org/ns/void#inDataset> <https://rdf.ag/o/hops#datasetdefinition> ;
                                      rdfs:isDefinedBy <https://rdf.ag/o/hops-2021-07-30> ;
                                      rdfs:label "Fuggle (US)"@en ;
                                      <http://www.w3.org/2004/02/skos/core#definition> "Fuggle (US) est dérivé du houblon Fuggle original du Royaume-Uni, mais il a été sélectionné de manière sélective pour être plus résistant aux maladies et avoir des rendements plus élevés. Être cultivé aux États-Unis peut également avoir des effets sur les propriétés de ce houblon."@fr ,
                                                                                       "Fuggle (US) is derived from the original Fuggle hops from the UK, but it has been selectively bred to be more resistant to disease and have higher yields. Being grown in the US may also have effects on the properties of this hop."@en ;
                                      <http://xmlns.com/foaf/0.1/name> "Fuggle (US)" .


###  https://rdf.ag/o/hops#HopsGalaxy
<https://rdf.ag/o/hops#HopsGalaxy> rdf:type owl:Class ;
                                   rdfs:subClassOf <https://rdf.ag/o/hops#Hops> ;
                                   <http://rdfs.org/ns/void#inDataset> <https://rdf.ag/o/hops#datasetdefinition> ;
                                   rdfs:isDefinedBy <https://rdf.ag/o/hops-2021-07-30> ;
                                   rdfs:label "Galaxy™"@en ;
                                   <http://www.w3.org/2004/02/skos/core#definition> "Galaxy™ est une variété australienne de houblon lancée pour la première fois en 2009 et dérivée de Perle. Il est surtout connu pour sa teneur élevée en huile."@fr ,
                                                                                    "Galaxy™ is an Australian variety of hops first released in 2009 that is derived from Perle. It is most prominantely known for its high oil content."@en ;
                                   <http://xmlns.com/foaf/0.1/name> "Galaxy™" ;
                                   <https://rdf.ag/o/hops#alphaAcidsContent> "11-16" ;
                                   <https://rdf.ag/o/hops#betaAcidsContent> "5-6.9" ;
                                   <https://rdf.ag/o/hops#perceivedAroma> "Agrumes, Fruit de la Passion, Pêche"@fr ,
                                                                          "Citrus, Passionfruit, Peach"@en ;
                                   <https://rdf.ag/o/hops#totalOilContent> "3-5" .


###  https://rdf.ag/o/hops#HopsGalena
<https://rdf.ag/o/hops#HopsGalena> rdf:type owl:Class ;
                                   rdfs:subClassOf <https://rdf.ag/o/hops#Hops> ;
                                   <http://rdfs.org/ns/void#inDataset> <https://rdf.ag/o/hops#datasetdefinition> ;
                                   rdfs:isDefinedBy <https://rdf.ag/o/hops-2021-07-30> ;
                                   rdfs:label "Galena"@en ;
                                   <http://www.w3.org/2004/02/skos/core#definition> "Galena a été sélectionnée en 1968 par R. R. Romanko dans l'Idaho à partir d'un croisement de pollinisation libre entre Brewer's Gold et un mâle inconnu. Il est connu pour avoir une teneur élevée en acide alpha, en acide bêta et en huile totale."@fr ,
                                                                                    "Galena was selected in 1968 by R. R. Romanko in Idaho from an open pollination cross between Brewer's Gold and an unknown male. It is known for having high alpha acid, beta acid and total oil content."@en ;
                                   <http://xmlns.com/foaf/0.1/isPrimaryTopicOf> <https://rdf.ag/o/hops#cropsci1979.0011183X001900040036x> ;
                                   <http://xmlns.com/foaf/0.1/name> "Galena" ;
                                   <https://rdf.ag/o/hops#alphaAcidsContent> "12" ;
                                   <https://rdf.ag/o/hops#betaAcidsContent> "7.5" ;
                                   <https://rdf.ag/o/hops#perceivedAroma> "Agrumes, Ananas, Brandy, Cassis, Citron Vert, Épicé, Groseille, Poire"@fr ,
                                                                          "Brandy, Blackcurrant, Citrus, Gooseberry, Lime, Pear, Pineapple, Spicy"@en ;
                                   <https://rdf.ag/o/hops#totalOilContent> "0.9-1.3" .


###  https://rdf.ag/o/hops#HopsGalenaVF
<https://rdf.ag/o/hops#HopsGalenaVF> rdf:type owl:Class ;
                                     rdfs:subClassOf <https://rdf.ag/o/hops#HopsGalena> ;
                                     <http://rdfs.org/ns/void#inDataset> <https://rdf.ag/o/hops#datasetdefinition> ;
                                     rdfs:isDefinedBy <https://rdf.ag/o/hops-2021-07-30> ;
                                     rdfs:label "Galena (VF)"@en ,
                                                "Virus Free Galena"@en ;
                                     <http://www.w3.org/2004/02/skos/core#definition> "Cette variété de Galène a été sélectionnée de manière sélective par le Dr Bob Romanko à Parma, ID, pour être plus résistante aux virus. Sinon, il est presque identique à Galena."@fr ,
                                                                                      "This variety of Galena was selectively bred by Dr. Bob Romanko at Parma, ID, to be more resistant to viruses. Otherwise, it is nearly identical to Galena."@en ;
                                     <http://xmlns.com/foaf/0.1/name> "Virus FreevGalena" .


###  https://rdf.ag/o/hops#HopsGlacier
<https://rdf.ag/o/hops#HopsGlacier> rdf:type owl:Class ;
                                    rdfs:subClassOf <https://rdf.ag/o/hops#Hops> ;
                                    <http://rdfs.org/ns/void#inDataset> <https://rdf.ag/o/hops#datasetdefinition> ;
                                    rdfs:isDefinedBy <https://rdf.ag/o/hops-2021-07-30> ;
                                    rdfs:label "Glacier"@en ;
                                    <http://www.w3.org/2004/02/skos/core#definition> "La variété de houblon Glacier a été développée par la Washington State University et a été lancée en 2000. Elle est connue pour avoir un rendement élevé et de faibles niveaux de cohumulone. C'est un descendant d'Elsasser, de Northern Brewer et de Brewer's Gold."@fr ,
                                                                                     "The Glacier hops variety was developed by Washington State University and was released in 2000. It is known for having a high yield and low cohumulone levels. It is a descendant of Elsasser, Northern Brewer and Brewer's Gold."@en ;
                                    <http://xmlns.com/foaf/0.1/name> "Glacier" ;
                                    <https://rdf.ag/o/hops#alphaAcidsContent> "3.3-9.7" ;
                                    <https://rdf.ag/o/hops#betaAcidsContent> "5.4-10" ;
                                    <https://rdf.ag/o/hops#totalOilContent> "0.7-1.6" .


###  https://rdf.ag/o/hops#HopsGolding
<https://rdf.ag/o/hops#HopsGolding> rdf:type owl:Class ;
                                    rdfs:subClassOf <https://rdf.ag/o/hops#Hops> ;
                                    <http://rdfs.org/ns/void#inDataset> <https://rdf.ag/o/hops#datasetdefinition> ;
                                    rdfs:isDefinedBy <https://rdf.ag/o/hops-2021-07-30> ;
                                    rdfs:label "Golding"@en ;
                                    <http://www.w3.org/2004/02/skos/core#definition> "Golding is a variety of hops from the United Kingdom. It is from this variety that many Golding varieties are derived from, with the exception of Styrian (or Yugoslavia) Golding, which is derived from Fuggle."@en ,
                                                                                     "Le Golding est une variété de houblon du Royaume-Uni. C'est de cette variété que sont dérivées de nombreuses variétés de Golding, à l'exception de la Golding de Styrie (ou de Yougoslavie) qui est dérivée de Fuggle."@fr ;
                                    <http://xmlns.com/foaf/0.1/name> "Golding" .


###  https://rdf.ag/o/hops#HopsGoldingBC
<https://rdf.ag/o/hops#HopsGoldingBC> rdf:type owl:Class ;
                                      rdfs:subClassOf <https://rdf.ag/o/hops#HopsEastKentGolding> ;
                                      <http://rdfs.org/ns/void#inDataset> <https://rdf.ag/o/hops#datasetdefinition> ;
                                      rdfs:isDefinedBy <https://rdf.ag/o/hops-2021-07-30> ;
                                      rdfs:label "Golding (BC)"@en ;
                                      <http://www.w3.org/2004/02/skos/core#definition> "Ce type de Golding, originaire du Royaume-Uni, généralement East Kent Golding, a été cultivé en Colombie-Britannique, ayant ainsi des propriétés différentes en raison de la différence de terroir."@fr ,
                                                                                       "This type of Golding, originated in the UK, usually East Kent Golding, and was grown in British Columbia, thus having different properties due to the difference in terroir."@en ;
                                      <http://xmlns.com/foaf/0.1/name> "Golding (BC)" ;
                                      <https://rdf.ag/o/hops#alphaAcidsContent> "4–7" .


###  https://rdf.ag/o/hops#HopsGoldingNZ
<https://rdf.ag/o/hops#HopsGoldingNZ> rdf:type owl:Class ;
                                      rdfs:subClassOf <https://rdf.ag/o/hops#HopsEastKentGolding> ;
                                      <http://rdfs.org/ns/void#inDataset> <https://rdf.ag/o/hops#datasetdefinition> ;
                                      rdfs:isDefinedBy <https://rdf.ag/o/hops-2021-07-30> ;
                                      rdfs:label "Golding (NZ)"@en ;
                                      <http://www.w3.org/2004/02/skos/core#definition> "Ce type de Golding, originaire du Royaume-Uni, généralement East Kent Golding, a été cultivé en Nouvelle-Zélande, ayant ainsi des propriétés différentes en raison de la différence de terroir."@fr ,
                                                                                       "This type of Golding, originated in the UK, usually East Kent Golding, and was grown in New Zealand, thus having different properties due to the difference in terroir."@en ;
                                      <http://xmlns.com/foaf/0.1/name> "Golding (NZ)" ;
                                      <https://rdf.ag/o/hops#alphaAcidsContent> "4–4.2" ;
                                      <https://rdf.ag/o/hops#betaAcidsContent> "4.6-4.8" .


###  https://rdf.ag/o/hops#HopsGoldingUS
<https://rdf.ag/o/hops#HopsGoldingUS> rdf:type owl:Class ;
                                      rdfs:subClassOf <https://rdf.ag/o/hops#HopsEastKentGolding> ;
                                      <http://rdfs.org/ns/void#inDataset> <https://rdf.ag/o/hops#datasetdefinition> ;
                                      rdfs:isDefinedBy <https://rdf.ag/o/hops-2021-07-30> ;
                                      rdfs:label "Golding (US)"@en ;
                                      <http://www.w3.org/2004/02/skos/core#definition> """Golding comes from the group of cultivars grown in East Kent, United Kingdom. US Golding are typically derived from Canterbury (village in East Kent) Golding hops.
      
      This hop was originally grown in British Columbia, Canada and it was then appearing in Washington and Oregon states in 1993. The hop that is grown in the US will have different properties from the same hop grown in the UK, due to differences in terroir.
      
      Golding is known for its delicate, sweet, and floral notes."""@en ,
                                                                                       """Golding provient du groupe de cultivars cultivés dans East Kent, Royaume-Uni. US Golding est généralement dérivé du houblon Golding de Canterbury (village dans l'est du Kent).
      
      Ce houblon a été cultivé à l'origine en Colombie-Britannique, au Canada, puis il est apparu dans les États de Washington et de l'Oregon en 1993. Le houblon cultivé aux États-Unis aura des propriétés différentes du même houblon cultivé au Royaume-Uni, en raison des différences de terroir.
      
      Golding est connu pour ses notes délicates, sucrées et florales."""@fr ;
                                      <http://xmlns.com/foaf/0.1/name> "Golding (US)" ;
                                      <https://rdf.ag/o/hops#alphaAcidsContent> "4–6" ;
                                      <https://rdf.ag/o/hops#betaAcidsContent> "2.0–3.0" ;
                                      <https://rdf.ag/o/hops#perceivedAroma> "Delicate, Floral, Sweet"@en ,
                                                                             "Délicat, Doux, Floral"@fr ;
                                      <https://rdf.ag/o/hops#totalOilContent> "0.7-1.0" .


###  https://rdf.ag/o/hops#HopsGreenBullet
<https://rdf.ag/o/hops#HopsGreenBullet> rdf:type owl:Class ;
                                        rdfs:subClassOf <https://rdf.ag/o/hops#Hops> ;
                                        <http://rdfs.org/ns/void#inDataset> <https://rdf.ag/o/hops#datasetdefinition> ;
                                        rdfs:isDefinedBy <https://rdf.ag/o/hops-2021-07-30> ;
                                        rdfs:label "Green Bullet"@en ;
                                        <http://www.w3.org/2004/02/skos/core#definition> "Green Bullet est un houblon néo-zélandais dérivé de Fuggle à la suite d'une sélection expérimentale effectuée pour lutter contre la pourriture noire des racines qui a frappé la Nouvelle-Zélande en 1949."@fr ,
                                                                                         "Green Bullet is a New Zealand hop derived from Fuggle as a result of experiemental breeding done to combat Black Root Rot that hit New Zealand in 1949."@en ;
                                        <http://xmlns.com/foaf/0.1/name> "Green Bullet" ;
                                        <https://rdf.ag/o/hops#alphaAcidsContent> "11-15" ;
                                        <https://rdf.ag/o/hops#betaAcidsContent> "2.9-7" ;
                                        <https://rdf.ag/o/hops#perceivedAroma> "Citron, Pin, Poivre, Raisin"@fr ,
                                                                               "Lemon, Pepper, Pine, Raisin"@en ;
                                        <https://rdf.ag/o/hops#totalOilContent> "0.46-1.13" .


###  https://rdf.ag/o/hops#HopsHallertau
<https://rdf.ag/o/hops#HopsHallertau> rdf:type owl:Class ;
                                      rdfs:subClassOf <https://rdf.ag/o/hops#Hops> ;
                                      <http://rdfs.org/ns/void#inDataset> <https://rdf.ag/o/hops#datasetdefinition> ;
                                      rdfs:comment "La raison de deux numéros d'accession USDA semble être deux échantillons différents du même houblon - Hallertau/Hallertau Mittelfrüher, provenant de deux régions différentes."@fr ,
                                                   "The reason for two USDA Accession Numbers seems to be two different samples of the same hop - Hallertau/Hallertau Mittelfrüher, from two different areas."@en ;
                                      rdfs:isDefinedBy <https://rdf.ag/o/hops-2021-07-30> ;
                                      rdfs:label "Hallertau"@en ,
                                                 "Hallertauer"@en ,
                                                 "Hallertauer Mittelfrüher"@en ;
                                      <http://www.w3.org/2004/02/skos/core#definition> "Hallertau est une race allemande qui existe depuis 100 ans. C'est l'ancêtre de nombreuses variétés afin de lutter contre sa sensibilité à la verticilliose et aux faibles rendements. Il est considéré comme l'une des quatre variétés \"nobles\" de houblon d'Allemagne."@fr ,
                                                                                       "Hallertau is a German landrace that has been around for the past 100 years. It is ancestor of many varieties in order to combat its susceptibility to verticillium wilt and poor yields. It is considered one of the four \"noble\" varieties of hops from Germany."@en ;
                                      <http://xmlns.com/foaf/0.1/name> "Hallertau" ;
                                      <https://rdf.ag/o/hops#alphaAcidsContent> "3.5-3.5" ;
                                      <https://rdf.ag/o/hops#betaAcidsContent> "3.5-4.5" ;
                                      <https://rdf.ag/o/hops#perceivedAroma> "Floral, Grassy, Spicy"@en ,
                                                                             "Épicé, Floral, Herbeux"@fr ;
                                      <https://rdf.ag/o/hops#totalOilContent> "0.6-1.2" .


###  https://rdf.ag/o/hops#HopsHallertau_Blanc
<https://rdf.ag/o/hops#HopsHallertau_Blanc> rdf:type owl:Class ;
                                            rdfs:subClassOf <https://rdf.ag/o/hops#HopsCascade> ;
                                            <http://rdfs.org/ns/void#inDataset> <https://rdf.ag/o/hops#datasetdefinition> ;
                                            rdfs:isDefinedBy <https://rdf.ag/o/hops-2021-07-30> ;
                                            rdfs:label "Hallertau Blanc"@en ;
                                            <http://www.w3.org/2004/02/skos/core#definition> "Hallertau Blanc is actually not variety of Hallertau, rather it is the daughter of Cascade and was bred in Germany in order to create American-style Ales."@en ,
                                                                                             "Hallertau Blanc n'est en fait pas une variété de Hallertau, c'est plutôt la fille de Cascade et a été élevée en Allemagne afin de créer des Ales de style américain."@fr ;
                                            <http://xmlns.com/foaf/0.1/name> "Hallertau Blanc" ;
                                            <https://rdf.ag/o/hops#alphaAcidsContent> "9-12" ;
                                            <https://rdf.ag/o/hops#betaAcidsContent> "4.5-6" ;
                                            <https://rdf.ag/o/hops#perceivedAroma> "Ananas, Cassis, Citronnelle, Fruité, Fruit de la passion, Groseille, Pamplemousse, Raisin, Vin Blanc"@fr ,
                                                                                   "Cassis, Fruity, Grapefruit, Grapes, Gooseberry, Lemongrass, Passionfruit, Pineapple, White Wine"@en ;
                                            <https://rdf.ag/o/hops#totalOilContent> "0.8-1.5" .


###  https://rdf.ag/o/hops#HopsHallertau_Gold
<https://rdf.ag/o/hops#HopsHallertau_Gold> rdf:type owl:Class ;
                                           rdfs:subClassOf <https://rdf.ag/o/hops#HopsHallertau> ;
                                           <http://rdfs.org/ns/void#inDataset> <https://rdf.ag/o/hops#datasetdefinition> ;
                                           rdfs:isDefinedBy <https://rdf.ag/o/hops-2021-07-30> ;
                                           rdfs:label "Hallertau Gold"@en ,
                                                      "Hallertauer Gold"@en ;
                                           <http://www.w3.org/2004/02/skos/core#definition> "Hallertau Gold est un descendant de Hallertau Mittelfrüher et a été élevé pour être plus résistant au flétrissement."@fr ,
                                                                                            "Hallertau Gold is a decendant of Hallertau Mittelfrüher and was bred to be more resisstant to wilt."@en ;
                                           <http://xmlns.com/foaf/0.1/name> "Hallertau Gold" ;
                                           <https://rdf.ag/o/hops#alphaAcidsContent> "7-10" ;
                                           <https://rdf.ag/o/hops#betaAcidsContent> "5-7" ;
                                           <https://rdf.ag/o/hops#totalOilContent> "1.78" .


###  https://rdf.ag/o/hops#HopsHallertau_Merkur
<https://rdf.ag/o/hops#HopsHallertau_Merkur> rdf:type owl:Class ;
                                             rdfs:subClassOf <https://rdf.ag/o/hops#HopsHallertau> ;
                                             <http://rdfs.org/ns/void#inDataset> <https://rdf.ag/o/hops#datasetdefinition> ;
                                             rdfs:isDefinedBy <https://rdf.ag/o/hops-2021-07-30> ;
                                             rdfs:label "Hallertau Merkur"@en ,
                                                        "Merkur"@en ;
                                             <http://www.w3.org/2004/02/skos/core#definition> "Hallertau Merker est un descendant du houblon Magnum et a été développé au Hull Hops Research Institute en Allemagne. Il est connu non seulement pour sa teneur élevée en acide alpha, mais également pour sa teneur élevée en myrcène et en huile humulène."@fr ,
                                                                                              "Hallertau Merker is a descendant of Magnum hops and was developed at the Hull Hops Research Institute in Germany. It is known for not just its high alpha acid content but its high myrcene and humulene oil content."@en ;
                                             <http://xmlns.com/foaf/0.1/name> "Hallertau Merkur" ;
                                             <https://rdf.ag/o/hops#alphaAcidsContent> "12-16.2" ;
                                             <https://rdf.ag/o/hops#betaAcidsContent> "5-7.3" ;
                                             <https://rdf.ag/o/hops#perceivedAroma> "Amer, Agrumes, Épicé, Terreux"@fr ,
                                                                                    "Bitter, Citrus, Earthy, Spicy"@en ;
                                             <https://rdf.ag/o/hops#totalOilContent> "2.6-3" .


###  https://rdf.ag/o/hops#HopsHallertau_NZ
<https://rdf.ag/o/hops#HopsHallertau_NZ> rdf:type owl:Class ;
                                         rdfs:subClassOf <https://rdf.ag/o/hops#HopsHallertau> ;
                                         <http://rdfs.org/ns/void#inDataset> <https://rdf.ag/o/hops#datasetdefinition> ;
                                         rdfs:isDefinedBy <https://rdf.ag/o/hops-2021-07-30> ;
                                         rdfs:label "Hallertau (NZ)"@en ,
                                                    "NNZ Hallertau"@en ,
                                                    "New Zealand Hallertauer"@en ;
                                         <http://www.w3.org/2004/02/skos/core#definition> "La variété néo-zélandaise de houblon Hallertau issue d'un croisement entre le Hallertau allemand d'origine et un houblon natif de Nouvelle-Zélande."@fr ,
                                                                                          "The New Zealand variety of Hallertau hops that was bred from a cross between the original German Hallertau and a New Zealand native hop."@en ;
                                         <http://xmlns.com/foaf/0.1/name> "Hallertau (NZ)" ;
                                         <https://rdf.ag/o/hops#alphaAcidsContent> "7-9" ;
                                         <https://rdf.ag/o/hops#betaAcidsContent> "5.8-8.5" ;
                                         <https://rdf.ag/o/hops#perceivedAroma> "Citron Vert, Floral"@fr ,
                                                                                "Floral, Lime"@en ;
                                         <https://rdf.ag/o/hops#totalOilContent> "0.9-1.1" .


###  https://rdf.ag/o/hops#HopsHallertau_Tradition
<https://rdf.ag/o/hops#HopsHallertau_Tradition> rdf:type owl:Class ;
                                                rdfs:subClassOf <https://rdf.ag/o/hops#HopsHallertau> ;
                                                <http://rdfs.org/ns/void#inDataset> <https://rdf.ag/o/hops#datasetdefinition> ;
                                                rdfs:isDefinedBy <https://rdf.ag/o/hops-2021-07-30> ;
                                                rdfs:label "German Tradition"@en ,
                                                           "H Tradition"@en ,
                                                           "Hallertau Tradition"@en ,
                                                           "Tradition"@en ;
                                                <http://www.w3.org/2004/02/skos/core#definition> "Hallertau Tradition a été sélectionné pour être plus résistant aux maladies et avoir une teneur en acide alpha plus élevée que ses parents : Hallertau Mittelfrüher, Hallertauer Gold et Saaz."@fr ,
                                                                                                 "Hallertau Tradition was bred to be more disease resistant and have a higher alpha acid content than its parents: Hallertau Mittelfrüher, Hallertauer Gold and Saaz."@en ;
                                                <http://xmlns.com/foaf/0.1/name> "Hallertau Tradition" ;
                                                <https://rdf.ag/o/hops#alphaAcidsContent> "4.6-7" ;
                                                <https://rdf.ag/o/hops#betaAcidsContent> "4-5" ;
                                                <https://rdf.ag/o/hops#totalOilContent> "0.9-1.9" .


###  https://rdf.ag/o/hops#HopsHallertau_US
<https://rdf.ag/o/hops#HopsHallertau_US> rdf:type owl:Class ;
                                         rdfs:subClassOf <https://rdf.ag/o/hops#HopsHallertau> ;
                                         <http://rdfs.org/ns/void#inDataset> <https://rdf.ag/o/hops#datasetdefinition> ;
                                         rdfs:isDefinedBy <https://rdf.ag/o/hops-2021-07-30> ;
                                         rdfs:label "Hallertau (US)"@en ,
                                                    "US Hallertau"@en ;
                                         <http://www.w3.org/2004/02/skos/core#definition> "Hallertau (US) est un houblon allemand Hallertau qui a été cultivé aux États-Unis et a donc des propriétés dues à la différence de climat et de terroir."@fr ,
                                                                                          "Hallertau (US) is a German Hallertau hop that was grown in the US and therefore has properties due to the difference in climate and terroir."@en ;
                                         <http://xmlns.com/foaf/0.1/name> "Hallertau (US)" ;
                                         <https://rdf.ag/o/hops#alphaAcidsContent> "3.5-5.5" ;
                                         <https://rdf.ag/o/hops#betaAcidsContent> "3.5-5.5" ;
                                         <https://rdf.ag/o/hops#perceivedAroma> "Floral, Spicy"@en ,
                                                                                "Épicé, Floral"@fr ;
                                         <https://rdf.ag/o/hops#totalOilContent> "0.6-1.0" .


###  https://rdf.ag/o/hops#HopsHelga
<https://rdf.ag/o/hops#HopsHelga> rdf:type owl:Class ;
                                  rdfs:subClassOf <https://rdf.ag/o/hops#HopsHallertau> ;
                                  <http://rdfs.org/ns/void#inDataset> <https://rdf.ag/o/hops#datasetdefinition> ;
                                  rdfs:isDefinedBy <https://rdf.ag/o/hops-2021-07-30> ;
                                  rdfs:label "Helga"@en ,
                                             "Southern Halltertau"@en ;
                                  <http://www.w3.org/2004/02/skos/core#definition> "Helga, or Southern Hallertau, is a descendant of Hallertau and was bred by Hop Products Australia in order to have similar 'noble hops' characteristics that could be grown in Australia."@en ,
                                                                                   "Helga, ou Southern Hallertau, est une descendante de Hallertau et a été élevée par Hop Products Australia afin d'avoir des caractéristiques de « houblon noble » similaires qui pourraient être cultivées en Australie."@fr ;
                                  <http://xmlns.com/foaf/0.1/name> "Helga" ;
                                  <https://rdf.ag/o/hops#alphaAcidsContent> "5.4-7.3" ;
                                  <https://rdf.ag/o/hops#betaAcidsContent> "5-7" ;
                                  <https://rdf.ag/o/hops#totalOilContent> "0.6-1.0 " .


###  https://rdf.ag/o/hops#HopsHerkules
<https://rdf.ag/o/hops#HopsHerkules> rdf:type owl:Class ;
                                     rdfs:subClassOf <https://rdf.ag/o/hops#HopsTaurus> ;
                                     <http://rdfs.org/ns/void#inDataset> <https://rdf.ag/o/hops#datasetdefinition> ;
                                     rdfs:isDefinedBy <https://rdf.ag/o/hops-2021-07-30> ;
                                     rdfs:label "Herkules"@en ;
                                     <http://www.w3.org/2004/02/skos/core#definition> "Herkules est un descendant de Taurus pour sa teneur élevée en acide alpha par l'Institut de recherche Hüll Hop et a été publié en 2005."@fr ,
                                                                                      "Herkules is a descendant of Taurus for its high alpha acid content by the Hüll Hop Research Institute and was released in 2005."@en ;
                                     <http://xmlns.com/foaf/0.1/name> "Herkules" ;
                                     <https://rdf.ag/o/hops#alphaAcidsContent> "12-17" ;
                                     <https://rdf.ag/o/hops#betaAcidsContent> "4-5.5" ;
                                     <https://rdf.ag/o/hops#perceivedAroma> "Black Pepper, Melon, Pine, Spicy"@en ,
                                                                            "Épicé, Melon, Pin, Poivre Noir"@fr ;
                                     <https://rdf.ag/o/hops#totalOilContent> "1.4-2.4" .


###  https://rdf.ag/o/hops#HopsHersbrucker
<https://rdf.ag/o/hops#HopsHersbrucker> rdf:type owl:Class ;
                                        rdfs:subClassOf <https://rdf.ag/o/hops#Hops> ;
                                        <http://rdfs.org/ns/void#inDataset> <https://rdf.ag/o/hops#datasetdefinition> ;
                                        rdfs:isDefinedBy <https://rdf.ag/o/hops-2021-07-30> ;
                                        rdfs:label "Hersbrucker"@en ,
                                                   "Hersbrucker Late"@en ,
                                                   "Hersbrucker Spaet"@en ,
                                                   "Hersbrucker Spat"@en ,
                                                   "Hersbrucker Spät"@en ,
                                                   "Hersbrucker-G"@en ;
                                        <http://www.w3.org/2004/02/skos/core#definition> "Hersbrucker est une variété allemande de houblon qui a été sélectionnée en remplacement du Hallertau Mittelfrüh et pour être plus résistante à la flétrissure verticillienne."@fr ,
                                                                                         "Hersbrucker is a German variety of hops that was bred as a replacement to Hallertau Mittelfrüh and to be more resistant to verticillium wilt."@en ;
                                        <http://xmlns.com/foaf/0.1/name> "Hersbrucker" ;
                                        <https://rdf.ag/o/hops#alphaAcidsContent> "2-5" ;
                                        <https://rdf.ag/o/hops#betaAcidsContent> "4-6" ;
                                        <https://rdf.ag/o/hops#perceivedAroma> "Floral, Fruity, Spicy"@en ,
                                                                               "Épicé, Floral, Fruité"@fr ;
                                        <https://rdf.ag/o/hops#totalOilContent> "0.5-1.3" .


###  https://rdf.ag/o/hops#HopsHersbrucker_E
<https://rdf.ag/o/hops#HopsHersbrucker_E> rdf:type owl:Class ;
                                          rdfs:subClassOf <https://rdf.ag/o/hops#Hops> ;
                                          <http://rdfs.org/ns/void#inDataset> <https://rdf.ag/o/hops#datasetdefinition> ;
                                          rdfs:isDefinedBy <https://rdf.ag/o/hops-2021-07-30> ;
                                          rdfs:label "Hersbrucker E"@en ,
                                                     "Hersbrucker England"@en ;
                                          <http://www.w3.org/2004/02/skos/core#definition> "Hersbrucker E est presque identique à la variété allemande d'origine, mais peut présenter des variations de propriétés en raison des différences de terroir et de climat par rapport à sa culture en Angleterre."@fr ,
                                                                                           "Hersbrucker E is nearly identical to the original German variety but may have some variations in properties due to differences in terroir and climate from being grown in England."@en ;
                                          <http://xmlns.com/foaf/0.1/name> "Hersbrucker E" ;
                                          <https://rdf.ag/o/hops#alphaAcidsContent> "4-6" ;
                                          <https://rdf.ag/o/hops#betaAcidsContent> "5-7" ;
                                          <https://rdf.ag/o/hops#totalOilContent> "0.63" .


###  https://rdf.ag/o/hops#HopsHersbrucker_Pure
<https://rdf.ag/o/hops#HopsHersbrucker_Pure> rdf:type owl:Class ;
                                             rdfs:subClassOf <https://rdf.ag/o/hops#Hops> ;
                                             <http://rdfs.org/ns/void#inDataset> <https://rdf.ag/o/hops#datasetdefinition> ;
                                             rdfs:isDefinedBy <https://rdf.ag/o/hops-2021-07-30> ;
                                             rdfs:label "Hersbrucker Pure"@en ;
                                             <http://www.w3.org/2004/02/skos/core#definition> "Hersbrucker Pure est le résultat du croisement entre Hallertau Mittelfrüh, Saaz et un houblon sauvage allemand afin de produire un agréable arôme de houblon 'noble'."@fr ,
                                                                                              "Hersbrucker Pure is a result of the cross between Hallertau Mittelfrüh, Saaz and a wild German hop in order to produce a pleasing 'noble' hop aroma."@en ;
                                             <http://xmlns.com/foaf/0.1/name> "Hersbrucker Pure" ;
                                             <https://rdf.ag/o/hops#alphaAcidsContent> "4.7-6" ;
                                             <https://rdf.ag/o/hops#betaAcidsContent> "2-3" ;
                                             <https://rdf.ag/o/hops#totalOilContent> "0.6-1.2" .


###  https://rdf.ag/o/hops#HopsHersbrucker_Red-Stem
<https://rdf.ag/o/hops#HopsHersbrucker_Red-Stem> rdf:type owl:Class ;
                                                 rdfs:subClassOf <https://rdf.ag/o/hops#Hops> ;
                                                 <http://rdfs.org/ns/void#inDataset> <https://rdf.ag/o/hops#datasetdefinition> ;
                                                 rdfs:isDefinedBy <https://rdf.ag/o/hops-2021-07-30> ;
                                                 rdfs:label "Hersbrucker Red-Stem"@en ;
                                                 <http://www.w3.org/2004/02/skos/core#definition> "Hersbrucker Red-Stem est une émanation clonale de l'original allemand Hersbrucker. Alors que tous les houblons Hersbrucker ont des tiges rouges, cette variété particulière de houblon a une tige qui est plus rouge et a peut-être une teneur en acide alpha plus élevée que les autres Hersbrucker."@fr ,
                                                                                                  "Hersbrucker Red-Stem is a clonal offshoot of the original German Hersbrucker. While all Hersbrucker hops have red stems, this particular variety of hop has a stem that is more prominently red and possibly has a higher alpha acid content than other Hersbruckers."@en ;
                                                 <http://xmlns.com/foaf/0.1/name> "Hersbrucker Red-Stem" ;
                                                 <https://rdf.ag/o/hops#alphaAcidsContent> "5-6" ;
                                                 <https://rdf.ag/o/hops#betaAcidsContent> "5-6" ;
                                                 <https://rdf.ag/o/hops#totalOilContent> "1.20" .


###  https://rdf.ag/o/hops#HopsHorizon
<https://rdf.ag/o/hops#HopsHorizon> rdf:type owl:Class ;
                                    rdfs:subClassOf <https://rdf.ag/o/hops#Hops> ;
                                    <http://rdfs.org/ns/void#inDataset> <https://rdf.ag/o/hops#datasetdefinition> ;
                                    rdfs:isDefinedBy <https://rdf.ag/o/hops-2021-07-30> ;
                                    rdfs:label "Horizon"@en ;
                                    <http://www.w3.org/2004/02/skos/core#definition> "Horizon hops is a versatile hops that was created in Corvallis, Oregon, USA in 1970 from a cross between Brewer's Gold and an Early Green-unknown male hop and Zattler seedling."@en ,
                                                                                     "Le houblon Horizon est un houblon polyvalent qui a été créé à Corvallis, Oregon, États-Unis en 1970 à partir d'un croisement entre Brewer's Gold et un houblon mâle Early Green-inconnu et un semis Zattler."@fr ;
                                    <http://xmlns.com/foaf/0.1/isPrimaryTopicOf> <https://rdf.ag/o/hops#cropsci1999.0011183X003900030052x> ;
                                    <http://xmlns.com/foaf/0.1/name> "Horizon" ;
                                    <https://rdf.ag/o/hops#alphaAcidsContent> "8.8-16.5" ;
                                    <https://rdf.ag/o/hops#betaAcidsContent> "5.5-8.5" ;
                                    <https://rdf.ag/o/hops#perceivedAroma> "Agrumes, Floral"@fr ,
                                                                           "Citrus, Floral"@en ;
                                    <https://rdf.ag/o/hops#totalOilContent> "0.8-1.22" .


###  https://rdf.ag/o/hops#HopsHuellMelon
<https://rdf.ag/o/hops#HopsHuellMelon> rdf:type owl:Class ;
                                       rdfs:subClassOf <https://rdf.ag/o/hops#Hops> ;
                                       <http://rdfs.org/ns/void#inDataset> <https://rdf.ag/o/hops#datasetdefinition> ;
                                       rdfs:isDefinedBy <https://rdf.ag/o/hops-2021-07-30> ;
                                       rdfs:label "Huell Melon"@en ,
                                                  "Hüll Melon"@en ;
                                       <http://www.w3.org/2004/02/skos/core#definition> "Huell Melon est une fille de Cascade, connue principalement pour son arôme de melon. Ce cultivar est sorti en 2012."@fr ,
                                                                                        "Huell Melon is a daughter of Cascade, known primarily for its melon aroma. This cultivar was released in 2012."@en ;
                                       <http://xmlns.com/foaf/0.1/name> "Huell Melon" ;
                                       <https://rdf.ag/o/hops#alphaAcidsContent> "6.9-7.5" ;
                                       <https://rdf.ag/o/hops#betaAcidsContent> "7.3-7.9" ;
                                       <https://rdf.ag/o/hops#perceivedAroma> "Abricot, Fraise, Melon Miel"@fr ,
                                                                              "Apricot, Honeydew Melon, Strawberry"@en ;
                                       <https://rdf.ag/o/hops#totalOilContent> "0.8" .


###  https://rdf.ag/o/hops#HopsJarrylo
<https://rdf.ag/o/hops#HopsJarrylo> rdf:type owl:Class ;
                                    rdfs:subClassOf <https://rdf.ag/o/hops#Hops> ;
                                    <http://rdfs.org/ns/void#inDataset> <https://rdf.ag/o/hops#datasetdefinition> ;
                                    rdfs:isDefinedBy <https://rdf.ag/o/hops-2021-07-30> ;
                                    rdfs:label "Jarrylo™"@en ,
                                               "Jaryllo"@en ;
                                    <http://www.w3.org/2004/02/skos/core#definition> "Jarrylo™ hops, named after the Slavic God Jarilo of fertility, vegetation, springtime, and war; was bred by the American Dwarf Hop Association from a descendant of Summit. Jarrylo™ was released commercially in 2013."@en ,
                                                                                     "Le houblon Jarrylo™, du nom du dieu slave Jarilo de la fertilité, de la végétation, du printemps et de la guerre ; a été élevé par l'American Dwarf Hop Association à partir d'un descendant de Summit. Jarrylo™ a été commercialisé en 2013."@fr ;
                                    <http://xmlns.com/foaf/0.1/name> "Jarrylo™" ;
                                    <https://rdf.ag/o/hops#alphaAcidsContent> "15–17" ;
                                    <https://rdf.ag/o/hops#betaAcidsContent> "6.0–7.5" ;
                                    <https://rdf.ag/o/hops#perceivedAroma> "Banana, Orange, Pear, Spice"@en ,
                                                                           "Banane, Épice, Orange, Poire"@fr ;
                                    <https://rdf.ag/o/hops#totalOilContent> "3.6–4.3" .


###  https://rdf.ag/o/hops#HopsJester
<https://rdf.ag/o/hops#HopsJester> rdf:type owl:Class ;
                                   rdfs:subClassOf <https://rdf.ag/o/hops#Hops> ;
                                   <http://rdfs.org/ns/void#inDataset> <https://rdf.ag/o/hops#datasetdefinition> ;
                                   rdfs:isDefinedBy <https://rdf.ag/o/hops-2021-07-30> ;
                                   rdfs:label "Jester®"@en ;
                                   <http://www.w3.org/2004/02/skos/core#definition> "Jester® est une fille de Cascade développée par le Charles Faram Hop Development Programme. Il a été commercialisé en 2013 par Charles Faram and Co Ltd."@fr ,
                                                                                    "Jester® is a daughter of Cascade developed by the Charles Faram Hop Development Programme in the UK. It was released commercially in 2013 by Charles Faram and Co Ltd."@en ;
                                   <http://xmlns.com/foaf/0.1/name> "Jester®" ;
                                   <https://rdf.ag/o/hops#alphaAcidsContent> "7-9" ;
                                   <https://rdf.ag/o/hops#betaAcidsContent> "4-6" ;
                                   <https://rdf.ag/o/hops#perceivedAroma> "Blackcurrant, Grapefruit, Lychee"@en ,
                                                                          "Cassis, Litchi, Pamplemousse"@fr ;
                                   <https://rdf.ag/o/hops#totalOilContent> "0.6-1.2" .


###  https://rdf.ag/o/hops#HopsLiberty
<https://rdf.ag/o/hops#HopsLiberty> rdf:type owl:Class ;
                                    rdfs:subClassOf <https://rdf.ag/o/hops#Hops> ;
                                    <http://rdfs.org/ns/void#inDataset> <https://rdf.ag/o/hops#datasetdefinition> ;
                                    rdfs:isDefinedBy <https://rdf.ag/o/hops-2021-07-30> ;
                                    rdfs:label "Liberty"@en ;
                                    <http://www.w3.org/2004/02/skos/core#definition> """Le houblon Liberty est le résultat d'un croisement entre Hallertau Mittelfrüher et un résistant au mildiou
      Masculin. C'est la demi-soeur de Crystal, Ultra et Mt. Hood et est le premier type de houblon « noble aromatique » à être cultivé aux États-Unis."""@fr ,
                                                                                     """Liberty hops are the result of a cross between Hallertau Mittelfrüher and a Downy Mildew resistant
      male. It is the half-sister to Crystal, Ultra and Mt. Hood and is the first 'noble aromatic' type of hops to be grown in the US."""@en ;
                                    <http://xmlns.com/foaf/0.1/isPrimaryTopicOf> <https://rdf.ag/o/hops#ropsci1992.0011183X003200040056x> ;
                                    <http://xmlns.com/foaf/0.1/name> "Liberty" ;
                                    <https://rdf.ag/o/hops#alphaAcidsContent> "3-6" ;
                                    <https://rdf.ag/o/hops#betaAcidsContent> "3.5" ;
                                    <https://rdf.ag/o/hops#perceivedAroma> "Citron, Épicé, Terreux"@fr ,
                                                                           "Lemon, Earthy, Spicy"@en ;
                                    <https://rdf.ag/o/hops#totalOilContent> "1.3" .


###  https://rdf.ag/o/hops#HopsMagnum
<https://rdf.ag/o/hops#HopsMagnum> rdf:type owl:Class ;
                                   rdfs:subClassOf <https://rdf.ag/o/hops#HopsHallertau> ;
                                   <http://rdfs.org/ns/void#inDataset> <https://rdf.ag/o/hops#datasetdefinition> ;
                                   rdfs:isDefinedBy <https://rdf.ag/o/hops-2021-07-30> ;
                                   rdfs:label "Hallertauer Magnum"@en ,
                                              "Magnum"@en ;
                                   <http://www.w3.org/2004/02/skos/core#definition> "Hallertauer Magnum, or Magnum, is a German hop variety that is known for its high bitterness. It was officially released in 1980 and created at German Hop Institute in Hull from a cross between Galena and a German male that is 50% Hallertau."@en ,
                                                                                    "Hallertauer Magnum, ou Magnum, est une variété de houblon allemand connue pour sa forte amertume. Il a été officiellement publié en 1980 et créé au German Hop Institute à Hull à partir d'un croisement entre Galena et un mâle allemand inconnu."@fr ;
                                   <http://xmlns.com/foaf/0.1/name> "Hallertauer Magnum" ;
                                   <https://rdf.ag/o/hops#alphaAcidsContent> "12.0–14.0" ;
                                   <https://rdf.ag/o/hops#betaAcidsContent> "4.5–5.5" ;
                                   <https://rdf.ag/o/hops#perceivedAroma> "Agrumes, Amer"@fr ,
                                                                          "Bitter, Citrus"@en ;
                                   <https://rdf.ag/o/hops#totalOilContent> "1.9-2.3" .


###  https://rdf.ag/o/hops#HopsMagnumUS
<https://rdf.ag/o/hops#HopsMagnumUS> rdf:type owl:Class ;
                                     rdfs:subClassOf <https://rdf.ag/o/hops#HopsMagnum> ;
                                     <http://rdfs.org/ns/void#inDataset> <https://rdf.ag/o/hops#datasetdefinition> ;
                                     rdfs:isDefinedBy <https://rdf.ag/o/hops-2021-07-30> ;
                                     rdfs:label "Hallertauer Magnum (US)"@en ,
                                                "Magnum (US)"@en ;
                                     <http://www.w3.org/2004/02/skos/core#definition> "Magnum, or Hallertauer Magnum, is a German hops cultivar from the cross between Galena and a native German hop. While genetically identical, Magnum that is grown in the US will have different characteristics due to the terroir and environmental differences in the US. It was received by the USDA in 1992. It is well known as a bittering hop due to its high alpha and cohumulone content."@en ,
                                                                                      "Magnum, ou Hallertauer Magnum, est un cultivar de houblon allemand issu du croisement entre la galène et un houblon allemand natif. Bien que génétiquement identique, le Magnum cultivé aux États-Unis aura des caractéristiques différentes en raison du terroir et des différences environnementales aux États-Unis. Il a été reçu par l'USDA en 1992. Il est bien connu comme houblon amer en raison de sa teneur élevée en alpha et en cohumulone."@fr ;
                                     <http://xmlns.com/foaf/0.1/name> "Hallertauer Magnumn (US)" ;
                                     <https://rdf.ag/o/hops#alphaAcidsContent> "12.0–14.0" ;
                                     <https://rdf.ag/o/hops#betaAcidsContent> "4.5–6.0" ;
                                     <https://rdf.ag/o/hops#perceivedAroma> "No distinct aroma"@en ,
                                                                            "Pas d'arôme distinct"@fr ;
                                     <https://rdf.ag/o/hops#totalOilContent> "1.9-2.3" .


###  https://rdf.ag/o/hops#HopsMandarinaBavaria
<https://rdf.ag/o/hops#HopsMandarinaBavaria> rdf:type owl:Class ;
                                             rdfs:subClassOf <https://rdf.ag/o/hops#Hops> ;
                                             <http://rdfs.org/ns/void#inDataset> <https://rdf.ag/o/hops#datasetdefinition> ;
                                             rdfs:isDefinedBy <https://rdf.ag/o/hops-2021-07-30> ;
                                             rdfs:label "Mandarina Bavaria"@en ;
                                             <http://www.w3.org/2004/02/skos/core#definition> "Le Mandarina Bavaria est un houblon originaire de Hüll, en Allemagne, issu d'un croisement entre Cascade (US), Hallertau Blanc et Hüll Melon."@fr ,
                                                                                              "Mandarina Bavaria is hop that originates from Hüll, Germany and is the product of a cross between Cascade (US), Hallertau Blanc and Hüll Melon."@en ;
                                             <http://xmlns.com/foaf/0.1/name> "Mandarina Bavaria" ;
                                             <https://rdf.ag/o/hops#alphaAcidsContent> "8.5-10.5" ;
                                             <https://rdf.ag/o/hops#betaAcidsContent> "5-6.5" ;
                                             <https://rdf.ag/o/hops#perceivedAroma> "Agrumes, Mandarine, Sucré"@fr ,
                                                                                    "Citrus, Sweet, Tangerine"@en ;
                                             <https://rdf.ag/o/hops#totalOilContent> "2.0" .


###  https://rdf.ag/o/hops#HopsMeridian
<https://rdf.ag/o/hops#HopsMeridian> rdf:type owl:Class ;
                                     rdfs:subClassOf <https://rdf.ag/o/hops#Hops> ;
                                     <http://rdfs.org/ns/void#inDataset> <https://rdf.ag/o/hops#datasetdefinition> ;
                                     rdfs:isDefinedBy <https://rdf.ag/o/hops-2021-07-30> ;
                                     rdfs:label "Meridian®"@en ;
                                     <http://www.w3.org/2004/02/skos/core#definition> "Le houblon Meridian® est un houblon américain déposé par Indie Hops, LLC. en 2014"@fr ,
                                                                                      "Meridian® hops is a US hop trademarked by Indie Hops, LLC. in 2014"@en ;
                                     <http://xmlns.com/foaf/0.1/name> "Meridian®" ;
                                     <https://rdf.ag/o/hops#alphaAcidsContent> "6.0-7.0" ;
                                     <https://rdf.ag/o/hops#betaAcidsContent> "6.0-9.0" ;
                                     <https://rdf.ag/o/hops#perceivedAroma> "Baies Mixtes, Citron, Fruits Tropicaux"@fr ,
                                                                            "Lemon, Mixed Berries, Tropical Fruit"@en ;
                                     <https://rdf.ag/o/hops#totalOilContent> "1.0-1.4" .


###  https://rdf.ag/o/hops#HopsMillennium
<https://rdf.ag/o/hops#HopsMillennium> rdf:type owl:Class ;
                                       rdfs:subClassOf <https://rdf.ag/o/hops#Hops> ;
                                       <http://rdfs.org/ns/void#inDataset> <https://rdf.ag/o/hops#datasetdefinition> ;
                                       rdfs:isDefinedBy <https://rdf.ag/o/hops-2021-07-30> ;
                                       rdfs:label "Millennium"@en ;
                                       <http://www.w3.org/2004/02/skos/core#definition> "Millennium a été libéré en 2000 du programme d'élevage John I. Haas. Il est principalement utilisé comme houblon amer et est un descendant de Nugget."@fr ,
                                                                                        "Millennium was released in 2000 from the John I. Haas Breeding Program. It is mostly used as a bittering hop and is a descendant from Nugget."@en ;
                                       <http://xmlns.com/foaf/0.1/name> "Millennium" ;
                                       <https://rdf.ag/o/hops#alphaAcidsContent> "14.5-16.5" ;
                                       <https://rdf.ag/o/hops#betaAcidsContent> "4.3–5.3" ;
                                       <https://rdf.ag/o/hops#perceivedAroma> "Herbaceous, Resin"@en ,
                                                                              "Herbacé, Résine"@fr ;
                                       <https://rdf.ag/o/hops#totalOilContent> "1.8-2.2" .


###  https://rdf.ag/o/hops#HopsMosaic
<https://rdf.ag/o/hops#HopsMosaic> rdf:type owl:Class ;
                                   rdfs:subClassOf <https://rdf.ag/o/hops#Hops> ;
                                   <http://rdfs.org/ns/void#inDataset> <https://rdf.ag/o/hops#datasetdefinition> ;
                                   rdfs:isDefinedBy <https://rdf.ag/o/hops-2021-07-30> ;
                                   rdfs:label "HBC369"@en ,
                                              "Mosaic®"@en ;
                                   <http://www.w3.org/2004/02/skos/core#definition> "Mosaic® est une variété de houblon brevetée par la Hop Breeding Company, L.L.C. et a été développé par Eugene G. Probasco et Jason Perrault."@fr ,
                                                                                    "Mosaic® is a hop variety patented by the Hop Breeding Company, L.L.C. and was developed by Eugene G. Probasco and Jason Perrault."@en ;
                                   <http://xmlns.com/foaf/0.1/isPrimaryTopicOf> <https://rdf.ag/o/hops#10.1094-ASBCJ-2017-1720-01> ;
                                   <http://xmlns.com/foaf/0.1/name> "Mosaic®" ;
                                   <https://rdf.ag/o/hops#alphaAcidsContent> "11.5-13.5" ;
                                   <https://rdf.ag/o/hops#betaAcidsContent> "3.2-3.9" ;
                                   <https://rdf.ag/o/hops#perceivedAroma> "Agrumes, Floral, Myrtille, Terreux, Tropical"@fr ,
                                                                          "Blueberry, Citrus, Earthy, Floral, Tropical"@en ;
                                   <https://rdf.ag/o/hops#totalOilContent> "1-1.5" .


###  https://rdf.ag/o/hops#HopsMotueka
<https://rdf.ag/o/hops#HopsMotueka> rdf:type owl:Class ;
                                    rdfs:subClassOf <https://rdf.ag/o/hops#Hops> ;
                                    <http://rdfs.org/ns/void#inDataset> <https://rdf.ag/o/hops#datasetdefinition> ;
                                    rdfs:isDefinedBy <https://rdf.ag/o/hops-2021-07-30> ;
                                    rdfs:label "B Saaz"@en ,
                                               "Belgian Saaz"@en ,
                                               "Motueka"@en ;
                                    <http://www.w3.org/2004/02/skos/core#definition> "Motueka est un houblon néo-zélandais développé par HortResearch. C'est un houblon triploïde qui est le résultat d'un croisement entre Saaz et un houblon natif de Nouvelle-Zélande."@fr ,
                                                                                     "Motueka is a New Zealand hop developed by HortResearch. It is a triploid hop that is the result of a cross between Saaz and a New Zealand native hop."@en ;
                                    <http://xmlns.com/foaf/0.1/name> "Motueka" ;
                                    <https://rdf.ag/o/hops#alphaAcidsContent> "6.5-8.5" ;
                                    <https://rdf.ag/o/hops#betaAcidsContent> "5-5.5" ;
                                    <https://rdf.ag/o/hops#perceivedAroma> "Agrumes, Citron, Citron Vert, Floral, Fruits Tropicaux"@fr ,
                                                                           "Citrus, Floral, Lemon, Lime, Tropical Fruit"@en ;
                                    <https://rdf.ag/o/hops#totalOilContent> "0.8" .


###  https://rdf.ag/o/hops#HopsMountHood
<https://rdf.ag/o/hops#HopsMountHood> rdf:type owl:Class ;
                                      rdfs:subClassOf <https://rdf.ag/o/hops#Hops> ;
                                      <http://rdfs.org/ns/void#inDataset> <https://rdf.ag/o/hops#datasetdefinition> ;
                                      rdfs:isDefinedBy <https://rdf.ag/o/hops-2021-07-30> ;
                                      rdfs:label "Mount Hood"@en ,
                                                 "Mt Hood"@en ,
                                                 "Mt. Hood"@en ;
                                      <http://www.w3.org/2004/02/skos/core#definition> "Mount Hood est le résultat d'un croisement entre Hallertau Mittelfruh et un mâle natif des États-Unis en 1983. C'est la demi-sœur de Crystal, Ultra et Liberty. En 1985, Mount Hood a reçu le numéro USDA 21455."@fr ,
                                                                                       "Mount Hood is the result of a cross between Hallertau Mittelfruh and native US male in 1983. It is the half-sister to Crystal, Ultra and Liberty. In 1985, Mount Hood was assigned the USDA number 21455."@en ;
                                      <http://xmlns.com/foaf/0.1/name> "Mount Hood" ;
                                      <https://rdf.ag/o/hops#alphaAcidsContent> "4-8" ;
                                      <https://rdf.ag/o/hops#betaAcidsContent> "5-8" ;
                                      <https://rdf.ag/o/hops#perceivedAroma> "Citron, Estragon, Fenouil, Herbes, Miel, Pamplemousse"@fr ,
                                                                             "Grapefruit, Fennel, Herbal, Honey, Lemon, Tarragon"@en ;
                                      <https://rdf.ag/o/hops#totalOilContent> "1-1.7" .


###  https://rdf.ag/o/hops#HopsMountRainier
<https://rdf.ag/o/hops#HopsMountRainier> rdf:type owl:Class ;
                                         rdfs:subClassOf <https://rdf.ag/o/hops#Hops> ;
                                         <http://rdfs.org/ns/void#inDataset> <https://rdf.ag/o/hops#datasetdefinition> ;
                                         rdfs:isDefinedBy <https://rdf.ag/o/hops-2021-07-30> ;
                                         rdfs:label "Mount Rainier"@en ;
                                         <http://www.w3.org/2004/02/skos/core#definition> "Mount Hood est le résultat d'un croisement entre Hallertau Mittelfruh et un mâle natif des États-Unis en 1983. C'est la demi-sœur de Crystal, Ultra et Liberty. En 1985, Mount Hood a reçu le numéro USDA 21455."@fr ,
                                                                                          "Mount Rainier is the product of Magnum and a native US male from the the USDA-ARS hop breeding program in collaboration with Oregon State University. This is hop is named after an active volcano in Washington State."@en ;
                                         <http://xmlns.com/foaf/0.1/name> "Mount Rainier" ;
                                         <https://rdf.ag/o/hops#alphaAcidsContent> "5-8.1" ;
                                         <https://rdf.ag/o/hops#betaAcidsContent> "5-7" ;
                                         <https://rdf.ag/o/hops#perceivedAroma> "Agrumes, Réglisse"@fr ,
                                                                                "Citrus, Licorice"@en .


###  https://rdf.ag/o/hops#HopsNelsonSauvin
<https://rdf.ag/o/hops#HopsNelsonSauvin> rdf:type owl:Class ;
                                         rdfs:subClassOf <https://rdf.ag/o/hops#Hops> ;
                                         <http://rdfs.org/ns/void#inDataset> <https://rdf.ag/o/hops#datasetdefinition> ;
                                         rdfs:isDefinedBy <https://rdf.ag/o/hops-2021-07-30> ;
                                         rdfs:label "Nelson Sauvin™"@en ;
                                         <http://www.w3.org/2004/02/skos/core#definition> "Nelson Sauvin™ est un houblon néo-zélandais déposé en 2000. Son nom est un dérivé du cépage Sauvignon Blanc, auquel beaucoup comparent son arôme."@fr ,
                                                                                          "Nelson Sauvin™ is a trademarked hop from New Zealand that was released in 2000. Its name is a derivative of Sauvignon Blanc wine grape, to which many compare its aroma."@en ;
                                         <http://xmlns.com/foaf/0.1/name> "Nelson Sauvin™" ;
                                         <https://rdf.ag/o/hops#alphaAcidsContent> "12-13" ;
                                         <https://rdf.ag/o/hops#betaAcidsContent> "6-8" ;
                                         <https://rdf.ag/o/hops#perceivedAroma> "Fruity, Grapefruit, Gooseberry, White Wine"@en ,
                                                                                "Fruité, Groseille, Pamplemousse, Vin Blanc"@fr ;
                                         <https://rdf.ag/o/hops#totalOilContent> "1.1" .


###  https://rdf.ag/o/hops#HopsNewport
<https://rdf.ag/o/hops#HopsNewport> rdf:type owl:Class ;
                                    rdfs:subClassOf <https://rdf.ag/o/hops#Hops> ;
                                    <http://rdfs.org/ns/void#inDataset> <https://rdf.ag/o/hops#datasetdefinition> ;
                                    rdfs:isDefinedBy <https://rdf.ag/o/hops-2021-07-30> ;
                                    rdfs:label "Newport"@en ,
                                               "Newport"@fr ;
                                    <http://www.w3.org/2004/02/skos/core#definition> """Newport est un houblon amer à haute teneur en acides alpha et bêta, développé par l'USDA-ARS et ayant reçu son numéro d'accession en 2000.
      
      Ce houblon est le résultat du croisement entre Hallertauer 'Magnum' et USDA 58111M en tant que nouveau houblon amer résistant aux maladies multiples."""@fr ,
                                                                                     """Newport is a bittering hop with high alpha and beta acid content, developed by the USDA-ARS and recieving its accession number in 2000.
      
      This hop is the result of the cross between Hallertauer 'Magnum' and USDA 58111M as a new multiple disease-resistant bittering hop."""@en ;
                                    <http://xmlns.com/foaf/0.1/isPrimaryTopicOf> <https://rdf.ag/o/hops#Henning2004> ;
                                    <http://xmlns.com/foaf/0.1/name> "Newport" ;
                                    <https://rdf.ag/o/hops#alphaAcidsContent> "13.5–17.0" ;
                                    <https://rdf.ag/o/hops#betaAcidsContent> "7.2–9.1" ;
                                    <https://rdf.ag/o/hops#perceivedAroma> "Balsamique, Vin"@fr ,
                                                                           "Wine, Balsamic"@en ;
                                    <https://rdf.ag/o/hops#totalOilContent> "1.6-3.4" .


###  https://rdf.ag/o/hops#HopsNorthdown
<https://rdf.ag/o/hops#HopsNorthdown> rdf:type owl:Class ;
                                      rdfs:subClassOf <https://rdf.ag/o/hops#Hops> ;
                                      <http://rdfs.org/ns/void#inDataset> <https://rdf.ag/o/hops#datasetdefinition> ;
                                      rdfs:isDefinedBy <https://rdf.ag/o/hops-2021-07-30> ;
                                      rdfs:label "Northdown"@en ,
                                                 "Wye Northdown"@en ;
                                      <http://www.w3.org/2004/02/skos/core#definition> "Northdown a été élevé au Wye College par le Dr Ray A. Neve en 1961 pour être plus résistant au mildiou. Il a été obtenu à partir d'une femelle Northern Brewer et d'un houblon mâle résistant au mildiou."@fr ,
                                                                                       "Northdown was bred at Wye College by Dr. Ray A. Neve in 1961 to be more resistant to Downy Mildew. It was bred from a Northern Brewer female and a Downy Mildew resistant male hops."@en ;
                                      <http://xmlns.com/foaf/0.1/name> "Northdown" ;
                                      <https://rdf.ag/o/hops#alphaAcidsContent> "7-10" ;
                                      <https://rdf.ag/o/hops#betaAcidsContent> "4-5.5" ;
                                      <https://rdf.ag/o/hops#perceivedAroma> "Baie, Épicé, Floral, Pin"@fr ,
                                                                             "Berry, Floral, Pine, Spicy"@en ;
                                      <https://rdf.ag/o/hops#totalOilContent> "1.2-2.5" .


###  https://rdf.ag/o/hops#HopsNorthernBrewer
<https://rdf.ag/o/hops#HopsNorthernBrewer> rdf:type owl:Class ;
                                           rdfs:subClassOf <https://rdf.ag/o/hops#Hops> ;
                                           <http://rdfs.org/ns/void#inDataset> <https://rdf.ag/o/hops#datasetdefinition> ;
                                           rdfs:isDefinedBy <https://rdf.ag/o/hops-2021-07-30> ;
                                           rdfs:label "Northern Brewer"@en ;
                                           <http://www.w3.org/2004/02/skos/core#definition> "Northern Brewer a été développé par le professeur Salmon au Wye College, Royaume-Uni en 1934 en croisant un East Kent Golding et un Brewer's Gold. Elle est identique à la variété cultivée en Allemagne; cependant, il est génétiquement différent de la version Américaine."@fr ,
                                                                                            "Northern Brewer was developed by Professor Salmon at Wye College, UK in 1934 by crossing an East Kent Golding and a Brewer's Gold. It is identical to the variety grown in Germany; however, it is genetically different from the US version."@en ;
                                           <http://xmlns.com/foaf/0.1/name> "Northern Brewer" ;
                                           <https://rdf.ag/o/hops#alphaAcidsContent> "9.5" ;
                                           <https://rdf.ag/o/hops#betaAcidsContent> "4" ;
                                           <https://rdf.ag/o/hops#perceivedAroma> "Herbal, Mint, Resin, Spicy"@en ,
                                                                                  "Épicé, Herbal, Menthe, Résine"@fr ;
                                           <https://rdf.ag/o/hops#totalOilContent> "1.61" .


###  https://rdf.ag/o/hops#HopsNorthernBrewer_US
<https://rdf.ag/o/hops#HopsNorthernBrewer_US> rdf:type owl:Class ;
                                              rdfs:subClassOf <https://rdf.ag/o/hops#Hops> ;
                                              <http://rdfs.org/ns/void#inDataset> <https://rdf.ag/o/hops#datasetdefinition> ;
                                              rdfs:isDefinedBy <https://rdf.ag/o/hops-2021-07-30> ;
                                              rdfs:label "Northern Brewer (US)"@en ;
                                              <http://www.w3.org/2004/02/skos/core#definition> "Northern Brewer a été développé par le professeur Salmon au Wye College, Royaume-Uni en 1934 en croisant un East Kent Golding et un Brewer's Gold. Elle diffère de la Northern Brewer originale car elle a subi une pollinisation croisée à partir de variétés indigènes Américaines et est donc plus adaptée aux climats Nord-Américains."@fr ,
                                                                                               "Northern Brewer was developed by Professor Salmon at Wye College, UK in 1934 by crossing an East Kent Golding and a Brewer's Gold. It differs from the original Northern Brewer as it has undergone cross pollination from native American varieties and thus is more suited for North American climates."@en ;
                                              <http://xmlns.com/foaf/0.1/name> "Northern Brewer (US)" ;
                                              <https://rdf.ag/o/hops#alphaAcidsContent> "8-10" ;
                                              <https://rdf.ag/o/hops#betaAcidsContent> "3-5" ;
                                              <https://rdf.ag/o/hops#totalOilContent> "1.5-2" .


###  https://rdf.ag/o/hops#HopsNugget
<https://rdf.ag/o/hops#HopsNugget> rdf:type owl:Class ;
                                   rdfs:subClassOf <https://rdf.ag/o/hops#Hops> ;
                                   <http://rdfs.org/ns/void#inDataset> <https://rdf.ag/o/hops#datasetdefinition> ;
                                   rdfs:isDefinedBy <https://rdf.ag/o/hops-2021-07-30> ;
                                   rdfs:label "Nugget"@en ,
                                              "Nugget"@fr ;
                                   <http://www.w3.org/2004/02/skos/core#definition> """Nugget est un houblon amer connu pour sa teneur élevée en alpha tout en ayant une faible teneur en bêta et en cohumolone. Par conséquent, ce houblon est un houblon approprié pour ajouter une base amère aux bières.
      
      Il a été élevé en 1970 à Corvallis, Oregon (alors appelé 7005-194), descendant de Brewer's Gold et East Kent Golding; son numéro d'accession lui a été attribué en 1978."""@fr ,
                                                                                    """Nugget is a bittering hop known for its high alpha content while having a low beta and cohumolone content. Therefore, this hop is a suitable hop to add bitter base to ales.
      
      It was bred in 1970 in Corvallis, Oregon (then called 7005-194), decending from Brewer's Gold and East Kent Golding; its accession number was assigned in 1978."""@en ;
                                   <http://xmlns.com/foaf/0.1/name> "Nugget" ;
                                   <https://rdf.ag/o/hops#alphaAcidsContent> "11.5–14.0" ;
                                   <https://rdf.ag/o/hops#betaAcidsContent> "4.2–5.8" ;
                                   <https://rdf.ag/o/hops#perceivedAroma> "Herbal, Peach, Pear, Spicy"@en ,
                                                                          "Épicé, Herbes, Pêche, Poire"@fr ;
                                   <https://rdf.ag/o/hops#totalOilContent> "1.8-2.2" .


###  https://rdf.ag/o/hops#HopsOlympic
<https://rdf.ag/o/hops#HopsOlympic> rdf:type owl:Class ;
                                    rdfs:subClassOf <https://rdf.ag/o/hops#Hops> ;
                                    <http://rdfs.org/ns/void#inDataset> <https://rdf.ag/o/hops#datasetdefinition> ;
                                    rdfs:isDefinedBy <https://rdf.ag/o/hops-2021-07-30> ;
                                    rdfs:label "Olympic"@en ;
                                    <http://www.w3.org/2004/02/skos/core#definition> "Olympic a été élevé par Prosser, WA, USA en 1974 par C. E. Zimmermann. Il a un pedigree compliqué et est un descendant de Brewer's Gold, Fuggle et East Kent Golding."@fr ,
                                                                                     "Olympic was bred by Prosser, WA, USA in 1974 by C. E. Zimmermann. It has a complicated pedigree and is a decendant of Brewer's Gold, Fuggle and East Kent Golding."@en ;
                                    <http://xmlns.com/foaf/0.1/isPrimaryTopicOf> <https://rdf.ag/o/hops#opsci1984.0011183X002400030046x> ;
                                    <http://xmlns.com/foaf/0.1/name> "Olympic" ;
                                    <https://rdf.ag/o/hops#alphaAcidsContent> "10.6-13.8" ;
                                    <https://rdf.ag/o/hops#betaAcidsContent> "3.8-6.1" ;
                                    <https://rdf.ag/o/hops#perceivedAroma> "Agrumes, Épicé"@fr ,
                                                                           "Citrus, Spicy"@en ;
                                    <https://rdf.ag/o/hops#totalOilContent> "0.86-2.55" .


###  https://rdf.ag/o/hops#HopsPacificGem
<https://rdf.ag/o/hops#HopsPacificGem> rdf:type owl:Class ;
                                       rdfs:subClassOf <https://rdf.ag/o/hops#Hops> ;
                                       <http://rdfs.org/ns/void#inDataset> <https://rdf.ag/o/hops#datasetdefinition> ;
                                       rdfs:isDefinedBy <https://rdf.ag/o/hops-2021-07-30> ;
                                       rdfs:label "Pacific Gem"@en ;
                                       <http://www.w3.org/2004/02/skos/core#definition> "Pacific Gem est un houblon néo-zélandais sorti en 1987. Il est le résultat d'un croisement entre Smooth Cone, California Late Cluster et Fuggle."@fr ,
                                                                                        "Pacific Gem is a New Zealand hop that was released in 1987. It is the result of a cross between Smooth Cone, California Late Cluster and Fuggle."@en ;
                                       <http://xmlns.com/foaf/0.1/name> "Pacific Gem" ;
                                       <https://rdf.ag/o/hops#alphaAcidsContent> "13-16" ;
                                       <https://rdf.ag/o/hops#betaAcidsContent> "7-9" ;
                                       <https://rdf.ag/o/hops#perceivedAroma> "Blackberry, Floral, Oak"@en ,
                                                                              "Chêne, Floral, Mûre"@fr ;
                                       <https://rdf.ag/o/hops#totalOilContent> "1.2-1.4" .


###  https://rdf.ag/o/hops#HopsPacificJade
<https://rdf.ag/o/hops#HopsPacificJade> rdf:type owl:Class ;
                                        rdfs:subClassOf <https://rdf.ag/o/hops#Hops> ;
                                        <http://rdfs.org/ns/void#inDataset> <https://rdf.ag/o/hops#datasetdefinition> ;
                                        rdfs:comment "Pacific Jade was trademarked, however it now has a status of Status: 602 - Abandoned-Failure To Respond Or Late Response according to Justia Trademarks."@en ,
                                                     "Pacific Jade était une marque déposée; cependant, il a maintenant le statut : 602 - Abandonné - Défaut de réponse ou réponse tardive selon Justia Trademarks."@fr ;
                                        rdfs:isDefinedBy <https://rdf.ag/o/hops-2021-07-30> ;
                                        rdfs:label "NZ Pacific Jade"@en ,
                                                   "Pacific Jade"@en ;
                                        <http://www.w3.org/2004/02/skos/core#definition> "Pacific Jade est un houblon élevé par le programme de recherche sur le houblon de Nouvelle-Zélande et sorti en 2004 par New Zealand Hops Limited."@fr ,
                                                                                         "Pacific Jade is a hop that was bred by the New Zealand Hop Research Program and was released in 2004 by New Zealand Hops Limited."@en ;
                                        <http://xmlns.com/foaf/0.1/name> "NZ Pacific Jade" ;
                                        <https://rdf.ag/o/hops#alphaAcidsContent> "12-14" ;
                                        <https://rdf.ag/o/hops#betaAcidsContent> "7-8" ;
                                        <https://rdf.ag/o/hops#perceivedAroma> "Citron, Herbal, Poivré"@fr ,
                                                                               "Herbal, Lemon, Peppery"@en ;
                                        <https://rdf.ag/o/hops#totalOilContent> "1.4" .


###  https://rdf.ag/o/hops#HopsPacifica
<https://rdf.ag/o/hops#HopsPacifica> rdf:type owl:Class ;
                                     rdfs:subClassOf <https://rdf.ag/o/hops#HopsHallertau> ;
                                     <http://rdfs.org/ns/void#inDataset> <https://rdf.ag/o/hops#datasetdefinition> ;
                                     rdfs:comment "Pacifica was trademarked, however it now has a status of Status: 602 - Abandoned-Failure To Respond Or Late Response according to Justia Trademarks."@en ,
                                                  "Pacifica était une marque déposée; cependant, il a maintenant le statut : 602 - Abandonné - Défaut de réponse ou réponse tardive selon Justia Trademarks."@fr ;
                                     rdfs:isDefinedBy <https://rdf.ag/o/hops-2021-07-30> ;
                                     rdfs:label "Pacific Hallertau"@en ,
                                                "Pacifica"@en ;
                                     <http://www.w3.org/2004/02/skos/core#definition> "Pacifica est un houblon élevé par HortResearch, programme néo-zélandais et sorti en 1994 par New Zealand Hops Limited. C'est le résultat de l'élevage à pollinisation libre de Hallertau Mittelfrüher."@fr ,
                                                                                      "Pacifica is a hop that was bred by HortResearch, New Zealand Program and was released in 1994 by New Zealand Hops Limited. It is the result of open pollination breeding of Hallertau Mittelfrüher."@en ;
                                     <http://xmlns.com/foaf/0.1/name> "Pacifica" ;
                                     <https://rdf.ag/o/hops#alphaAcidsContent> "5-6" ;
                                     <https://rdf.ag/o/hops#betaAcidsContent> "6" ;
                                     <https://rdf.ag/o/hops#perceivedAroma> "Agrumes, Épicé, Floral, Herbal, Orange"@fr ,
                                                                            "Citrusy, Floral, Herbal, Orange, Spicy"@en ;
                                     <https://rdf.ag/o/hops#totalOilContent> "1.0" .


###  https://rdf.ag/o/hops#HopsPerle
<https://rdf.ag/o/hops#HopsPerle> rdf:type owl:Class ;
                                  rdfs:subClassOf <https://rdf.ag/o/hops#Hops> ;
                                  <http://rdfs.org/ns/void#inDataset> <https://rdf.ag/o/hops#datasetdefinition> ;
                                  rdfs:isDefinedBy <https://rdf.ag/o/hops-2021-07-30> ;
                                  rdfs:label "Perle"@en ;
                                  <http://www.w3.org/2004/02/skos/core#definition> "Perle a été rendu public en 1978 et a été créé en Allemagne à partir d'un croisement entre Northern Brewer et une variété allemande native."@fr ,
                                                                                   "Perle was released in 1978 to the public and was created in Germany from a cross between Northern Brewer and a native German variety."@en ;
                                  <http://xmlns.com/foaf/0.1/name> "Perle" ;
                                  <https://rdf.ag/o/hops#alphaAcidsContent> "8-9" ;
                                  <https://rdf.ag/o/hops#betaAcidsContent> "8" ;
                                  <https://rdf.ag/o/hops#perceivedAroma> "Cedar, Orange, Spicy"@en ,
                                                                         "Cèdre, Épicé, Orange"@fr ;
                                  <https://rdf.ag/o/hops#totalOilContent> "0.6-1.2" .


###  https://rdf.ag/o/hops#HopsPerle_US
<https://rdf.ag/o/hops#HopsPerle_US> rdf:type owl:Class ;
                                     rdfs:subClassOf <https://rdf.ag/o/hops#Hops> ;
                                     <http://rdfs.org/ns/void#inDataset> <https://rdf.ag/o/hops#datasetdefinition> ;
                                     rdfs:isDefinedBy <https://rdf.ag/o/hops-2021-07-30> ;
                                     rdfs:label "Perle (US)"@en ;
                                     <http://www.w3.org/2004/02/skos/core#definition> "Perle a été rendu public en 1978 et a été créé en Allemagne à partir d'un croisement entre Northern Brewer et une variété allemande native. Bien que génétiquement identique à la Perle du Royaume-Uni, il a été noté que la Perle cultivée en Amérique du Nord a une teneur plus élevée en acide alpha et en myrcène, mais plus faible en humulène. La différence de propriétés rend ce houblon légèrement plus apprécié comme houblon amer que la variété cultivée au Royaume-Uni."@fr ,
                                                                                      "Perle was released in 1978 to the public and was created in Germany from a cross between Northern Brewer and a native German variety. While genetically identical to Perle from the UK, it has been noted that Perle grown in North America has higher alpha acid and myrcene contents, but lower in humulene. The difference in properties makes this hop favored slightly more as a bittering hop than the variety grown in the UK."@en ;
                                     <http://xmlns.com/foaf/0.1/name> "Perle (US)" ;
                                     <https://rdf.ag/o/hops#alphaAcidsContent> "6-10" ;
                                     <https://rdf.ag/o/hops#betaAcidsContent> "3-5" ;
                                     <https://rdf.ag/o/hops#perceivedAroma> "Floral, Herbal, Spicy"@en ,
                                                                            "Épicé, Floral, Herbal"@fr ;
                                     <https://rdf.ag/o/hops#totalOilContent> "0.7-1.2" .


###  https://rdf.ag/o/hops#HopsPethamGolding
<https://rdf.ag/o/hops#HopsPethamGolding> rdf:type owl:Class ;
                                          rdfs:subClassOf <https://rdf.ag/o/hops#HopsGolding> ;
                                          <http://rdfs.org/ns/void#inDataset> <https://rdf.ag/o/hops#datasetdefinition> ;
                                          rdfs:isDefinedBy <https://rdf.ag/o/hops-2021-07-30> ;
                                          rdfs:label "Petham Golding"@en ;
                                          <http://www.w3.org/2004/02/skos/core#definition> "Although Petham Golding was one of the most popular variety of hops from East Kent, England in the late 1800s, it is no longer grown in favor of varieties with larger yields and that are less prone to breaking at the branching point. Chinook, a hop popular in the US, owes its lineage to Petham Golding. Petham is named after the village of Petham, located near Canterbury in the UK."@en ,
                                                                                           "Bien que Petham Golding ait été l'une des variétés de houblon les plus populaires de l'East Kent, en Angleterre, à la fin des années 1800, il n'est plus cultivé en faveur de variétés avec des rendements plus élevés et moins susceptibles de se casser au point de ramification. Le chinook, un houblon populaire aux États-Unis, doit sa lignée à Petham Golding. Petham tire son nom du village de Petham, situé près de Canterbury au Royaume-Uni."@fr ;
                                          <http://xmlns.com/foaf/0.1/name> "Petham Golding" ;
                                          <https://rdf.ag/o/hops#alphaAcidsContent> "6.9" ;
                                          <https://rdf.ag/o/hops#betaAcidsContent> "2" ;
                                          <https://rdf.ag/o/hops#totalOilContent> "1.15" .


###  https://rdf.ag/o/hops#HopsPioneer
<https://rdf.ag/o/hops#HopsPioneer> rdf:type owl:Class ;
                                    rdfs:subClassOf <https://rdf.ag/o/hops#Hops> ;
                                    <http://rdfs.org/ns/void#inDataset> <https://rdf.ag/o/hops#datasetdefinition> ;
                                    rdfs:isDefinedBy <https://rdf.ag/o/hops-2021-07-30> ;
                                    rdfs:label "Pioneer"@en ;
                                    <http://www.w3.org/2004/02/skos/core#definition> "Pioneer and its sister Herald were bred from Omega at Wye College, UK."@en ,
                                                                                     "Pioneer et sa sœur Herald ont été élevés à partir d'Omega au Wye College, au Royaume-Uni."@fr ;
                                    <http://xmlns.com/foaf/0.1/name> "Pioneer" ;
                                    <https://rdf.ag/o/hops#alphaAcidsContent> "8-10" ;
                                    <https://rdf.ag/o/hops#betaAcidsContent> "3.5-4" ;
                                    <https://rdf.ag/o/hops#perceivedAroma> "Agrumes, Cèdre, Citron, Herbes, Pamplemousse"@fr ,
                                                                           "Cedar, Citrus, Grapefruit, Herbs, Lemon"@en ;
                                    <https://rdf.ag/o/hops#totalOilContent> "1-1.8" .


###  https://rdf.ag/o/hops#HopsPolaris
<https://rdf.ag/o/hops#HopsPolaris> rdf:type owl:Class ;
                                    rdfs:subClassOf <https://rdf.ag/o/hops#Hops> ;
                                    <http://rdfs.org/ns/void#inDataset> <https://rdf.ag/o/hops#datasetdefinition> ;
                                    rdfs:isDefinedBy <https://rdf.ag/o/hops-2021-07-30> ;
                                    rdfs:label "Polaris"@en ;
                                    <http://www.w3.org/2004/02/skos/core#definition> "Polaris a été publié par le Hop Research Institute de Hüll, en Allemagne, a publié Polaris en 2012 et est connu pour avoir une teneur élevée en acide alpha."@fr ,
                                                                                     "Polaris was released by the Hop Research Institute in Hüll, Germany released Polaris in 2012 and is known for having a high alpha acid content."@en ;
                                    <http://xmlns.com/foaf/0.1/name> "Polaris" ;
                                    <https://rdf.ag/o/hops#alphaAcidsContent> "18-23" ;
                                    <https://rdf.ag/o/hops#betaAcidsContent> "4.5-6" ;
                                    <https://rdf.ag/o/hops#perceivedAroma> "Floral, Fruity, Mint, Pine, Spice"@en ,
                                                                           "Épice, Floral, Fruité, Menthe, Pin"@fr ;
                                    <https://rdf.ag/o/hops#totalOilContent> "4.0-5.0" .


###  https://rdf.ag/o/hops#HopsPrideofRingwood
<https://rdf.ag/o/hops#HopsPrideofRingwood> rdf:type owl:Class ;
                                            rdfs:subClassOf <https://rdf.ag/o/hops#Hops> ;
                                            <http://rdfs.org/ns/void#inDataset> <https://rdf.ag/o/hops#datasetdefinition> ;
                                            rdfs:isDefinedBy <https://rdf.ag/o/hops-2021-07-30> ;
                                            rdfs:label "Pride of Ringwood"@en ;
                                            <http://www.w3.org/2004/02/skos/core#definition> "Pride of Ringwood est un descendant de Pride of Kent et élevé par pollinisation libre par Bill Nash à la Ringwood Hop Research Station à Ringwood, Victoria, Australie. Il est sorti en 1958 et était à cette époque le houblon avec la teneur en acide alpha la plus élevée au monde."@fr ,
                                                                                             "Pride of Ringwood is a descendant of Pride of Kent and bred through open pollination by Bill Nash at the Ringwood Hop Research Station in Ringwood, Victoria, Australia. It was released in 1958 and at that time was the hop with the highest alpha acid content in the world."@en ;
                                            <http://xmlns.com/foaf/0.1/name> "Pride of Ringwood" ;
                                            <https://rdf.ag/o/hops#alphaAcidsContent> "7-11" ;
                                            <https://rdf.ag/o/hops#betaAcidsContent> "4-8" ;
                                            <https://rdf.ag/o/hops#perceivedAroma> "Cedar, Fruity, Herbal, Spicy, Oak"@en ,
                                                                                   "Cèdre, Chêne, Épicé, Fruité, Herbal"@fr ;
                                            <https://rdf.ag/o/hops#totalOilContent> "1.21" .


###  https://rdf.ag/o/hops#HopsProgress
<https://rdf.ag/o/hops#HopsProgress> rdf:type owl:Class ;
                                     rdfs:subClassOf <https://rdf.ag/o/hops#Hops> ;
                                     <http://rdfs.org/ns/void#inDataset> <https://rdf.ag/o/hops#datasetdefinition> ;
                                     rdfs:isDefinedBy <https://rdf.ag/o/hops-2021-07-30> ;
                                     rdfs:label "Progress"@en ;
                                     <http://www.w3.org/2004/02/skos/core#definition> "Progress a été conçu pour être un substitut alternatif et peu coûteux à Fuggle. Il a été élevé pour la première fois au Wye College, au Royaume-Uni, en 1951 et a été relâché en 1964. Il s'agit d'un descendant de Whitbread Golding et d'une variété amérindienne."@fr ,
                                                                                      "Progress was bred to be an alternative, low-cost, substitute for Fuggle. It was first bred at Wye College, UK in the 1951 and was released in 1964. It is a descendant of Whitbread Golding and a native American variety."@en ;
                                     <http://xmlns.com/foaf/0.1/name> "Progress" ;
                                     <https://rdf.ag/o/hops#alphaAcidsContent> "6-7.5" ;
                                     <https://rdf.ag/o/hops#betaAcidsContent> "2-3.3" ;
                                     <https://rdf.ag/o/hops#perceivedAroma> "Earthy, Grass, Honey, Mint, Spicy"@en ,
                                                                            "Épicé, Herbe, Menthe, Miel, Terreux"@fr ;
                                     <https://rdf.ag/o/hops#totalOilContent> "0.5-1.2" .


###  https://rdf.ag/o/hops#HopsSaaz
<https://rdf.ag/o/hops#HopsSaaz> rdf:type owl:Class ;
                                 rdfs:subClassOf <https://rdf.ag/o/hops#Hops> ;
                                 <http://rdfs.org/ns/void#inDataset> <https://rdf.ag/o/hops#datasetdefinition> ;
                                 rdfs:isDefinedBy <https://rdf.ag/o/hops-2021-07-30> ;
                                 rdfs:label "Czech Saaz"@en ,
                                            "Saaz"@en ;
                                 <http://www.w3.org/2004/02/skos/core#definition> "Saaz a été officiellement publié en 1952, mais il a été largement utilisé dans le brassage de la bière au cours des 700 dernières années. Il est originaire de Bohême, aujourd'hui République tchèque, et est principalement utilisé comme houblon aromatique en raison de sa faible teneur en acide alpha."@fr ,
                                                                                  "Saaz was officially released in 1952 but it has been prominently used in beer brewing for the last 700 years. It originated in Bohemia, now Czech Republic, and is mostly used as an aroma hop due to its low alpha acid content."@en ;
                                 <http://xmlns.com/foaf/0.1/name> "Saaz" ;
                                 <https://rdf.ag/o/hops#alphaAcidsContent> "2.5-4.5" ;
                                 <https://rdf.ag/o/hops#betaAcidsContent> "4-6" ;
                                 <https://rdf.ag/o/hops#perceivedAroma> "Earthy, Floral, Herbal"@en ,
                                                                        "Floral, Herbal, Terreux"@fr ;
                                 <https://rdf.ag/o/hops#totalOilContent> "0.4-0.8" .


###  https://rdf.ag/o/hops#HopsSaaz_US
<https://rdf.ag/o/hops#HopsSaaz_US> rdf:type owl:Class ;
                                    rdfs:subClassOf <https://rdf.ag/o/hops#HopsSaaz> ;
                                    <http://rdfs.org/ns/void#inDataset> <https://rdf.ag/o/hops#datasetdefinition> ;
                                    rdfs:isDefinedBy <https://rdf.ag/o/hops-2021-07-30> ;
                                    rdfs:label "Czech Saaz (US)"@en ,
                                               "Saaz (US)"@en ;
                                    <http://www.w3.org/2004/02/skos/core#definition> "Saaz (US) is Saaz hops that has been grown in the US, or North America, and therefore may have different properties due to terroir or cross-pollination from North American native hop varieties."@en ,
                                                                                     "Saaz (États-Unis) est un houblon Saaz qui a été cultivé aux États-Unis ou en Amérique du Nord et peut donc avoir des propriétés différentes en raison du terroir ou de la pollinisation croisée à partir de variétés de houblon indigènes d'Amérique du Nord."@fr ;
                                    <http://xmlns.com/foaf/0.1/name> "Saaz" ;
                                    <https://rdf.ag/o/hops#alphaAcidsContent> "3-4.5" ;
                                    <https://rdf.ag/o/hops#betaAcidsContent> "3-4.5" ;
                                    <https://rdf.ag/o/hops#perceivedAroma> "Earthy, Herbal, Spicy"@en ,
                                                                           "Épicé, Herbal, Terreux"@fr ;
                                    <https://rdf.ag/o/hops#totalOilContent> "0.5-1" .


###  https://rdf.ag/o/hops#HopsSantiam
<https://rdf.ag/o/hops#HopsSantiam> rdf:type owl:Class ;
                                    rdfs:subClassOf <https://rdf.ag/o/hops#Hops> ;
                                    <http://rdfs.org/ns/void#inDataset> <https://rdf.ag/o/hops#datasetdefinition> ;
                                    rdfs:isDefinedBy <https://rdf.ag/o/hops-2021-07-30> ;
                                    rdfs:label "Santiam"@en ;
                                    <http://www.w3.org/2004/02/skos/core#definition> "Santiam a été relâché en 1997 et élevé par l'Agriculture Research Service à Corvallis, Oregon. Sa lignée comprend le suisse Tettnanger, l'allemand Hallertauer Mittelfrüher et Cascade (États-Unis)."@fr ,
                                                                                     "Santiam was released in 1997 and bred by the Agriculture Research Service in Corvallis, Oregon. Its lineage includes Swiss Tettnanger, German Hallertauer Mittelfrüher and Cascade (US)."@en ;
                                    <http://xmlns.com/foaf/0.1/isPrimaryTopicOf> <https://rdf.ag/o/cropsci1999.0011183X003900030051x> ;
                                    <http://xmlns.com/foaf/0.1/name> "Santiam" ;
                                    <https://rdf.ag/o/hops#alphaAcidsContent> "5-8" ;
                                    <https://rdf.ag/o/hops#betaAcidsContent> "5.3-8.5" ;
                                    <https://rdf.ag/o/hops#perceivedAroma> "Citron, Épicé, Fruité, Herbal, Pêche, Poivre"@fr ,
                                                                           "Herbal, Fruity, Lemon, Peach, Pepper, Spicy"@en ;
                                    <https://rdf.ag/o/hops#totalOilContent> "1.3-1.7" .


###  https://rdf.ag/o/hops#HopsSaphir
<https://rdf.ag/o/hops#HopsSaphir> rdf:type owl:Class ;
                                   rdfs:subClassOf <https://rdf.ag/o/hops#Hops> ;
                                   <http://rdfs.org/ns/void#inDataset> <https://rdf.ag/o/hops#datasetdefinition> ;
                                   rdfs:isDefinedBy <https://rdf.ag/o/hops-2021-07-30> ;
                                   rdfs:label "Saphir"@en ;
                                   <http://www.w3.org/2004/02/skos/core#definition> "Saphir a été élevé au Hop Research Center de Hüll comme alternative à Hallertau Mittelfrüh qui est plus disponible dans le commerce et est sorti en 2002."@fr ,
                                                                                    "Saphir was bred at the Hop Research Center in Hüll as an alternative to Hallertau Mittelfrüh that is more commercially available and was released in 2002."@en ;
                                   <http://xmlns.com/foaf/0.1/name> "Saphir" ;
                                   <https://rdf.ag/o/hops#alphaAcidsContent> "2-4.5" ;
                                   <https://rdf.ag/o/hops#betaAcidsContent> "4-7" ;
                                   <https://rdf.ag/o/hops#perceivedAroma> "Agrumes, Épicé, Fruité"@fr ,
                                                                          "Citrus, Fruity, Spicy"@en ;
                                   <https://rdf.ag/o/hops#totalOilContent> "0.8-1.4" .


###  https://rdf.ag/o/hops#HopsSavinskiGolding
<https://rdf.ag/o/hops#HopsSavinskiGolding> rdf:type owl:Class ;
                                            owl:equivalentClass <https://rdf.ag/o/hops#HopsStyrianGolding> ;
                                            rdfs:subClassOf <https://rdf.ag/o/hops#HopsFuggle> ;
                                            <http://rdfs.org/ns/void#inDataset> <https://rdf.ag/o/hops#datasetdefinition> ;
                                            rdfs:isDefinedBy <https://rdf.ag/o/hops-2021-07-30> ;
                                            rdfs:label "Sanutaler"@en ,
                                                       "Savinski Golding"@en ,
                                                       "Steirer Hopfen"@en ,
                                                       "Styrian"@en ;
                                            <http://www.w3.org/2004/02/skos/core#definition> "Il s'agit d'une sélection clonale d'un Fuggle (Styrian Golding) de Yougoslavie pris au tournant du siècle."@fr ,
                                                                                             "This is clonal selection of a Fuggle (Styrian Golding) from Yugoslavia taken at the turn of the century."@en ;
                                            <http://xmlns.com/foaf/0.1/name> "Savinski Golding" .


###  https://rdf.ag/o/hops#HopsSimcoe
<https://rdf.ag/o/hops#HopsSimcoe> rdf:type owl:Class ;
                                   rdfs:subClassOf <https://rdf.ag/o/hops#Hops> ;
                                   <http://rdfs.org/ns/void#inDataset> <https://rdf.ag/o/hops#datasetdefinition> ;
                                   rdfs:isDefinedBy <https://rdf.ag/o/hops-2021-07-30> ;
                                   rdfs:label "Simcoe®"@en ;
                                   <http://www.w3.org/2004/02/skos/core#definition> "Simcoe® est une variété de houblon déposée développée par le professeur Zimmerman et détenue par Yakima Chief Ranches, Inc."@fr ,
                                                                                    "Simcoe® is a trademarked hops variety developed Professor Zimmerman and owned by Yakima Chief Ranches, Inc."@en ;
                                   <http://xmlns.com/foaf/0.1/name> "Simcoe®" ;
                                   <https://rdf.ag/o/hops#alphaAcidsContent> "12.0–14.0" ;
                                   <https://rdf.ag/o/hops#betaAcidsContent> "4-5" ;
                                   <https://rdf.ag/o/hops#perceivedAroma> "Agrumes, Fruit de la Passion, Herbes, Pamplemousse, Pin, Terreux"@fr ,
                                                                          "Citrus, Earthy, Grapefruit, Herbal, Passionfruit, Pine"@en ;
                                   <https://rdf.ag/o/hops#totalOilContent> "2-2.5" .


###  https://rdf.ag/o/hops#HopsSorachiAce
<https://rdf.ag/o/hops#HopsSorachiAce> rdf:type owl:Class ;
                                       rdfs:subClassOf <https://rdf.ag/o/hops#Hops> ;
                                       <http://rdfs.org/ns/void#inDataset> <https://rdf.ag/o/hops#datasetdefinition> ;
                                       rdfs:isDefinedBy <https://rdf.ag/o/hops-2021-07-30> ;
                                       rdfs:label "Sorachi Ace"@en ,
                                                  "Sorachi Ace"@fr ;
                                       <http://www.w3.org/2004/02/skos/core#definition> "Sorachi Ace a été développé par le Dr Mori sor Sapporo Breweries Co. Ltd au Japon en 1984; un croisement entre Brewer's Gold, Saaz et Beikei n ° 2 mâle.Un houblon aromatique apprécié des brasseurs artisanaux."@fr ,
                                                                                        "Sorachi Ace was developed by Dr. Mori for Sapporo Breweries Co. Ltd in Japan 1984; a cross between Brewer's Gold, Saaz and Beikei No. 2 male. An aromatic hop that is popular among craft brewers."@en ;
                                       <http://xmlns.com/foaf/0.1/isPrimaryTopicOf> <https://rdf.ag/o/hops#Sanekata:2018aa> ;
                                       <http://xmlns.com/foaf/0.1/name> "Sorachi Ace" ;
                                       <https://rdf.ag/o/hops#alphaAcidsContent> "12.0–13.0" ;
                                       <https://rdf.ag/o/hops#betaAcidsContent> "8.8–9.9" ;
                                       <https://rdf.ag/o/hops#perceivedAroma> "Agrumes, Aneth, Citron, Orange"@fr ,
                                                                              "Lemmon, Citrus, Orange, Dill"@en ;
                                       <https://rdf.ag/o/hops#totalOilContent> "2.8-3.2" .


###  https://rdf.ag/o/hops#HopsSpalter
<https://rdf.ag/o/hops#HopsSpalter> rdf:type owl:Class ;
                                    rdfs:subClassOf <https://rdf.ag/o/hops#Hops> ;
                                    <http://rdfs.org/ns/void#inDataset> <https://rdf.ag/o/hops#datasetdefinition> ;
                                    rdfs:isDefinedBy <https://rdf.ag/o/hops-2021-07-30> ;
                                    rdfs:label "Spalt"@en ,
                                               "Spalter"@en ;
                                    <http://www.w3.org/2004/02/skos/core#definition> "Le spalt est l'un des houblons les plus anciens au monde, datant du 8ème siècle. Il s'agit d'une race locale cultivée principalement dans la région de Spalt en Allemagne."@fr ,
                                                                                     "Spalt is one of the oldest hops in the world, dating back to 8th century. They are a landrace grown predominantly in the Spalt region of Germany."@en ;
                                    <http://xmlns.com/foaf/0.1/name> "Spalter" ;
                                    <https://rdf.ag/o/hops#alphaAcidsContent> "2.5-5.7" ;
                                    <https://rdf.ag/o/hops#betaAcidsContent> "3-5" ;
                                    <https://rdf.ag/o/hops#perceivedAroma> "Earthy, Spicy"@en ,
                                                                           "Épicé, Terreux"@fr ;
                                    <https://rdf.ag/o/hops#totalOilContent> "0.5-0.9" .


###  https://rdf.ag/o/hops#HopsSpalterSelect
<https://rdf.ag/o/hops#HopsSpalterSelect> rdf:type owl:Class ;
                                          rdfs:subClassOf <https://rdf.ag/o/hops#Hops> ;
                                          <http://rdfs.org/ns/void#inDataset> <https://rdf.ag/o/hops#datasetdefinition> ;
                                          rdfs:isDefinedBy <https://rdf.ag/o/hops-2021-07-30> ;
                                          rdfs:label "Select Spalt"@en ,
                                                     "Spalt Select"@en ,
                                                     "Spalter Select"@en ;
                                          <http://www.w3.org/2004/02/skos/core#definition> "Spalter Select a été élevé à Hüll, en Allemagne, comme alternative commerciale à Spalt et est le résultat d'un croisement entre Spalt et Hallertau Mittelfrühe. Il est sorti en 1993."@fr ,
                                                                                           "Spalter Select was bred in Hüll, Germany as a commercial alternative to Spalt and is the result of a cross between Spalt and Hallertau Mittelfrühe. It was released in 1993."@en ;
                                          <http://xmlns.com/foaf/0.1/name> "Spalter Select" ;
                                          <https://rdf.ag/o/hops#alphaAcidsContent> "3-6.5" ;
                                          <https://rdf.ag/o/hops#betaAcidsContent> "2-5" ;
                                          <https://rdf.ag/o/hops#perceivedAroma> "Earthy, Floral, Herbal, Spicy"@en ,
                                                                                 "Épicé, Floral, Herbal, Terreux"@fr ;
                                          <https://rdf.ag/o/hops#totalOilContent> "0.5-1.2" .


###  https://rdf.ag/o/hops#HopsStrisselspalt
<https://rdf.ag/o/hops#HopsStrisselspalt> rdf:type owl:Class ;
                                          rdfs:subClassOf <https://rdf.ag/o/hops#Hops> ;
                                          <http://rdfs.org/ns/void#inDataset> <https://rdf.ag/o/hops#datasetdefinition> ;
                                          rdfs:isDefinedBy <https://rdf.ag/o/hops-2021-07-30> ;
                                          rdfs:label "French Strisselspalt"@en ,
                                                     "Strisselspalt"@en ,
                                                     "Strisselspalter"@en ;
                                          <http://www.w3.org/2004/02/skos/core#definition> "Strisselspalt est une ancienne race locale de la région Alsace en France et est un descendant de Spalt, Hersbrucker ou d'un croisement entre les deux."@fr ,
                                                                                           "Strisselspalt is an old landrace from the Alsace region of France and is a descendant of either Spalt, Hersbrucker or a cross between the two."@en ;
                                          <http://xmlns.com/foaf/0.1/name> "Strisselspalt" ;
                                          <https://rdf.ag/o/hops#alphaAcidsContent> "1.8-5.7" ;
                                          <https://rdf.ag/o/hops#betaAcidsContent> "2.5-6" ;
                                          <https://rdf.ag/o/hops#perceivedAroma> "Agrumes, Épicé, Floral, Fruits, Herbes"@fr ,
                                                                                 "Citrus, Floral, Fruit, Herbal, Spicy"@en ;
                                          <https://rdf.ag/o/hops#totalOilContent> "0.6-0.9" .


###  https://rdf.ag/o/hops#HopsStyrianGolding
<https://rdf.ag/o/hops#HopsStyrianGolding> rdf:type owl:Class ;
                                           owl:equivalentClass <https://rdf.ag/o/hops#HopsYugoslaviaGolding> ;
                                           rdfs:subClassOf <https://rdf.ag/o/hops#HopsFuggle> ;
                                           <http://rdfs.org/ns/void#inDataset> <https://rdf.ag/o/hops#datasetdefinition> ;
                                           rdfs:isDefinedBy <https://rdf.ag/o/hops-2021-07-30> ;
                                           rdfs:label "Savinja Golding"@en ,
                                                      "Savinjski Golding"@en ,
                                                      "Styrian"@en ,
                                                      "Styrian Golding"@en ,
                                                      "Styrian Savinjski Golding"@en ;
                                           <http://www.w3.org/2004/02/skos/core#definition> "Styrian Golding est en fait un descendant de Fuggle et non de Golding. Dans les années 1930, une souche de verticilliose a ravagé l'industrie du houblon yougoslave, donc un houblon résistant du Royaume-Uni a été introduit pour reconstruire l'industrie du houblon. Malheureusement, il a été confondu avec un Golding alors qu'il s'agissait en fait d'un Fuggle. Il s'appelait Styrian, à l'origine Steirer - un houblon poussant le long de la frontière slovène (anciennement Yougoslavie)/autrichienne, la deuxième partie du nom venant de la gaffe susmentionnée."@fr ,
                                                                                            "Styrian Golding is actually a descendant of Fuggle not Golding. In the 1930s a Verticillium Wilt strain ravaged the Yugoslavian hop industry, so a resistant hop from the UK was brought in to rebuild the hop industry. Unfortunately, it was mistaken for a Golding when it was in fact a Fuggle. It was named Styrian, originally Steirer - a hop growing along the Slovenia (formerly Yugoslavia)/Austrian border, with the second part of the name coming from the aforementioned blunder."@en ;
                                           <http://xmlns.com/foaf/0.1/name> "Styrian Golding" ;
                                           <https://rdf.ag/o/hops#alphaAcidsContent> "2.8-6" ;
                                           <https://rdf.ag/o/hops#betaAcidsContent> "2-3" ;
                                           <https://rdf.ag/o/hops#totalOilContent> "0.5-1" .


###  https://rdf.ag/o/hops#HopsSummer
<https://rdf.ag/o/hops#HopsSummer> rdf:type owl:Class ;
                                   rdfs:subClassOf <https://rdf.ag/o/hops#Hops> ;
                                   <http://rdfs.org/ns/void#inDataset> <https://rdf.ag/o/hops#datasetdefinition> ;
                                   rdfs:isDefinedBy <https://rdf.ag/o/hops-2021-07-30> ;
                                   rdfs:label "Summer"@en ;
                                   <http://www.w3.org/2004/02/skos/core#definition> "Summer est un houblon Australien créé en 1997 par Hop Products Australia. C'est un descendant du houblon Saaz."@fr ,
                                                                                    "Summer is an Australian hop that was created in 1997 by Hop Products Australia. It is a descendant of Saaz hops."@en ;
                                   <http://xmlns.com/foaf/0.1/name> "Summer" ;
                                   <https://rdf.ag/o/hops#alphaAcidsContent> "5.6-6.4" ;
                                   <https://rdf.ag/o/hops#betaAcidsContent> "4.8-6.1" ;
                                   <https://rdf.ag/o/hops#perceivedAroma> "Abricot, Herbe, Melon, Pêche"@fr ,
                                                                          "Apricot, Grass, Melon, Peach"@en ;
                                   <https://rdf.ag/o/hops#totalOilContent> "1.4-2.0" .


###  https://rdf.ag/o/hops#HopsSummit
<https://rdf.ag/o/hops#HopsSummit> rdf:type owl:Class ;
                                   rdfs:subClassOf <https://rdf.ag/o/hops#Hops> ;
                                   <http://rdfs.org/ns/void#inDataset> <https://rdf.ag/o/hops#datasetdefinition> ;
                                   rdfs:isDefinedBy <https://rdf.ag/o/hops-2021-07-30> ;
                                   rdfs:label "Summit™"@en ;
                                   <http://www.w3.org/2004/02/skos/core#definition> "Summit™ est une variété de houblon semi-naine qui a été lancée en 2000 dans le cadre d'une joint-venture entre Roy Farms et Green Acre Farms. Il a été développé en 1998 par l'American Dwarf Hop Association."@fr ,
                                                                                    "Summit™ is a semi-dwarf hop variety that was released in 2000 in a joint venture between Roy Farms and Green Acre Farms. It was developed in 1998 by the American Dwarf Hop Association."@en ;
                                   <http://xmlns.com/foaf/0.1/name> "Summit™" ;
                                   <https://rdf.ag/o/hops#alphaAcidsContent> "16-18" ;
                                   <https://rdf.ag/o/hops#betaAcidsContent> "3.3-4.3" ;
                                   <https://rdf.ag/o/hops#perceivedAroma> "Agrumes, Terreux"@fr ,
                                                                          "Citrus, Earthy"@en ;
                                   <https://rdf.ag/o/hops#totalOilContent> "1.5-3" .


###  https://rdf.ag/o/hops#HopsTarget
<https://rdf.ag/o/hops#HopsTarget> rdf:type owl:Class ;
                                   rdfs:subClassOf <https://rdf.ag/o/hops#Hops> ;
                                   <http://rdfs.org/ns/void#inDataset> <https://rdf.ag/o/hops#datasetdefinition> ;
                                   rdfs:isDefinedBy <https://rdf.ag/o/hops-2021-07-30> ;
                                   rdfs:label "Target"@en ,
                                              "Wye Target"@en ;
                                   <http://www.w3.org/2004/02/skos/core#definition> "Le houblon Target, un descendant de Northern Brewer et d'Eastwell Golding, a été élevé par le Dr Ray A. Neve en 1965 au Wye College au Royaume-Uni."@fr ,
                                                                                    "Target hops, a descendant of Northern Brewer and Eastwell Golding, was bred by Dr. Ray A. Neve in 1965 at Wye College in the UK."@en ;
                                   <http://xmlns.com/foaf/0.1/name> "Target" ;
                                   <https://rdf.ag/o/hops#alphaAcidsContent> "8-12.5" ;
                                   <https://rdf.ag/o/hops#betaAcidsContent> "5-5.5" ;
                                   <https://rdf.ag/o/hops#perceivedAroma> "Cedar, Liquorice, Pine"@en ,
                                                                          "Cèdre, Pin, Réglisse"@fr ;
                                   <https://rdf.ag/o/hops#totalOilContent> "1.6-2.6" .


###  https://rdf.ag/o/hops#HopsTarget_VF
<https://rdf.ag/o/hops#HopsTarget_VF> rdf:type owl:Class ;
                                      rdfs:subClassOf <https://rdf.ag/o/hops#HopsTarget> ;
                                      <http://rdfs.org/ns/void#inDataset> <https://rdf.ag/o/hops#datasetdefinition> ;
                                      rdfs:isDefinedBy <https://rdf.ag/o/hops-2021-07-30> ;
                                      rdfs:label "Target (VF)"@en ,
                                                 "Wye Target (VF)"@en ;
                                      <http://www.w3.org/2004/02/skos/core#definition> "Il s'agit d'une sélection sans virus des houblons Target."@fr ,
                                                                                       "This is a virus free selection of the Target hops."@en ;
                                      <http://xmlns.com/foaf/0.1/name> "Target (VF)" ;
                                      <https://rdf.ag/o/hops#alphaAcidsContent> "8.9-15.2" ;
                                      <https://rdf.ag/o/hops#betaAcidsContent> "3.9-6.9" ;
                                      <https://rdf.ag/o/hops#perceivedAroma> "Cedar, Liquorice, Pine"@en ,
                                                                             "Cèdre, Pin, Réglisse"@fr ;
                                      <https://rdf.ag/o/hops#totalOilContent> "0.82-2.32" .


###  https://rdf.ag/o/hops#HopsTaurus
<https://rdf.ag/o/hops#HopsTaurus> rdf:type owl:Class ;
                                   rdfs:subClassOf <https://rdf.ag/o/hops#Hops> ;
                                   <http://rdfs.org/ns/void#inDataset> <https://rdf.ag/o/hops#datasetdefinition> ;
                                   rdfs:isDefinedBy <https://rdf.ag/o/hops-2021-07-30> ;
                                   rdfs:label "Hallertau Taurus"@en ,
                                              "Taurus"@en ;
                                   <http://www.w3.org/2004/02/skos/core#definition> "Taurus est une variété allemande de houblon qui a une teneur élevée en acide alpha et a été sélectionnée par le Hüll Hop Research Institute. Ce houblon est sorti en 1995."@fr ,
                                                                                    "Taurus is a German variety of hops that has a high alpha acid content and was bred by the Hüll Hop Research Institute. This hop was released in 1995."@en ;
                                   <http://xmlns.com/foaf/0.1/name> "Taurus" ;
                                   <https://rdf.ag/o/hops#alphaAcidsContent> "12.3-17.9" ;
                                   <https://rdf.ag/o/hops#betaAcidsContent> "4-6" ;
                                   <https://rdf.ag/o/hops#totalOilContent> "0.9-1.5" .


###  https://rdf.ag/o/hops#HopsTeamaker
<https://rdf.ag/o/hops#HopsTeamaker> rdf:type owl:Class ;
                                     rdfs:subClassOf <https://rdf.ag/o/hops#Hops> ;
                                     <http://rdfs.org/ns/void#inDataset> <https://rdf.ag/o/hops#datasetdefinition> ;
                                     rdfs:isDefinedBy <https://rdf.ag/o/hops-2021-07-30> ;
                                     rdfs:label "Teamaker"@en ;
                                     <http://www.w3.org/2004/02/skos/core#definition> """Teamaker a été développé par l'USDA et a été publié par l'ARS Forage, Seed and Cereal Research Unit à Corvallis, Oregon. Il est unique dans le sens où il a été élevé pour avoir une teneur bas en acide alpha et une teneur élevée en acide bêta.
      
      En raison de ses propriétés antibiotiques, il est utilisé comme antibiotique alternatif dans l'alimentation du bétail. Il est également connu pour être utilisé dans les thés, comme son nom l'indique."""@fr ,
                                                                                      """Teamaker was developed by the USDA and was released by the ARS Forage, Seed and Cereal Research Unit in Corvallis, Oregon. It is unique in the sense that it was bred to have low alpha acid content and high beta acid content.
      
      Due to its antibiotic properties, it is used as an alternative anitibiotic in livestock feed. It is also known for being used in teas, as the name suggests."""@en ;
                                     <http://xmlns.com/foaf/0.1/isPrimaryTopicOf> <https://rdf.ag/o/hops#jpr2007.02.0105crc> ;
                                     <http://xmlns.com/foaf/0.1/name> "Teamaker" ;
                                     <https://rdf.ag/o/hops#alphaAcidsContent> "0.6-1.8" ;
                                     <https://rdf.ag/o/hops#betaAcidsContent> "5.4-13.2" ;
                                     <https://rdf.ag/o/hops#perceivedAroma> "Aucune amertume"@fr ,
                                                                            "No bitterness"@en .


###  https://rdf.ag/o/hops#HopsTettnanger
<https://rdf.ag/o/hops#HopsTettnanger> rdf:type owl:Class ;
                                       rdfs:subClassOf <https://rdf.ag/o/hops#Hops> ;
                                       <http://rdfs.org/ns/void#inDataset> <https://rdf.ag/o/hops#datasetdefinition> ;
                                       rdfs:isDefinedBy <https://rdf.ag/o/hops-2021-07-30> ;
                                       rdfs:label "Deutscher Frühopfen"@de ,
                                                  "Schwetzinger"@de ,
                                                  "Tettnang"@en ,
                                                  "Tettnang Tettnanger"@en ,
                                                  "Tettnanger"@en ,
                                                  "Tettnanger (GR)"@en ;
                                       <http://www.w3.org/2004/02/skos/core#definition> "Le Tettnanger est une ancienne variété locale de houblon cultivée autour de Tettnang, un village en Allemagne. Cette variété est proche de Hallertau caractéristiquement et de Saaz génétiquement. Le Tettnanger cultivé ailleurs a très probablement été hybride avec Fuggle."@fr ,
                                                                                        "Tettnanger is old landrace variety of hops that is grown around Tettnang, a village in Germany. This variety is similar to Hallertau chariteristically and to Saaz genetically. Tettnanger grown elsewhere most likely have been hybridized with Fuggle."@en ;
                                       <http://xmlns.com/foaf/0.1/name> "Tettnanger" ;
                                       <https://rdf.ag/o/hops#alphaAcidsContent> "3-5.8" ;
                                       <https://rdf.ag/o/hops#betaAcidsContent> "2.8-5.3" ;
                                       <https://rdf.ag/o/hops#totalOilContent> "0.36-1.07" .


###  https://rdf.ag/o/hops#HopsTettnanger_A
<https://rdf.ag/o/hops#HopsTettnanger_A> rdf:type owl:Class ;
                                         rdfs:subClassOf <https://rdf.ag/o/hops#HopsTettnanger> ;
                                         <http://rdfs.org/ns/void#inDataset> <https://rdf.ag/o/hops#datasetdefinition> ;
                                         rdfs:isDefinedBy <https://rdf.ag/o/hops-2021-07-30> ;
                                         rdfs:label "Tettnanger A"@en ;
                                         <http://www.w3.org/2004/02/skos/core#definition> "Tettnanger A, similaire à son frère Tettnanger B, est une sélection clonale du Tettnanger allemand par le Dr Schmutz à l'Université de Hohenheim, en Allemagne, dans les années 1970. Ces deux sélections auraient un taux d'acide alpha plus élevé, mais les tests effectués aux États-Unis n'ont pas pu confirmer cette affirmation."@fr ,
                                                                                          "Tettnanger A, similar to its sibling Tettnanger B, is a clonal selection of the German Tettnanger by Dr. Schmutz at the University of Hohenheim, Germany, in the 1970s. These two selections are said to have higher alpha acid, however testing done in the US was unable to confirm this claim."@en ;
                                         <http://xmlns.com/foaf/0.1/name> "Tettnanger A" ;
                                         <https://rdf.ag/o/hops#alphaAcidsContent> "4.4" ;
                                         <https://rdf.ag/o/hops#betaAcidsContent> "5" ;
                                         <https://rdf.ag/o/hops#totalOilContent> "0.85" .


###  https://rdf.ag/o/hops#HopsTettnanger_B
<https://rdf.ag/o/hops#HopsTettnanger_B> rdf:type owl:Class ;
                                         rdfs:subClassOf <https://rdf.ag/o/hops#HopsTettnanger> ;
                                         <http://rdfs.org/ns/void#inDataset> <https://rdf.ag/o/hops#datasetdefinition> ;
                                         rdfs:isDefinedBy <https://rdf.ag/o/hops-2021-07-30> ;
                                         rdfs:label "Tettnanger B"@en ;
                                         <http://www.w3.org/2004/02/skos/core#definition> "Tettnanger B, similaire à son frère Tettnanger A, est une sélection clonale du Tettnanger allemand par le Dr Schmutz à l'Université de Hohenheim, en Allemagne, dans les années 1970. Ces deux sélections auraient un taux d'acide alpha plus élevé, mais les tests effectués aux États-Unis n'ont pas pu confirmer cette affirmation."@fr ,
                                                                                          "Tettnanger B, similar to its sibling Tettnanger A, is a clonal selection of the German Tettnanger by Dr. Schmutz at the University of Hohenheim, Germany, in the 1970s. These two selections are said to have higher alpha acid, however testing done in the US was unable to confirm this claim."@en ;
                                         <http://xmlns.com/foaf/0.1/name> "Tettnanger B" ;
                                         <https://rdf.ag/o/hops#alphaAcidsContent> "5.3" ;
                                         <https://rdf.ag/o/hops#betaAcidsContent> "5.2" ;
                                         <https://rdf.ag/o/hops#totalOilContent> "0.90" .


###  https://rdf.ag/o/hops#HopsTettnanger_CH
<https://rdf.ag/o/hops#HopsTettnanger_CH> rdf:type owl:Class ;
                                          rdfs:subClassOf <https://rdf.ag/o/hops#Hops> ;
                                          <http://rdfs.org/ns/void#inDataset> <https://rdf.ag/o/hops#datasetdefinition> ;
                                          rdfs:isDefinedBy <https://rdf.ag/o/hops-2021-07-30> ;
                                          rdfs:label "Tettnanger (Swiss)"@en ;
                                          <http://www.w3.org/2004/02/skos/core#definition> "Le Tettnanger Suisse est génétiquement différent du Tettnanger Allemand car il a été découvert que la variété cultivée en Suisse était en fait dérivée de Fuggle. Il est, cependant, toujours caractéristiquement similaire au Tettnanger allemand."@fr ,
                                                                                           "Swiss Tettnanger is genetically different from the German Tettnanger as the variety grown in Switzerland has been found to have actually been derived from Fuggle. It is, however, still characteristically similar to the German Tettnanger."@en ;
                                          <http://xmlns.com/foaf/0.1/name> "Tettnanger (Swiss)" ;
                                          <https://rdf.ag/o/hops#alphaAcidsContent> "4.1-6.3" ;
                                          <https://rdf.ag/o/hops#betaAcidsContent> "3.6-5.7" ;
                                          <https://rdf.ag/o/hops#totalOilContent> "0.42-1.13" .


###  https://rdf.ag/o/hops#HopsTettnanger_US
<https://rdf.ag/o/hops#HopsTettnanger_US> rdf:type owl:Class ;
                                          rdfs:subClassOf <https://rdf.ag/o/hops#HopsTettnanger_CH> ;
                                          <http://rdfs.org/ns/void#inDataset> <https://rdf.ag/o/hops#datasetdefinition> ;
                                          rdfs:isDefinedBy <https://rdf.ag/o/hops-2021-07-30> ;
                                          rdfs:label "Tettnanger (US)"@en ;
                                          <http://www.w3.org/2004/02/skos/core#definition> "US Tettnanger est un clone de rhizome du Tettnanger suisse importé aux États-Unis. Les propriétés peuvent différer légèrement en raison du terroir ou de la pollinisation croisée."@fr ,
                                                                                           "US Tettnanger is a rhizome clone of the Swiss Tettnanger brought over to the US. The properties may differ slightly due to terroir or from cross pollination."@en ;
                                          <http://xmlns.com/foaf/0.1/name> "Tettnanger (US)" ;
                                          <https://rdf.ag/o/hops#alphaAcidsContent> "4-5" ;
                                          <https://rdf.ag/o/hops#betaAcidsContent> "3-4.5" ;
                                          <https://rdf.ag/o/hops#totalOilContent> "0.4-0.8" .


###  https://rdf.ag/o/hops#HopsTomahawk
<https://rdf.ag/o/hops#HopsTomahawk> rdf:type owl:Class ;
                                     rdfs:subClassOf <https://rdf.ag/o/hops#Hops> ;
                                     <http://rdfs.org/ns/void#inDataset> <https://rdf.ag/o/hops#datasetdefinition> ;
                                     rdfs:isDefinedBy <https://rdf.ag/o/hops-2021-07-30> ;
                                     rdfs:label "Tomahawk®"@en ;
                                     <http://www.w3.org/2004/02/skos/core#definition> "La lignée de Tomahawk® n'est pas connue. Il est génétiquement identique à Columbus, mais en raison d'un différend juridique entre Hopunion et Yakima Chief, les deux noms ont été enregistrés lorsque les deux parties ont tenté de breveter indépendamment la même variété. Columbus/Tomahawk® a été élevé pour sa teneur élevée en acide alpha et est souvent vendu avec Zeus en tant que CTZ."@fr ,
                                                                                      "The lineage of Tomahawk® is not known. It is genetically identical to Columbus, however due to a legal dispute between Hopunion and Yakima Chief both names were registered when the two parties tried to independently patent the same variety. Columbus/Tomahawk® was bred for its high alpha acid content and is often sold with Zeus as CTZ."@en ;
                                     <http://xmlns.com/foaf/0.1/name> "Tomahawk®" ;
                                     <https://rdf.ag/o/hops#alphaAcidsContent> "14-18" ;
                                     <https://rdf.ag/o/hops#betaAcidsContent> "4.5-6" ;
                                     <https://rdf.ag/o/hops#totalOilContent> "1.5-4.5" .


###  https://rdf.ag/o/hops#HopsTriplePearl
<https://rdf.ag/o/hops#HopsTriplePearl> rdf:type owl:Class ;
                                        rdfs:subClassOf <https://rdf.ag/o/hops#Hops> ;
                                        <http://rdfs.org/ns/void#inDataset> <https://rdf.ag/o/hops#datasetdefinition> ;
                                        rdfs:isDefinedBy <https://rdf.ag/o/hops-2021-07-30> ;
                                        rdfs:label "TriplePearl"@en ,
                                                   "TriplePearl"@fr ;
                                        <http://www.w3.org/2004/02/skos/core#definition> "TriplePearl a été développé par l'USDA-ARS comme une variété de «Perle» sans pépins et plus résistante aux virus. Le projet de recherche USDA-ARS n ° 425226 a réussi à créer un houblon triploïde (stérile) en 2013."@fr ,
                                                                                         "TriplePearl was developped by the USDA-ARS as a seedless, more virus-resistant variety of 'Perle'. The USDA-ARS Research Project #425226 succeeded in creating a triploid (sterile) hop in 2013."@en ;
                                        <http://xmlns.com/foaf/0.1/name> "Triple Pearl" ;
                                        <https://rdf.ag/o/hops#alphaAcidsContent> "10.2–11.2" ;
                                        <https://rdf.ag/o/hops#betaAcidsContent> "3.3-4.2" ;
                                        <https://rdf.ag/o/hops#perceivedAroma> "Melon, Orange Rind/Zest, Orange-Citrus, Pepper, Resin, Spicy"@en ,
                                                                               "Épicé, Melon, Orange-agrumes, Poivre, Résine, Zeste d'orange"@fr ;
                                        <https://rdf.ag/o/hops#totalOilContent> "1.1-1.8" .


###  https://rdf.ag/o/hops#HopsUltra
<https://rdf.ag/o/hops#HopsUltra> rdf:type owl:Class ;
                                  rdfs:subClassOf <https://rdf.ag/o/hops#Hops> ;
                                  <http://rdfs.org/ns/void#inDataset> <https://rdf.ag/o/hops#datasetdefinition> ;
                                  rdfs:isDefinedBy <https://rdf.ag/o/hops-2021-07-30> ;
                                  rdfs:label "Ultra"@en ;
                                  <http://www.w3.org/2004/02/skos/core#definition> "Le houblon Ultra a été développé en Oregon, aux États-Unis et a été commercialisé en 1995. Il est connu pour sa teneur élevée en humulène, qui donne un arôme épicé."@fr ,
                                                                                   "Ultra hops were developed in Oregon, US and was commercially released in 1995. It is known for its high humulene content, which results in a spicy aroma."@en ;
                                  <http://xmlns.com/foaf/0.1/name> "Ultra" ;
                                  <https://rdf.ag/o/hops#alphaAcidsContent> "3-5" ;
                                  <https://rdf.ag/o/hops#betaAcidsContent> "3.6-5" ;
                                  <https://rdf.ag/o/hops#perceivedAroma> "Earthy, Floral, herbal, Spicy"@en ,
                                                                         "Épicé, Floral, Herbal, Terreux"@fr ;
                                  <https://rdf.ag/o/hops#totalOilContent> "0.8-1.2" .


###  https://rdf.ag/o/hops#HopsVanguard
<https://rdf.ag/o/hops#HopsVanguard> rdf:type owl:Class ;
                                     rdfs:subClassOf <https://rdf.ag/o/hops#Hops> ;
                                     <http://rdfs.org/ns/void#inDataset> <https://rdf.ag/o/hops#datasetdefinition> ;
                                     rdfs:isDefinedBy <https://rdf.ag/o/hops-2021-07-30> ;
                                     rdfs:label "Vanguard"@en ;
                                     <http://www.w3.org/2004/02/skos/core#definition> "Vanguard est un produit du programme de sélection de houblon de l'USDA et a été publié en 1997. Il a les propriétés uniques d'avoir une teneur bas en acide alpha, une teneur élevée en acide bêta, des niveaux élevés d'humulène et de faibles niveaux de cohumulone."@fr ,
                                                                                      "Vanguard is a product of the USDA’s hop breeding program and was released in 1997. It has the unique properties of having a low alpha acid content, high beta acid content, high levels of humulene and low levels cohumulone."@en ;
                                     <http://xmlns.com/foaf/0.1/name> "Vanguard" ;
                                     <https://rdf.ag/o/hops#alphaAcidsContent> "4.40-6" ;
                                     <https://rdf.ag/o/hops#betaAcidsContent> "6-7" ;
                                     <https://rdf.ag/o/hops#perceivedAroma> "Blackcurrant, Floral, Herbal"@en ,
                                                                            "Cassis, Floral, Herbacé"@fr ;
                                     <https://rdf.ag/o/hops#totalOilContent> "0.9-1.2" .


###  https://rdf.ag/o/hops#HopsWaiiti
<https://rdf.ag/o/hops#HopsWaiiti> rdf:type owl:Class ;
                                   rdfs:subClassOf <https://rdf.ag/o/hops#Hops> ;
                                   <http://rdfs.org/ns/void#inDataset> <https://rdf.ag/o/hops#datasetdefinition> ;
                                   rdfs:isDefinedBy <https://rdf.ag/o/hops-2021-07-30> ;
                                   rdfs:label "Wai-iti™"@en ;
                                   <http://www.w3.org/2004/02/skos/core#definition> "Wai-iti™ est un houblon de marque élevé par New Zealand Plant and Food Research avec son pedigree composé de Hallertauer Mittelfrüh et Liberty et il appartient à New Zealand Hops Limited. Il a été publié en 2011 et est connu pour ses teneurs élevées en acides alpha et bêta et sa teneur bas en cohumulone."@fr ,
                                                                                    "Wai-iti™ is a trademarked hop bred by New Zealand Plant and Food Research with its pedigree consisting of Hallertauer Mittelfrüh and Liberty and it is owned by New Zealand Hops Limited. It was released in 2011 and is known for high alpha and beta acid contents and low cohumulone."@en ;
                                   <http://xmlns.com/foaf/0.1/name> "Wai-iti™" ;
                                   <https://rdf.ag/o/hops#alphaAcidsContent> "2.5-3.5" ;
                                   <https://rdf.ag/o/hops#betaAcidsContent> "4.5-5.5" ;
                                   <https://rdf.ag/o/hops#perceivedAroma> "Citron Vert, Fruits à Noyau"@fr ,
                                                                          "Lime, Stone Fruit"@en ;
                                   <https://rdf.ag/o/hops#totalOilContent> "1.6" .


###  https://rdf.ag/o/hops#HopsWaimea
<https://rdf.ag/o/hops#HopsWaimea> rdf:type owl:Class ;
                                   rdfs:subClassOf <https://rdf.ag/o/hops#Hops> ;
                                   <http://rdfs.org/ns/void#inDataset> <https://rdf.ag/o/hops#datasetdefinition> ;
                                   rdfs:isDefinedBy <https://rdf.ag/o/hops-2021-07-30> ;
                                   rdfs:label "Waimea™"@en ;
                                   <http://www.w3.org/2004/02/skos/core#definition> "Waimea™ est un houblon de marque appartenant à New Zealand Hops Limited qui a été lancé en 2012, un descendant du Californian Late Cluster, Fuggle et Saaz et élevé pour avoir une teneur élevée en acide alpha."@fr ,
                                                                                    "Waimea™ is a trademarked hop owned by New Zealand Hops Limited that was released in 2012, a descendant of Californian Late Cluster, Fuggle and Saaz and bred to have a high alpha acid content."@en ;
                                   <http://xmlns.com/foaf/0.1/name> "Waimea™" ;
                                   <https://rdf.ag/o/hops#alphaAcidsContent> "16-19" ;
                                   <https://rdf.ag/o/hops#betaAcidsContent> "7-9" ;
                                   <https://rdf.ag/o/hops#perceivedAroma> "Agrumes, Pin"@fr ,
                                                                          "Citrus, Pine"@en ;
                                   <https://rdf.ag/o/hops#totalOilContent> "2.1" .


###  https://rdf.ag/o/hops#HopsWakatu
<https://rdf.ag/o/hops#HopsWakatu> rdf:type owl:Class ;
                                   rdfs:subClassOf <https://rdf.ag/o/hops#Hops> ;
                                   <http://rdfs.org/ns/void#inDataset> <https://rdf.ag/o/hops#datasetdefinition> ;
                                   rdfs:comment "Ce houblon a le statut de marque 602 - Abandonné - Échec de réponse ou réponse tardive"@fr ,
                                                "This hop has the trademark status 602 - Abandoned-Failure To Respond Or Late Response"@en ;
                                   rdfs:isDefinedBy <https://rdf.ag/o/hops-2021-07-30> ;
                                   rdfs:label "Wakatu"@en ;
                                   <http://www.w3.org/2004/02/skos/core#definition> "Wakatu est un descendant de Hallertauer Mittelfrüher et un houblon originaire de Nouvelle-Zélande. Il a été élevé par le programme de sélection de houblon de l'Institut néo-zélandais de recherche sur les plantes et l'alimentation et publié en 1988."@fr ,
                                                                                    "Wakatu is a descendant of Hallertauer Mittelfrüher and a native New Zealand hop. It was bred by the New Zealand Institute for Plant and Food Research’s hop breeding program and released in 1988."@en ;
                                   <http://xmlns.com/foaf/0.1/name> "Wakatu" ;
                                   <https://rdf.ag/o/hops#alphaAcidsContent> "6.5-8.5" ;
                                   <https://rdf.ag/o/hops#betaAcidsContent> "8.5" ;
                                   <https://rdf.ag/o/hops#perceivedAroma> "Citron Vert, Floral, Vanille"@fr ,
                                                                          "Lime, Floral, Vanilla"@en ;
                                   <https://rdf.ag/o/hops#totalOilContent> "1.0" .


###  https://rdf.ag/o/hops#HopsWarrior
<https://rdf.ag/o/hops#HopsWarrior> rdf:type owl:Class ;
                                    rdfs:subClassOf <https://rdf.ag/o/hops#Hops> ;
                                    <http://rdfs.org/ns/void#inDataset> <https://rdf.ag/o/hops#datasetdefinition> ;
                                    rdfs:isDefinedBy <https://rdf.ag/o/hops-2021-07-30> ;
                                    rdfs:label "Warrior®"@en ,
                                               "Warrior® Brand YCR 5"@en ;
                                    <http://www.w3.org/2004/02/skos/core#definition> "Warrior® a été développé par Select Botanicals Group, maintenant Yakima Chief Ranches, pour sa teneur élevée en acide alpha."@fr ,
                                                                                     "Warrior® was developed by Select Botanicals Group, now Yakima Chief Ranches, for its high alpha acid content."@en ;
                                    <http://xmlns.com/foaf/0.1/name> "Warrior®" ;
                                    <https://rdf.ag/o/hops#alphaAcidsContent> "14.5-18" ;
                                    <https://rdf.ag/o/hops#betaAcidsContent> "4.3-6" ;
                                    <https://rdf.ag/o/hops#perceivedAroma> "Agrumes, Épicé"@fr ,
                                                                           "Citrus, Spicy"@en ;
                                    <https://rdf.ag/o/hops#totalOilContent> "1-2" .


###  https://rdf.ag/o/hops#HopsWhitbreadGolding
<https://rdf.ag/o/hops#HopsWhitbreadGolding> rdf:type owl:Class ;
                                             rdfs:subClassOf <https://rdf.ag/o/hops#HopsGolding> ;
                                             <http://rdfs.org/ns/void#inDataset> <https://rdf.ag/o/hops#datasetdefinition> ;
                                             rdfs:isDefinedBy <https://rdf.ag/o/hops-2021-07-30> ;
                                             rdfs:label "WGV"@en ,
                                                        "Whitbread Golding"@en ;
                                             <http://www.w3.org/2004/02/skos/core#definition> "Connu à l'origine sous le nom de White's Golding parce qu'il a été cultivé en 1911 par M. White, il a ensuite été remplacé par Whitbread lorsque la brasserie Whitbread a acheté la ferme de M. White."@fr ,
                                                                                              "Originally known as White's Golding because it was grown in 1911 by Mr. White, it was then changed to Whitbread when Whitbread Brewery purchased Mr. White's farm."@en ;
                                             <http://xmlns.com/foaf/0.1/name> "Whitbread Golding" ;
                                             <https://rdf.ag/o/hops#alphaAcidsContent> "5-7.5" ;
                                             <https://rdf.ag/o/hops#betaAcidsContent> "2.5-3.5" ;
                                             <https://rdf.ag/o/hops#totalOilContent> "0.8-1.22" .


###  https://rdf.ag/o/hops#HopsWillamette
<https://rdf.ag/o/hops#HopsWillamette> rdf:type owl:Class ;
                                       rdfs:subClassOf <https://rdf.ag/o/hops#Hops> ;
                                       <http://rdfs.org/ns/void#inDataset> <https://rdf.ag/o/hops#datasetdefinition> ;
                                       rdfs:isDefinedBy <https://rdf.ag/o/hops-2021-07-30> ;
                                       rdfs:label "Willamette"@en ,
                                                  "Willamette"@fr ;
                                       <http://www.w3.org/2004/02/skos/core#definition> "Willamette est l'un des cultivars de houblon les plus populaires cultivés aux États-Unis et un descendant de Fuggle. Il a été nommé d'après la rivière Willamette qui traverse l'Oregon, où il a été développé par le programme de sélection USDA et publié en 1976. Il se caractérise par une faible teneur en acide alpha."@fr ,
                                                                                        "Willamette is one of the most popular hop cultivars grown in the US and a descendant of Fuggle. It was named after Willamette River that runs through Oregon, where it was developed by the USDA breeding program and released in 1976. It is characterized by having a low alpha acid content."@en ;
                                       <http://xmlns.com/foaf/0.1/isPrimaryTopicOf> <https://rdf.ag/o/hops#sci1976.0011183X001600050043x> ;
                                       <http://xmlns.com/foaf/0.1/name> "Willamette" ;
                                       <https://rdf.ag/o/hops#alphaAcidsContent> "4.0–6.0" ;
                                       <https://rdf.ag/o/hops#betaAcidsContent> "3.5–4.5" ;
                                       <https://rdf.ag/o/hops#perceivedAroma> "Agrumes, Caramel, Curry, Encens, Sureau"@fr ,
                                                                              "Caramel, Citrus, Curry, Elderberry, Incense"@en ;
                                       <https://rdf.ag/o/hops#substitute> "Fuggle (US), Glacier, Styrian Golding, Tettnanger (US)" ;
                                       <https://rdf.ag/o/hops#totalOilContent> "1.0-1.5" .


###  https://rdf.ag/o/hops#HopsYugoslaviaGolding
<https://rdf.ag/o/hops#HopsYugoslaviaGolding> rdf:type owl:Class ;
                                              rdfs:subClassOf <https://rdf.ag/o/hops#HopsFuggle> ;
                                              <http://rdfs.org/ns/void#inDataset> <https://rdf.ag/o/hops#datasetdefinition> ;
                                              rdfs:isDefinedBy <https://rdf.ag/o/hops-2021-07-30> ;
                                              rdfs:label "Yugoslavia Golding"@en ;
                                              <http://www.w3.org/2004/02/skos/core#definition> "Identical to Styrian Golding, however the USDA has an accession number for Yugoslavia Golding. It was received in 1961 under PI No. 250809 from Ljubljana, Yugoslavia."@en ,
                                                                                               "Identique à Styrian Golding, cependant l'USDA a un numéro d'accession pour Yougoslavia Golding. Il a été reçu en 1961 sous le numéro PI 250809 de Ljubljana, Yougoslavie."@fr ;
                                              <http://xmlns.com/foaf/0.1/name> "Yugoslavia Golding" .


###  https://rdf.ag/o/hops#HopsZeus
<https://rdf.ag/o/hops#HopsZeus> rdf:type owl:Class ;
                                 rdfs:subClassOf <https://rdf.ag/o/hops#Hops> ;
                                 <http://rdfs.org/ns/void#inDataset> <https://rdf.ag/o/hops#datasetdefinition> ;
                                 rdfs:isDefinedBy <https://rdf.ag/o/hops-2021-07-30> ;
                                 rdfs:label "Zeus"@en ;
                                 <http://www.w3.org/2004/02/skos/core#definition> "Zeus est un houblon hybride américain qui a été sélectionné pour sa teneur élevée en acide alpha. Il est souvent vendu dans le cadre du mélange CTZ (Columbus, Tomahawk®, Zeus)."@fr ,
                                                                                  "Zeus is an American hybrid hop that was bred for its high alpha acid content. It is often sold as part of the blend CTZ (Columbus, Tomahawk®, Zeus)."@en ;
                                 <http://xmlns.com/foaf/0.1/name> "Zeus" ;
                                 <https://rdf.ag/o/hops#alphaAcidsContent> "13-17.5" ;
                                 <https://rdf.ag/o/hops#betaAcidsContent> "4.5-6.5" ;
                                 <https://rdf.ag/o/hops#perceivedAroma> "Agrumes, Herbes"@fr ,
                                                                        "Citrus, Herbal"@en ;
                                 <https://rdf.ag/o/hops#totalOilContent> "2.4-4.5" .


###  https://rdf.ag/o/hops#Rakau
<https://rdf.ag/o/hops#Rakau> rdf:type owl:Class ;
                              rdfs:subClassOf <https://rdf.ag/o/hops#Hops> ;
                              <http://rdfs.org/ns/void#inDataset> <https://rdf.ag/o/hops#datasetdefinition> ;
                              rdfs:comment "La marque déposée de Rakau a le statut 602 - Abandonné - Défaut de réponse ou réponse tardive."@fr ,
                                           "Rakau's trademark has status 602 - Abandoned-Failure To Respond Or Late Response."@en ;
                              rdfs:isDefinedBy <https://rdf.ag/o/hops-2021-07-30> ;
                              rdfs:label "AlphAroma"@en ,
                                         "Rakau"@en ;
                              <http://www.w3.org/2004/02/skos/core#definition> "Rakau, anciennement connu sous le nom d'AlphAroma, a été élevé en Nouvelle-Zélande à la fin des années 1970 à partir de Smooth Cone par pollinisation libre. Il est sorti en 1983 sous le nom d'AlphAroma et a ensuite été réédité sous le nom de Rakau en 2007 par New Zealand Hops Limited."@fr ,
                                                                               "Rakau, formerly known as AlphAroma, was bred in New Zealand in the late 1970’s from Smooth Cone through open pollination. It was released in 1983 under the name AlphAroma and was then re-released under the name Rakau in 2007 by New Zealand Hops Limited."@en ;
                              <http://xmlns.com/foaf/0.1/name> "Rakau" ;
                              <https://rdf.ag/o/hops#alphaAcidsContent> "5.8-10.9" ;
                              <https://rdf.ag/o/hops#betaAcidsContent> "2.6-4.8" ;
                              <https://rdf.ag/o/hops#perceivedAroma> "Fruit De La Passion, Fruits Tropicaux, Pin"@fr ,
                                                                     "Passionfruit, Pine, Tropical Fruit"@en ;
                              <https://rdf.ag/o/hops#totalOilContent> "1.21" .


###  https://rdf.ag/o/malt#AcidatedMalt
<https://rdf.ag/o/malt#AcidatedMalt> rdf:type owl:Class ;
                                     rdfs:subClassOf <https://rdf.ag/o/malt#Malt> ;
                                     <http://rdfs.org/ns/void#inDataset> <https://rdf.ag/o/malt#datasetdefinition> ;
                                     rdfs:isDefinedBy <http://rdf.ag/o/malt-2021-03-24> ;
                                     rdfs:label "Acid Malt"@en ,
                                                "Acidated Malt"@en ,
                                                "Malt Acide"@fr ,
                                                "Malt Acidulé"@fr ;
                                     <http://www.w3.org/2004/02/skos/core#definition> """Grâce à quelques moyens de traitement, les malts acidulés sont des malts qui sont acides et sont utilisés pour abaisser le pH de la purée pour obtenir une activité enzymatique plus souhaitable et pour augmenter la récupération de l'extrait.
        
        L'acidation peut être obtenue par fermentation d'acide lactique après le séchage, la germination du grain macéré dans des conditions anaérobies jusqu'à ce qu'il devienne acide, ou par pulvérisation de malt vert avec Lactobacillus delbrückii (une bactérie lactique), puis maintenu à 50°C (122°F) pendant 24-36h avant la cuisson."""@fr ,
                                                                                      """Through a few processing means, acidated malts are malts that are acidic and are used to lower the pH of mash to achieve more desireable enzymatic activity and to increase extract recovery.
    
    Acidation can be achieved through lactic acid fermentation after kilning, germinating macerated grain in anaerobic conditions until it becomes acidic, or by spraying green malt with Lactobacillus delbrückii (a lactic acid bacteria) and then held at 50˚C (122˚F) for 24-36h before kilning."""@en .


###  https://rdf.ag/o/malt#BarleyMalt
<https://rdf.ag/o/malt#BarleyMalt> rdf:type owl:Class ;
                                   rdfs:subClassOf <https://rdf.ag/o/malt#Malt> ;
                                   <http://rdfs.org/ns/void#inDataset> <https://rdf.ag/o/malt#datasetdefinition> ;
                                   rdfs:isDefinedBy <http://rdf.ag/o/malt-2021-03-24> ;
                                   rdfs:label "Barley Malt"@en ,
                                              "Malt d'Orge"@fr ;
                                   <http://www.w3.org/2004/02/skos/core#definition> "Malt qui utilise de l'orge comme base."@fr ,
                                                                                    "Malt that uses barley as a base."@en .


###  https://rdf.ag/o/malt#CaramelMalt
<https://rdf.ag/o/malt#CaramelMalt> rdf:type owl:Class ;
                                    rdfs:subClassOf <https://rdf.ag/o/malt#Malt> ;
                                    <http://rdfs.org/ns/void#inDataset> <https://rdf.ag/o/malt#datasetdefinition> ;
                                    rdfs:isDefinedBy <http://rdf.ag/o/malt-2021-03-24> ;
                                    rdfs:label "Caramel Malt"@en ,
                                               "Malt au Caramel"@fr ;
                                    <http://www.w3.org/2004/02/skos/core#definition> "Caramel malts are malts that are the result of the endosperm of the base grain being liquified during the malting process and can even crystalize. The moisture content of the final product is higher due to stewing process that occurs between germination and kilning. Caramel malts come in a variety of colors from 20 EBC to 500 EBC, which gives beers a golden caramel color. This malt adds a sweet, caramel or toffee aroma. These malts quickly lose their aroma while in storage so they must be used soon after manufacture."@en ,
                                                                                     "Les malts de caramel sont des malts qui sont le résultat de la liquéfaction de l'endosperme du grain de base pendant le processus de maltage et peuvent même cristalliser. La teneur en humidité du produit final est plus élevée en raison du processus de cuisson qui se produit entre la germination et la cuisson. Les malts au caramel sont disponibles dans une variété de couleurs allant de 20 EBC à 500 EBC, ce qui donne aux bières une couleur caramel dorée. Ce malt ajoute un arôme sucré, caramel ou caramel. Ces malts perdent rapidement leur arôme au cours du stockage, ils doivent donc être utilisés peu de temps après leur fabrication."@fr .


###  https://rdf.ag/o/malt#ChocolateMalt
<https://rdf.ag/o/malt#ChocolateMalt> rdf:type owl:Class ;
                                      rdfs:subClassOf <https://rdf.ag/o/malt#RoastedMalt> ;
                                      <http://rdfs.org/ns/void#inDataset> <https://rdf.ag/o/malt#datasetdefinition> ;
                                      rdfs:comment "For roasted malts, the classes Pale Chocolate Malt, Standard Chocolate Malt and Black Malt have the general ranges of EBC coloring assigned to each of these classes. It is important to note that there are significant gaps between these ranges despite all being in the same Roasted Malt class. This is due to the fact that much of the coloring is at the decretion of the operator of the roasting drum, therefore coloring may vary from malters or even between batches. In the end, it is the malters who decide under which class the product will be marketed."@en ,
                                                   "Pour les malts torréfiés, les classes Malt au Chocolat Pâle, Malt au Chocolat Standard et Malt Noir ont les gammes générales de coloration EBC attribuées à chacune de ces classes. Il est important de noter qu'il existe des écarts importants entre ces gammes, bien qu'elles appartiennent toutes à la même classe de malt torréfié. Cela est dû au fait qu'une grande partie de la coloration est à la décrétion de l'opérateur du tambour de torréfaction, donc la coloration peut varier d'un malter ou même d'un lot à l'autre. En fin de compte, ce sont les malters qui décident sous quelle classe le produit sera commercialisé."@fr ;
                                      rdfs:isDefinedBy <http://rdf.ag/o/malt-2021-03-24> ;
                                      rdfs:label "Chocolate Malt"@en ,
                                                 "Malt au Chocolat"@fr ;
                                      <http://www.w3.org/2004/02/skos/core#definition> "Malts torréfiés qui ont un arôme quelque peu chocolaté et dont la coloration varie de 500-1100 EBC."@fr ,
                                                                                       "Roasted malts that that have a somewhat chocolatey aroma and whose coloring varies from 500-1100 EBC."@en .


###  https://rdf.ag/o/malt#Malt
<https://rdf.ag/o/malt#Malt> rdf:type owl:Class ;
                             rdfs:subClassOf <http://www.beerecipe.com/ontology#Ingredient> ;
                             <http://rdfs.org/ns/void#inDataset> <https://rdf.ag/o/malt#datasetdefinition> ;
                             rdfs:isDefinedBy <http://rdf.ag/o/malt-2021-03-24> ;
                             rdfs:label "Malt"@en ,
                                        "Malt"@fr ;
                             <http://www.w3.org/2004/02/skos/core#definition> """Le malt est le résultat du processus de maltage par lequel un grain (ou parfois des légumineuses), généralement de l'orge, est partiellement germé puis soumis à un processus de séchage ou de torréfaction.
       
       Le malt est un élément essentiel du brassage de la bière. En démarrant le processus de germination des grains (ou légumineuses), des enzymes sont activées pour commencer à convertir l'amidon de la graine en sucre (principalement maltose) et en acides aminés. Ensuite, les grains sont séchés ou torréfiés pour arrêter l'activité enzymatique jusqu'à ce que le brasseur soit prêt à brasser de la bière."""@fr ,
                                                                              """Malt is the result of the malting process by which a grain (or sometimes pulse), usually barley is partially germinated and then subjected to a drying or roasting process.
       
       Malt is an essential part of brewing beer. By starting the germination process of the grains (or pulses), enzymes are activated to start converting the starch in the seed into sugar (mainly maltose) and amino acids. Then the grains are dried or roasted to halt enzyme activity until the brewer is ready to brew the beer."""@en .


###  https://rdf.ag/o/malt#MunichMalt
<https://rdf.ag/o/malt#MunichMalt> rdf:type owl:Class ;
                                   rdfs:subClassOf <https://rdf.ag/o/malt#TwoRowBarleyMalt> ;
                                   <http://rdfs.org/ns/void#inDataset> <https://rdf.ag/o/malt#datasetdefinition> ;
                                   rdfs:isDefinedBy <http://rdf.ag/o/malt-2021-03-24> ;
                                   rdfs:label "Malt de Munich"@fr ,
                                              "Munich Malt"@en ,
                                              "Münchener Malz"@de ;
                                   <http://www.w3.org/2004/02/skos/core#definition> "Les malts de Munich sont généralement utilisés pour les bières d'Oktoberfest. Ce sont des malts plus foncés (15-30 EBC) et riches en arômes en raison d'une cuisson plus longue. Comparés aux malts pâles, les malts de Munich ne sont pas aussi fermentescibles, ont des temps de conversion plus lents et sont pauvres en enzymes."@fr ,
                                                                                    "Munich malts are typically used for Oktoberfest beers. They are darker malts (15-30 EBC) and rich in aroma due to longer kilning. Compared to pale malts, Munich malts are are not as fermentable, slower coversion times, and are poor in enzymes."@en .


###  https://rdf.ag/o/malt#PaleAleMalt
<https://rdf.ag/o/malt#PaleAleMalt> rdf:type owl:Class ;
                                    rdfs:subClassOf <https://rdf.ag/o/malt#TwoRowBarleyMalt> ;
                                    <http://rdfs.org/ns/void#inDataset> <https://rdf.ag/o/malt#datasetdefinition> ;
                                    rdfs:comment "English malters typically favor local barley cultivars."@en ,
                                                 "Les malters anglais préfèrent généralement les cultivars d'orge locaux."@fr ;
                                    rdfs:isDefinedBy <http://rdf.ag/o/malt-2021-03-24> ;
                                    rdfs:label "Malt de Bière Pâle"@fr ,
                                               "Pale Ale Malt"@en ;
                                    <http://www.w3.org/2004/02/skos/core#definition> """Les malts de bière pâles et doux sont généralement utilisés pour brasser des bières de style britannique. L'orge à deux rangs à faible teneur en azote (1,35 à 1.5%) est généralement utilisée comme base pour les malts de bière blonde. Les malts de bière légère utilisent généralement de l'orge à deux rangs avec des pourcentages plus élevés de nigtrogen (1.6-1.65%).
                
        Les malts finis sont généralement plus foncés que les malts lager et plus aromatisés au malt, ont environ 4-6.5 unités EBC, ont une valeur TSN de 0.5-0.7% et des ratios TSN: TN d'environ 40%."""@fr ,
                                                                                     """Pale and mild ale malts are typically used to brew British-style ales. Low nitrogen (1.35-1.5%), two-row barley are typically used as a base for pale ale malts. Mild ale malts generally use two-row barley with higher percentages of nigtrogen (1.6-1.65%).
        
        Finished malts are typically darker than lager malts and more malty flavored, have about 4-6.5 EBC units, have a TSN value of 0.5-0.7%, and TSN:TN ratios of about 40%."""@en .


###  https://rdf.ag/o/malt#PaleAleMaltingActivity
<https://rdf.ag/o/malt#PaleAleMaltingActivity> rdf:type owl:Class ;
                                               rdfs:subClassOf <https://rdf.ag/o/MaltingActivity> ;
                                               <http://rdfs.org/ns/void#inDataset> <https://rdf.ag/o/malt#datasetdefinition> ;
                                               rdfs:isDefinedBy <http://rdf.ag/o/malt-2021-03-24> ;
                                               rdfs:label "Maltage de la Bière Pâle"@fr ,
                                                          "Pale Ale Malting"@en ;
                                               <http://www.w3.org/2004/02/skos/core#definition> """ The barley grain must be well and evenly modified (the part of the germination process where the endosperm breaks down), although slightly less well-modified grains lead to better head retention. Under-modified grains lead to problems with beer infiltration and instability, poor extract recoveries, and slow wort recovery rates.
        
        The grains must then be dried with cool and rapid airflow. The airflow temperature is then raised to 60-90˚C (140-194˚F) and then cured at a temperature of around 105˚C and are removed from the kiln until they have a moisture content of about 1%, although the acceptance higher delivered moisture contents (up to 4%) has reduced kilning costs."""@en ,
                                                                                                """Le grain d'orge doit être bien et uniformément modifié (la partie du processus de germination où l'endosperme se décompose), bien que des grains légèrement moins bien modifiés conduisent à une meilleure rétention de la tête. Les grains sous-modifiés entraînent des problèmes d'infiltration et d'instabilité de la bière, de mauvaises récupérations d'extrait et des taux de récupération du moût lents.
        
        Les grains doivent ensuite être séchés avec un flux d'air frais et rapide. La température du flux d'air est ensuite élevée à 60-90°C (140-194°F), puis durcie à une température d'environ 105°C et est retirée du four jusqu'à ce qu'elle ait une teneur en humidité d'environ 1%, bien que l'acceptation des teneurs plus élevées en humidité (jusqu'à 4%) ont réduit les coûts de cuisson."""@fr .


###  https://rdf.ag/o/malt#PilsnerMalt
<https://rdf.ag/o/malt#PilsnerMalt> rdf:type owl:Class ;
                                    rdfs:subClassOf <https://rdf.ag/o/malt#TwoRowBarleyMalt> ;
                                    <http://rdfs.org/ns/void#inDataset> <https://rdf.ag/o/malt#datasetdefinition> ;
                                    rdfs:isDefinedBy <http://rdf.ag/o/malt-2021-03-24> ;
                                    rdfs:label "Malt de Pilsner"@fr ,
                                               "Pilsner Malt"@en ;
                                    <http://www.w3.org/2004/02/skos/core#definition> "La Pilsner, ainsi que d'autres malts de bière blonde, ont une couleur très pâle et des arômes faibles. Ils sont fabriqués avec de l'orge à deux rangs (TN 1,52-1,84%, protéines brutes 9,5-11,5%) qui est trempé à une teneur en humidité d'environ 43%. La période de germination est généralement plus longue et plus fraîche avec une température maximale de 17°C (62.6°F). Une fois que les grains ont germé, ils sont ensuite séchés en utilisant un flux d'air frais et rapide jusqu'à ce que la teneur en humidité soit d'environ 8%. Les grains sont ensuite lentement durcis avec des températures à montée lente qui ont un maximum de 70-85°C (158-185°F)."@fr ,
                                                                                     "Pilsner, as well as other lager malts, have a very pale color and weak aromas. They are made with two-row barley (TN 1.52-1.84%, crude protein 9.5-11.5%) that is steeped to a moisture content of about 43%. The germination period is typically longer and cooler with a maximum temperature of 17˚C (62.6˚F). Once the grains have germinated they are then dried using cool and fast airflow until the moisture content is about 8%. The grains are then slowly cured with slow-rising temperatures that have a maximum of 70-85˚C (158-185˚F)."@en .


###  https://rdf.ag/o/malt#RoastedMalt
<https://rdf.ag/o/malt#RoastedMalt> rdf:type owl:Class ;
                                    rdfs:subClassOf <https://rdf.ag/o/malt#Malt> ;
                                    <http://rdfs.org/ns/void#inDataset> <https://rdf.ag/o/malt#datasetdefinition> ;
                                    rdfs:isDefinedBy <http://rdf.ag/o/malt-2021-03-24> ;
                                    rdfs:label "Malt Torréfié"@fr ,
                                               "Roasted Malt"@en ;
                                    <http://www.w3.org/2004/02/skos/core#definition> "Malts dont les grains de base subissent un processus de torréfaction en fûts à haute température après germination. Les malts torréfiés sont souvent décrits comme ayant un arôme amer, riche ou chocolaté, une coloration qui varie de 500-1400 EBC à la discrétion de l'opérateur et avec peu ou pas d'activité enzymatique. L'enveloppe du grain fini doit être polie et brillante, l'endosperme ne doit pas être d'acier, carbonisé ou vitreux, mais doit être friable."@fr ,
                                                                                     "Malts whose base grains undergo a roasting process in drums at high temperatures after germination. Roasted malts are often decribed as having bitter, rich or chocolate aroma, coloring that varies from 500-1400 EBC at the descretion of the operator and with little to no enzymatic activity. The husk of the finished grain must be polished and shiny, the endosperm must not be steely, charred or glassy, rather they should be friable."@en .


###  https://rdf.ag/o/malt#SixRowBarleyMalt
<https://rdf.ag/o/malt#SixRowBarleyMalt> rdf:type owl:Class ;
                                         rdfs:subClassOf <https://rdf.ag/o/malt#BarleyMalt> ;
                                         <http://rdfs.org/ns/void#inDataset> <https://rdf.ag/o/malt#datasetdefinition> ;
                                         rdfs:isDefinedBy <http://rdf.ag/o/malt-2021-03-24> ;
                                         rdfs:label "Malt d'Orge à Six Rangs"@fr ,
                                                    "Six-Row Barley Malt"@en ;
                                         <http://www.w3.org/2004/02/skos/core#definition> "Malt qui utilise de l'orge à six rangs comme base."@fr ,
                                                                                          "Malt that uses six-row barley as a base."@en .


###  https://rdf.ag/o/malt#TwoRowBarleyMalt
<https://rdf.ag/o/malt#TwoRowBarleyMalt> rdf:type owl:Class ;
                                         rdfs:subClassOf <https://rdf.ag/o/malt#BarleyMalt> ;
                                         <http://rdfs.org/ns/void#inDataset> <https://rdf.ag/o/malt#datasetdefinition> ;
                                         rdfs:isDefinedBy <http://rdf.ag/o/malt-2021-03-24> ;
                                         rdfs:label "Malt d'Orge à Deux Rangs"@fr ,
                                                    "Two-Row Barley Malt"@en ;
                                         <http://www.w3.org/2004/02/skos/core#definition> "Malt qui utilise de l'orge à deux rangs comme base. L'orge à deux rangs est préférée pour le maltage car les grains sont souvent plus charnus que les grains d'orge à six rangs en raison du nombre plus faible de grains par tête d'orge."@fr ,
                                                                                          "Malt that uses two-row barley as a base. Two-row barley is preferred for malting since the grains are often plumper than six-row barley grain due to the lower number of grains per head of barley."@en .


###  https://rdf.ag/o/malt#ViennaMalt
<https://rdf.ag/o/malt#ViennaMalt> rdf:type owl:Class ;
                                   rdfs:subClassOf <https://rdf.ag/o/malt#TwoRowBarleyMalt> ;
                                   <http://rdfs.org/ns/void#inDataset> <https://rdf.ag/o/malt#datasetdefinition> ;
                                   rdfs:isDefinedBy <http://rdf.ag/o/malt-2021-03-24> ;
                                   rdfs:label "Malt de Vienna"@fr ,
                                              "Vienna Malt"@en ,
                                              "Weiner Malz"@de ;
                                   <http://www.w3.org/2004/02/skos/core#definition> "Les malts de Vienne se situent entre les malts Pilsner et Munich en termes de couleur (5-10 EBC) et fournissent la coloration pour les lagers brun doré. L'orge avec une teneur en protéines plus élevée est souvent utilisée. Les malts sont bons mais pas sur-modifiés, le processus de séchage est long, utilisant la recurculation de l'air dans le four et le processus de durcissement est terminé à environ 90°C (194°F). Contrairement aux malts caramalisés, l'endosperme n'est pas liquéfié."@fr ,
                                                                                    "Vienna malts fall between Pilsner and Munich malts in terms of color (5-10 EBC) and provide the coloring for golden brown lagers. Barley with higher protein content is often used. The malts are well but not over-modified, the drying process is long, using air recurculation in the kiln and the curing process is completed at around 90˚C (194˚F). Unlike caramalized malts, the endosperm is not liquified."@en .


###  https://rdf.ag/o/malt#WheatMalt
<https://rdf.ag/o/malt#WheatMalt> rdf:type owl:Class ;
                                  rdfs:subClassOf <https://rdf.ag/o/malt#Malt> ;
                                  <http://rdfs.org/ns/void#inDataset> <https://rdf.ag/o/malt#datasetdefinition> ;
                                  rdfs:isDefinedBy <http://rdf.ag/o/malt-2021-03-24> ;
                                  rdfs:label "Malt de Blé"@fr ,
                                             "Wheat Malt"@en ;
                                  <http://www.w3.org/2004/02/skos/core#definition> "Malt qui utilise du blé comme base."@fr ,
                                                                                   "Malt that uses wheat as a base."@en .


###  https://rdf.ag/o/malt#marisOtterMalt
<https://rdf.ag/o/malt#marisOtterMalt> rdf:type owl:Class ;
                                       rdfs:subClassOf <https://rdf.ag/o/malt#PaleAleMalt> ;
                                       <http://rdfs.org/ns/void#inDataset> <https://rdf.ag/o/malt#datasetdefinition> ;
                                       rdfs:isDefinedBy <http://rdf.ag/o/malt-2021-03-24> ;
                                       rdfs:label "Malt de Maris Otter"@fr ,
                                                  "Maris Otter Malt"@en ;
                                       <http://www.w3.org/2004/02/skos/core#definition> "A pale ale malt that has a barley grain base of the cultivar Maris Otter."@en ,
                                                                                        "Un malt de bière blonde à base de grains d'orge du cultivar Maris Otter."@fr .


###  https://schema.org/ProductGroup
<https://schema.org/ProductGroup> rdf:type owl:Class .


#################################################################
#    Individuals
#################################################################

###  http://www.beerecipe.com/ontology#US05_Yeast
<http://www.beerecipe.com/ontology#US05_Yeast> rdf:type owl:NamedIndividual ;
                                               <http://www.beerecipe.com/ontology#ingredientName> "Safale US-05 Dry Ale Yeast" ;
                                               <http://www.beerecipe.com/ontology#maxAttenuation> 0.82 ;
                                               <http://www.beerecipe.com/ontology#minAttenuation> 0.78 ;
                                               <http://www.beerecipe.com/ontology#optimalTemperature> "22.0"^^xsd:float ;
                                               <http://www.beerecipe.com/ontology#yeastDescription> "Neutral, well-balanced American ale yeast producing clean and crisp profiles; suitable for a wide range of ales including American Pale Ale, IPA and stouts." ;
                                               <http://www.beerecipe.com/ontology#yeastName> "SafAle US-05" ;
                                               rdfs:comment "Clean, neutral American ale yeast producing crisp profiles with medium attenuation, ideal for hop-forward beers." ;
                                               rdfs:label "Safale US-05" .


###  http://www.beerecipe.com/ontology#WLP001_Yeast
<http://www.beerecipe.com/ontology#WLP001_Yeast> rdf:type owl:NamedIndividual ,
                                                          <http://www.beerecipe.com/ontology#Yeast> ;
                                                 rdfs:comment "Clean, versatile ale yeast. Perfect for American IPAs" ;
                                                 rdfs:label "WLP001 California Ale Yeast" .


###  http://www.beerecipe.com/ontology#WLP007_Yeast
<http://www.beerecipe.com/ontology#WLP007_Yeast> rdf:type owl:NamedIndividual ;
                                                 <http://www.beerecipe.com/ontology#ingredientName> "WLP007 Dry English Ale" ;
                                                 <http://www.beerecipe.com/ontology#maxAttenuation> 80 ;
                                                 <http://www.beerecipe.com/ontology#minAttenuation> 70 ;
                                                 <http://www.beerecipe.com/ontology#optimalTemperature> "20.0"^^xsd:float ;
                                                 <http://www.beerecipe.com/ontology#yeastDescription> "Highly attenuative English ale yeast producing dry, clean finishes. Suitable for stouts and strong ales." ;
                                                 <http://www.beerecipe.com/ontology#yeastName> "WLP007 Dry English Ale" .


###  http://www.semanticweb.org/matte/ontologies/2025/10/untitled-ontology-4#AhtanumHop
:AhtanumHop rdf:type owl:NamedIndividual ,
                     <https://rdf.ag/o/hops#Hops> ;
            <http://www.beerecipe.com/ontology#alphaAcidPercentage> "6.0"^^xsd:float ;
            <http://www.beerecipe.com/ontology#hopName> "Ahtanum" ;
            rdfs:comment "American hop with floral, citrus and piney notes. Used for aroma" ;
            rdfs:label "Ahtanum" .


###  http://www.semanticweb.org/matte/ontologies/2025/10/untitled-ontology-4#Airlock
:Airlock rdf:type owl:NamedIndividual ,
                  <http://www.beerecipe.com/ontology#Equipment> ;
         <http://www.beerecipe.com/ontology#isRequiredBy> :BrewDog_PunkIPA_Recipe ;
         rdfs:comment "One-way valve allowing CO2 to escape during fermentation while preventing oxygen and contaminants from entering." ;
         rdfs:label "Airlock" .


###  http://www.semanticweb.org/matte/ontologies/2025/10/untitled-ontology-4#AmericanIPA
:AmericanIPA rdf:type owl:NamedIndividual ,
                      <http://www.beerecipe.com/ontology#BeerStyle> ;
             <http://www.beerecipe.com/ontology#maxABV> "7.5"^^xsd:float ;
             <http://www.beerecipe.com/ontology#maxIBU> 70 ;
             <http://www.beerecipe.com/ontology#minABV> "5.5"^^xsd:float ;
             <http://www.beerecipe.com/ontology#minIBU> 40 ;
             <http://www.beerecipe.com/ontology#styleDescription> "Hoppy, bitter, citrus-forward" ;
             <http://www.beerecipe.com/ontology#styleName> "American IPA" .


###  http://www.semanticweb.org/matte/ontologies/2025/10/untitled-ontology-4#BeginnerBoil60min
:BeginnerBoil60min rdf:type owl:NamedIndividual ,
                            <http://www.beerecipe.com/ontology#BrewingStep> ;
                   <http://www.beerecipe.com/ontology#stepDuration> 60 ;
                   <http://www.beerecipe.com/ontology#stepName> "Boil" ;
                   <http://www.beerecipe.com/ontology#stepOrder> 2 ;
                   <http://www.beerecipe.com/ontology#stepTemperature> "100.0"^^xsd:float .


###  http://www.semanticweb.org/matte/ontologies/2025/10/untitled-ontology-4#BeginnerMash45min
:BeginnerMash45min rdf:type owl:NamedIndividual ,
                            <http://www.beerecipe.com/ontology#BrewingStep> ;
                   <http://www.beerecipe.com/ontology#stepDuration> 45 ;
                   <http://www.beerecipe.com/ontology#stepName> "Mash" ;
                   <http://www.beerecipe.com/ontology#stepOrder> 1 ;
                   <http://www.beerecipe.com/ontology#stepTemperature> "66.0"^^xsd:float .


###  http://www.semanticweb.org/matte/ontologies/2025/10/untitled-ontology-4#Boil60min
:Boil60min rdf:type owl:NamedIndividual ,
                    <http://www.beerecipe.com/ontology#BoilStep> ;
           <http://www.beerecipe.com/ontology#stepDuration> 60 ;
           <http://www.beerecipe.com/ontology#stepName> "Boil" ;
           <http://www.beerecipe.com/ontology#stepOrder> 4 ;
           <http://www.beerecipe.com/ontology#stepTemperature> "100.0"^^xsd:float ;
           rdfs:comment "Sterilizes the wort, isomerizes hop alpha acids, and drives off unwanted volatile compounds."@en .


###  http://www.semanticweb.org/matte/ontologies/2025/10/untitled-ontology-4#BottlingEquipment
:BottlingEquipment rdf:type owl:NamedIndividual ,
                            <http://www.beerecipe.com/ontology#Equipment> ;
                   <http://www.beerecipe.com/ontology#isRequiredBy> :BrewDog_PunkIPA_Recipe ;
                   rdfs:comment "Bottles, caps, capper, and bottling wand for packaging finished beer. Alternative: kegging system." ;
                   rdfs:label "Bottling Equipment" .


###  http://www.semanticweb.org/matte/ontologies/2025/10/untitled-ontology-4#Bran_russinaImperialStout
:Bran_russinaImperialStout rdf:type owl:NamedIndividual ,
                                    <https://rdf.ag/o/beer#Beer> ;
                           rdfs:comment "Full-bodied Russian Imperial Stout with intense roasted malt character, 10.82% ABV and 64 IBU." ;
                           rdfs:label "Russian Imperial Stout" .


###  http://www.semanticweb.org/matte/ontologies/2025/10/untitled-ontology-4#BrewDog_PunkIPA_Recipe
:BrewDog_PunkIPA_Recipe rdf:type owl:NamedIndividual ,
                                 <http://www.beerecipe.com/ontology#Recipe> ;
                        <http://www.beerecipe.com/ontology#hasHop> :AhtanumHop ,
                                                                   :ChinookHop ,
                                                                   :NelsonSauvinHop ,
                                                                   :SimcoeHop ;
                        <http://www.beerecipe.com/ontology#hasMalt> :Caramalt ,
                                                                    :ExtraPaleMalt ;
                        <http://www.beerecipe.com/ontology#hasStyle> :IPA ;
                        <http://www.beerecipe.com/ontology#hasYeast> <http://www.beerecipe.com/ontology#WLP001_Yeast> ;
                        <http://www.beerecipe.com/ontology#producesBeer> :PunkIPA_Beer ;
                        <http://www.beerecipe.com/ontology#requiresEquipment> :Airlock ,
                                                                              :BottlingEquipment ,
                                                                              :BrewKettle ,
                                                                              :FermentationVessel ,
                                                                              :Hydrometer ,
                                                                              :MashTun ,
                                                                              :Sanitizer ,
                                                                              :Thermometer ,
                                                                              :WortChiller ;
                        :hasWater :Water ;
                        <http://www.beerecipe.com/ontology#author> "BrewDog" ;
                        <http://www.beerecipe.com/ontology#batchSize> "20.0"^^xsd:float ;
                        <http://www.beerecipe.com/ontology#boilingTime> 60 ;
                        <http://www.beerecipe.com/ontology#conditioningDuration> 14 ;
                        <http://www.beerecipe.com/ontology#creationDate> "2007-04-15"^^xsd:date ;
                        <http://www.beerecipe.com/ontology#difficultyLevel> "intermediate" ;
                        <http://www.beerecipe.com/ontology#estimatedABV> "5.6"^^xsd:float ;
                        <http://www.beerecipe.com/ontology#estimatedEBC> 17 ;
                        <http://www.beerecipe.com/ontology#estimatedIBU> 40 ;
                        <http://www.beerecipe.com/ontology#fermentationDuration> 10 ;
                        <http://www.beerecipe.com/ontology#finalGravity> "1.012"^^xsd:float ;
                        <http://www.beerecipe.com/ontology#isGlutenFree> "false"^^xsd:boolean ;
                        <http://www.beerecipe.com/ontology#isVegan> "true"^^xsd:boolean ;
                        <http://www.beerecipe.com/ontology#mashingTime> 65 ;
                        <http://www.beerecipe.com/ontology#originalGravity> "1.054"^^xsd:float ;
                        <http://www.beerecipe.com/ontology#recipeDescription> "Post Modern Classic. Layered with new world hops to create an explosion of tropical fruit and an all-out riot of grapefruit, pineapple and lychee before a spiky bitter finish. This is the beer that started it all - and it's not done yet." ;
                        <http://www.beerecipe.com/ontology#recipeName> "BrewDog Punk IPA" ;
                        <http://www.beerecipe.com/ontology#servingTemperature> "7.0"^^xsd:float ;
                        <http://www.beerecipe.com/ontology#totalBrewingTime> 300 .


###  http://www.semanticweb.org/matte/ontologies/2025/10/untitled-ontology-4#BrewKettle
:BrewKettle rdf:type owl:NamedIndividual ,
                     <http://www.beerecipe.com/ontology#Equipment> ;
            <http://www.beerecipe.com/ontology#isRequiredBy> :BrewDog_PunkIPA_Recipe ;
            rdfs:comment "Large pot or kettle for boiling wort with hops. Typically 25-30L capacity for homebrewing." ;
            rdfs:label "Brew Kettle" .


###  http://www.semanticweb.org/matte/ontologies/2025/10/untitled-ontology-4#CanadaWinterWheat
:CanadaWinterWheat rdf:type owl:NamedIndividual ;
                   <http://www.beerecipe.com/ontology#cerealName> "Canada winter wheat" ;
                   <http://www.beerecipe.com/ontology#glutenContent> "false"^^xsd:boolean .


###  http://www.semanticweb.org/matte/ontologies/2025/10/untitled-ontology-4#Caramalt
:Caramalt rdf:type owl:NamedIndividual ;
          <http://www.beerecipe.com/ontology#maltName> "Caramalt" ;
          <http://www.beerecipe.com/ontology#ebc> 30 ;
          rdfs:comment "Crystal malt for body, sweetness and golden color" ;
          rdfs:label "Caramalt" .


###  http://www.semanticweb.org/matte/ontologies/2025/10/untitled-ontology-4#CascadeHop
:CascadeHop rdf:type owl:NamedIndividual ,
                     <https://rdf.ag/o/hops#Hops> ;
            <http://www.beerecipe.com/ontology#alphaAcidPercentage> "5.5"^^xsd:float ;
            <http://www.beerecipe.com/ontology#hopName> "Cascade" ;
            rdfs:comment "Classic American aroma hop with floral and citrus (grapefruit) character, signature hop of American Pale Ales." ;
            rdfs:label "Cascade" .


###  http://www.semanticweb.org/matte/ontologies/2025/10/untitled-ontology-4#Cereal_RiceWheat
:Cereal_RiceWheat rdf:type owl:NamedIndividual ,
                           :Cereal ,
                           :RiceWheat ;
                  <http://www.beerecipe.com/ontology#cerealName> "Rice Wheat" ;
                  <http://www.beerecipe.com/ontology#glutenContent> "false"^^xsd:boolean .


###  http://www.semanticweb.org/matte/ontologies/2025/10/untitled-ontology-4#ChinookHop
:ChinookHop rdf:type owl:NamedIndividual ;
            <http://www.beerecipe.com/ontology#alphaAcidPercentage> "13.0"^^xsd:float ;
            <http://www.beerecipe.com/ontology#hopName> "Chinook" ;
            rdfs:comment "American hop variety with piney, spicy character. High alpha acids for bittering" ;
            rdfs:label "Chinook" .


###  http://www.semanticweb.org/matte/ontologies/2025/10/untitled-ontology-4#ChocolateMalt
:ChocolateMalt rdf:type owl:NamedIndividual ;
               <http://www.beerecipe.com/ontology#maltName> "Chocolate Malt" .


###  http://www.semanticweb.org/matte/ontologies/2025/10/untitled-ontology-4#Conditioning14days
:Conditioning14days rdf:type owl:NamedIndividual ,
                             <http://www.beerecipe.com/ontology#BrewingStep> ,
                             <http://www.beerecipe.com/ontology#ConditioningStep> ;
                    <http://www.beerecipe.com/ontology#stepDuration> 336 ;
                    <http://www.beerecipe.com/ontology#stepName> "Conditioning" ;
                    <http://www.beerecipe.com/ontology#stepOrder> 8 ;
                    <http://www.beerecipe.com/ontology#stepTemperature> "12.0"^^xsd:float ;
                    rdfs:comment "Maturation phase where flavors develop, beer clarifies and stabilizes."@en .


###  http://www.semanticweb.org/matte/ontologies/2025/10/untitled-ontology-4#CoolingToPitchTemp
:CoolingToPitchTemp rdf:type owl:NamedIndividual ,
                             <http://www.beerecipe.com/ontology#BrewingStep> ,
                             <http://www.beerecipe.com/ontology#CoolingStep> ;
                    <http://www.beerecipe.com/ontology#stepDuration> 30 ;
                    <http://www.beerecipe.com/ontology#stepName> "Cooling" ;
                    <http://www.beerecipe.com/ontology#stepOrder> 6 ;
                    <http://www.beerecipe.com/ontology#stepTemperature> "20.0"^^xsd:float ;
                    rdfs:comment "Rapidly cools the wort to the optimal fermentation temperature for pitching yeast."@en .


###  http://www.semanticweb.org/matte/ontologies/2025/10/untitled-ontology-4#EPA_Boil60min
:EPA_Boil60min rdf:type owl:NamedIndividual ,
                        <http://www.beerecipe.com/ontology#BoilStep> ,
                        <http://www.beerecipe.com/ontology#BrewingStep> ;
               <http://www.beerecipe.com/ontology#isStepOf> :EasyPaleAleRecipe ;
               <http://www.beerecipe.com/ontology#stepDuration> 60 ;
               <http://www.beerecipe.com/ontology#stepName> "Boil" ;
               <http://www.beerecipe.com/ontology#stepOrder> 4 ;
               <http://www.beerecipe.com/ontology#stepTemperature> "100.0"^^xsd:float ;
               rdfs:comment "Boil wort to sterilize, isomerize hops, and drive off volatiles for a clean pale ale flavor."@en .


###  http://www.semanticweb.org/matte/ontologies/2025/10/untitled-ontology-4#EPA_Conditioning14days
:EPA_Conditioning14days rdf:type owl:NamedIndividual ,
                                 <http://www.beerecipe.com/ontology#BrewingStep> ,
                                 <http://www.beerecipe.com/ontology#ConditioningStep> ;
                        <http://www.beerecipe.com/ontology#isStepOf> :EasyPaleAleRecipe ;
                        <http://www.beerecipe.com/ontology#stepDuration> 20160 ;
                        <http://www.beerecipe.com/ontology#stepName> "Conditioning" ;
                        <http://www.beerecipe.com/ontology#stepOrder> 8 ;
                        <http://www.beerecipe.com/ontology#stepTemperature> "12.0"^^xsd:float ;
                        rdfs:comment "Maturation phase: flavors develop and beer clarifies."@en .


###  http://www.semanticweb.org/matte/ontologies/2025/10/untitled-ontology-4#EPA_CoolingToPitchTemp
:EPA_CoolingToPitchTemp rdf:type owl:NamedIndividual ,
                                 <http://www.beerecipe.com/ontology#BrewingStep> ,
                                 <http://www.beerecipe.com/ontology#CoolingStep> ;
                        <http://www.beerecipe.com/ontology#isStepOf> :EasyPaleAleRecipe ;
                        <http://www.beerecipe.com/ontology#stepDuration> 20 ;
                        <http://www.beerecipe.com/ontology#stepName> "Cooling" ;
                        <http://www.beerecipe.com/ontology#stepOrder> 6 ;
                        <http://www.beerecipe.com/ontology#stepTemperature> "18.0"^^xsd:float ;
                        rdfs:comment "Rapidly cool wort to yeast pitching temperature for clean fermentation."@en .


###  http://www.semanticweb.org/matte/ontologies/2025/10/untitled-ontology-4#EPA_Fermentation10days
:EPA_Fermentation10days rdf:type owl:NamedIndividual ,
                                 <http://www.beerecipe.com/ontology#BrewingStep> ,
                                 <http://www.beerecipe.com/ontology#FermentationStep> ;
                        <http://www.beerecipe.com/ontology#isStepOf> :EasyPaleAleRecipe ;
                        <http://www.beerecipe.com/ontology#stepDuration> 14400 ;
                        <http://www.beerecipe.com/ontology#stepName> "Fermentation" ;
                        <http://www.beerecipe.com/ontology#stepOrder> 7 ;
                        <http://www.beerecipe.com/ontology#stepTemperature> "20.0"^^xsd:float ;
                        rdfs:comment "Primary fermentation: yeast converts sugars to alcohol and CO2 for a balanced pale ale."@en .


###  http://www.semanticweb.org/matte/ontologies/2025/10/untitled-ontology-4#EPA_Mash60min
:EPA_Mash60min rdf:type owl:NamedIndividual ,
                        <http://www.beerecipe.com/ontology#BrewingStep> ,
                        <http://www.beerecipe.com/ontology#MashStep> ,
                        [ rdf:type owl:Restriction ;
                          owl:onProperty <http://www.beerecipe.com/ontology#stepTemperature> ;
                          owl:someValuesFrom xsd:float
                        ] ;
               <http://www.beerecipe.com/ontology#isStepOf> :EasyPaleAleRecipe ;
               <http://www.beerecipe.com/ontology#stepDuration> 60 ;
               <http://www.beerecipe.com/ontology#stepName> "Mash" ;
               <http://www.beerecipe.com/ontology#stepOrder> 1 ;
               <http://www.beerecipe.com/ontology#stepTemperature> "66.0"^^xsd:float ;
               rdfs:comment "Convert malt starches to fermentable sugars for a balanced pale ale body."@en .


###  http://www.semanticweb.org/matte/ontologies/2025/10/untitled-ontology-4#EPA_MashOut10min
:EPA_MashOut10min rdf:type owl:NamedIndividual ,
                           <http://www.beerecipe.com/ontology#BrewingStep> ,
                           <http://www.beerecipe.com/ontology#MashOutStep> ,
                           <http://www.beerecipe.com/ontology#MashStep> ,
                           [ rdf:type owl:Restriction ;
                             owl:onProperty <http://www.beerecipe.com/ontology#stepTemperature> ;
                             owl:someValuesFrom xsd:float
                           ] ;
                  <http://www.beerecipe.com/ontology#isStepOf> :EasyPaleAleRecipe ;
                  <http://www.beerecipe.com/ontology#stepDuration> 10 ;
                  <http://www.beerecipe.com/ontology#stepName> "MashOut" ;
                  <http://www.beerecipe.com/ontology#stepOrder> 2 ;
                  <http://www.beerecipe.com/ontology#stepTemperature> "76.0"^^xsd:float ;
                  rdfs:comment "Stop enzymatic activity and prepare for lautering."@en .


###  http://www.semanticweb.org/matte/ontologies/2025/10/untitled-ontology-4#EPA_Sparge15min
:EPA_Sparge15min rdf:type owl:NamedIndividual ,
                          <http://www.beerecipe.com/ontology#BrewingStep> ,
                          <http://www.beerecipe.com/ontology#SpargeStep> ;
                 <http://www.beerecipe.com/ontology#isStepOf> :EasyPaleAleRecipe ;
                 <http://www.beerecipe.com/ontology#stepDuration> 15 ;
                 <http://www.beerecipe.com/ontology#stepName> "Sparge" ;
                 <http://www.beerecipe.com/ontology#stepOrder> 3 ;
                 <http://www.beerecipe.com/ontology#stepTemperature> "76.0"^^xsd:float ;
                 rdfs:comment "Rinse grains to extract remaining sugars for a lighter, balanced pale ale."@en .


###  http://www.semanticweb.org/matte/ontologies/2025/10/untitled-ontology-4#EPA_Whirlpool10min
:EPA_Whirlpool10min rdf:type owl:NamedIndividual ,
                             <http://www.beerecipe.com/ontology#BrewingStep> ,
                             <http://www.beerecipe.com/ontology#WhirlpoolStep> ;
                    <http://www.beerecipe.com/ontology#isStepOf> :EasyPaleAleRecipe ;
                    <http://www.beerecipe.com/ontology#stepDuration> 10 ,
                                                                     40320 ;
                    <http://www.beerecipe.com/ontology#stepName> "Whirlpool" ;
                    <http://www.beerecipe.com/ontology#stepOrder> 5 ;
                    <http://www.beerecipe.com/ontology#stepTemperature> "85.0"^^xsd:float ;
                    rdfs:comment "Separate hops and trub for clarity before cooling."@en .


###  http://www.semanticweb.org/matte/ontologies/2025/10/untitled-ontology-4#EasyPaleAleRecipe
:EasyPaleAleRecipe rdf:type owl:NamedIndividual ,
                            <http://www.beerecipe.com/ontology#Recipe> ;
                   <http://www.beerecipe.com/ontology#hasCereal> :CanadaWinterWheat ,
                                                                 :Cereal_RiceWheat ;
                   <http://www.beerecipe.com/ontology#hasHop> :CascadeHop ;
                   <http://www.beerecipe.com/ontology#hasMalt> :PaleAleMalt ;
                   <http://www.beerecipe.com/ontology#hasStyle> :PaleAle ;
                   <http://www.beerecipe.com/ontology#hasYeast> <http://www.beerecipe.com/ontology#US05_Yeast> ;
                   :hasWater :Water ;
                   <http://www.beerecipe.com/ontology#author> "Unknown" ;
                   <http://www.beerecipe.com/ontology#batchSize> "20.0"^^xsd:float ;
                   <http://www.beerecipe.com/ontology#boilingTime> 60 ;
                   <http://www.beerecipe.com/ontology#conditioningDuration> 14 ;
                   <http://www.beerecipe.com/ontology#difficultyLevel> "beginner" ;
                   <http://www.beerecipe.com/ontology#estimatedABV> "4.8"^^xsd:float ;
                   <http://www.beerecipe.com/ontology#estimatedEBC> 10 ;
                   <http://www.beerecipe.com/ontology#estimatedIBU> 30 ;
                   <http://www.beerecipe.com/ontology#fermentationDuration> 10 ;
                   <http://www.beerecipe.com/ontology#finalGravity> "1.01"^^xsd:float ;
                   <http://www.beerecipe.com/ontology#mashingTime> 60 ;
                   <http://www.beerecipe.com/ontology#originalGravity> "1.048"^^xsd:float ;
                   <http://www.beerecipe.com/ontology#recipeDescription> "Fresh and balanced American Pale Ale with Cascade hops." ;
                   <http://www.beerecipe.com/ontology#recipeName> "Easy Pale Ale" ;
                   <http://www.beerecipe.com/ontology#servingTemperature> "8.0"^^xsd:float ;
                   <http://www.beerecipe.com/ontology#totalBrewingTime> 360 .


###  http://www.semanticweb.org/matte/ontologies/2025/10/untitled-ontology-4#ExtraPaleMalt
:ExtraPaleMalt rdf:type owl:NamedIndividual ;
               <http://www.beerecipe.com/ontology#maltName> "Extra Pale Malt" ;
               <http://www.beerecipe.com/ontology#ebc> 5.5 ;
               rdfs:comment "Base malt for pale ales and IPAs, provides fermentable sugars" ;
               rdfs:label "Extra Pale Malt" .


###  http://www.semanticweb.org/matte/ontologies/2025/10/untitled-ontology-4#Fermentation7days
:Fermentation7days rdf:type owl:NamedIndividual ,
                            <http://www.beerecipe.com/ontology#BrewingStep> ,
                            <http://www.beerecipe.com/ontology#FermentationStep> ;
                   <http://www.beerecipe.com/ontology#stepDuration> 10080 ,
                                                                    168 ;
                   <http://www.beerecipe.com/ontology#stepName> "Fermentation" ;
                   <http://www.beerecipe.com/ontology#stepOrder> 7 ;
                   <http://www.beerecipe.com/ontology#stepTemperature> "20.0"^^xsd:float ;
                   rdfs:comment "Yeast converts sugars into alcohol and CO2; primary fermentation phase."@en .


###  http://www.semanticweb.org/matte/ontologies/2025/10/untitled-ontology-4#FermentationVessel
:FermentationVessel rdf:type owl:NamedIndividual ,
                             <http://www.beerecipe.com/ontology#Equipment> ;
                    <http://www.beerecipe.com/ontology#isRequiredBy> :BrewDog_PunkIPA_Recipe ;
                    rdfs:comment "Airtight container (plastic bucket or glass carboy) for primary fermentation. Must hold at least 25L for this batch size." ;
                    rdfs:label "Fermentation Vessel" .


###  http://www.semanticweb.org/matte/ontologies/2025/10/untitled-ontology-4#FlakedOats
:FlakedOats rdf:type owl:NamedIndividual ;
            <http://www.beerecipe.com/ontology#cerealName> "Flaked Oats" ;
            <http://www.beerecipe.com/ontology#glutenContent> "true"^^xsd:boolean .


###  http://www.semanticweb.org/matte/ontologies/2025/10/untitled-ontology-4#GAS_RussianImperialStout
:GAS_RussianImperialStout rdf:type owl:NamedIndividual ,
                                   <http://www.beerecipe.com/ontology#Recipe> ;
                          <http://www.beerecipe.com/ontology#hasCereal> :FlakedOats ,
                                                                        :MarisOtter ,
                                                                        :RoastedBarley ;
                          <http://www.beerecipe.com/ontology#hasHop> :MagnumHop ;
                          <http://www.beerecipe.com/ontology#hasMalt> :ChocolateMalt ;
                          <http://www.beerecipe.com/ontology#hasStyle> :RussianImperialStout ;
                          <http://www.beerecipe.com/ontology#hasYeast> <http://www.beerecipe.com/ontology#WLP007_Yeast> ;
                          <http://www.beerecipe.com/ontology#producesBeer> :Bran_russinaImperialStout ;
                          :hasWater :Water ;
                          <http://www.beerecipe.com/ontology#author> "Brewing Ben (Brewer's Friend)" ;
                          <http://www.beerecipe.com/ontology#batchSize> "5.0"^^xsd:float ;
                          <http://www.beerecipe.com/ontology#boilingTime> 75 ;
                          <http://www.beerecipe.com/ontology#conditioningDuration> 60 ;
                          <http://www.beerecipe.com/ontology#creationDate> "2023-11-01"^^xsd:date ;
                          <http://www.beerecipe.com/ontology#difficultyLevel> "advanced" ;
                          <http://www.beerecipe.com/ontology#estimatedABV> "10.82"^^xsd:float ;
                          <http://www.beerecipe.com/ontology#estimatedEBC> 98 ;
                          <http://www.beerecipe.com/ontology#estimatedIBU> 64 ;
                          <http://www.beerecipe.com/ontology#fermentationDuration> 21 ;
                          <http://www.beerecipe.com/ontology#finalGravity> "1.027"^^xsd:float ;
                          <http://www.beerecipe.com/ontology#isGlutenFree> "false"^^xsd:boolean ;
                          <http://www.beerecipe.com/ontology#isVegan> "false"^^xsd:boolean ;
                          <http://www.beerecipe.com/ontology#mashingTime> 60 ;
                          <http://www.beerecipe.com/ontology#originalGravity> "1.109"^^xsd:float ;
                          <http://www.beerecipe.com/ontology#recipeDescription> "Russian Imperial Stout — ricetta all-grain ad alta gravità con maris otter, roasted barley, chocolate malts e flaked oats. Versione ricetta pubblicata su Brewer's Friend." ;
                          <http://www.beerecipe.com/ontology#recipeName> "GAS RIS (Russian Imperial Stout)" ;
                          <http://www.beerecipe.com/ontology#servingTemperature> "12.0"^^xsd:float ;
                          <http://www.beerecipe.com/ontology#totalBrewingTime> 180 .


###  http://www.semanticweb.org/matte/ontologies/2025/10/untitled-ontology-4#Hydrometer
:Hydrometer rdf:type owl:NamedIndividual ,
                     <http://www.beerecipe.com/ontology#Equipment> ;
            <http://www.beerecipe.com/ontology#isRequiredBy> :BrewDog_PunkIPA_Recipe ;
            rdfs:comment "Instrument to measure specific gravity of wort/beer, essential for calculating ABV and monitoring fermentation." ;
            rdfs:label "Hydrometer" .


###  http://www.semanticweb.org/matte/ontologies/2025/10/untitled-ontology-4#IPA
:IPA rdf:type owl:NamedIndividual ,
              <http://www.beerecipe.com/ontology#BeerStyle> ;
     rdfs:comment "India Pale Ale: hop-forward beer style with pronounced bitterness and citrus/tropical fruit aromas, typically 5.5-7.5% ABV." ;
     rdfs:label "IPA" .


###  http://www.semanticweb.org/matte/ontologies/2025/10/untitled-ontology-4#MagnumHop
:MagnumHop rdf:type owl:NamedIndividual ,
                    <https://rdf.ag/o/hops#Hops> ;
           <http://www.beerecipe.com/ontology#alphaAcidPercentage> "13.5"^^xsd:float ;
           <http://www.beerecipe.com/ontology#hopName> "Magnum" ;
           rdfs:comment "German high-alpha bittering hop with clean, neutral bitterness and mild hop aroma, excellent for high-gravity beers." ;
           rdfs:label "Magnum" .


###  http://www.semanticweb.org/matte/ontologies/2025/10/untitled-ontology-4#MarisOtter
:MarisOtter rdf:type owl:NamedIndividual ,
                     :Cereal ;
            rdfs:comment "Premium British two-row spring barley variety prized for its rich, malty flavor and excellent extract efficiency." ;
            rdfs:label "Maris Otter" .


###  http://www.semanticweb.org/matte/ontologies/2025/10/untitled-ontology-4#MarisOtterMalt
:MarisOtterMalt rdf:type owl:NamedIndividual ;
                <http://www.beerecipe.com/ontology#ebcColor> 8 ;
                <http://www.beerecipe.com/ontology#maltName> "Maris Otter Malt" .


###  http://www.semanticweb.org/matte/ontologies/2025/10/untitled-ontology-4#MashOut10min
:MashOut10min rdf:type owl:NamedIndividual ,
                       <http://www.beerecipe.com/ontology#BrewingStep> ,
                       <http://www.beerecipe.com/ontology#MashStep> ,
                       [ rdf:type owl:Restriction ;
                         owl:onProperty <http://www.beerecipe.com/ontology#stepTemperature> ;
                         owl:someValuesFrom xsd:float
                       ] ;
              <http://www.beerecipe.com/ontology#stepDuration> 10 ;
              <http://www.beerecipe.com/ontology#stepName> "MashOut" ;
              <http://www.beerecipe.com/ontology#stepOrder> 2 ;
              <http://www.beerecipe.com/ontology#stepTemperature> "76.0"^^xsd:float ;
              rdfs:comment "Stop enzymatic activity and raise mash temperature to prepare for lautering or sparging."@en .


###  http://www.semanticweb.org/matte/ontologies/2025/10/untitled-ontology-4#MashTun
:MashTun rdf:type owl:NamedIndividual ,
                  <http://www.beerecipe.com/ontology#Equipment> ;
         <http://www.beerecipe.com/ontology#isRequiredBy> :BrewDog_PunkIPA_Recipe ;
         rdfs:comment "Insulated vessel for mashing grains at controlled temperatures to convert starches to fermentable sugars." ;
         rdfs:label "Mash Tun" .


###  http://www.semanticweb.org/matte/ontologies/2025/10/untitled-ontology-4#NelsonSauvinHop
:NelsonSauvinHop rdf:type owl:NamedIndividual ,
                          <https://rdf.ag/o/hops#Hops> ;
                 <http://www.beerecipe.com/ontology#alphaAcidPercentage> "12.0"^^xsd:float ;
                 <http://www.beerecipe.com/ontology#hopName> "Nelson Sauvin" ;
                 rdfs:comment "New Zealand hop with distinctive white wine, gooseberry character. Signature BrewDog hop" ;
                 rdfs:label "Nelson Sauvin" .


###  http://www.semanticweb.org/matte/ontologies/2025/10/untitled-ontology-4#NewZealand
:NewZealand rdf:type owl:NamedIndividual ,
                     <http://www.beerecipe.com/ontology#Country> ;
            rdfs:comment "Origin of Nelson Sauvin hop variety with distinctive white wine character. Known for unique southern hemisphere hop varieties." ;
            rdfs:label "New Zealand" .


###  http://www.semanticweb.org/matte/ontologies/2025/10/untitled-ontology-4#PaleAle
:PaleAle rdf:type owl:NamedIndividual ,
                  <http://www.beerecipe.com/ontology#BeerStyle> ;
         <http://www.beerecipe.com/ontology#styleName> "Pale Ale" .


###  http://www.semanticweb.org/matte/ontologies/2025/10/untitled-ontology-4#PaleAleMalt
:PaleAleMalt rdf:type owl:NamedIndividual ;
             <http://www.beerecipe.com/ontology#ebcColor> 6 ;
             <http://www.beerecipe.com/ontology#maltName> "Pale Ale Malt" .


###  http://www.semanticweb.org/matte/ontologies/2025/10/untitled-ontology-4#PunkIPA_Beer
:PunkIPA_Beer rdf:type owl:NamedIndividual ,
                       <https://rdf.ag/o/beer#Beer> ;
              rdfs:comment "BrewDog's flagship craft beer: post-modern pale ale with tropical fruit character, 5.6% ABV and 40 IBU." ;
              rdfs:label "Punk IPA" .


###  http://www.semanticweb.org/matte/ontologies/2025/10/untitled-ontology-4#PunkIPA_Boil60min
:PunkIPA_Boil60min rdf:type owl:NamedIndividual ,
                            <http://www.beerecipe.com/ontology#BoilStep> ,
                            <http://www.beerecipe.com/ontology#BrewingStep> ;
                   <http://www.beerecipe.com/ontology#isStepOf> :BrewDog_PunkIPA_Recipe ;
                   <http://www.beerecipe.com/ontology#stepDuration> 60 ;
                   <http://www.beerecipe.com/ontology#stepName> "Boil" ;
                   <http://www.beerecipe.com/ontology#stepOrder> 4 ;
                   <http://www.beerecipe.com/ontology#stepTemperature> "100.0"^^xsd:float ;
                   rdfs:comment "60 minute boil with hop additions at 60min (bittering), 15min and flameout (aroma)"@en .


###  http://www.semanticweb.org/matte/ontologies/2025/10/untitled-ontology-4#PunkIPA_Conditioning14days
:PunkIPA_Conditioning14days rdf:type owl:NamedIndividual ,
                                     <http://www.beerecipe.com/ontology#BrewingStep> ,
                                     <http://www.beerecipe.com/ontology#ConditioningStep> ;
                            <http://www.beerecipe.com/ontology#isStepOf> :BrewDog_PunkIPA_Recipe ;
                            <http://www.beerecipe.com/ontology#stepDuration> 20160 ;
                            <http://www.beerecipe.com/ontology#stepName> "Conditioning" ;
                            <http://www.beerecipe.com/ontology#stepOrder> 8 ;
                            <http://www.beerecipe.com/ontology#stepTemperature> "7.0"^^xsd:float ;
                            rdfs:comment "Cold conditioning for clarity and carbonation"@en .


###  http://www.semanticweb.org/matte/ontologies/2025/10/untitled-ontology-4#PunkIPA_Cooling30min
:PunkIPA_Cooling30min rdf:type owl:NamedIndividual ,
                               <http://www.beerecipe.com/ontology#BrewingStep> ,
                               <http://www.beerecipe.com/ontology#CoolingStep> ;
                      <http://www.beerecipe.com/ontology#isStepOf> :BrewDog_PunkIPA_Recipe ;
                      <http://www.beerecipe.com/ontology#stepDuration> 30 ;
                      <http://www.beerecipe.com/ontology#stepName> "Cooling" ;
                      <http://www.beerecipe.com/ontology#stepOrder> 6 ;
                      <http://www.beerecipe.com/ontology#stepTemperature> "18.0"^^xsd:float ;
                      rdfs:comment "Rapidly cool wort to yeast pitching temperature"@en .


###  http://www.semanticweb.org/matte/ontologies/2025/10/untitled-ontology-4#PunkIPA_Fermentation10days
:PunkIPA_Fermentation10days rdf:type owl:NamedIndividual ,
                                     <http://www.beerecipe.com/ontology#BrewingStep> ,
                                     <http://www.beerecipe.com/ontology#FermentationStep> ;
                            <http://www.beerecipe.com/ontology#isStepOf> :BrewDog_PunkIPA_Recipe ;
                            <http://www.beerecipe.com/ontology#stepDuration> 14400 ;
                            <http://www.beerecipe.com/ontology#stepName> "Fermentation" ;
                            <http://www.beerecipe.com/ontology#stepOrder> 7 ;
                            <http://www.beerecipe.com/ontology#stepTemperature> "19.0"^^xsd:float ;
                            rdfs:comment "Primary fermentation with dry hop addition on day 4"@en .


###  http://www.semanticweb.org/matte/ontologies/2025/10/untitled-ontology-4#PunkIPA_Mash65min
:PunkIPA_Mash65min rdf:type owl:NamedIndividual ,
                            <http://www.beerecipe.com/ontology#BrewingStep> ,
                            <http://www.beerecipe.com/ontology#MashStep> ;
                   <http://www.beerecipe.com/ontology#isStepOf> :BrewDog_PunkIPA_Recipe ;
                   <http://www.beerecipe.com/ontology#stepDuration> 65 ;
                   <http://www.beerecipe.com/ontology#stepName> "Mash" ;
                   <http://www.beerecipe.com/ontology#stepOrder> 1 ;
                   <http://www.beerecipe.com/ontology#stepTemperature> "65.0"^^xsd:float ;
                   rdfs:comment "Single infusion mash to convert starches to fermentable sugars"@en .


###  http://www.semanticweb.org/matte/ontologies/2025/10/untitled-ontology-4#PunkIPA_MashOut10min
:PunkIPA_MashOut10min rdf:type owl:NamedIndividual ,
                               <http://www.beerecipe.com/ontology#BrewingStep> ,
                               <http://www.beerecipe.com/ontology#MashOutStep> ,
                               <http://www.beerecipe.com/ontology#MashStep> ;
                      <http://www.beerecipe.com/ontology#isStepOf> :BrewDog_PunkIPA_Recipe ;
                      <http://www.beerecipe.com/ontology#stepDuration> 10 ;
                      <http://www.beerecipe.com/ontology#stepName> "MashOut" ;
                      <http://www.beerecipe.com/ontology#stepOrder> 2 ;
                      <http://www.beerecipe.com/ontology#stepTemperature> "75.0"^^xsd:float ;
                      rdfs:comment "Stop enzymatic activity and prepare for lautering"@en .


###  http://www.semanticweb.org/matte/ontologies/2025/10/untitled-ontology-4#PunkIPA_Sparge15min
:PunkIPA_Sparge15min rdf:type owl:NamedIndividual ,
                              <http://www.beerecipe.com/ontology#BrewingStep> ,
                              <http://www.beerecipe.com/ontology#SpargeStep> ;
                     <http://www.beerecipe.com/ontology#isStepOf> :BrewDog_PunkIPA_Recipe ;
                     <http://www.beerecipe.com/ontology#stepDuration> 15 ;
                     <http://www.beerecipe.com/ontology#stepName> "Sparge" ;
                     <http://www.beerecipe.com/ontology#stepOrder> 3 ;
                     <http://www.beerecipe.com/ontology#stepTemperature> "75.0"^^xsd:float ;
                     rdfs:comment "Rinse grains to extract remaining sugars"@en .


###  http://www.semanticweb.org/matte/ontologies/2025/10/untitled-ontology-4#PunkIPA_Whirlpool20min
:PunkIPA_Whirlpool20min rdf:type owl:NamedIndividual ,
                                 <http://www.beerecipe.com/ontology#BrewingStep> ,
                                 <http://www.beerecipe.com/ontology#WhirlpoolStep> ;
                        <http://www.beerecipe.com/ontology#isStepOf> :BrewDog_PunkIPA_Recipe ;
                        <http://www.beerecipe.com/ontology#stepDuration> 20 ;
                        <http://www.beerecipe.com/ontology#stepName> "Whirlpool" ;
                        <http://www.beerecipe.com/ontology#stepOrder> 5 ;
                        <http://www.beerecipe.com/ontology#stepTemperature> "80.0"^^xsd:float ;
                        rdfs:comment "Whirlpool at 80°C with hop additions for enhanced aroma"@en .


###  http://www.semanticweb.org/matte/ontologies/2025/10/untitled-ontology-4#RIS_Boil90min
:RIS_Boil90min rdf:type owl:NamedIndividual ,
                        <http://www.beerecipe.com/ontology#BoilStep> ,
                        <http://www.beerecipe.com/ontology#BrewingStep> ;
               <http://www.beerecipe.com/ontology#isStepOf> :GAS_RussianImperialStout ;
               <http://www.beerecipe.com/ontology#stepDuration> 90 ;
               <http://www.beerecipe.com/ontology#stepName> "Boil" ;
               <http://www.beerecipe.com/ontology#stepOrder> 4 ;
               <http://www.beerecipe.com/ontology#stepTemperature> "100.0"^^xsd:float ;
               rdfs:comment "Sterilizes the wort, isomerizes hop alpha acids, and drives off unwanted volatile compounds."@en .


###  http://www.semanticweb.org/matte/ontologies/2025/10/untitled-ontology-4#RIS_Conditioning28days
:RIS_Conditioning28days rdf:type owl:NamedIndividual ,
                                 <http://www.beerecipe.com/ontology#BrewingStep> ,
                                 <http://www.beerecipe.com/ontology#ConditioningStep> ;
                        <http://www.beerecipe.com/ontology#stepDuration> 40320 ;
                        <http://www.beerecipe.com/ontology#stepName> "Conditioning" ;
                        <http://www.beerecipe.com/ontology#stepOrder> 8 ;
                        <http://www.beerecipe.com/ontology#stepTemperature> "12.0"^^xsd:float ;
                        rdfs:comment "Maturation phase: flavors develop, beer clarifies and stabilizes."@en .


###  http://www.semanticweb.org/matte/ontologies/2025/10/untitled-ontology-4#RIS_CoolingToPitchTemp
:RIS_CoolingToPitchTemp rdf:type owl:NamedIndividual ,
                                 <http://www.beerecipe.com/ontology#BrewingStep> ,
                                 <http://www.beerecipe.com/ontology#CoolingStep> ;
                        <http://www.beerecipe.com/ontology#isStepOf> :GAS_RussianImperialStout ;
                        <http://www.beerecipe.com/ontology#stepDuration> 40 ;
                        <http://www.beerecipe.com/ontology#stepName> "Cooling" ;
                        <http://www.beerecipe.com/ontology#stepOrder> 6 ;
                        <http://www.beerecipe.com/ontology#stepTemperature> "20.0"^^xsd:float ;
                        rdfs:comment "Rapidly cool wort to yeast pitching temperature."@en .


###  http://www.semanticweb.org/matte/ontologies/2025/10/untitled-ontology-4#RIS_Fermentation14days
:RIS_Fermentation14days rdf:type owl:NamedIndividual ,
                                 <http://www.beerecipe.com/ontology#BrewingStep> ,
                                 <http://www.beerecipe.com/ontology#FermentationStep> ;
                        <http://www.beerecipe.com/ontology#isStepOf> :GAS_RussianImperialStout ;
                        <http://www.beerecipe.com/ontology#stepDuration> 20160 ;
                        <http://www.beerecipe.com/ontology#stepName> "Fermentation" ;
                        <http://www.beerecipe.com/ontology#stepOrder> 7 ;
                        <http://www.beerecipe.com/ontology#stepTemperature> "20.0"^^xsd:float ;
                        rdfs:comment "Primary fermentation: yeast converts sugars into alcohol and CO2."@en .


###  http://www.semanticweb.org/matte/ontologies/2025/10/untitled-ontology-4#RIS_Mash60min
:RIS_Mash60min rdf:type owl:NamedIndividual ,
                        <http://www.beerecipe.com/ontology#BrewingStep> ,
                        <http://www.beerecipe.com/ontology#MashStep> ,
                        [ rdf:type owl:Restriction ;
                          owl:onProperty <http://www.beerecipe.com/ontology#stepTemperature> ;
                          owl:someValuesFrom xsd:float
                        ] ;
               <http://www.beerecipe.com/ontology#isStepOf> :GAS_RussianImperialStout ;
               <http://www.beerecipe.com/ontology#stepDuration> 60 ;
               <http://www.beerecipe.com/ontology#stepName> "Mash" ;
               <http://www.beerecipe.com/ontology#stepOrder> 1 ;
               <http://www.beerecipe.com/ontology#stepTemperature> "68.0"^^xsd:float ;
               rdfs:comment "Conversion of starches in the malt to fermentable sugars via enzymatic activity."@en .


###  http://www.semanticweb.org/matte/ontologies/2025/10/untitled-ontology-4#RIS_MashOut10min
:RIS_MashOut10min rdf:type owl:NamedIndividual ,
                           <http://www.beerecipe.com/ontology#BrewingStep> ,
                           <http://www.beerecipe.com/ontology#MashOutStep> ,
                           <http://www.beerecipe.com/ontology#MashStep> ,
                           [ rdf:type owl:Restriction ;
                             owl:onProperty <http://www.beerecipe.com/ontology#stepTemperature> ;
                             owl:someValuesFrom xsd:float
                           ] ;
                  <http://www.beerecipe.com/ontology#isStepOf> :GAS_RussianImperialStout ;
                  <http://www.beerecipe.com/ontology#stepDuration> 10 ;
                  <http://www.beerecipe.com/ontology#stepName> "MashOut" ;
                  <http://www.beerecipe.com/ontology#stepOrder> 2 ;
                  <http://www.beerecipe.com/ontology#stepTemperature> "76.0"^^xsd:float ;
                  rdfs:comment "Stop enzymatic activity and raise mash temperature to prepare for lautering or sparging."@en .


###  http://www.semanticweb.org/matte/ontologies/2025/10/untitled-ontology-4#RIS_Sparge20min
:RIS_Sparge20min rdf:type owl:NamedIndividual ,
                          <http://www.beerecipe.com/ontology#BrewingStep> ,
                          <http://www.beerecipe.com/ontology#SpargeStep> ;
                 <http://www.beerecipe.com/ontology#isStepOf> :GAS_RussianImperialStout ;
                 <http://www.beerecipe.com/ontology#stepDuration> 20 ;
                 <http://www.beerecipe.com/ontology#stepName> "Sparge" ;
                 <http://www.beerecipe.com/ontology#stepOrder> 3 ;
                 <http://www.beerecipe.com/ontology#stepTemperature> "76.0"^^xsd:float ;
                 rdfs:comment "Rinse the grains to extract remaining sugars and increase wort yield."@en .


###  http://www.semanticweb.org/matte/ontologies/2025/10/untitled-ontology-4#RIS_Whirlpool15min
:RIS_Whirlpool15min rdf:type owl:NamedIndividual ,
                             <http://www.beerecipe.com/ontology#BrewingStep> ,
                             <http://www.beerecipe.com/ontology#WhirlpoolStep> ;
                    <http://www.beerecipe.com/ontology#isStepOf> :GAS_RussianImperialStout ;
                    <http://www.beerecipe.com/ontology#stepDuration> 15 ;
                    <http://www.beerecipe.com/ontology#stepName> "Whirlpool" ;
                    <http://www.beerecipe.com/ontology#stepOrder> 5 ;
                    <http://www.beerecipe.com/ontology#stepTemperature> "85.0"^^xsd:float ;
                    rdfs:comment "Separates hops and trub from the wort via vortexing; helps clarify the wort before cooling."@en .


###  http://www.semanticweb.org/matte/ontologies/2025/10/untitled-ontology-4#RoastedBarley
:RoastedBarley rdf:type owl:NamedIndividual ;
               <http://www.beerecipe.com/ontology#cerealName> "Roasted Barley" ;
               <http://www.beerecipe.com/ontology#glutenContent> "true"^^xsd:boolean .


###  http://www.semanticweb.org/matte/ontologies/2025/10/untitled-ontology-4#RussianImperialStout
:RussianImperialStout rdf:type owl:NamedIndividual ,
                               <http://www.beerecipe.com/ontology#BeerStyle> ;
                      <http://www.beerecipe.com/ontology#maxABV> "12.0"^^xsd:float ;
                      <http://www.beerecipe.com/ontology#maxIBU> 90 ;
                      <http://www.beerecipe.com/ontology#minABV> "8.0"^^xsd:float ;
                      <http://www.beerecipe.com/ontology#minIBU> 30 ;
                      <http://www.beerecipe.com/ontology#styleDescription> "Rich, intense, full-bodied stout with strong roasted and dark fruit notes." ;
                      <http://www.beerecipe.com/ontology#styleName> "Russian Imperial Stout" .


###  http://www.semanticweb.org/matte/ontologies/2025/10/untitled-ontology-4#Sanitizer
:Sanitizer rdf:type owl:NamedIndividual ,
                    <http://www.beerecipe.com/ontology#Equipment> ;
           <http://www.beerecipe.com/ontology#isRequiredBy> :BrewDog_PunkIPA_Recipe ;
           rdfs:comment "No-rinse sanitizer (e.g., Star San) essential for sanitizing all equipment that contacts wort/beer post-boil." ;
           rdfs:label "Sanitizer" .


###  http://www.semanticweb.org/matte/ontologies/2025/10/untitled-ontology-4#Scotland
:Scotland rdf:type owl:NamedIndividual ,
                   <http://www.beerecipe.com/ontology#Country> ;
          <http://www.beerecipe.com/ontology#isOriginOf> :BrewDog_PunkIPA_Recipe ;
          rdfs:comment "Home of BrewDog brewery in Ellon, Aberdeenshire. Known for craft beer revolution and innovative brewing techniques." ;
          rdfs:label "Scotland" .


###  http://www.semanticweb.org/matte/ontologies/2025/10/untitled-ontology-4#SimcoeHop
:SimcoeHop rdf:type owl:NamedIndividual ,
                    <https://rdf.ag/o/hops#Hops> ;
           <http://www.beerecipe.com/ontology#alphaAcidPercentage> "13.0"^^xsd:float ;
           <http://www.beerecipe.com/ontology#hopName> "Simcoe" ;
           rdfs:comment "American hop with passion fruit, pine and earthy character" ;
           rdfs:label "Simcoe" .


###  http://www.semanticweb.org/matte/ontologies/2025/10/untitled-ontology-4#Sparge20min
:Sparge20min rdf:type owl:NamedIndividual ,
                      <http://www.beerecipe.com/ontology#SpargeStep> ;
             <http://www.beerecipe.com/ontology#stepDuration> 20 ;
             <http://www.beerecipe.com/ontology#stepName> "Sparge" ;
             <http://www.beerecipe.com/ontology#stepOrder> 3 ;
             <http://www.beerecipe.com/ontology#stepTemperature> "76.0"^^xsd:float ;
             rdfs:comment "Rinse the grains to extract remaining sugars and increase wort yield."@en .


###  http://www.semanticweb.org/matte/ontologies/2025/10/untitled-ontology-4#StandardMash45min
:StandardMash45min rdf:type owl:NamedIndividual ,
                            <http://www.beerecipe.com/ontology#MashStep> ;
                   <http://www.beerecipe.com/ontology#stepDuration> 45 ;
                   <http://www.beerecipe.com/ontology#stepName> "Mash" ;
                   <http://www.beerecipe.com/ontology#stepOrder> 1 ;
                   <http://www.beerecipe.com/ontology#stepTemperature> "66.0"^^xsd:float ;
                   rdfs:comment "Conversion of starches in the malt to fermentable sugars via enzymatic activity."@en .


###  http://www.semanticweb.org/matte/ontologies/2025/10/untitled-ontology-4#Thermometer
:Thermometer rdf:type owl:NamedIndividual ,
                      <http://www.beerecipe.com/ontology#Equipment> ;
             <http://www.beerecipe.com/ontology#isRequiredBy> :BrewDog_PunkIPA_Recipe ;
             rdfs:comment "Digital or analog thermometer (range 0-110°C) for monitoring mash, boil, and fermentation temperatures." ;
             rdfs:label "Brewing Thermometer" .


###  http://www.semanticweb.org/matte/ontologies/2025/10/untitled-ontology-4#TripleHoppedIPA
:TripleHoppedIPA rdf:type owl:NamedIndividual ;
                 <http://www.beerecipe.com/ontology#hasStyle> :AmericanIPA ;
                 <http://www.beerecipe.com/ontology#difficultyLevel> "advanced" ;
                 <http://www.beerecipe.com/ontology#estimatedABV> "7.2"^^xsd:float ;
                 <http://www.beerecipe.com/ontology#estimatedIBU> 65 .


###  http://www.semanticweb.org/matte/ontologies/2025/10/untitled-ontology-4#UnitedKingdom
:UnitedKingdom rdf:type owl:NamedIndividual ,
                        <http://www.beerecipe.com/ontology#Country> ;
               rdfs:comment "Origin of pale ale malt varieties and traditional British brewing techniques. Home to Maris Otter barley." ;
               rdfs:label "United Kingdom" .


###  http://www.semanticweb.org/matte/ontologies/2025/10/untitled-ontology-4#UnitedStates
:UnitedStates rdf:type owl:NamedIndividual ,
                       <http://www.beerecipe.com/ontology#Country> ;
              rdfs:comment "Origin of American hop varieties (Chinook, Simcoe, Ahtanum) and American IPA style. Major craft beer innovation hub." ;
              rdfs:label "United States" .


###  http://www.semanticweb.org/matte/ontologies/2025/10/untitled-ontology-4#Water
:Water rdf:type owl:NamedIndividual ,
                :Water .


###  http://www.semanticweb.org/matte/ontologies/2025/10/untitled-ontology-4#Whirlpool15min
:Whirlpool15min rdf:type owl:NamedIndividual ,
                         <http://www.beerecipe.com/ontology#WhirlpoolStep> ;
                <http://www.beerecipe.com/ontology#stepDuration> 15 ;
                <http://www.beerecipe.com/ontology#stepName> "Whirlpool" ;
                <http://www.beerecipe.com/ontology#stepOrder> 5 ;
                <http://www.beerecipe.com/ontology#stepTemperature> "85.0"^^xsd:float ;
                rdfs:comment "Separates hops and trub from the wort via vortexing; helps clarify the wort before cooling."@en .


###  http://www.semanticweb.org/matte/ontologies/2025/10/untitled-ontology-4#WortChiller
:WortChiller rdf:type owl:NamedIndividual ,
                      <http://www.beerecipe.com/ontology#Equipment> ;
             <http://www.beerecipe.com/ontology#isRequiredBy> :BrewDog_PunkIPA_Recipe ;
             rdfs:comment "Immersion or counterflow chiller to rapidly cool wort from boiling to pitching temperature (18-20°C)." ;
             rdfs:label "Wort Chiller" .


#################################################################
#    Annotations
#################################################################

<http://www.beerecipe.com/ontology#hasBrewingStep> rdfs:comment "Connects a recipe to its brewing steps" ;
                                                   rdfs:label "has brewing step" .


<http://www.beerecipe.com/ontology#hasCereal> rdfs:comment "Connects a recipe to the cereals used, especially for gluten-free recipes" ;
                                              rdfs:label "has cereal" .


<http://www.beerecipe.com/ontology#hasHop> rdfs:comment "Connects a recipe to the hops used" ;
                                           rdfs:label "has hop" .


<http://www.beerecipe.com/ontology#hasIngredient> rdfs:comment "Connects a recipe to its ingredients" ;
                                                  rdfs:label "has ingredient" .


<http://www.beerecipe.com/ontology#hasMalt> rdfs:comment "Connects a recipe to the malts used" ;
                                            rdfs:label "has malt" .


<http://www.beerecipe.com/ontology#hasStyle> rdfs:comment "Connects a recipe to its beer style (IPA, Stout, Lager, etc.)" ;
                                             rdfs:label "has style" .


<http://www.beerecipe.com/ontology#isCerealOf> rdfs:comment "Indicates that a cereal is used in a recipe" ;
                                               rdfs:label "is cereal of" .


<http://www.beerecipe.com/ontology#isHopOf> rdfs:comment "Indicates that a hop is used in a recipe" ;
                                            rdfs:label "is hop of" .


<http://www.beerecipe.com/ontology#isIngredientOf> rdfs:comment "Indicates that an ingredient is part of a recipe" ;
                                                   rdfs:label "is ingredient of" .


<http://www.beerecipe.com/ontology#isMaltOf> rdfs:comment "Indicates that a malt is used in a recipe" ;
                                             rdfs:label "is malt of" .


<http://www.beerecipe.com/ontology#isOriginOf> rdfs:comment "Indicates ingredients that originate from this country" ;
                                               rdfs:label "is origin of" .


<http://www.beerecipe.com/ontology#isProducedBy> rdfs:comment "Indicates that a beer is produced by a specific recipe" ;
                                                 rdfs:label "is produced by" .


<http://www.beerecipe.com/ontology#isRequiredBy> rdfs:comment "Indicates which recipes require this equipment" ;
                                                 rdfs:label "is required by" .


<http://www.beerecipe.com/ontology#isSimilarTo> rdfs:comment "Indicates that two recipes are similar. This is a symmetric and transitive property." ;
                                                rdfs:label "is similar to" .


<http://www.beerecipe.com/ontology#isStepOf> rdfs:comment "Indicates that a brewing step belongs to a recipe" ;
                                             rdfs:label "is step of" .


<http://www.beerecipe.com/ontology#isStyleOf> rdfs:comment "Indicates recipes that belong to this beer style" ;
                                              rdfs:label "is style of" .


<http://www.beerecipe.com/ontology#isYeastOf> rdfs:comment "Indicates that a yeast is used in a recipe" ;
                                              rdfs:label "is yeast of" .


<http://www.beerecipe.com/ontology#producesBeer> rdfs:comment "Connects a recipe to the beer it produces. A recipe produces exactly one type of beer." ;
                                                 rdfs:label "produces beer" .


:Water rdfs:comment "Brewing water - the primary ingredient in beer, comprising 90-95% of the final product. Water chemistry significantly affects beer flavor." ;
       rdfs:label "Water" .


<https://rdf.ag/o/cerealstoo#EasternCanadaWheat> <http://rdfs.org/ns/void#inDataset> <https://rdf.ag/o/cerealstoo#datasetdefinition> ;
                                                 rdfs:isDefinedBy <https://rdf.ag/o/cerealstoo-2021-02-18> ;
                                                 rdfs:label "Blé de l'Est du Canada"@fr ,
                                                            "Eastern Canada Wheat"@en ;
                                                 <http://www.w3.org/2004/02/skos/core#definition> "Eastern Canadian grains are regulated by the Canadian Eastern Grain Commission and they include the classes and varieties of grains grown in the eastern Canadian provences of Ontario, Quebéc,New Brunswick, Nova Scotia, Prince Edward Island and Newfoundland and Labrador."@en ,
                                                                                                  "Les grains de l'est du Canada sont réglementés par la Commission canadienne des grains de l'Est et comprennent les classes et les variétés de grains cultivés dans les provinces de l'est du Canada de l'Ontario, du Québec, du Nouveau-Brunswick, de la Nouvelle-Écosse, de l'Île-du-Prince-Édouard et de Terre-Neuve-et-Labrador."@fr ;
                                                 <http://www.w3.org/ns/prov#hadPrimarySource> <https://rdf.ag/o/cerealstoo#CanadianGrainCommission2019Canadian-Wheat-Classes> .


<https://rdf.ag/o/cerealstoo#HRS> <http://rdfs.org/ns/void#inDataset> <https://rdf.ag/o/cerealstoo#datasetdefinition> ;
                                  rdfs:isDefinedBy <https://rdf.ag/o/cerealstoo-2021-02-18> ;
                                  rdfs:label "Blé de Force Rouge de Printemps"@fr ,
                                             "Hard Red Spring Wheat"@en ;
                                  <http://www.w3.org/2004/02/skos/core#definition> "Cette classe comprend toutes les variétés de Blé de Force Rouge de printemps."@fr ,
                                                                                   "This class consists of all varieties of Hard Red Spring Wheat."@en ;
                                  <http://www.w3.org/ns/prov#hadPrimarySource> <https://rdf.ag/o/cerealstoo#USDA2014StandardsforWheat> ;
                                  <http://xmlns.com/foaf/0.1/name> "HRS" .


<https://rdf.ag/o/cerealstoo#SWW> <http://rdfs.org/ns/void#inDataset> <https://rdf.ag/o/cerealstoo#datasetdefinition> ;
                                  rdfs:isDefinedBy <https://rdf.ag/o/cerealstoo-2021-02-18> ;
                                  rdfs:label "Blé Tendre Blanc (SWW)"@fr ,
                                             "Soft White Wheat (SWW)"@en ;
                                  <http://www.w3.org/2004/02/skos/core#definition> "Cette classe comprend tous les types de blé blanc dont les grains ont des endospermes mous."@fr ,
                                                                                   "This class consists of all types of white wheat whose kernels have soft endosperms."@en ;
                                  <http://www.w3.org/ns/prov#hadPrimarySource> <https://rdf.ag/o/cerealstoo#USDA2014StandardsforWheat> ;
                                  <http://xmlns.com/foaf/0.1/name> "SWW" .


###  Generated by the OWL API (version 5.1.18) https://github.com/owlcs/owlapi/
